<?xml version="1.0"?>
<rdf:RDF xmlns="http://www.semanticweb.org/macoda/ontologies/PMO#"
     xml:base="http://www.semanticweb.org/macoda/ontologies/PMO"
     xmlns:owl="http://www.w3.org/2002/07/owl#"
     xmlns:rdf="http://www.w3.org/1999/02/22-rdf-syntax-ns#"
     xmlns:xml="http://www.w3.org/XML/1998/namespace"
     xmlns:xsd="http://www.w3.org/2001/XMLSchema#"
     xmlns:PEMO="http://www.semanticweb.org/macoda/ontologies/PEMO#"
     xmlns:rdfs="http://www.w3.org/2000/01/rdf-schema#"
     xmlns:PMOEA="http://www.semanticweb.org/macoda/ontologies/PMOEA#">
    <owl:Ontology rdf:about="http://www.semanticweb.org/macoda/ontologies/PMOEA"/>
    


    <!-- 
    ///////////////////////////////////////////////////////////////////////////////////////
    //
    // Object Properties
    //
    ///////////////////////////////////////////////////////////////////////////////////////
     -->

    


    <!-- http://www.semanticweb.org/macoda/ontologies/PMOEA#hasPreferenceModel -->

    <owl:ObjectProperty rdf:about="http://www.semanticweb.org/macoda/ontologies/PMOEA#hasPreferenceModel">
        <rdfs:domain rdf:resource="http://www.semanticweb.org/macoda/ontologies/PMOEA#PMOEA"/>
        <rdfs:range rdf:resource="http://www.semanticweb.org/macoda/ontologies/PMOEA#PreferenceModel"/>
        <rdfs:label xml:lang="en">hasPreferenceModel</rdfs:label>
    </owl:ObjectProperty>
    


    <!-- http://www.semanticweb.org/macoda/ontologies/PMOEA#hasPreferenceInformationFromDM -->

    <owl:ObjectProperty rdf:about="http://www.semanticweb.org/macoda/ontologies/PMOEA#hasPreferenceInformationFromDM">
        <rdfs:domain rdf:resource="http://www.semanticweb.org/macoda/ontologies/PMOEA#PMOEA"/>
        <rdfs:range rdf:resource="http://www.semanticweb.org/macoda/ontologies/PMOEA#PreferenceInformationFromDM"/>
        <rdfs:label xml:lang="en">hasPreferenceInformationFromDM</rdfs:label>
    </owl:ObjectProperty>
    


    <!-- http://www.semanticweb.org/macoda/ontologies/PMOEA#hasInteractionTime -->

    <owl:ObjectProperty rdf:about="http://www.semanticweb.org/macoda/ontologies/PMOEA#hasInteractionTime">
        <rdfs:domain rdf:resource="http://www.semanticweb.org/macoda/ontologies/PMOEA#PMOEA"/>
        <rdfs:range rdf:resource="http://www.semanticweb.org/macoda/ontologies/PMOEA#InteractionTime"/>
        <rdfs:label xml:lang="en">hasInteractionTime</rdfs:label>
    </owl:ObjectProperty>
    


    <!-- http://www.semanticweb.org/macoda/ontologies/PMOEA#hasPreferenceIntegration -->

    <owl:ObjectProperty rdf:about="http://www.semanticweb.org/macoda/ontologies/PMOEA#hasPreferenceIntegration">
        <rdfs:domain rdf:resource="http://www.semanticweb.org/macoda/ontologies/PMOEA#PMOEA"/>
        <rdfs:range rdf:resource="http://www.semanticweb.org/macoda/ontologies/PMOEA#PreferenceIntegration"/>
        <rdfs:label xml:lang="en">hasPreferenceIntegration</rdfs:label>
    </owl:ObjectProperty>
    


    <!-- http://www.semanticweb.org/macoda/ontologies/PMOEA#isInteractiveVersionOf -->

    <owl:ObjectProperty rdf:about="http://www.semanticweb.org/macoda/ontologies/PMOEA#isInteractiveVersionOf">
        <owl:inverseOf rdf:resource="http://www.semanticweb.org/macoda/ontologies/PMOEA#hasInteractiveVersion"/>
        <rdfs:domain rdf:resource="http://www.semanticweb.org/macoda/ontologies/PMOEA#PMOEA"/>
        <rdfs:range rdf:resource="http://www.semanticweb.org/macoda/ontologies/PMOEA#PMOEA"/>
        <rdfs:label xml:lang="en">isInteractiveVersionOf</rdfs:label>
    </owl:ObjectProperty>
    


    <!-- http://www.semanticweb.org/macoda/ontologies/PMOEA#hasLearningMethod -->

    <owl:ObjectProperty rdf:about="http://www.semanticweb.org/macoda/ontologies/PMOEA#hasLearningMethod">
        <rdfs:domain rdf:resource="http://www.semanticweb.org/macoda/ontologies/PMOEA#PMOEA"/>
        <rdfs:range rdf:resource="http://www.semanticweb.org/macoda/ontologies/PMOEA#LearningMethod"/>
        <rdfs:label xml:lang="en">hasLearningMethod</rdfs:label>
    </owl:ObjectProperty>
    


    <!-- http://www.semanticweb.org/macoda/ontologies/PMOEA#hasComparison -->

    <owl:ObjectProperty rdf:about="http://www.semanticweb.org/macoda/ontologies/PMOEA#hasComparison">
        <rdfs:domain rdf:resource="http://www.semanticweb.org/macoda/ontologies/PMOEA#PMOEA"/>
        <rdfs:range rdf:resource="http://www.semanticweb.org/macoda/ontologies/PMOEA#PMOEA"/>
        <rdfs:label xml:lang="en">hasComparison</rdfs:label>
    </owl:ObjectProperty>
    


    <!-- http://www.semanticweb.org/macoda/ontologies/PMOEA#hasInteractiveVersion -->

    <owl:ObjectProperty rdf:about="http://www.semanticweb.org/macoda/ontologies/PMOEA#hasInteractiveVersion">
        <rdfs:domain rdf:resource="http://www.semanticweb.org/macoda/ontologies/PMOEA#PMOEA"/>
        <rdfs:range rdf:resource="http://www.semanticweb.org/macoda/ontologies/PMOEA#PMOEA"/>
        <rdfs:label xml:lang="en">hasInteractiveVersion</rdfs:label>
    </owl:ObjectProperty>
    


    <!-- http://www.semanticweb.org/macoda/ontologies/PMOEA#canSolve -->

    <owl:ObjectProperty rdf:about="http://www.semanticweb.org/macoda/ontologies/PMOEA#canSolve">
        <rdfs:domain rdf:resource="http://www.semanticweb.org/macoda/ontologies/PMOEA#MetaHeuristic"/>
        <rdfs:range rdf:resource="http://www.semanticweb.org/macoda/ontologies/PMOEA#MOP"/>
        <rdfs:label xml:lang="en">canSolve</rdfs:label>
    </owl:ObjectProperty>
    


    <!-- http://www.semanticweb.org/macoda/ontologies/PMOEA#hasResultInfluence -->

    <owl:ObjectProperty rdf:about="http://www.semanticweb.org/macoda/ontologies/PMOEA#hasResultInfluence">
        <rdfs:domain rdf:resource="http://www.semanticweb.org/macoda/ontologies/PMOEA#PMOEA"/>
        <rdfs:range rdf:resource="http://www.semanticweb.org/macoda/ontologies/PMOEA#ResultInfluence"/>
        <rdfs:label xml:lang="en">hasResultInfluence</rdfs:label>
    </owl:ObjectProperty>
    


    <!-- http://www.semanticweb.org/macoda/ontologies/PMOEA#hasAuthor -->

    <owl:ObjectProperty rdf:about="http://www.semanticweb.org/macoda/ontologies/PMOEA#hasAuthor">
        <rdfs:domain rdf:resource="http://www.semanticweb.org/macoda/ontologies/PMOEA#MetaHeuristic"/>
        <rdfs:range rdf:resource="http://www.semanticweb.org/macoda/ontologies/PMOEA#Researcher"/>
        <rdfs:label xml:lang="en">hasAuthor</rdfs:label>
    </owl:ObjectProperty>
    


    <!-- http://www.semanticweb.org/macoda/ontologies/PMOEA#hasExtension -->

    <owl:ObjectProperty rdf:about="http://www.semanticweb.org/macoda/ontologies/PMOEA#hasExtension">
        <owl:inverseOf rdf:resource="http://www.semanticweb.org/macoda/ontologies/PMOEA#isExtensionOf"/>
        <rdf:type rdf:resource="http://www.w3.org/2002/07/owl#TransitiveProperty"/>
        <rdfs:domain rdf:resource="http://www.semanticweb.org/macoda/ontologies/PMOEA#PMOEA"/>
        <rdfs:range rdf:resource="http://www.semanticweb.org/macoda/ontologies/PMOEA#PMOEA"/>
        <rdfs:label xml:lang="en">hasExtension</rdfs:label>
    </owl:ObjectProperty>
    


    <!-- http://www.semanticweb.org/macoda/ontologies/PMOEA#useLibrary -->

    <owl:ObjectProperty rdf:about="http://www.semanticweb.org/macoda/ontologies/PMOEA#useLibrary">
        <rdfs:domain rdf:resource="http://www.semanticweb.org/macoda/ontologies/PMOEA#MetaHeuristic"/>
        <rdfs:range rdf:resource="http://www.semanticweb.org/macoda/ontologies/PMOEA#ImplementationLibrary"/>
        <rdfs:label xml:lang="en">useLibrary</rdfs:label>
    </owl:ObjectProperty>
    


    <!-- http://www.semanticweb.org/macoda/ontologies/PMOEA#isExtensionOf -->

    <owl:ObjectProperty rdf:about="http://www.semanticweb.org/macoda/ontologies/PMOEA#isExtensionOf">
        <rdf:type rdf:resource="http://www.w3.org/2002/07/owl#TransitiveProperty"/>
        <rdfs:domain rdf:resource="http://www.semanticweb.org/macoda/ontologies/PMOEA#MetaHeuristic"/>
        <rdfs:range rdf:resource="http://www.semanticweb.org/macoda/ontologies/PMOEA#MetaHeuristic"/>
        <rdfs:label xml:lang="en">isExtensionOf</rdfs:label>
    </owl:ObjectProperty>
    


    <!-- http://www.semanticweb.org/macoda/ontologies/PMOEA#hasSearchAlgorithm -->

    <owl:ObjectProperty rdf:about="http://www.semanticweb.org/macoda/ontologies/PMOEA#hasSearchAlgorithm">
        <rdfs:domain rdf:resource="http://www.semanticweb.org/macoda/ontologies/PMOEA#PMOEA"/>
        <rdfs:range rdf:resource="http://www.semanticweb.org/macoda/ontologies/PMOEA#MetaHeuristic"/>
        <rdfs:label xml:lang="en">hasSearchAlgorithm</rdfs:label>
    </owl:ObjectProperty>
    


    <!-- http://www.semanticweb.org/macoda/ontologies/PMOEA#hasImplementationLanguage -->

    <owl:ObjectProperty rdf:about="http://www.semanticweb.org/macoda/ontologies/PMOEA#hasImplementationLanguage">
        <rdfs:domain rdf:resource="http://www.semanticweb.org/macoda/ontologies/PMOEA#MetaHeuristic"/>
        <rdfs:range rdf:resource="http://www.semanticweb.org/macoda/ontologies/PMOEA#ProgrammingLanguage"/>
        <rdfs:label xml:lang="en">hasImplementationLanguage</rdfs:label>
    </owl:ObjectProperty>
    


    <!-- http://www.semanticweb.org/macoda/ontologies/PMOEA#discussedIn -->

    <owl:ObjectProperty rdf:about="http://www.semanticweb.org/macoda/ontologies/PMOEA#discussedIn">
        <rdfs:comment>The topic is discussed in a bibliographic reference.</rdfs:comment>
    </owl:ObjectProperty>
    


    <!-- 
    ///////////////////////////////////////////////////////////////////////////////////////
    //
    // Data properties
    //
    ///////////////////////////////////////////////////////////////////////////////////////
     -->

    


    <!-- http://www.semanticweb.org/macoda/ontologies/PMOEA#isDiscreteProblem -->

    <owl:DatatypeProperty rdf:about="http://www.semanticweb.org/macoda/ontologies/PMOEA#isDiscreteProblem">
        <rdfs:domain rdf:resource="http://www.semanticweb.org/macoda/ontologies/PMOEA#MOP"/>
        <rdfs:range rdf:resource="http://www.w3.org/2001/XMLSchema#boolean"/>
        <rdfs:label xml:lang="en">isDiscreteProblem</rdfs:label>
    </owl:DatatypeProperty>
    


    <!-- http://www.semanticweb.org/macoda/ontologies/PMOEA#hasDevelopingYear -->

    <owl:DatatypeProperty rdf:about="http://www.semanticweb.org/macoda/ontologies/PMOEA#hasDevelopingYear">
        <rdfs:domain rdf:resource="http://www.semanticweb.org/macoda/ontologies/PMOEA#MetaHeuristic"/>
        <rdfs:range rdf:resource="http://www.w3.org/2001/XMLSchema#integer"/>
        <rdfs:label xml:lang="en">hasDevelopingYear</rdfs:label>
    </owl:DatatypeProperty>
    


    <!-- http://www.semanticweb.org/macoda/ontologies/PMOEA#hasLibraryDescription -->

    <owl:DatatypeProperty rdf:about="http://www.semanticweb.org/macoda/ontologies/PMOEA#hasLibraryDescription">
        <rdfs:domain rdf:resource="http://www.semanticweb.org/macoda/ontologies/PMOEA#ImplementationLibrary"/>
        <rdfs:range rdf:resource="http://www.w3.org/2001/XMLSchema#string"/>
        <rdfs:label xml:lang="en">hasLibraryDescription</rdfs:label>
    </owl:DatatypeProperty>
    


    <!-- http://www.semanticweb.org/macoda/ontologies/PMOEA#isMixedInteger -->

    <owl:DatatypeProperty rdf:about="http://www.semanticweb.org/macoda/ontologies/PMOEA#isMixedInteger">
        <rdfs:domain rdf:resource="http://www.semanticweb.org/macoda/ontologies/PMOEA#MOP"/>
        <rdfs:range rdf:resource="http://www.w3.org/2001/XMLSchema#boolean"/>
        <rdfs:label xml:lang="en">isMixedInteger</rdfs:label>
    </owl:DatatypeProperty>
    


    <!-- http://www.semanticweb.org/macoda/ontologies/PMOEA#hasRemarks -->

    <owl:DatatypeProperty rdf:about="http://www.semanticweb.org/macoda/ontologies/PMOEA#hasRemarks">
        <rdfs:range rdf:resource="http://www.w3.org/2001/XMLSchema#string"/>
        <rdfs:label xml:lang="en">hasRemarks</rdfs:label>
    </owl:DatatypeProperty>
    


    <!-- http://www.semanticweb.org/macoda/ontologies/PMOEA#hasExpensiveEvaluation -->

    <owl:DatatypeProperty rdf:about="http://www.semanticweb.org/macoda/ontologies/PMOEA#hasExpensiveEvaluation">
        <rdfs:domain rdf:resource="http://www.semanticweb.org/macoda/ontologies/PMOEA#MOP"/>
        <rdfs:range rdf:resource="http://www.w3.org/2001/XMLSchema#boolean"/>
        <rdfs:label xml:lang="en">hasExpensiveEvaluation</rdfs:label>
    </owl:DatatypeProperty>
    


    <!-- http://www.semanticweb.org/macoda/ontologies/PMOEA#OWLDataProperty_61d3cd95_fde4_4c1b_af08_1eaf73473aea -->

    <owl:DatatypeProperty rdf:about="http://www.semanticweb.org/macoda/ontologies/PMOEA#OWLDataProperty_61d3cd95_fde4_4c1b_af08_1eaf73473aea">
        <rdfs:domain rdf:resource="http://www.semanticweb.org/macoda/ontologies/PMOEA#MOP"/>
        <rdfs:range rdf:resource="http://www.w3.org/2001/XMLSchema#boolean"/>
        <rdfs:label xml:lang="en">isMultimodalProblem</rdfs:label>
    </owl:DatatypeProperty>
    


    <!-- http://www.semanticweb.org/macoda/ontologies/PMOEA#isNoisy -->

    <owl:DatatypeProperty rdf:about="http://www.semanticweb.org/macoda/ontologies/PMOEA#isNoisy">
        <rdfs:domain rdf:resource="http://www.semanticweb.org/macoda/ontologies/PMOEA#MOP"/>
        <rdfs:range rdf:resource="http://www.w3.org/2001/XMLSchema#boolean"/>
        <rdfs:label xml:lang="en">isNoisy</rdfs:label>
    </owl:DatatypeProperty>
    


    <!-- http://www.semanticweb.org/macoda/ontologies/PMOEA#MultipleRegionOfInterest -->

    <owl:DatatypeProperty rdf:about="http://www.semanticweb.org/macoda/ontologies/PMOEA#MultipleRegionOfInterest">
        <rdfs:domain rdf:resource="http://www.semanticweb.org/macoda/ontologies/PMOEA#PMOEA"/>
        <rdfs:range rdf:resource="http://www.w3.org/2001/XMLSchema#boolean"/>
        <rdfs:label xml:lang="en">MultipleRegionOfInterest</rdfs:label>
    </owl:DatatypeProperty>
    


    <!-- http://www.semanticweb.org/macoda/ontologies/PMOEA#useProgrammingLanguage -->

    <owl:DatatypeProperty rdf:about="http://www.semanticweb.org/macoda/ontologies/PMOEA#useProgrammingLanguage">
        <rdfs:domain rdf:resource="http://www.semanticweb.org/macoda/ontologies/PMOEA#PMOEA"/>
        <rdfs:range rdf:resource="http://www.w3.org/2001/XMLSchema#string"/>
        <rdfs:label xml:lang="en">useProgrammingLanguage</rdfs:label>
    </owl:DatatypeProperty>
    


    <!-- http://www.semanticweb.org/macoda/ontologies/PMOEA#isContinuousProblem -->

    <owl:DatatypeProperty rdf:about="http://www.semanticweb.org/macoda/ontologies/PMOEA#isContinuousProblem">
        <rdfs:domain rdf:resource="http://www.semanticweb.org/macoda/ontologies/PMOEA#MOP"/>
        <rdfs:range rdf:resource="http://www.w3.org/2001/XMLSchema#boolean"/>
        <rdfs:label xml:lang="en">isContinuousProblem</rdfs:label>
    </owl:DatatypeProperty>
    


    <!-- http://www.semanticweb.org/macoda/ontologies/PMOEA#SpreadControl -->

    <owl:DatatypeProperty rdf:about="http://www.semanticweb.org/macoda/ontologies/PMOEA#SpreadControl">
        <rdfs:domain rdf:resource="http://www.semanticweb.org/macoda/ontologies/PMOEA#PMOEA"/>
        <rdfs:range rdf:resource="http://www.w3.org/2001/XMLSchema#boolean"/>
        <rdfs:label xml:lang="en">SpreadControl</rdfs:label>
    </owl:DatatypeProperty>
    


    <!-- http://www.semanticweb.org/macoda/ontologies/PMOEA#ParetoDominancePreservation -->

    <owl:DatatypeProperty rdf:about="http://www.semanticweb.org/macoda/ontologies/PMOEA#ParetoDominancePreservation">
        <rdfs:domain rdf:resource="http://www.semanticweb.org/macoda/ontologies/PMOEA#PMOEA"/>
        <rdfs:range rdf:resource="http://www.w3.org/2001/XMLSchema#boolean"/>
        <rdfs:label xml:lang="en">ParetoDominancePreservation</rdfs:label>
    </owl:DatatypeProperty>
    


    <!-- http://www.semanticweb.org/macoda/ontologies/PMOEA#ObjectiveNumber -->

    <owl:DatatypeProperty rdf:about="http://www.semanticweb.org/macoda/ontologies/PMOEA#ObjectiveNumber">
        <rdfs:domain rdf:resource="http://www.semanticweb.org/macoda/ontologies/PMOEA#MOP"/>
        <rdfs:range rdf:resource="http://www.w3.org/2001/XMLSchema#integer"/>
        <rdfs:label xml:lang="en">ObjectiveNumber</rdfs:label>
    </owl:DatatypeProperty>
    


    <!-- http://www.semanticweb.org/macoda/ontologies/PMOEA#hasReference -->

    <owl:DatatypeProperty rdf:about="http://www.semanticweb.org/macoda/ontologies/PMOEA#hasReference">
        <rdfs:range rdf:resource="http://www.w3.org/2001/XMLSchema#string"/>
        <rdfs:label xml:lang="en">hasReference</rdfs:label>
    </owl:DatatypeProperty>
    


    <!-- http://www.semanticweb.org/macoda/ontologies/PMOEA#isManyObjectiveProblem -->

    <owl:DatatypeProperty rdf:about="http://www.semanticweb.org/macoda/ontologies/PMOEA#isManyObjectiveProblem">
        <rdfs:domain rdf:resource="http://www.semanticweb.org/macoda/ontologies/PMOEA#MOP"/>
        <rdfs:range rdf:resource="http://www.w3.org/2001/XMLSchema#boolean"/>
        <rdfs:label xml:lang="en">isManyObjectiveProblem</rdfs:label>
    </owl:DatatypeProperty>
    


    <!-- http://www.semanticweb.org/macoda/ontologies/PMOEA#hasHeterogeneousConstraints -->

    <owl:DatatypeProperty rdf:about="http://www.semanticweb.org/macoda/ontologies/PMOEA#hasHeterogeneousConstraints">
        <rdfs:domain rdf:resource="http://www.semanticweb.org/macoda/ontologies/PMOEA#MOP"/>
        <rdfs:range rdf:resource="http://www.w3.org/2001/XMLSchema#boolean"/>
        <rdfs:comment>Constraint function components of a problem that differ in complexity, latency, uncertainty, domain type, co-domain type, black box vs analytically known, or in other ways that might affect search.</rdfs:comment>
    </owl:DatatypeProperty>
    


    <!-- http://www.semanticweb.org/macoda/ontologies/PMOEA#hasHeterogeneousObjectives -->

    <owl:DatatypeProperty rdf:about="http://www.semanticweb.org/macoda/ontologies/PMOEA#hasHeterogeneousObjectives">
        <rdfs:domain rdf:resource="http://www.semanticweb.org/macoda/ontologies/PMOEA#MOP"/>
        <rdfs:range rdf:resource="http://www.w3.org/2001/XMLSchema#boolean"/>
        <rdfs:comment>Objective function components of a problem that differ in complexity, latency, uncertainty, domain type, co-domain type, black box vs analytically known, or in other ways that might affect search.</rdfs:comment>
    </owl:DatatypeProperty>
    


    <!-- 
    ///////////////////////////////////////////////////////////////////////////////////////
    //
    // Classes
    //
    ///////////////////////////////////////////////////////////////////////////////////////
     -->

    


    <!-- http://www.semanticweb.org/macoda/ontologies/PMOEA#AlphaDominance -->

    <owl:Class rdf:about="http://www.semanticweb.org/macoda/ontologies/PMOEA#AlphaDominance">
        <rdfs:subClassOf rdf:resource="http://www.semanticweb.org/macoda/ontologies/PMOEA#OrderRelation"/>
        <rdfs:comment>Dominance relation considering trade-off between objectives to prevent dominance resistant points</rdfs:comment>
    </owl:Class>
    


    <!-- http://www.semanticweb.org/macoda/ontologies/PMOEA#AsynchronousEA -->

    <owl:Class rdf:about="http://www.semanticweb.org/macoda/ontologies/PMOEA#AsynchronousEA">
        <rdfs:subClassOf rdf:resource="http://www.semanticweb.org/macoda/ontologies/PMOEA#Parallelisation"/>
        <rdfs:comment>Evolutionary algorithms that work on parallel architectures supporting asynchronous solution evaluations, selection and search operators.</rdfs:comment>
    </owl:Class>
    


    <!-- http://www.semanticweb.org/macoda/ontologies/PMOEA#Constraints -->

    <owl:Class rdf:about="http://www.semanticweb.org/macoda/ontologies/PMOEA#Constraints">
        <rdfs:subClassOf rdf:resource="http://www.semanticweb.org/macoda/ontologies/PMOEA#PreferenceIntegration"/>
    </owl:Class>
    


    <!-- http://www.semanticweb.org/macoda/ontologies/PMOEA#EdgeRotatedConeOrder -->

    <owl:Class rdf:about="http://www.semanticweb.org/macoda/ontologies/PMOEA#EdgeRotatedConeOrder">
        <rdfs:subClassOf rdf:resource="http://www.semanticweb.org/macoda/ontologies/PMOEA#OrderRelation"/>
        <rdfs:comment>Dominance relation with parameter epsilon. used in the componentwise comparison to increase/decrease the coordinates of one of the solutions.</rdfs:comment>
    </owl:Class>
    


    <!-- http://www.semanticweb.org/macoda/ontologies/PMOEA#FavourRelation -->

    <owl:Class rdf:about="http://www.semanticweb.org/macoda/ontologies/PMOEA#FavourRelation">
        <rdfs:subClassOf rdf:resource="http://www.semanticweb.org/macoda/ontologies/PMOEA#OrderRelation"/>
        <rdfs:comment>Order relation proposed for many objective optimization. This in-transitive relation counts in how many objectives one solution is better than another solution.</rdfs:comment>
    </owl:Class>
    


    <!-- http://www.semanticweb.org/macoda/ontologies/PMOEA#HeterogeneousObjectives -->

    <owl:Class rdf:about="http://www.semanticweb.org/macoda/ontologies/PMOEA#HeterogeneousObjectives">
        <rdfs:subClassOf rdf:resource="http://www.semanticweb.org/macoda/ontologies/PMOEA#MOP"/>
        <rdfs:comment>Objective function components of a problem that differ in complexity, latency, uncertainty, domain type, co-domain type, black box vs analytically known, or in other ways that might affect search.</rdfs:comment>
    </owl:Class>
    


    <!-- http://www.semanticweb.org/macoda/ontologies/PMOEA#LeaderSelection -->

    <owl:Class rdf:about="http://www.semanticweb.org/macoda/ontologies/PMOEA#LeaderSelection">
        <rdfs:subClassOf rdf:resource="http://www.semanticweb.org/macoda/ontologies/PMOEA#PreferenceIntegration"/>
        <rdfs:label>ParticleUpdate</rdfs:label>
    </owl:Class>
    


    <!-- http://www.semanticweb.org/macoda/ontologies/PMOEA#LightBeamSearch -->

    <owl:Class rdf:about="http://www.semanticweb.org/macoda/ontologies/PMOEA#LightBeamSearch">
        <rdfs:subClassOf rdf:resource="http://www.semanticweb.org/macoda/ontologies/PMOEA#PreferenceModel"/>
    </owl:Class>
    


    <!-- http://www.semanticweb.org/macoda/ontologies/PMOEA#ReferencePoint_based -->

    <owl:Class rdf:about="http://www.semanticweb.org/macoda/ontologies/PMOEA#ReferencePoint_based">
        <owl:equivalentClass>
            <owl:Restriction>
                <owl:onProperty rdf:resource="http://www.semanticweb.org/macoda/ontologies/PMOEA#hasPreferenceInformationFromDM"/>
                <owl:someValuesFrom rdf:resource="http://www.semanticweb.org/macoda/ontologies/PMOEA#ReferencePoint"/>
            </owl:Restriction>
        </owl:equivalentClass>
        <rdfs:subClassOf rdf:resource="http://www.semanticweb.org/macoda/ontologies/PMOEA#PMOEA"/>
        <rdfs:label xml:lang="en">ReferencePoint_based</rdfs:label>
    </owl:Class>
    


    <!-- http://www.semanticweb.org/macoda/ontologies/PMOEA#GeneralAdditive -->

    <owl:Class rdf:about="http://www.semanticweb.org/macoda/ontologies/PMOEA#GeneralAdditive">
        <rdfs:subClassOf rdf:resource="http://www.semanticweb.org/macoda/ontologies/PMOEA#UtilityFunction"/>
        <rdfs:label xml:lang="en">GeneralAdditive</rdfs:label>
    </owl:Class>
    


    <!-- http://www.semanticweb.org/macoda/ontologies/PMOEA#SetPreferenceRelation -->

    <owl:Class rdf:about="http://www.semanticweb.org/macoda/ontologies/PMOEA#SetPreferenceRelation">
        <rdfs:subClassOf rdf:resource="http://www.semanticweb.org/macoda/ontologies/PMOEA#PreferenceModel"/>
        <rdfs:label xml:lang="en">SetPreferenceRelation</rdfs:label>
    </owl:Class>
    


    <!-- http://www.semanticweb.org/macoda/ontologies/PMOEA#ReferenceDirection -->

    <owl:Class rdf:about="http://www.semanticweb.org/macoda/ontologies/PMOEA#ReferenceDirection">
        <rdfs:subClassOf rdf:resource="http://www.semanticweb.org/macoda/ontologies/PMOEA#PreferenceInformationFromDM"/>
        <rdfs:label xml:lang="en">ReferenceDirection</rdfs:label>
    </owl:Class>
    


    <!-- http://www.semanticweb.org/macoda/ontologies/PMOEA#PreferenceRegion -->

    <owl:Class rdf:about="http://www.semanticweb.org/macoda/ontologies/PMOEA#PreferenceRegion">
        <rdfs:subClassOf rdf:resource="http://www.semanticweb.org/macoda/ontologies/PMOEA#PreferenceModel"/>
        <rdfs:label xml:lang="en">PreferenceRegion</rdfs:label>
    </owl:Class>
    


    <!-- http://www.semanticweb.org/macoda/ontologies/PMOEA#SolutionComparison -->

    <owl:Class rdf:about="http://www.semanticweb.org/macoda/ontologies/PMOEA#SolutionComparison">
        <rdfs:subClassOf rdf:resource="http://www.semanticweb.org/macoda/ontologies/PMOEA#PreferenceInformationFromDM"/>
        <rdfs:label xml:lang="en">SolutionComparison</rdfs:label>
    </owl:Class>
    


    <!-- http://www.semanticweb.org/macoda/ontologies/PMOEA#BoundedRegion -->

    <owl:Class rdf:about="http://www.semanticweb.org/macoda/ontologies/PMOEA#BoundedRegion">
        <rdfs:subClassOf rdf:resource="http://www.semanticweb.org/macoda/ontologies/PMOEA#SetOfSolutions"/>
        <owl:disjointWith rdf:resource="http://www.semanticweb.org/macoda/ontologies/PMOEA#BiasedDistribution"/>
        <rdfs:label xml:lang="en">BoundedRegion</rdfs:label>
    </owl:Class>
    


    <!-- http://www.semanticweb.org/macoda/ontologies/PMOEA#GroupDecisionMaking -->

    <owl:Class rdf:about="http://www.semanticweb.org/macoda/ontologies/PMOEA#GroupDecisionMaking">
        <rdfs:subClassOf rdf:resource="http://www.semanticweb.org/macoda/ontologies/PMOEA#PreferenceInformationFromDM"/>
        <rdfs:label xml:lang="en">GroupDecisionMaking</rdfs:label>
    </owl:Class>
    


    <!-- http://www.semanticweb.org/macoda/ontologies/PMOEA#DiversityVSConvergence_based -->

    <owl:Class rdf:about="http://www.semanticweb.org/macoda/ontologies/PMOEA#DiversityVSConvergence_based">
        <rdfs:subClassOf rdf:resource="http://www.semanticweb.org/macoda/ontologies/PMOEA#MOEA"/>
        <rdfs:label xml:lang="en">DiversityVSConvergence_based</rdfs:label>
    </owl:Class>
    


    <!-- http://www.semanticweb.org/macoda/ontologies/PMOEA#SetPreference -->

    <owl:Class rdf:about="http://www.semanticweb.org/macoda/ontologies/PMOEA#SetPreference">
        <rdfs:subClassOf rdf:resource="http://www.semanticweb.org/macoda/ontologies/PMOEA#PreferenceInformationFromDM"/>
        <rdfs:label xml:lang="en">SetPreference</rdfs:label>
    </owl:Class>
    


    <!-- http://www.semanticweb.org/macoda/ontologies/PMOEA#PolyhedralConeBased -->

    <owl:Class rdf:about="http://www.semanticweb.org/macoda/ontologies/PMOEA#PolyhedralConeBased">
        <rdfs:subClassOf rdf:resource="http://www.semanticweb.org/macoda/ontologies/PMOEA#PreferenceModel"/>
        <rdfs:label xml:lang="en">PolyhedralConeBased</rdfs:label>
    </owl:Class>
    


    <!-- http://www.semanticweb.org/macoda/ontologies/PMOEA#WFG -->

    <owl:Class rdf:about="http://www.semanticweb.org/macoda/ontologies/PMOEA#WFG">
        <rdfs:subClassOf rdf:resource="http://www.semanticweb.org/macoda/ontologies/PMOEA#Academic_Problem"/>
        <rdfs:label xml:lang="en">WFG</rdfs:label>
    </owl:Class>
    


    <!-- http://www.semanticweb.org/macoda/ontologies/PMOEA#ResultInfluence -->

    <owl:Class rdf:about="http://www.semanticweb.org/macoda/ontologies/PMOEA#ResultInfluence">
        <rdfs:comment>Result of the method,  range or distribution or only one Solution</rdfs:comment>
        <rdfs:label xml:lang="en">ResultInfluence</rdfs:label>
    </owl:Class>
    


    <!-- http://www.semanticweb.org/macoda/ontologies/PMOEA#ChoquetIntegral -->

    <owl:Class rdf:about="http://www.semanticweb.org/macoda/ontologies/PMOEA#ChoquetIntegral">
        <rdfs:subClassOf rdf:resource="http://www.semanticweb.org/macoda/ontologies/PMOEA#UtilityFunction"/>
        <rdfs:label xml:lang="en">ChoquetIntegral</rdfs:label>
    </owl:Class>
    


    <!-- http://www.semanticweb.org/macoda/ontologies/PMOEA#Linear -->

    <owl:Class rdf:about="http://www.semanticweb.org/macoda/ontologies/PMOEA#Linear">
        <rdfs:subClassOf rdf:resource="http://www.semanticweb.org/macoda/ontologies/PMOEA#UtilityFunction"/>
        <rdfs:label xml:lang="en">Linear</rdfs:label>
    </owl:Class>
    


    <!-- http://www.semanticweb.org/macoda/ontologies/PMOEA#QuasiConcave -->

    <owl:Class rdf:about="http://www.semanticweb.org/macoda/ontologies/PMOEA#QuasiConcave">
        <rdfs:subClassOf rdf:resource="http://www.semanticweb.org/macoda/ontologies/PMOEA#UtilityFunction"/>
        <rdfs:label xml:lang="en">QuasiConcave</rdfs:label>
    </owl:Class>
    


    <!-- http://www.semanticweb.org/macoda/ontologies/PMOEA#PreferenceRegion -->

    <owl:Class rdf:about="http://www.semanticweb.org/macoda/ontologies/PMOEA#PreferenceRegion">
        <rdfs:subClassOf rdf:resource="http://www.semanticweb.org/macoda/ontologies/PMOEA#PreferenceInformationFromDM"/>
        <rdfs:label xml:lang="en">PreferenceRegion</rdfs:label>
    </owl:Class>
    


    <!-- http://www.semanticweb.org/macoda/ontologies/PMOEA#Indicator -->

    <owl:Class rdf:about="http://www.semanticweb.org/macoda/ontologies/PMOEA#Indicator">
        <rdfs:subClassOf rdf:resource="http://www.semanticweb.org/macoda/ontologies/PMOEA#PreferenceInformationFromDM"/>
        <rdfs:label xml:lang="en">Indicator</rdfs:label>
    </owl:Class>
    


    <!-- http://www.semanticweb.org/macoda/ontologies/PMOEA#SelectionCriterion -->

    <owl:Class rdf:about="http://www.semanticweb.org/macoda/ontologies/PMOEA#SelectionCriterion">
        <rdfs:subClassOf rdf:resource="http://www.semanticweb.org/macoda/ontologies/PMOEA#PreferenceIntegration"/>
        <rdfs:label xml:lang="en">SelectionCriterion</rdfs:label>
    </owl:Class>
    


    <!-- http://www.semanticweb.org/macoda/ontologies/PMOEA#Probabilistic_based -->

    <owl:Class rdf:about="http://www.semanticweb.org/macoda/ontologies/PMOEA#Probabilistic_based">
        <rdfs:subClassOf rdf:resource="http://www.semanticweb.org/macoda/ontologies/PMOEA#MOEA"/>
        <rdfs:label xml:lang="en">Probabilistic_based</rdfs:label>
    </owl:Class>
    


    <!-- http://www.semanticweb.org/macoda/ontologies/PMOEA#OrdinalRegression -->

    <owl:Class rdf:about="http://www.semanticweb.org/macoda/ontologies/PMOEA#OrdinalRegression">
        <rdfs:subClassOf rdf:resource="http://www.semanticweb.org/macoda/ontologies/PMOEA#LearningMethod"/>
        <rdfs:label xml:lang="en">OrdinalRegression</rdfs:label>
    </owl:Class>
    


    <!-- http://www.semanticweb.org/macoda/ontologies/PMOEA#FrontSorting -->

    <owl:Class rdf:about="http://www.semanticweb.org/macoda/ontologies/PMOEA#FrontSorting">
        <rdfs:subClassOf rdf:resource="http://www.semanticweb.org/macoda/ontologies/PMOEA#PreferenceIntegration"/>
        <rdfs:label xml:lang="en">FrontSorting</rdfs:label>
    </owl:Class>
    


    <!-- http://www.semanticweb.org/macoda/ontologies/PMOEA#Knapsack -->

    <owl:Class rdf:about="http://www.semanticweb.org/macoda/ontologies/PMOEA#Knapsack">
        <rdfs:subClassOf rdf:resource="http://www.semanticweb.org/macoda/ontologies/PMOEA#Academic_Problem"/>
        <rdfs:label xml:lang="en">Knapsack</rdfs:label>
    </owl:Class>
    


    <!-- http://www.semanticweb.org/macoda/ontologies/PMOEA#UtilityFunction -->

    <owl:Class rdf:about="http://www.semanticweb.org/macoda/ontologies/PMOEA#UtilityFunction">
        <rdfs:subClassOf rdf:resource="http://www.semanticweb.org/macoda/ontologies/PMOEA#PreferenceModel"/>
        <rdfs:label xml:lang="en">UtilityFunction</rdfs:label>
    </owl:Class>
    


    <!-- http://www.semanticweb.org/macoda/ontologies/PMOEA#Memetic -->

    <owl:Class rdf:about="http://www.semanticweb.org/macoda/ontologies/PMOEA#Memetic">
        <rdfs:subClassOf rdf:resource="http://www.semanticweb.org/macoda/ontologies/PMOEA#MOEA"/>
        <rdfs:label xml:lang="en">Memetic</rdfs:label>
    </owl:Class>
    


    <!-- http://www.semanticweb.org/macoda/ontologies/PMOEA#Initalization -->

    <owl:Class rdf:about="http://www.semanticweb.org/macoda/ontologies/PMOEA#Initalization">
        <rdfs:subClassOf rdf:resource="http://www.semanticweb.org/macoda/ontologies/PMOEA#PreferenceIntegration"/>
        <rdfs:label xml:lang="en">Initalization</rdfs:label>
    </owl:Class>
    


    <!-- http://www.semanticweb.org/macoda/ontologies/PMOEA#BudgetofDMcalls -->

    <owl:Class rdf:about="http://www.semanticweb.org/macoda/ontologies/PMOEA#BudgetofDMcalls">
        <rdfs:subClassOf rdf:resource="http://www.semanticweb.org/macoda/ontologies/PMOEA#PreferenceInformationFromDM"/>
        <rdfs:label xml:lang="en">BudgetofDMcalls</rdfs:label>
    </owl:Class>
    


    <!-- http://www.semanticweb.org/macoda/ontologies/PMOEA#TerminationCriterion -->

    <owl:Class rdf:about="http://www.semanticweb.org/macoda/ontologies/PMOEA#TerminationCriterion">
        <rdfs:subClassOf rdf:resource="http://www.semanticweb.org/macoda/ontologies/PMOEA#PreferenceIntegration"/>
        <rdfs:label xml:lang="en">TerminationCriterion</rdfs:label>
    </owl:Class>
    


    <!-- http://www.semanticweb.org/macoda/ontologies/PMOEA#DecisionRules -->

    <owl:Class rdf:about="http://www.semanticweb.org/macoda/ontologies/PMOEA#DecisionRules">
        <rdfs:subClassOf rdf:resource="http://www.semanticweb.org/macoda/ontologies/PMOEA#PreferenceModel"/>
        <rdfs:label xml:lang="en">DecisionRules</rdfs:label>
    </owl:Class>
    


    <!-- http://www.semanticweb.org/macoda/ontologies/PMOEA#TerritorySize -->

    <owl:Class rdf:about="http://www.semanticweb.org/macoda/ontologies/PMOEA#TerritorySize">
        <rdfs:subClassOf rdf:resource="http://www.semanticweb.org/macoda/ontologies/PMOEA#PreferenceIntegration"/>
        <rdfs:label xml:lang="en">TerritorySize</rdfs:label>
    </owl:Class>
    


    <!-- http://www.semanticweb.org/macoda/ontologies/PMOEA#KneePoint -->

    <owl:Class rdf:about="http://www.semanticweb.org/macoda/ontologies/PMOEA#KneePoint">
        <rdfs:subClassOf rdf:resource="http://www.semanticweb.org/macoda/ontologies/PMOEA#PreferenceModel"/>
        <rdfs:label xml:lang="en">KneePoint</rdfs:label>
    </owl:Class>
    


    <!-- http://www.semanticweb.org/macoda/ontologies/PMOEA#SOEA -->

    <owl:Class rdf:about="http://www.semanticweb.org/macoda/ontologies/PMOEA#SOEA">
        <rdfs:subClassOf rdf:resource="http://www.semanticweb.org/macoda/ontologies/PMOEA#MetaHeuristic"/>
        <rdfs:comment>single-objective evolutionary algorithm</rdfs:comment>
        <rdfs:label xml:lang="en">SOEA</rdfs:label>
    </owl:Class>
    


    <!-- http://www.semanticweb.org/macoda/ontologies/PMOEA#AchievementScalarizingFunction -->

    <owl:Class rdf:about="http://www.semanticweb.org/macoda/ontologies/PMOEA#AchievementScalarizingFunction">
        <rdfs:subClassOf rdf:resource="http://www.semanticweb.org/macoda/ontologies/PMOEA#PreferenceModel"/>
        <rdfs:label xml:lang="en">AchievementScalarizingFunction</rdfs:label>
    </owl:Class>
    


    <!-- http://www.semanticweb.org/macoda/ontologies/PMOEA#LinearProgramming -->

    <owl:Class rdf:about="http://www.semanticweb.org/macoda/ontologies/PMOEA#LinearProgramming">
        <rdfs:subClassOf rdf:resource="http://www.semanticweb.org/macoda/ontologies/PMOEA#LearningMethod"/>
        <rdfs:label xml:lang="en">LinearProgramming</rdfs:label>
    </owl:Class>
    


    <!-- http://www.semanticweb.org/macoda/ontologies/PMOEA#SampleSorts -->

    <owl:Class rdf:about="http://www.semanticweb.org/macoda/ontologies/PMOEA#SampleSorts">
        <rdfs:subClassOf rdf:resource="http://www.semanticweb.org/macoda/ontologies/PMOEA#SolutionComparison"/>
        <rdfs:label xml:lang="en">SampleSorts</rdfs:label>
    </owl:Class>
    


    <!-- http://www.semanticweb.org/macoda/ontologies/PMOEA#ObjectiveSpaceTransformation_basedPEMO -->

    <owl:Class rdf:about="http://www.semanticweb.org/macoda/ontologies/PMOEA#ObjectiveSpaceTransformation_basedPEMO">
        <owl:equivalentClass>
            <owl:Restriction>
                <owl:onProperty rdf:resource="http://www.semanticweb.org/macoda/ontologies/PMOEA#hasPreferenceIntegration"/>
                <owl:hasValue rdf:resource="http://www.semanticweb.org/macoda/ontologies/PMOEA#ObjectiveTransformation"/>
            </owl:Restriction>
        </owl:equivalentClass>
        <rdfs:subClassOf rdf:resource="http://www.semanticweb.org/macoda/ontologies/PMOEA#PMOEA"/>
        <rdfs:label xml:lang="en">ObjectiveSpaceTransformation_basedPEMO</rdfs:label>
    </owl:Class>
    


    <!-- http://www.semanticweb.org/macoda/ontologies/PMOEA#QuadraticProgramming -->

    <owl:Class rdf:about="http://www.semanticweb.org/macoda/ontologies/PMOEA#QuadraticProgramming">
        <rdfs:subClassOf rdf:resource="http://www.semanticweb.org/macoda/ontologies/PMOEA#LearningMethod"/>
        <rdfs:label xml:lang="en">QuadraticProgramming</rdfs:label>
    </owl:Class>
    


    <!-- http://www.semanticweb.org/macoda/ontologies/PMOEA#AdditivePiecewiseLinear -->

    <owl:Class rdf:about="http://www.semanticweb.org/macoda/ontologies/PMOEA#AdditivePiecewiseLinear">
        <rdfs:subClassOf rdf:resource="http://www.semanticweb.org/macoda/ontologies/PMOEA#UtilityFunction"/>
        <rdfs:label xml:lang="en">AdditivePiecewiseLinear</rdfs:label>
    </owl:Class>
    


    <!-- http://www.semanticweb.org/macoda/ontologies/PMOEA#PreferenceInformationFromDM -->

    <owl:Class rdf:about="http://www.semanticweb.org/macoda/ontologies/PMOEA#PreferenceInformationFromDM">
        <rdfs:label xml:lang="en">PreferenceInformationFromDM</rdfs:label>
    </owl:Class>
    


    <!-- http://www.semanticweb.org/macoda/ontologies/PMOEA#a-priori -->

    <owl:Class rdf:about="http://www.semanticweb.org/macoda/ontologies/PMOEA#a-priori">
        <rdfs:subClassOf rdf:resource="http://www.semanticweb.org/macoda/ontologies/PMOEA#InteractionTime"/>
        <rdfs:label xml:lang="en">a-priori</rdfs:label>
    </owl:Class>
    


    <!-- http://www.semanticweb.org/macoda/ontologies/PMOEA#Trade-off -->

    <owl:Class rdf:about="http://www.semanticweb.org/macoda/ontologies/PMOEA#Trade-off">
        <rdfs:subClassOf rdf:resource="http://www.semanticweb.org/macoda/ontologies/PMOEA#PreferenceInformationFromDM"/>
        <rdfs:label xml:lang="en">Trade-off</rdfs:label>
    </owl:Class>
    


    <!-- http://www.semanticweb.org/macoda/ontologies/PMOEA#PMOEA -->

    <owl:Class rdf:about="http://www.semanticweb.org/macoda/ontologies/PMOEA#PMOEA">
        <rdfs:subClassOf rdf:resource="http://www.semanticweb.org/macoda/ontologies/PMOEA#MOEA"/>
        <rdfs:comment>preference_based multi-objective evolutionary algorithms</rdfs:comment>
        <rdfs:label xml:lang="en">PMOEA</rdfs:label>
    </owl:Class>
    


    <!-- http://www.semanticweb.org/macoda/ontologies/PMOEA#PreferenceModel -->

    <owl:Class rdf:about="http://www.semanticweb.org/macoda/ontologies/PMOEA#PreferenceModel">
        <rdfs:label xml:lang="en">PreferenceModel</rdfs:label>
    </owl:Class>
    


    <!-- http://www.semanticweb.org/macoda/ontologies/PMOEA#Academic_Problem -->

    <owl:Class rdf:about="http://www.semanticweb.org/macoda/ontologies/PMOEA#Academic_Problem">
        <rdfs:subClassOf rdf:resource="http://www.semanticweb.org/macoda/ontologies/PMOEA#MOP"/>
        <rdfs:comment>preference_based evolutionary multi-objective optimization</rdfs:comment>
        <rdfs:label xml:lang="en">Academic_Problem</rdfs:label>
    </owl:Class>
    


    <!-- http://www.semanticweb.org/macoda/ontologies/PMOEA#OneSolution -->

    <owl:Class rdf:about="http://www.semanticweb.org/macoda/ontologies/PMOEA#OneSolution">
        <rdfs:subClassOf rdf:resource="http://www.semanticweb.org/macoda/ontologies/PMOEA#ResultInfluence"/>
        <owl:disjointWith rdf:resource="http://www.semanticweb.org/macoda/ontologies/PMOEA#SetOfSolutions"/>
        <rdfs:label xml:lang="en">OneSolution</rdfs:label>
    </owl:Class>
    


    <!-- http://www.semanticweb.org/macoda/ontologies/PMOEA#PSO_based -->

    <owl:Class rdf:about="http://www.semanticweb.org/macoda/ontologies/PMOEA#PSO_based">
        <rdfs:subClassOf rdf:resource="http://www.semanticweb.org/macoda/ontologies/PMOEA#Swarm_based"/>
        <rdfs:label xml:lang="en">PSO_based</rdfs:label>
    </owl:Class>
    


    <!-- http://www.semanticweb.org/macoda/ontologies/PMOEA#ASF -->

    <owl:Class rdf:about="http://www.semanticweb.org/macoda/ontologies/PMOEA#ASF">
        <rdfs:subClassOf rdf:resource="http://www.semanticweb.org/macoda/ontologies/PMOEA#PreferenceIntegration"/>
        <rdfs:label xml:lang="en">ASF</rdfs:label>
    </owl:Class>
    


    <!-- http://www.semanticweb.org/macoda/ontologies/PMOEA#DesirabilityFunction -->

    <owl:Class rdf:about="http://www.semanticweb.org/macoda/ontologies/PMOEA#DesirabilityFunction">
        <rdfs:subClassOf rdf:resource="http://www.semanticweb.org/macoda/ontologies/PMOEA#UtilityFunction"/>
        <rdfs:label xml:lang="en">DesirabilityFunction</rdfs:label>
    </owl:Class>
    


    <!-- http://www.semanticweb.org/macoda/ontologies/PMOEA#a-posteriori -->

    <owl:Class rdf:about="http://www.semanticweb.org/macoda/ontologies/PMOEA#a-posteriori">
        <rdfs:subClassOf rdf:resource="http://www.semanticweb.org/macoda/ontologies/PMOEA#InteractionTime"/>
        <rdfs:label xml:lang="en">a-posteriori</rdfs:label>
    </owl:Class>
    


    <!-- http://www.semanticweb.org/macoda/ontologies/PMOEA#Objectives -->

    <owl:Class rdf:about="http://www.semanticweb.org/macoda/ontologies/PMOEA#Objectives">
        <rdfs:subClassOf rdf:resource="http://www.semanticweb.org/macoda/ontologies/PMOEA#PreferenceIntegration"/>
        <rdfs:label xml:lang="en">Objectives</rdfs:label>
    </owl:Class>
    


    <!-- http://www.semanticweb.org/macoda/ontologies/PMOEA#ProgrammingLanguage -->

    <owl:Class rdf:about="http://www.semanticweb.org/macoda/ontologies/PMOEA#ProgrammingLanguage">
        <rdfs:label xml:lang="en">ProgrammingLanguage</rdfs:label>
    </owl:Class>
    


    <!-- http://www.semanticweb.org/macoda/ontologies/PMOEA#SetOfSolutions -->

    <owl:Class rdf:about="http://www.semanticweb.org/macoda/ontologies/PMOEA#SetOfSolutions">
        <rdfs:subClassOf rdf:resource="http://www.semanticweb.org/macoda/ontologies/PMOEA#ResultInfluence"/>
        <rdfs:label xml:lang="en">SetOfSolutions</rdfs:label>
    </owl:Class>
    


    <!-- http://www.semanticweb.org/macoda/ontologies/PMOEA#DominanceRelation -->

    <owl:Class rdf:about="http://www.semanticweb.org/macoda/ontologies/PMOEA#DominanceRelation">
        <rdfs:subClassOf rdf:resource="http://www.semanticweb.org/macoda/ontologies/PMOEA#PreferenceIntegration"/>
        <rdfs:label xml:lang="en">DominanceRelation</rdfs:label>
    </owl:Class>
    


    <!-- http://www.semanticweb.org/macoda/ontologies/PMOEA#NeuralNetwork -->

    <owl:Class rdf:about="http://www.semanticweb.org/macoda/ontologies/PMOEA#NeuralNetwork">
        <rdfs:subClassOf rdf:resource="http://www.semanticweb.org/macoda/ontologies/PMOEA#LearningMethod"/>
        <rdfs:label xml:lang="en">NeuralNetwork</rdfs:label>
    </owl:Class>
    


    <!-- http://www.semanticweb.org/macoda/ontologies/PMOEA#MetaHeuristic -->

    <owl:Class rdf:about="http://www.semanticweb.org/macoda/ontologies/PMOEA#MetaHeuristic">
        <rdfs:label xml:lang="en">MetaHeuristic</rdfs:label>
    </owl:Class>
    


    <!-- http://www.semanticweb.org/macoda/ontologies/PMOEA#Fitness -->

    <owl:Class rdf:about="http://www.semanticweb.org/macoda/ontologies/PMOEA#Fitness">
        <rdfs:subClassOf rdf:resource="http://www.semanticweb.org/macoda/ontologies/PMOEA#PreferenceIntegration"/>
        <rdfs:label xml:lang="en">Fitness</rdfs:label>
    </owl:Class>
    


    <!-- http://www.semanticweb.org/macoda/ontologies/PMOEA#SetQualityIndicator -->

    <owl:Class rdf:about="http://www.semanticweb.org/macoda/ontologies/PMOEA#SetQualityIndicator">
        <rdfs:subClassOf rdf:resource="http://www.semanticweb.org/macoda/ontologies/PMOEA#PreferenceIntegration"/>
        <rdfs:label xml:lang="en">SetQualityIndicator</rdfs:label>
    </owl:Class>
    


    <!-- http://www.semanticweb.org/macoda/ontologies/PMOEA#CrowdingDistance -->

    <owl:Class rdf:about="http://www.semanticweb.org/macoda/ontologies/PMOEA#CrowdingDistance">
        <rdfs:subClassOf rdf:resource="http://www.semanticweb.org/macoda/ontologies/PMOEA#PreferenceIntegration"/>
        <rdfs:label xml:lang="en">CrowdingDistance</rdfs:label>
    </owl:Class>
    


    <!-- http://www.semanticweb.org/macoda/ontologies/PMOEA#OutrankingRelation -->

    <owl:Class rdf:about="http://www.semanticweb.org/macoda/ontologies/PMOEA#OutrankingRelation">
        <rdfs:subClassOf rdf:resource="http://www.semanticweb.org/macoda/ontologies/PMOEA#PreferenceModel"/>
        <rdfs:label xml:lang="en">OutrankingRelation</rdfs:label>
    </owl:Class>
    


    <!-- http://www.semanticweb.org/macoda/ontologies/PMOEA#Researcher -->

    <owl:Class rdf:about="http://www.semanticweb.org/macoda/ontologies/PMOEA#Researcher">
        <rdfs:label xml:lang="en">Researcher</rdfs:label>
    </owl:Class>
    


    <!-- http://www.semanticweb.org/macoda/ontologies/PMOEA#ObjectiveComparison -->

    <owl:Class rdf:about="http://www.semanticweb.org/macoda/ontologies/PMOEA#ObjectiveComparison">
        <rdfs:subClassOf rdf:resource="http://www.semanticweb.org/macoda/ontologies/PMOEA#PreferenceInformationFromDM"/>
        <rdfs:label xml:lang="en">ObjectiveComparison</rdfs:label>
    </owl:Class>
    


    <!-- http://www.semanticweb.org/macoda/ontologies/PMOEA#Decomposition_based -->

    <owl:Class rdf:about="http://www.semanticweb.org/macoda/ontologies/PMOEA#Decomposition_based">
        <rdfs:subClassOf rdf:resource="http://www.semanticweb.org/macoda/ontologies/PMOEA#MOEA"/>
        <rdfs:label xml:lang="en">Decomposition_based</rdfs:label>
    </owl:Class>
    


    <!-- http://www.semanticweb.org/macoda/ontologies/PMOEA#ReferencePoint -->

    <owl:Class rdf:about="http://www.semanticweb.org/macoda/ontologies/PMOEA#ReferencePoint">
        <rdfs:subClassOf rdf:resource="http://www.semanticweb.org/macoda/ontologies/PMOEA#PreferenceInformationFromDM"/>
        <rdfs:label xml:lang="en">ReferencePoint</rdfs:label>
    </owl:Class>
    


    <!-- http://www.semanticweb.org/macoda/ontologies/PMOEA#SupportVectorMachine -->

    <owl:Class rdf:about="http://www.semanticweb.org/macoda/ontologies/PMOEA#SupportVectorMachine">
        <rdfs:subClassOf rdf:resource="http://www.semanticweb.org/macoda/ontologies/PMOEA#LearningMethod"/>
        <rdfs:label xml:lang="en">SupportVectorMachine</rdfs:label>
    </owl:Class>
    


    <!-- http://www.semanticweb.org/macoda/ontologies/PMOEA#DTLZ -->

    <owl:Class rdf:about="http://www.semanticweb.org/macoda/ontologies/PMOEA#DTLZ">
        <rdfs:subClassOf rdf:resource="http://www.semanticweb.org/macoda/ontologies/PMOEA#Academic_Problem"/>
        <rdfs:label xml:lang="en">DTLZ</rdfs:label>
    </owl:Class>
    


    <!-- http://www.semanticweb.org/macoda/ontologies/PMOEA#Polynomial -->

    <owl:Class rdf:about="http://www.semanticweb.org/macoda/ontologies/PMOEA#Polynomial">
        <rdfs:subClassOf rdf:resource="http://www.semanticweb.org/macoda/ontologies/PMOEA#UtilityFunction"/>
        <rdfs:label xml:lang="en">Polynomial</rdfs:label>
    </owl:Class>
    


    <!-- http://www.semanticweb.org/macoda/ontologies/PMOEA#Ranking -->

    <owl:Class rdf:about="http://www.semanticweb.org/macoda/ontologies/PMOEA#Ranking">
        <rdfs:subClassOf rdf:resource="http://www.semanticweb.org/macoda/ontologies/PMOEA#PreferenceModel"/>
        <rdfs:label xml:lang="en">Ranking</rdfs:label>
    </owl:Class>
    


    <!-- http://www.semanticweb.org/macoda/ontologies/PMOEA#ACO_based -->

    <owl:Class rdf:about="http://www.semanticweb.org/macoda/ontologies/PMOEA#ACO_based">
        <rdfs:subClassOf rdf:resource="http://www.semanticweb.org/macoda/ontologies/PMOEA#Probabilistic_based"/>
        <rdfs:label xml:lang="en">ACO_based</rdfs:label>
    </owl:Class>
    


    <!-- http://www.semanticweb.org/macoda/ontologies/PMOEA#BiasedDistribution -->

    <owl:Class rdf:about="http://www.semanticweb.org/macoda/ontologies/PMOEA#BiasedDistribution">
        <rdfs:subClassOf rdf:resource="http://www.semanticweb.org/macoda/ontologies/PMOEA#SetOfSolutions"/>
        <rdfs:label xml:lang="en">BiasedDistribution</rdfs:label>
    </owl:Class>
    


    <!-- http://www.semanticweb.org/macoda/ontologies/PMOEA#LearningMethod -->

    <owl:Class rdf:about="http://www.semanticweb.org/macoda/ontologies/PMOEA#LearningMethod">
        <rdfs:label xml:lang="en">LearningMethod</rdfs:label>
    </owl:Class>
    


    <!-- http://www.semanticweb.org/macoda/ontologies/PMOEA#Swarm_based -->

    <owl:Class rdf:about="http://www.semanticweb.org/macoda/ontologies/PMOEA#Swarm_based">
        <rdfs:subClassOf rdf:resource="http://www.semanticweb.org/macoda/ontologies/PMOEA#MOEA"/>
        <rdfs:label xml:lang="en">Swarm_based</rdfs:label>
    </owl:Class>
    


    <!-- http://www.semanticweb.org/macoda/ontologies/PMOEA#Coevolution_based -->

    <owl:Class rdf:about="http://www.semanticweb.org/macoda/ontologies/PMOEA#Coevolution_based">
        <rdfs:subClassOf rdf:resource="http://www.semanticweb.org/macoda/ontologies/PMOEA#MOEA"/>
        <rdfs:label xml:lang="en">Coevolution_based</rdfs:label>
    </owl:Class>
    


    <!-- http://www.semanticweb.org/macoda/ontologies/PMOEA#InteractionTime -->

    <owl:Class rdf:about="http://www.semanticweb.org/macoda/ontologies/PMOEA#InteractionTime">
        <rdfs:label xml:lang="en">InteractionTime</rdfs:label>
    </owl:Class>
    


    <!-- http://www.semanticweb.org/macoda/ontologies/PMOEA#PreferenceIntegration -->

    <owl:Class rdf:about="http://www.semanticweb.org/macoda/ontologies/PMOEA#PreferenceIntegration">
        <rdfs:comment>Modification of the search algorithm to incorporate preference</rdfs:comment>
        <rdfs:label xml:lang="en">PreferenceIntegration</rdfs:label>
    </owl:Class>
    


    <!-- http://www.semanticweb.org/macoda/ontologies/PMOEA#progressive -->

    <owl:Class rdf:about="http://www.semanticweb.org/macoda/ontologies/PMOEA#progressive">
        <rdfs:subClassOf rdf:resource="http://www.semanticweb.org/macoda/ontologies/PMOEA#InteractionTime"/>
        <rdfs:label xml:lang="en">progressive</rdfs:label>
    </owl:Class>
    


    <!-- http://www.semanticweb.org/macoda/ontologies/PMOEA#DesirabilityFunction -->

    <owl:Class rdf:about="http://www.semanticweb.org/macoda/ontologies/PMOEA#DesirabilityFunction">
        <rdfs:subClassOf rdf:resource="http://www.semanticweb.org/macoda/ontologies/PMOEA#PreferenceInformationFromDM"/>
        <rdfs:label xml:lang="en">DesirabilityFunction</rdfs:label>
    </owl:Class>
    


    <!-- http://www.semanticweb.org/macoda/ontologies/PMOEA#Indicator_based -->

    <owl:Class rdf:about="http://www.semanticweb.org/macoda/ontologies/PMOEA#Indicator_based">
        <rdfs:subClassOf rdf:resource="http://www.semanticweb.org/macoda/ontologies/PMOEA#MOEA"/>
        <rdfs:label xml:lang="en">Indicator_based</rdfs:label>
    </owl:Class>
    


    <!-- http://www.semanticweb.org/macoda/ontologies/PMOEA#ImplementationLibrary -->

    <owl:Class rdf:about="http://www.semanticweb.org/macoda/ontologies/PMOEA#ImplementationLibrary">
        <rdfs:label xml:lang="en">ImplementationLibrary</rdfs:label>
    </owl:Class>
    


    <!-- http://www.semanticweb.org/macoda/ontologies/PMOEA#ZDT -->

    <owl:Class rdf:about="http://www.semanticweb.org/macoda/ontologies/PMOEA#ZDT">
        <rdfs:subClassOf rdf:resource="http://www.semanticweb.org/macoda/ontologies/PMOEA#Academic_Problem"/>
        <rdfs:label xml:lang="en">ZDT</rdfs:label>
    </owl:Class>
    


    <!-- http://www.semanticweb.org/macoda/ontologies/PMOEA#FuzzyLogic -->

    <owl:Class rdf:about="http://www.semanticweb.org/macoda/ontologies/PMOEA#FuzzyLogic">
        <rdfs:subClassOf rdf:resource="http://www.semanticweb.org/macoda/ontologies/PMOEA#PreferenceModel"/>
        <rdfs:label xml:lang="en">FuzzyLogic</rdfs:label>
    </owl:Class>
    


    <!-- http://www.semanticweb.org/macoda/ontologies/PMOEA#MOP -->

    <owl:Class rdf:about="http://www.semanticweb.org/macoda/ontologies/PMOEA#MOP">
        <rdfs:comment>MultiobjectiveOptimizationProblem</rdfs:comment>
        <rdfs:label xml:lang="en">MOP</rdfs:label>
    </owl:Class>
    


    <!-- http://www.semanticweb.org/macoda/ontologies/PMOEA#MOEA -->

    <owl:Class rdf:about="http://www.semanticweb.org/macoda/ontologies/PMOEA#MOEA">
        <rdfs:subClassOf rdf:resource="http://www.semanticweb.org/macoda/ontologies/PMOEA#MetaHeuristic"/>
        <rdfs:label xml:lang="en">MOEA</rdfs:label>
    </owl:Class>
    


    <!-- http://www.semanticweb.org/macoda/ontologies/PMOEA#WeightFunctionInObjectiveSpace -->

    <owl:Class rdf:about="http://www.semanticweb.org/macoda/ontologies/PMOEA#WeightFunctionInObjectiveSpace">
        <rdfs:subClassOf rdf:resource="http://www.semanticweb.org/macoda/ontologies/PMOEA#PreferenceRegion"/>
        <rdfs:label xml:lang="en">WeightFunctionInObjectiveSpace</rdfs:label>
    </owl:Class>
    


    <!-- http://www.semanticweb.org/macoda/ontologies/PMOEA#DistributionFunctionInObjectiveSpace -->

    <owl:Class rdf:about="http://www.semanticweb.org/macoda/ontologies/PMOEA#DistributionFunctionInObjectiveSpace">
        <rdfs:subClassOf rdf:resource="http://www.semanticweb.org/macoda/ontologies/PMOEA#PreferenceRegion"/>
        <rdfs:label xml:lang="en">DistributionFunctionInObjectiveSpace</rdfs:label>
    </owl:Class>
    


    <!-- http://www.semanticweb.org/macoda/ontologies/PMOEA#SampleRanks -->

    <owl:Class rdf:about="http://www.semanticweb.org/macoda/ontologies/PMOEA#SampleRanks">
        <rdfs:subClassOf rdf:resource="http://www.semanticweb.org/macoda/ontologies/PMOEA#SolutionComparison"/>
        <rdfs:label xml:lang="en">SampleRanks</rdfs:label>
    </owl:Class>
    


    <!-- http://www.semanticweb.org/macoda/ontologies/PMOEA#Realworld_Problem -->

    <owl:Class rdf:about="http://www.semanticweb.org/macoda/ontologies/PMOEA#Realworld_Problem">
        <rdfs:subClassOf rdf:resource="http://www.semanticweb.org/macoda/ontologies/PMOEA#MOP"/>
        <rdfs:label xml:lang="en">Realworld_Problem</rdfs:label>
    </owl:Class>
    


    <!-- http://www.semanticweb.org/macoda/ontologies/PMOEA#ObjectiveRelativeImportance -->

    <owl:Class rdf:about="http://www.semanticweb.org/macoda/ontologies/PMOEA#ObjectiveRelativeImportance">
        <rdfs:subClassOf rdf:resource="http://www.semanticweb.org/macoda/ontologies/PMOEA#PreferenceModel"/>
    </owl:Class>
    


    <!-- http://www.semanticweb.org/macoda/ontologies/PMOEA#OrderRelation -->

    <owl:Class rdf:about="http://www.semanticweb.org/macoda/ontologies/PMOEA#OrderRelation"/>
    


    <!-- http://www.semanticweb.org/macoda/ontologies/PMOEA#OutrankingParameters -->

    <owl:Class rdf:about="http://www.semanticweb.org/macoda/ontologies/PMOEA#OutrankingParameters">
        <rdfs:subClassOf rdf:resource="http://www.semanticweb.org/macoda/ontologies/PMOEA#PreferenceInformationFromDM"/>
        <rdfs:label>OutrankingParameters</rdfs:label>
    </owl:Class>
    


    <!-- http://www.semanticweb.org/macoda/ontologies/PMOEA#Parallelisation -->

    <owl:Class rdf:about="http://www.semanticweb.org/macoda/ontologies/PMOEA#Parallelisation">
        <rdfs:comment>Algorithm&apos;s schemes used for parallelisation and interleaving evaluations</rdfs:comment>
    </owl:Class>
    


    <!-- http://www.semanticweb.org/macoda/ontologies/PMOEA#PreferencePoint -->

    <owl:Class rdf:about="http://www.semanticweb.org/macoda/ontologies/PMOEA#PreferencePoint">
        <rdfs:subClassOf rdf:resource="http://www.semanticweb.org/macoda/ontologies/PMOEA#PreferenceModel"/>
    </owl:Class>
    


    <!-- http://www.semanticweb.org/macoda/ontologies/PMOEA#Publication -->

    <owl:Class rdf:about="http://www.semanticweb.org/macoda/ontologies/PMOEA#Publication"/>
    


    <!-- http://www.semanticweb.org/macoda/ontologies/PMOEA#k-Dominance -->

    <owl:Class rdf:about="http://www.semanticweb.org/macoda/ontologies/PMOEA#k-Dominance">
        <rdfs:subClassOf rdf:resource="http://www.semanticweb.org/macoda/ontologies/PMOEA#OrderRelation"/>
        <rdfs:comment>Also (1-k)-dominance. Dominance relation based on counting results of component-wise comparisons. Not transitive.</rdfs:comment>
    </owl:Class>
    


    <!-- 
    ///////////////////////////////////////////////////////////////////////////////////////
    //
    // Individuals
    //
    ///////////////////////////////////////////////////////////////////////////////////////
     -->

    


    <!-- http://www.semanticweb.org/macoda/ontologies/PMOEA#Abhay_Kumar -->

    <owl:NamedIndividual rdf:about="http://www.semanticweb.org/macoda/ontologies/PMOEA#Abhay_Kumar">
        <rdf:type rdf:resource="http://www.semanticweb.org/macoda/ontologies/PMOEA#Researcher"/>
        <rdfs:label>Abhay Kumar</rdfs:label>
    </owl:NamedIndividual>
    


    <!-- http://www.semanticweb.org/macoda/ontologies/PMOEA#AdditiveEpsilonIndicator -->

    <owl:NamedIndividual rdf:about="http://www.semanticweb.org/macoda/ontologies/PMOEA#AdditiveEpsilonIndicator">
        <rdf:type rdf:resource="http://www.semanticweb.org/macoda/ontologies/PMOEA#SetQualityIndicator"/>
        <rdfs:label>AdditiveEpsilonIndicator</rdfs:label>
    </owl:NamedIndividual>
    


    <!-- http://www.semanticweb.org/macoda/ontologies/PMOEA#AirfoilShapeOptimization -->

    <owl:NamedIndividual rdf:about="http://www.semanticweb.org/macoda/ontologies/PMOEA#AirfoilShapeOptimization">
        <rdf:type rdf:resource="http://www.semanticweb.org/macoda/ontologies/PMOEA#Realworld_Problem"/>
        <PMOEA:isContinuousProblem rdf:datatype="http://www.w3.org/2001/XMLSchema#boolean">true</PMOEA:isContinuousProblem>
        <PMOEA:ObjectiveNumber rdf:datatype="http://www.w3.org/2001/XMLSchema#integer">6</PMOEA:ObjectiveNumber>
        <PMOEA:isManyObjectiveProblem rdf:datatype="http://www.w3.org/2001/XMLSchema#boolean">true</PMOEA:isManyObjectiveProblem>
        <rdfs:label>AirfoilShapeOptimization_6</rdfs:label>
    </owl:NamedIndividual>
    


    <!-- http://www.semanticweb.org/macoda/ontologies/PMOEA#AirfoilShapeOptimization_3 -->

    <owl:NamedIndividual rdf:about="http://www.semanticweb.org/macoda/ontologies/PMOEA#AirfoilShapeOptimization_3">
        <rdf:type rdf:resource="http://www.semanticweb.org/macoda/ontologies/PMOEA#Realworld_Problem"/>
        <PMOEA:isContinuousProblem rdf:datatype="http://www.w3.org/2001/XMLSchema#boolean">true</PMOEA:isContinuousProblem>
        <PMOEA:ObjectiveNumber rdf:datatype="http://www.w3.org/2001/XMLSchema#integer">3</PMOEA:ObjectiveNumber>
        <PMOEA:hasReference>A. Szollos, M. Smd, and J. Hajek, Aerodynamic optimization
via multi-objective micro-genetic algorithm with range adaptation,
knowledge-based reinitialization, crowding and epsilon-dominance, Advances in Engineering Software, vol. 40, no. 6, pp. 419430, 2009</PMOEA:hasReference>
        <rdfs:label>AirfoilShapeOptimization_3</rdfs:label>
    </owl:NamedIndividual>
    


    <!-- http://www.semanticweb.org/macoda/ontologies/PMOEA#Alfredo_G._Hernndez-Daz -->

    <owl:NamedIndividual rdf:about="http://www.semanticweb.org/macoda/ontologies/PMOEA#Alfredo_G._Hernndez-Daz">
        <rdf:type rdf:resource="http://www.semanticweb.org/macoda/ontologies/PMOEA#Researcher"/>
        <rdfs:label>Alfredo G. Hernndez-Daz</rdfs:label>
    </owl:NamedIndividual>
    


    <!-- http://www.semanticweb.org/macoda/ontologies/PMOEA#Alfredo_Montano -->

    <owl:NamedIndividual rdf:about="http://www.semanticweb.org/macoda/ontologies/PMOEA#Alfredo_Montano">
        <rdf:type rdf:resource="http://www.semanticweb.org/macoda/ontologies/PMOEA#Researcher"/>
        <rdfs:label>Alfredo Montano</rdfs:label>
    </owl:NamedIndividual>
    


    <!-- http://www.semanticweb.org/macoda/ontologies/PMOEA#Ana_Beln_Ruiz -->

    <owl:NamedIndividual rdf:about="http://www.semanticweb.org/macoda/ontologies/PMOEA#Ana_Beln_Ruiz">
        <rdf:type rdf:resource="http://www.semanticweb.org/macoda/ontologies/PMOEA#Researcher"/>
        <rdfs:label>Ana Beln Ruiz</rdfs:label>
    </owl:NamedIndividual>
    


    <!-- http://www.semanticweb.org/macoda/ontologies/PMOEA#Andrzej_Jaszkiewicz -->

    <owl:NamedIndividual rdf:about="http://www.semanticweb.org/macoda/ontologies/PMOEA#Andrzej_Jaszkiewicz">
        <rdf:type rdf:resource="http://www.semanticweb.org/macoda/ontologies/PMOEA#Researcher"/>
        <rdfs:label>Andrzej Jaszkiewicz</rdfs:label>
    </owl:NamedIndividual>
    


    <!-- http://www.semanticweb.org/macoda/ontologies/PMOEA#Antonio_Jaimes -->

    <owl:NamedIndividual rdf:about="http://www.semanticweb.org/macoda/ontologies/PMOEA#Antonio_Jaimes">
        <rdf:type rdf:resource="http://www.semanticweb.org/macoda/ontologies/PMOEA#Researcher"/>
        <rdfs:label>Antonio Jaimes</rdfs:label>
    </owl:NamedIndividual>
    


    <!-- http://www.semanticweb.org/macoda/ontologies/PMOEA#Carlos_Coello_Coello -->

    <owl:NamedIndividual rdf:about="http://www.semanticweb.org/macoda/ontologies/PMOEA#Carlos_Coello_Coello">
        <rdf:type rdf:resource="http://www.semanticweb.org/macoda/ontologies/PMOEA#Researcher"/>
        <rdfs:label>Carlos Coello Coello</rdfs:label>
    </owl:NamedIndividual>
    


    <!-- http://www.semanticweb.org/macoda/ontologies/PMOEA#ChebyshevPreferenceRelation -->

    <owl:NamedIndividual rdf:about="http://www.semanticweb.org/macoda/ontologies/PMOEA#ChebyshevPreferenceRelation">
        <rdf:type rdf:resource="http://www.semanticweb.org/macoda/ontologies/PMOEA#DominanceRelation"/>
        <rdfs:comment>Solutions in ROI are compared using the usual Pareto dominance relation, while solutions outside of the ROI are compared using their achievement function value</rdfs:comment>
        <rdfs:label>ChebyshevPreferenceRelation</rdfs:label>
    </owl:NamedIndividual>
    


    <!-- http://www.semanticweb.org/macoda/ontologies/PMOEA#Claudia_Gomez -->

    <owl:NamedIndividual rdf:about="http://www.semanticweb.org/macoda/ontologies/PMOEA#Claudia_Gomez">
        <rdf:type rdf:resource="http://www.semanticweb.org/macoda/ontologies/PMOEA#Researcher"/>
        <rdfs:label>Claudia Gomez</rdfs:label>
    </owl:NamedIndividual>
    


    <!-- http://www.semanticweb.org/macoda/ontologies/PMOEA#CompositeScalarizingFunctions -->

    <owl:NamedIndividual rdf:about="http://www.semanticweb.org/macoda/ontologies/PMOEA#CompositeScalarizingFunctions">
        <rdf:type rdf:resource="http://www.semanticweb.org/macoda/ontologies/PMOEA#AchievementScalarizingFunction"/>
        <rdfs:comment>used in iPMA</rdfs:comment>
        <rdfs:label>CompositeScalarizingFunctions</rdfs:label>
    </owl:NamedIndividual>
    


    <!-- http://www.semanticweb.org/macoda/ontologies/PMOEA#DTLZ2_10 -->

    <owl:NamedIndividual rdf:about="http://www.semanticweb.org/macoda/ontologies/PMOEA#DTLZ2_10">
        <rdf:type rdf:resource="http://www.semanticweb.org/macoda/ontologies/PMOEA#DTLZ"/>
        <PMOEA:isContinuousProblem rdf:datatype="http://www.w3.org/2001/XMLSchema#boolean">true</PMOEA:isContinuousProblem>
        <PMOEA:ObjectiveNumber rdf:datatype="http://www.w3.org/2001/XMLSchema#integer">10</PMOEA:ObjectiveNumber>
        <PMOEA:isManyObjectiveProblem rdf:datatype="http://www.w3.org/2001/XMLSchema#boolean">true</PMOEA:isManyObjectiveProblem>
        <rdfs:label>DTLZ2_10</rdfs:label>
    </owl:NamedIndividual>
    


    <!-- http://www.semanticweb.org/macoda/ontologies/PMOEA#DTLZ2_6 -->

    <owl:NamedIndividual rdf:about="http://www.semanticweb.org/macoda/ontologies/PMOEA#DTLZ2_6">
        <rdf:type rdf:resource="http://www.semanticweb.org/macoda/ontologies/PMOEA#DTLZ"/>
        <PMOEA:isContinuousProblem rdf:datatype="http://www.w3.org/2001/XMLSchema#boolean">true</PMOEA:isContinuousProblem>
        <PMOEA:ObjectiveNumber rdf:datatype="http://www.w3.org/2001/XMLSchema#integer">6</PMOEA:ObjectiveNumber>
        <PMOEA:isManyObjectiveProblem rdf:datatype="http://www.w3.org/2001/XMLSchema#boolean">true</PMOEA:isManyObjectiveProblem>
    </owl:NamedIndividual>
    


    <!-- http://www.semanticweb.org/macoda/ontologies/PMOEA#DTLZ3_3 -->

    <owl:NamedIndividual rdf:about="http://www.semanticweb.org/macoda/ontologies/PMOEA#DTLZ3_3">
        <rdf:type rdf:resource="http://www.semanticweb.org/macoda/ontologies/PMOEA#DTLZ"/>
        <PMOEA:OWLDataProperty_61d3cd95_fde4_4c1b_af08_1eaf73473aea rdf:datatype="http://www.w3.org/2001/XMLSchema#boolean">true</PMOEA:OWLDataProperty_61d3cd95_fde4_4c1b_af08_1eaf73473aea>
        <PMOEA:isContinuousProblem rdf:datatype="http://www.w3.org/2001/XMLSchema#boolean">true</PMOEA:isContinuousProblem>
        <PMOEA:ObjectiveNumber rdf:datatype="http://www.w3.org/2001/XMLSchema#integer">3</PMOEA:ObjectiveNumber>
    </owl:NamedIndividual>
    


    <!-- http://www.semanticweb.org/macoda/ontologies/PMOEA#DTLZ3_4 -->

    <owl:NamedIndividual rdf:about="http://www.semanticweb.org/macoda/ontologies/PMOEA#DTLZ3_4">
        <rdf:type rdf:resource="http://www.semanticweb.org/macoda/ontologies/PMOEA#DTLZ"/>
        <PMOEA:OWLDataProperty_61d3cd95_fde4_4c1b_af08_1eaf73473aea rdf:datatype="http://www.w3.org/2001/XMLSchema#boolean">true</PMOEA:OWLDataProperty_61d3cd95_fde4_4c1b_af08_1eaf73473aea>
        <PMOEA:isContinuousProblem rdf:datatype="http://www.w3.org/2001/XMLSchema#boolean">true</PMOEA:isContinuousProblem>
        <PMOEA:ObjectiveNumber rdf:datatype="http://www.w3.org/2001/XMLSchema#integer">4</PMOEA:ObjectiveNumber>
        <PMOEA:isManyObjectiveProblem rdf:datatype="http://www.w3.org/2001/XMLSchema#boolean">true</PMOEA:isManyObjectiveProblem>
    </owl:NamedIndividual>
    


    <!-- http://www.semanticweb.org/macoda/ontologies/PMOEA#DTLZ3_6 -->

    <owl:NamedIndividual rdf:about="http://www.semanticweb.org/macoda/ontologies/PMOEA#DTLZ3_6">
        <rdf:type rdf:resource="http://www.semanticweb.org/macoda/ontologies/PMOEA#DTLZ"/>
        <PMOEA:OWLDataProperty_61d3cd95_fde4_4c1b_af08_1eaf73473aea rdf:datatype="http://www.w3.org/2001/XMLSchema#boolean">true</PMOEA:OWLDataProperty_61d3cd95_fde4_4c1b_af08_1eaf73473aea>
        <PMOEA:isContinuousProblem rdf:datatype="http://www.w3.org/2001/XMLSchema#boolean">true</PMOEA:isContinuousProblem>
        <PMOEA:ObjectiveNumber rdf:datatype="http://www.w3.org/2001/XMLSchema#integer">6</PMOEA:ObjectiveNumber>
        <PMOEA:isManyObjectiveProblem rdf:datatype="http://www.w3.org/2001/XMLSchema#boolean">true</PMOEA:isManyObjectiveProblem>
    </owl:NamedIndividual>
    


    <!-- http://www.semanticweb.org/macoda/ontologies/PMOEA#DTLZ4_4 -->

    <owl:NamedIndividual rdf:about="http://www.semanticweb.org/macoda/ontologies/PMOEA#DTLZ4_4">
        <rdf:type rdf:resource="http://www.semanticweb.org/macoda/ontologies/PMOEA#DTLZ"/>
        <PMOEA:isContinuousProblem rdf:datatype="http://www.w3.org/2001/XMLSchema#boolean">true</PMOEA:isContinuousProblem>
        <PMOEA:ObjectiveNumber rdf:datatype="http://www.w3.org/2001/XMLSchema#integer">4</PMOEA:ObjectiveNumber>
        <PMOEA:isManyObjectiveProblem rdf:datatype="http://www.w3.org/2001/XMLSchema#boolean">true</PMOEA:isManyObjectiveProblem>
    </owl:NamedIndividual>
    


    <!-- http://www.semanticweb.org/macoda/ontologies/PMOEA#DTLZ4_6 -->

    <owl:NamedIndividual rdf:about="http://www.semanticweb.org/macoda/ontologies/PMOEA#DTLZ4_6">
        <rdf:type rdf:resource="http://www.semanticweb.org/macoda/ontologies/PMOEA#DTLZ"/>
        <PMOEA:isContinuousProblem rdf:datatype="http://www.w3.org/2001/XMLSchema#boolean">true</PMOEA:isContinuousProblem>
        <PMOEA:ObjectiveNumber rdf:datatype="http://www.w3.org/2001/XMLSchema#integer">6</PMOEA:ObjectiveNumber>
        <PMOEA:isManyObjectiveProblem rdf:datatype="http://www.w3.org/2001/XMLSchema#boolean">true</PMOEA:isManyObjectiveProblem>
    </owl:NamedIndividual>
    


    <!-- http://www.semanticweb.org/macoda/ontologies/PMOEA#DTLZ5_3 -->

    <owl:NamedIndividual rdf:about="http://www.semanticweb.org/macoda/ontologies/PMOEA#DTLZ5_3">
        <rdf:type rdf:resource="http://www.semanticweb.org/macoda/ontologies/PMOEA#DTLZ"/>
        <PMOEA:isContinuousProblem rdf:datatype="http://www.w3.org/2001/XMLSchema#boolean">true</PMOEA:isContinuousProblem>
        <PMOEA:ObjectiveNumber rdf:datatype="http://www.w3.org/2001/XMLSchema#integer">3</PMOEA:ObjectiveNumber>
    </owl:NamedIndividual>
    


    <!-- http://www.semanticweb.org/macoda/ontologies/PMOEA#DTLZ5_4 -->

    <owl:NamedIndividual rdf:about="http://www.semanticweb.org/macoda/ontologies/PMOEA#DTLZ5_4">
        <rdf:type rdf:resource="http://www.semanticweb.org/macoda/ontologies/PMOEA#DTLZ"/>
        <PMOEA:isContinuousProblem rdf:datatype="http://www.w3.org/2001/XMLSchema#boolean">true</PMOEA:isContinuousProblem>
        <PMOEA:ObjectiveNumber rdf:datatype="http://www.w3.org/2001/XMLSchema#integer">4</PMOEA:ObjectiveNumber>
        <PMOEA:isManyObjectiveProblem rdf:datatype="http://www.w3.org/2001/XMLSchema#boolean">true</PMOEA:isManyObjectiveProblem>
    </owl:NamedIndividual>
    


    <!-- http://www.semanticweb.org/macoda/ontologies/PMOEA#DTLZ5_6 -->

    <owl:NamedIndividual rdf:about="http://www.semanticweb.org/macoda/ontologies/PMOEA#DTLZ5_6">
        <rdf:type rdf:resource="http://www.semanticweb.org/macoda/ontologies/PMOEA#DTLZ"/>
        <PMOEA:isContinuousProblem rdf:datatype="http://www.w3.org/2001/XMLSchema#boolean">true</PMOEA:isContinuousProblem>
        <PMOEA:ObjectiveNumber rdf:datatype="http://www.w3.org/2001/XMLSchema#integer">6</PMOEA:ObjectiveNumber>
        <PMOEA:isManyObjectiveProblem rdf:datatype="http://www.w3.org/2001/XMLSchema#boolean">true</PMOEA:isManyObjectiveProblem>
    </owl:NamedIndividual>
    


    <!-- http://www.semanticweb.org/macoda/ontologies/PMOEA#DTLZ6_3 -->

    <owl:NamedIndividual rdf:about="http://www.semanticweb.org/macoda/ontologies/PMOEA#DTLZ6_3">
        <rdf:type rdf:resource="http://www.semanticweb.org/macoda/ontologies/PMOEA#DTLZ"/>
        <PMOEA:isContinuousProblem rdf:datatype="http://www.w3.org/2001/XMLSchema#boolean">true</PMOEA:isContinuousProblem>
        <PMOEA:ObjectiveNumber rdf:datatype="http://www.w3.org/2001/XMLSchema#integer">3</PMOEA:ObjectiveNumber>
    </owl:NamedIndividual>
    


    <!-- http://www.semanticweb.org/macoda/ontologies/PMOEA#DTLZ7_3 -->

    <owl:NamedIndividual rdf:about="http://www.semanticweb.org/macoda/ontologies/PMOEA#DTLZ7_3">
        <rdf:type rdf:resource="http://www.semanticweb.org/macoda/ontologies/PMOEA#DTLZ"/>
        <PMOEA:isContinuousProblem rdf:datatype="http://www.w3.org/2001/XMLSchema#boolean">true</PMOEA:isContinuousProblem>
        <PMOEA:ObjectiveNumber rdf:datatype="http://www.w3.org/2001/XMLSchema#integer">3</PMOEA:ObjectiveNumber>
        <rdfs:label>DTLZ7_3</rdfs:label>
    </owl:NamedIndividual>
    


    <!-- http://www.semanticweb.org/macoda/ontologies/PMOEA#Deb32 -->

    <owl:NamedIndividual rdf:about="http://www.semanticweb.org/macoda/ontologies/PMOEA#Deb32">
        <rdf:type rdf:resource="http://www.semanticweb.org/macoda/ontologies/PMOEA#Academic_Problem"/>
        <PMOEA:isContinuousProblem rdf:datatype="http://www.w3.org/2001/XMLSchema#boolean">true</PMOEA:isContinuousProblem>
        <PMOEA:ObjectiveNumber rdf:datatype="http://www.w3.org/2001/XMLSchema#integer">2</PMOEA:ObjectiveNumber>
        <rdfs:comment>K. Deb, Multi-Objective Genetic Algorithms: Problem Difficulties and
Construction of Test Problems, Evolutionary Computation 7 (3) (1999) 205
230. Fall</rdfs:comment>
        <rdfs:label>Deb32</rdfs:label>
    </owl:NamedIndividual>
    


    <!-- http://www.semanticweb.org/macoda/ontologies/PMOEA#Dipti_Srinivasan -->

    <owl:NamedIndividual rdf:about="http://www.semanticweb.org/macoda/ontologies/PMOEA#Dipti_Srinivasan">
        <rdf:type rdf:resource="http://www.semanticweb.org/macoda/ontologies/PMOEA#Researcher"/>
        <rdfs:label>Dipti Srinivasan</rdfs:label>
    </owl:NamedIndividual>
    


    <!-- http://www.semanticweb.org/macoda/ontologies/PMOEA#ELECTRE -->

    <owl:NamedIndividual rdf:about="http://www.semanticweb.org/macoda/ontologies/PMOEA#ELECTRE">
        <rdf:type rdf:resource="http://www.semanticweb.org/macoda/ontologies/PMOEA#OutrankingRelation"/>
        <rdfs:comment>A proposition xSy (x outranks y) (x seems at least as good as y) holds if and only if the coalition of criteria in agreement with this proposition is strong enough and there is no important coalition
discordant with it . Let c(x,y) and d(x,y) denote the degree of truth of the predicates C(x,y) and D(x,y). the truth of  xSy can be calculated as :deta(x, y) = c(x, y)  N(d(x, y))</rdfs:comment>
        <rdfs:label>ELECTRE_based</rdfs:label>
    </owl:NamedIndividual>
    


    <!-- http://www.semanticweb.org/macoda/ontologies/PMOEA#ELECTREParameters -->

    <owl:NamedIndividual rdf:about="http://www.semanticweb.org/macoda/ontologies/PMOEA#ELECTREParameters">
        <rdf:type rdf:resource="http://www.semanticweb.org/macoda/ontologies/PMOEA#OutrankingParameters"/>
        <rdfs:comment>including weights that express the importance of different objectives,Indifferencethresholds,Vetothresholds, strict outranking parameter</rdfs:comment>
        <rdfs:label>ELECTREParameters</rdfs:label>
    </owl:NamedIndividual>
    


    <!-- http://www.semanticweb.org/macoda/ontologies/PMOEA#Eduardo_Fernandez -->

    <owl:NamedIndividual rdf:about="http://www.semanticweb.org/macoda/ontologies/PMOEA#Eduardo_Fernandez">
        <rdf:type rdf:resource="http://www.semanticweb.org/macoda/ontologies/PMOEA#Researcher"/>
        <rdfs:label>Eduardo Fernandez</rdfs:label>
    </owl:NamedIndividual>
    


    <!-- http://www.semanticweb.org/macoda/ontologies/PMOEA#Edy_Lopez -->

    <owl:NamedIndividual rdf:about="http://www.semanticweb.org/macoda/ontologies/PMOEA#Edy_Lopez">
        <rdf:type rdf:resource="http://www.semanticweb.org/macoda/ontologies/PMOEA#Researcher"/>
        <rdfs:label>Edy Lopez</rdfs:label>
    </owl:NamedIndividual>
    


    <!-- http://www.semanticweb.org/macoda/ontologies/PMOEA#Fonseca_test -->

    <owl:NamedIndividual rdf:about="http://www.semanticweb.org/macoda/ontologies/PMOEA#Fonseca_test">
        <rdf:type rdf:resource="http://www.semanticweb.org/macoda/ontologies/PMOEA#Academic_Problem"/>
        <owl:sameAs rdf:resource="http://www.semanticweb.org/macoda/ontologies/PMOEA#FF"/>
        <PMOEA:isContinuousProblem rdf:datatype="http://www.w3.org/2001/XMLSchema#boolean">true</PMOEA:isContinuousProblem>
        <PMOEA:ObjectiveNumber rdf:datatype="http://www.w3.org/2001/XMLSchema#integer">2</PMOEA:ObjectiveNumber>
        <rdfs:comment>C. M. M. Fonseca, Multiobjective genetic algorithms with application
to control engineering problems, Ph.D. dissertation, Dept. Autom.
Control Syst. Eng., Univ. Sheffield, Sheffield, U.K., 1995</rdfs:comment>
        <rdfs:label>FonsecaTest</rdfs:label>
    </owl:NamedIndividual>
    


    <!-- http://www.semanticweb.org/macoda/ontologies/PMOEA#GF-NSGA-II -->

    <owl:NamedIndividual rdf:about="http://www.semanticweb.org/macoda/ontologies/PMOEA#GF-NSGA-II">
        <rdf:type rdf:resource="http://www.semanticweb.org/macoda/ontologies/PMOEA#PMOEA"/>
        <PMOEA:hasPreferenceModel rdf:resource="http://www.semanticweb.org/macoda/ontologies/PMOEA#GaussionFunctionOnHyperplane"/>
        <PMOEA:hasPreferenceInformationFromDM rdf:resource="http://www.semanticweb.org/macoda/ontologies/PMOEA#ParametersInGaussionFunction"/>
        <PMOEA:hasInteractionTime rdf:resource="http://www.semanticweb.org/macoda/ontologies/PMOEA#a-priori"/>
        <PMOEA:hasPreferenceIntegration rdf:resource="http://www.semanticweb.org/macoda/ontologies/PMOEA#CrowdingDistance"/>
        <PMOEA:hasComparison rdf:resource="http://www.semanticweb.org/macoda/ontologies/PMOEA#R-NSGA-II"/>
        <PMOEA:canSolve rdf:resource="http://www.semanticweb.org/macoda/ontologies/PMOEA#DTLZ5_3"/>
        <PMOEA:canSolve rdf:resource="http://www.semanticweb.org/macoda/ontologies/PMOEA#DTLZ7_3"/>
        <PMOEA:canSolve rdf:resource="http://www.semanticweb.org/macoda/ontologies/PMOEA#HybridCarControllerOptimizationProblem"/>
        <PMOEA:canSolve rdf:resource="http://www.semanticweb.org/macoda/ontologies/PMOEA#Knapsack_2"/>
        <PMOEA:canSolve rdf:resource="http://www.semanticweb.org/macoda/ontologies/PMOEA#Knapsack_4"/>
        <PMOEA:canSolve rdf:resource="http://www.semanticweb.org/macoda/ontologies/PMOEA#Knapsack_10"/>
        <PMOEA:canSolve rdf:resource="http://www.semanticweb.org/macoda/ontologies/PMOEA#DTLZ1_3"/>
        <PMOEA:canSolve rdf:resource="http://www.semanticweb.org/macoda/ontologies/PMOEA#DTLZ2_3"/>
        <PMOEA:canSolve rdf:resource="http://www.semanticweb.org/macoda/ontologies/PMOEA#Knapsack_8"/>
        <PMOEA:canSolve rdf:resource="http://www.semanticweb.org/macoda/ontologies/PMOEA#WeldedBeamDesign"/>
        <PMOEA:hasResultInfluence rdf:resource="http://www.semanticweb.org/macoda/ontologies/PMOEA#BoundedRegion"/>
        <PMOEA:hasAuthor rdf:resource="http://www.semanticweb.org/macoda/ontologies/PMOEA#Kaname_Narukawa"/>
        <PMOEA:hasAuthor rdf:resource="http://www.semanticweb.org/macoda/ontologies/PMOEA#Markus_Olhofer"/>
        <PMOEA:hasAuthor rdf:resource="http://www.semanticweb.org/macoda/ontologies/PMOEA#Yu_Setoguchi"/>
        <PMOEA:hasAuthor rdf:resource="http://www.semanticweb.org/macoda/ontologies/PMOEA#Yuki_Tanigaki"/>
        <PMOEA:hasSearchAlgorithm rdf:resource="http://www.semanticweb.org/macoda/ontologies/PMOEA#NSGA-II"/>
        <PMOEA:hasDevelopingYear rdf:datatype="http://www.w3.org/2001/XMLSchema#integer">2015</PMOEA:hasDevelopingYear>
        <PMOEA:MultipleRegionOfInterest rdf:datatype="http://www.w3.org/2001/XMLSchema#boolean">true</PMOEA:MultipleRegionOfInterest>
        <PMOEA:SpreadControl rdf:datatype="http://www.w3.org/2001/XMLSchema#boolean">true</PMOEA:SpreadControl>
        <PMOEA:ParetoDominancePreservation rdf:datatype="http://www.w3.org/2001/XMLSchema#boolean">true</PMOEA:ParetoDominancePreservation>
        <PMOEA:hasReference>Narukawa, K., Y. Setoguchi, Y. Tanigaki, M. Olhofer, B. Sendhoff and H. Ishibuchi (2015). &quot;Preference representation using Gaussian functions on a hyperplane in evolutionary multi-objective optimization.&quot; Soft Computing</PMOEA:hasReference>
        <PMOEA:hasReference>Tanigaki, Yuki, et al. &quot;Preference-based NSGA-II for many-objective knapsack problems.&quot; Soft Computing and Intelligent Systems (SCIS), 2014 Joint 7th International Conference on and Advanced Intelligent Systems (ISIS), 15th International Symposium on. IEEE, 2014.</PMOEA:hasReference>
        <rdfs:comment>We previously proposed to represent the preference of the DM using Gaussian functions on a hyperplane. The DM specifies the center and spread vectors of the Gaussian functions so as to represent his/her preference. The preference handling is integrated into the framework of NSGA-II. This paper extends our previous work by considering an allowable radius and a shortest distance to realize a distribution that follows Gaussian functions. Our aim is to obtain dense solutions around center vectors and sparse solutions far away from the center vectors on a hyperplane.</rdfs:comment>
        <rdfs:label>GF-NSGA-II</rdfs:label>
    </owl:NamedIndividual>
    


    <!-- http://www.semanticweb.org/macoda/ontologies/PMOEA#GaussionFunctionOnHyperplane -->

    <owl:NamedIndividual rdf:about="http://www.semanticweb.org/macoda/ontologies/PMOEA#GaussionFunctionOnHyperplane">
        <rdf:type rdf:resource="http://www.semanticweb.org/macoda/ontologies/PMOEA#PreferenceRegion"/>
        <rdfs:comment>a Gaussian function on the hyperplane in the objective space defined by a center vecter and spread vecter, solutions near the  center vecter is preferred by the DM</rdfs:comment>
        <rdfs:label>GaussianFunctionsOnTheHyperplane</rdfs:label>
    </owl:NamedIndividual>
    


    <!-- http://www.semanticweb.org/macoda/ontologies/PMOEA#H-MCSGA -->

    <owl:NamedIndividual rdf:about="http://www.semanticweb.org/macoda/ontologies/PMOEA#H-MCSGA">
        <rdf:type rdf:resource="http://www.semanticweb.org/macoda/ontologies/PMOEA#PMOEA"/>
        <PMOEA:hasPreferenceModel rdf:resource="http://www.semanticweb.org/macoda/ontologies/PMOEA#THESEUS"/>
        <PMOEA:hasPreferenceInformationFromDM rdf:resource="http://www.semanticweb.org/macoda/ontologies/PMOEA#SortSampleIntoCategory"/>
        <PMOEA:hasInteractionTime rdf:resource="http://www.semanticweb.org/macoda/ontologies/PMOEA#a-priori"/>
        <PMOEA:hasPreferenceIntegration rdf:resource="http://www.semanticweb.org/macoda/ontologies/PMOEA#FrontSorting"/>
        <PMOEA:canSolve rdf:resource="http://www.semanticweb.org/macoda/ontologies/PMOEA#ProjectPortfolioProblem_9"/>
        <PMOEA:hasResultInfluence rdf:resource="http://www.semanticweb.org/macoda/ontologies/PMOEA#SetOfSolutions"/>
        <PMOEA:hasAuthor rdf:resource="http://www.semanticweb.org/macoda/ontologies/PMOEA#Claudia_Gomez"/>
        <PMOEA:hasAuthor rdf:resource="http://www.semanticweb.org/macoda/ontologies/PMOEA#Eduardo_Fernandez"/>
        <PMOEA:hasAuthor rdf:resource="http://www.semanticweb.org/macoda/ontologies/PMOEA#Laura_Cruz-Reyes"/>
        <PMOEA:hasAuthor rdf:resource="http://www.semanticweb.org/macoda/ontologies/PMOEA#Patricia_Sanchez"/>
        <PMOEA:hasSearchAlgorithm rdf:resource="http://www.semanticweb.org/macoda/ontologies/PMOEA#NSGA-II"/>
        <PMOEA:hasDevelopingYear rdf:datatype="http://www.w3.org/2001/XMLSchema#integer">2014</PMOEA:hasDevelopingYear>
        <PMOEA:hasReference>Cruz-Reyes, L., E. Fernandez, C. Gomez and P. Sanchez (2014). Preference Incorporation into Evolutionary Multiobjective Optimization Using a Multi-Criteria Evaluation Method. Recent Advances on Hybrid Approaches for Designing Intelligent Systems, Springer: 533-542</PMOEA:hasReference>
        <rdfs:comment>we introduce a new way to incorporate and update the DMs preferences into a Multiobjective Evolutionary Algorithm, expressed in a set of solutions assigned to ordered categories. We propose a variant of the well-known Non-dominated Sorting Genetic Algorithm II (NSGA-II), called Hybrid-MultiCriteria Sorting Genetic Algorithm (H-MCSGA). In this algorithm, we strengthen the selective pressure based on dominance adding selective pressure based on assignments to categories. Particularly, we make selective pressure towards non-dominated solutions that belong to the best category</rdfs:comment>
        <rdfs:label>H-MCSGA</rdfs:label>
    </owl:NamedIndividual>
    


    <!-- http://www.semanticweb.org/macoda/ontologies/PMOEA#HybridCarControllerOptimizationProblem -->

    <owl:NamedIndividual rdf:about="http://www.semanticweb.org/macoda/ontologies/PMOEA#HybridCarControllerOptimizationProblem">
        <rdf:type rdf:resource="http://www.semanticweb.org/macoda/ontologies/PMOEA#Realworld_Problem"/>
        <PMOEA:isContinuousProblem rdf:datatype="http://www.w3.org/2001/XMLSchema#boolean">true</PMOEA:isContinuousProblem>
        <PMOEA:ObjectiveNumber rdf:datatype="http://www.w3.org/2001/XMLSchema#integer">7</PMOEA:ObjectiveNumber>
        <PMOEA:hasReference>Narukawa K, Rodemann T (2012) Examining the performance of evolutionary many-objective optimization algorithms on a real-world
application. In: Proceedings of 2012 IEEE International Conference
on Genetic and Evolutionary Computing, pp 316319. IEEE</PMOEA:hasReference>
        <PMOEA:isManyObjectiveProblem rdf:datatype="http://www.w3.org/2001/XMLSchema#boolean">true</PMOEA:isManyObjectiveProblem>
        <rdfs:comment>HCCOP is given as a black box that has 11 decision variables
and 7 objectives</rdfs:comment>
        <rdfs:label>HybridCarControllerOptimizationProblem</rdfs:label>
    </owl:NamedIndividual>
    


    <!-- http://www.semanticweb.org/macoda/ontologies/PMOEA#J._Sundar -->

    <owl:NamedIndividual rdf:about="http://www.semanticweb.org/macoda/ontologies/PMOEA#J._Sundar">
        <rdf:type rdf:resource="http://www.semanticweb.org/macoda/ontologies/PMOEA#Researcher"/>
        <rdfs:label>J. Sundar</rdfs:label>
    </owl:NamedIndividual>
    


    <!-- http://www.semanticweb.org/macoda/ontologies/PMOEA#Jorge_Navarro -->

    <owl:NamedIndividual rdf:about="http://www.semanticweb.org/macoda/ontologies/PMOEA#Jorge_Navarro">
        <rdf:type rdf:resource="http://www.semanticweb.org/macoda/ontologies/PMOEA#Researcher"/>
        <rdfs:label>Jorge Navarro</rdfs:label>
    </owl:NamedIndividual>
    


    <!-- http://www.semanticweb.org/macoda/ontologies/PMOEA#Julin_Molina -->

    <owl:NamedIndividual rdf:about="http://www.semanticweb.org/macoda/ontologies/PMOEA#Julin_Molina">
        <rdf:type rdf:resource="http://www.semanticweb.org/macoda/ontologies/PMOEA#Researcher"/>
        <rdfs:label>Julin Molina</rdfs:label>
    </owl:NamedIndividual>
    


    <!-- http://www.semanticweb.org/macoda/ontologies/PMOEA#KUR -->

    <owl:NamedIndividual rdf:about="http://www.semanticweb.org/macoda/ontologies/PMOEA#KUR">
        <rdf:type rdf:resource="http://www.semanticweb.org/macoda/ontologies/PMOEA#Academic_Problem"/>
        <PMOEA:isContinuousProblem rdf:datatype="http://www.w3.org/2001/XMLSchema#boolean">true</PMOEA:isContinuousProblem>
        <PMOEA:ObjectiveNumber rdf:datatype="http://www.w3.org/2001/XMLSchema#integer">2</PMOEA:ObjectiveNumber>
        <rdfs:comment>used in LBS-EMO, no reference found</rdfs:comment>
        <rdfs:label>KUR</rdfs:label>
    </owl:NamedIndividual>
    


    <!-- http://www.semanticweb.org/macoda/ontologies/PMOEA#Kaisa_Miettinen -->

    <owl:NamedIndividual rdf:about="http://www.semanticweb.org/macoda/ontologies/PMOEA#Kaisa_Miettinen">
        <rdf:type rdf:resource="http://www.semanticweb.org/macoda/ontologies/PMOEA#Researcher"/>
        <rdfs:label>Kaisa Miettinen</rdfs:label>
    </owl:NamedIndividual>
    


    <!-- http://www.semanticweb.org/macoda/ontologies/PMOEA#KanGAL -->

    <owl:NamedIndividual rdf:about="http://www.semanticweb.org/macoda/ontologies/PMOEA#KanGAL">
        <rdfs:label>KanGAL</rdfs:label>
    </owl:NamedIndividual>
    


    <!-- http://www.semanticweb.org/macoda/ontologies/PMOEA#Kaname_Narukawa -->

    <owl:NamedIndividual rdf:about="http://www.semanticweb.org/macoda/ontologies/PMOEA#Kaname_Narukawa">
        <rdf:type rdf:resource="http://www.semanticweb.org/macoda/ontologies/PMOEA#Researcher"/>
        <rdfs:label>Kaname Narukawa</rdfs:label>
    </owl:NamedIndividual>
    


    <!-- http://www.semanticweb.org/macoda/ontologies/PMOEA#Khaled_Ghdira -->

    <owl:NamedIndividual rdf:about="http://www.semanticweb.org/macoda/ontologies/PMOEA#Khaled_Ghdira">
        <rdf:type rdf:resource="http://www.semanticweb.org/macoda/ontologies/PMOEA#Researcher"/>
        <rdfs:label>Khaled Ghdira</rdfs:label>
    </owl:NamedIndividual>
    


    <!-- http://www.semanticweb.org/macoda/ontologies/PMOEA#Knapsack_9 -->

    <owl:NamedIndividual rdf:about="http://www.semanticweb.org/macoda/ontologies/PMOEA#Knapsack_9">
        <rdf:type rdf:resource="http://www.semanticweb.org/macoda/ontologies/PMOEA#Knapsack"/>
        <PMOEA:isDiscreteProblem rdf:datatype="http://www.w3.org/2001/XMLSchema#boolean">true</PMOEA:isDiscreteProblem>
        <PMOEA:ObjectiveNumber rdf:datatype="http://www.w3.org/2001/XMLSchema#integer">9</PMOEA:ObjectiveNumber>
        <PMOEA:isManyObjectiveProblem rdf:datatype="http://www.w3.org/2001/XMLSchema#boolean">true</PMOEA:isManyObjectiveProblem>
        <rdfs:label>knapsack_9</rdfs:label>
    </owl:NamedIndividual>
    


    <!-- http://www.semanticweb.org/macoda/ontologies/PMOEA#LBS-EMO -->

    <owl:NamedIndividual rdf:about="http://www.semanticweb.org/macoda/ontologies/PMOEA#LBS-EMO">
        <rdf:type rdf:resource="http://www.semanticweb.org/macoda/ontologies/PMOEA#PMOEA"/>
        <PMOEA:hasPreferenceModel rdf:resource="http://www.semanticweb.org/macoda/ontologies/PMOEA#LightBeamSearch"/>
        <PMOEA:hasPreferenceModel rdf:resource="http://www.semanticweb.org/macoda/ontologies/PMOEA#WierzbickiASF"/>
        <PMOEA:hasPreferenceInformationFromDM rdf:resource="http://www.semanticweb.org/macoda/ontologies/PMOEA#LBSParameters"/>
        <PMOEA:hasInteractionTime rdf:resource="http://www.semanticweb.org/macoda/ontologies/PMOEA#progressive"/>
        <PMOEA:hasPreferenceIntegration rdf:resource="http://www.semanticweb.org/macoda/ontologies/PMOEA#CrowdingDistance"/>
        <PMOEA:hasComparison rdf:resource="http://www.semanticweb.org/macoda/ontologies/PMOEA#RD-NSGA-II"/>
        <PMOEA:hasComparison rdf:resource="http://www.semanticweb.org/macoda/ontologies/PMOEA#R-NSGA-II"/>
        <PMOEA:canSolve rdf:resource="http://www.semanticweb.org/macoda/ontologies/PMOEA#DTLZ2_10"/>
        <PMOEA:canSolve rdf:resource="http://www.semanticweb.org/macoda/ontologies/PMOEA#KUR"/>
        <PMOEA:canSolve rdf:resource="http://www.semanticweb.org/macoda/ontologies/PMOEA#CarSideImpactProblem"/>
        <PMOEA:canSolve rdf:resource="http://www.semanticweb.org/macoda/ontologies/PMOEA#DTLZ2_5"/>
        <PMOEA:canSolve rdf:resource="http://www.semanticweb.org/macoda/ontologies/PMOEA#ZDT3"/>
        <PMOEA:canSolve rdf:resource="http://www.semanticweb.org/macoda/ontologies/PMOEA#DTLZ2_3"/>
        <PMOEA:canSolve rdf:resource="http://www.semanticweb.org/macoda/ontologies/PMOEA#ZDT1"/>
        <PMOEA:canSolve rdf:resource="http://www.semanticweb.org/macoda/ontologies/PMOEA#SpringDesignProblem"/>
        <PMOEA:canSolve rdf:resource="http://www.semanticweb.org/macoda/ontologies/PMOEA#WeldedBeamDesign"/>
        <PMOEA:hasResultInfluence rdf:resource="http://www.semanticweb.org/macoda/ontologies/PMOEA#BoundedRegion"/>
        <PMOEA:hasAuthor rdf:resource="http://www.semanticweb.org/macoda/ontologies/PMOEA#Abhay_Kumar"/>
        <PMOEA:hasAuthor rdf:resource="http://www.semanticweb.org/macoda/ontologies/PMOEA#Kalyanmoy_Deb"/>
        <PMOEA:hasSearchAlgorithm rdf:resource="http://www.semanticweb.org/macoda/ontologies/PMOEA#NSGA-II"/>
        <PMOEA:hasDevelopingYear rdf:datatype="http://www.w3.org/2001/XMLSchema#integer">2007</PMOEA:hasDevelopingYear>
        <PMOEA:hasRemarks>EMO in MCDM</PMOEA:hasRemarks>
        <PMOEA:MultipleRegionOfInterest rdf:datatype="http://www.w3.org/2001/XMLSchema#boolean">true</PMOEA:MultipleRegionOfInterest>
        <PMOEA:SpreadControl rdf:datatype="http://www.w3.org/2001/XMLSchema#boolean">true</PMOEA:SpreadControl>
        <PMOEA:ParetoDominancePreservation rdf:datatype="http://www.w3.org/2001/XMLSchema#boolean">true</PMOEA:ParetoDominancePreservation>
        <PMOEA:hasReference>Deb, K. and A. Kumar (2007). Light beam search based multi-objective optimization using evolutionary algorithms. Evolutionary Computation, 2007. CEC 2007. IEEE Congress on, IEEE</PMOEA:hasReference>
        <rdfs:comment>The light beam search uses a reference direction and additional thresholds which are then used to find some possibly interesting neighboring solutions around the most preferred solution. In this approach, the decision maker is asked to provide one or more pairs of aspiration and reservation points, the preference threshold vector and the  parameter used to control the density of the final identified solutions. The hybrid procedure has the ability to find the part of the Pareto optimal region illuminated by the light beam emanating from the starting point to the aspiration point with a span controlled by the veto threshold</rdfs:comment>
        <rdfs:label>LBS-EMO</rdfs:label>
    </owl:NamedIndividual>
    


    <!-- http://www.semanticweb.org/macoda/ontologies/PMOEA#Laura_Cruz-Reyes -->

    <owl:NamedIndividual rdf:about="http://www.semanticweb.org/macoda/ontologies/PMOEA#Laura_Cruz-Reyes">
        <rdf:type rdf:resource="http://www.semanticweb.org/macoda/ontologies/PMOEA#Researcher"/>
        <rdfs:label>Laura Cruz-Reyes</rdfs:label>
    </owl:NamedIndividual>
    


    <!-- http://www.semanticweb.org/macoda/ontologies/PMOEA#LeaderParticleSelection -->

    <owl:NamedIndividual rdf:about="http://www.semanticweb.org/macoda/ontologies/PMOEA#LeaderParticleSelection">
        <rdf:type rdf:resource="http://www.semanticweb.org/macoda/ontologies/PMOEA#LeaderSelection"/>
        <rdfs:comment>In particle swarm optimization</rdfs:comment>
        <rdfs:label>GlobalBestParticleSelection</rdfs:label>
    </owl:NamedIndividual>
    


    <!-- http://www.semanticweb.org/macoda/ontologies/PMOEA#LightBeamSearch -->

    <owl:NamedIndividual rdf:about="http://www.semanticweb.org/macoda/ontologies/PMOEA#LightBeamSearch">
        <rdf:type rdf:resource="http://www.semanticweb.org/macoda/ontologies/PMOEA#LightBeamSearch"/>
    </owl:NamedIndividual>
    


    <!-- http://www.semanticweb.org/macoda/ontologies/PMOEA#Lily_Rachmawati -->

    <owl:NamedIndividual rdf:about="http://www.semanticweb.org/macoda/ontologies/PMOEA#Lily_Rachmawati">
        <rdf:type rdf:resource="http://www.semanticweb.org/macoda/ontologies/PMOEA#Researcher"/>
        <rdfs:label>Lily Rachmawati</rdfs:label>
    </owl:NamedIndividual>
    


    <!-- http://www.semanticweb.org/macoda/ontologies/PMOEA#Luis_V._Santana -->

    <owl:NamedIndividual rdf:about="http://www.semanticweb.org/macoda/ontologies/PMOEA#Luis_V._Santana">
        <rdf:type rdf:resource="http://www.semanticweb.org/macoda/ontologies/PMOEA#Researcher"/>
        <rdfs:label>Luis V. Santana</rdfs:label>
    </owl:NamedIndividual>
    


    <!-- http://www.semanticweb.org/macoda/ontologies/PMOEA#Mariano_Luque -->

    <owl:NamedIndividual rdf:about="http://www.semanticweb.org/macoda/ontologies/PMOEA#Mariano_Luque">
        <rdf:type rdf:resource="http://www.semanticweb.org/macoda/ontologies/PMOEA#Researcher"/>
        <rdfs:label>Mariano Luque</rdfs:label>
    </owl:NamedIndividual>
    


    <!-- http://www.semanticweb.org/macoda/ontologies/PMOEA#Markus_Olhofer -->

    <owl:NamedIndividual rdf:about="http://www.semanticweb.org/macoda/ontologies/PMOEA#Markus_Olhofer">
        <rdf:type rdf:resource="http://www.semanticweb.org/macoda/ontologies/PMOEA#Researcher"/>
        <rdfs:label>Markus Olhofer</rdfs:label>
    </owl:NamedIndividual>
    


    <!-- http://www.semanticweb.org/macoda/ontologies/PMOEA#NOSGA -->

    <owl:NamedIndividual rdf:about="http://www.semanticweb.org/macoda/ontologies/PMOEA#NOSGA">
        <rdf:type rdf:resource="http://www.semanticweb.org/macoda/ontologies/PMOEA#PMOEA"/>
        <PMOEA:hasPreferenceModel rdf:resource="http://www.semanticweb.org/macoda/ontologies/PMOEA#ELECTRE"/>
        <PMOEA:hasPreferenceInformationFromDM rdf:resource="http://www.semanticweb.org/macoda/ontologies/PMOEA#ELECTREParameters"/>
        <PMOEA:hasInteractionTime rdf:resource="http://www.semanticweb.org/macoda/ontologies/PMOEA#a-priori"/>
        <PMOEA:hasPreferenceIntegration rdf:resource="http://www.semanticweb.org/macoda/ontologies/PMOEA#CrowdingDistance"/>
        <PMOEA:hasPreferenceIntegration rdf:resource="http://www.semanticweb.org/macoda/ontologies/PMOEA#FrontSorting"/>
        <PMOEA:canSolve rdf:resource="http://www.semanticweb.org/macoda/ontologies/PMOEA#ProjectPortfolioProblem_9"/>
        <PMOEA:hasResultInfluence rdf:resource="http://www.semanticweb.org/macoda/ontologies/PMOEA#SetOfSolutions"/>
        <PMOEA:hasAuthor rdf:resource="http://www.semanticweb.org/macoda/ontologies/PMOEA#Carlos_Coello_Coello"/>
        <PMOEA:hasAuthor rdf:resource="http://www.semanticweb.org/macoda/ontologies/PMOEA#Eduardo_Fernandez"/>
        <PMOEA:hasAuthor rdf:resource="http://www.semanticweb.org/macoda/ontologies/PMOEA#Edy_Lopez"/>
        <PMOEA:hasAuthor rdf:resource="http://www.semanticweb.org/macoda/ontologies/PMOEA#Jorge_Navarro"/>
        <PMOEA:hasAuthor rdf:resource="http://www.semanticweb.org/macoda/ontologies/PMOEA#Sergio_Bernal"/>
        <PMOEA:hasExtension rdf:resource="http://www.semanticweb.org/macoda/ontologies/PMOEA#NOSGA-II"/>
        <PMOEA:hasSearchAlgorithm rdf:resource="http://www.semanticweb.org/macoda/ontologies/PMOEA#NSGA-II"/>
        <PMOEA:hasImplementationLanguage rdf:resource="http://www.semanticweb.org/macoda/ontologies/PMOEA#C++"/>
        <PMOEA:hasDevelopingYear rdf:datatype="http://www.w3.org/2001/XMLSchema#integer">2010</PMOEA:hasDevelopingYear>
        <PMOEA:hasReference>Fernandez, E., E. Lopez, S. Bernal, C. A. C. Coello and J. Navarro (2010). &quot;Evolutionary multiobjective optimization using an outranking-based dominance generalization.&quot; Computers &amp; Operations Research 37(2): 390-395.</PMOEA:hasReference>
        <rdfs:comment>The proposal is based on finding a subset of the Pareto frontier composed of solutions for which no other solutions strictly outrank them. This non-outranked concept will be used instead of dominance when performing the evolutionary search.</rdfs:comment>
        <rdfs:label>NOSGA</rdfs:label>
    </owl:NamedIndividual>
    


    <!-- http://www.semanticweb.org/macoda/ontologies/PMOEA#NOSGA-II -->

    <owl:NamedIndividual rdf:about="http://www.semanticweb.org/macoda/ontologies/PMOEA#NOSGA-II">
        <rdf:type rdf:resource="http://www.semanticweb.org/macoda/ontologies/PMOEA#PMOEA"/>
        <PMOEA:hasPreferenceModel rdf:resource="http://www.semanticweb.org/macoda/ontologies/PMOEA#ELECTRE"/>
        <PMOEA:hasPreferenceInformationFromDM rdf:resource="http://www.semanticweb.org/macoda/ontologies/PMOEA#ELECTREParameters"/>
        <PMOEA:hasInteractionTime rdf:resource="http://www.semanticweb.org/macoda/ontologies/PMOEA#a-priori"/>
        <PMOEA:hasPreferenceIntegration rdf:resource="http://www.semanticweb.org/macoda/ontologies/PMOEA#CrowdingDistance"/>
        <PMOEA:hasPreferenceIntegration rdf:resource="http://www.semanticweb.org/macoda/ontologies/PMOEA#FrontSorting"/>
        <PMOEA:canSolve rdf:resource="http://www.semanticweb.org/macoda/ontologies/PMOEA#ProjectPortfolioProblem_9"/>
        <PMOEA:hasResultInfluence rdf:resource="http://www.semanticweb.org/macoda/ontologies/PMOEA#BoundedRegion"/>
        <PMOEA:hasAuthor rdf:resource="http://www.semanticweb.org/macoda/ontologies/PMOEA#Carlos_Coello_Coello"/>
        <PMOEA:hasAuthor rdf:resource="http://www.semanticweb.org/macoda/ontologies/PMOEA#Eduardo_Fernandez"/>
        <PMOEA:hasAuthor rdf:resource="http://www.semanticweb.org/macoda/ontologies/PMOEA#Edy_Lopez"/>
        <PMOEA:hasAuthor rdf:resource="http://www.semanticweb.org/macoda/ontologies/PMOEA#Fernando_Lopez,"/>
        <PMOEA:hasSearchAlgorithm rdf:resource="http://www.semanticweb.org/macoda/ontologies/PMOEA#NSGA-II"/>
        <PMOEA:hasDevelopingYear rdf:datatype="http://www.w3.org/2001/XMLSchema#integer">2011</PMOEA:hasDevelopingYear>
        <PMOEA:hasRemarks>compared to NOSGA, the preference model is more complex here, which considers best compromise solution</PMOEA:hasRemarks>
        <PMOEA:hasReference>Fernandez, E., E. Lopez, F. Lopez and C. A. C. Coello (2011). &quot;Increasing selective pressure towards the best compromise in evolutionary multiobjective optimization: The extended NOSGA method.&quot; Information Sciences 181(1): 44-56</PMOEA:hasReference>
        <rdfs:comment>Compared to NSGA, the model of DMs preferences is better than before, and a good theoretical characterization of the best compromise solution is achieved. Using this characterization, we improve convergence to a privileged zone on the Pareto frontier. This makes easier the solution of problems with many objectives.</rdfs:comment>
        <rdfs:label>NOSGA-II</rdfs:label>
    </owl:NamedIndividual>
    


    <!-- http://www.semanticweb.org/macoda/ontologies/PMOEA#ExponentialFunctionPreferOneObjective -->

    <owl:NamedIndividual rdf:about="http://www.semanticweb.org/macoda/ontologies/PMOEA#ExponentialFunctionPreferOneObjective">
        <rdf:type rdf:resource="http://www.semanticweb.org/macoda/ontologies/PMOEA#DistributionFunctionInObjectiveSpace"/>
        <rdfs:label xml:lang="en">ExponentialFunctionPreferOneObjective</rdfs:label>
    </owl:NamedIndividual>
    


    <!-- http://www.semanticweb.org/macoda/ontologies/PMOEA#DTLZ3_8 -->

    <owl:NamedIndividual rdf:about="http://www.semanticweb.org/macoda/ontologies/PMOEA#DTLZ3_8">
        <rdf:type rdf:resource="http://www.semanticweb.org/macoda/ontologies/PMOEA#DTLZ"/>
        <PMOEA:OWLDataProperty_61d3cd95_fde4_4c1b_af08_1eaf73473aea rdf:datatype="http://www.w3.org/2001/XMLSchema#boolean">true</PMOEA:OWLDataProperty_61d3cd95_fde4_4c1b_af08_1eaf73473aea>
        <PMOEA:isContinuousProblem rdf:datatype="http://www.w3.org/2001/XMLSchema#boolean">true</PMOEA:isContinuousProblem>
        <PMOEA:ObjectiveNumber rdf:datatype="http://www.w3.org/2001/XMLSchema#integer">8</PMOEA:ObjectiveNumber>
        <PMOEA:isManyObjectiveProblem rdf:datatype="http://www.w3.org/2001/XMLSchema#boolean">true</PMOEA:isManyObjectiveProblem>
        <rdfs:label xml:lang="en">DTLZ3_8</rdfs:label>
    </owl:NamedIndividual>
    


    <!-- http://www.semanticweb.org/macoda/ontologies/PMOEA#WierzbickiASF -->

    <owl:NamedIndividual rdf:about="http://www.semanticweb.org/macoda/ontologies/PMOEA#WierzbickiASF">
        <rdf:type rdf:resource="http://www.semanticweb.org/macoda/ontologies/PMOEA#AchievementScalarizingFunction"/>
        <rdfs:comment>Tchebycheff with augmentation part</rdfs:comment>
        <rdfs:label xml:lang="en">WierzbickiASF</rdfs:label>
    </owl:NamedIndividual>
    


    <!-- http://www.semanticweb.org/macoda/ontologies/PMOEA#NEMO-II -->

    <owl:NamedIndividual rdf:about="http://www.semanticweb.org/macoda/ontologies/PMOEA#NEMO-II">
        <rdf:type rdf:resource="http://www.semanticweb.org/macoda/ontologies/PMOEA#PMOEA"/>
        <PMOEA:hasPreferenceModel rdf:resource="http://www.semanticweb.org/macoda/ontologies/PMOEA#ChoquetIntegral"/>
        <PMOEA:hasPreferenceModel rdf:resource="http://www.semanticweb.org/macoda/ontologies/PMOEA#LinearUtilityFunction"/>
        <PMOEA:hasPreferenceModel rdf:resource="http://www.semanticweb.org/macoda/ontologies/PMOEA#AdditivePiecewiseLinear"/>
        <PMOEA:hasPreferenceModel rdf:resource="http://www.semanticweb.org/macoda/ontologies/PMOEA#GeneralAdditiveUtilityFunction"/>
        <PMOEA:hasPreferenceInformationFromDM rdf:resource="http://www.semanticweb.org/macoda/ontologies/PMOEA#PairwiseComparison"/>
        <PMOEA:hasInteractionTime rdf:resource="http://www.semanticweb.org/macoda/ontologies/PMOEA#progressive"/>
        <PMOEA:hasPreferenceIntegration rdf:resource="http://www.semanticweb.org/macoda/ontologies/PMOEA#FrontSorting"/>
        <PMOEA:hasLearningMethod rdf:resource="http://www.semanticweb.org/macoda/ontologies/PMOEA#RobustOrdinalRegression"/>
        <PMOEA:canSolve rdf:resource="http://www.semanticweb.org/macoda/ontologies/PMOEA#DTLZ1_5"/>
        <PMOEA:canSolve rdf:resource="http://www.semanticweb.org/macoda/ontologies/PMOEA#ZDT2"/>
        <PMOEA:canSolve rdf:resource="http://www.semanticweb.org/macoda/ontologies/PMOEA#DTLZ2_5"/>
        <PMOEA:canSolve rdf:resource="http://www.semanticweb.org/macoda/ontologies/PMOEA#DTLZ1_3"/>
        <PMOEA:canSolve rdf:resource="http://www.semanticweb.org/macoda/ontologies/PMOEA#DTLZ2_3"/>
        <PMOEA:canSolve rdf:resource="http://www.semanticweb.org/macoda/ontologies/PMOEA#ZDT1"/>
        <PMOEA:hasResultInfluence rdf:resource="http://www.semanticweb.org/macoda/ontologies/PMOEA#BiasedDistribution"/>
        <PMOEA:hasAuthor rdf:resource="http://www.semanticweb.org/macoda/ontologies/PMOEA#Piotr_Zielniewicz"/>
        <PMOEA:hasAuthor rdf:resource="http://www.semanticweb.org/macoda/ontologies/PMOEA#Salvatore_Greco
"/>
        <PMOEA:hasAuthor rdf:resource="http://www.semanticweb.org/macoda/ontologies/PMOEA#Salvatore_Corrente"/>
        <PMOEA:hasAuthor rdf:resource="http://www.semanticweb.org/macoda/ontologies/PMOEA#Juergen_Branke"/>
        <PMOEA:hasAuthor rdf:resource="http://www.semanticweb.org/macoda/ontologies/PMOEA#Roman_Sowinski"/>
        <PMOEA:isExtensionOf rdf:resource="http://www.semanticweb.org/macoda/ontologies/PMOEA#NEMO-I"/>
        <PMOEA:hasSearchAlgorithm rdf:resource="http://www.semanticweb.org/macoda/ontologies/PMOEA#NSGA-II"/>
        <PMOEA:hasDevelopingYear rdf:datatype="http://www.w3.org/2001/XMLSchema#integer">2014</PMOEA:hasDevelopingYear>
        <PMOEA:ParetoDominancePreservation rdf:datatype="http://www.w3.org/2001/XMLSchema#boolean">true</PMOEA:ParetoDominancePreservation>
        <PMOEA:hasReference>Branke, Juergen, Corrente, Salvatore, Greco, Salvatore, Slowinski, Roman and
Zielniewicz, Piotr (2014) Using Choquet integral as preference model in interactive
evolutionary multiobjective optimization. Working Paper. Coventry, UK: WBS, University of Warwick. WBS working papers</PMOEA:hasReference>
        <rdfs:comment>NEMO-I has shown a satisfactory convergence to the best compromise solution, the calculation of the necessary preference relation requires a considerable computational effort. For this reason, in this paper, we are using an alternative method called NEMO-II, which overcomes the problem of prohibitive computational effort. NEMO-II accepts any type of value function. We are considering four types of value functions within NEMO-II: linear, additive piecewise-linear, general additive, and (for the first time in combination with evolutionary multiobjective algorithms) the Choquet integral</rdfs:comment>
        <rdfs:label xml:lang="en">NEMO-II</rdfs:label>
    </owl:NamedIndividual>
    


    <!-- http://www.semanticweb.org/macoda/ontologies/PMOEA#Maoguo_Gong -->

    <owl:NamedIndividual rdf:about="http://www.semanticweb.org/macoda/ontologies/PMOEA#Maoguo_Gong">
        <rdf:type rdf:resource="http://www.semanticweb.org/macoda/ontologies/PMOEA#Researcher"/>
        <rdfs:label xml:lang="en">Maoguo Gong</rdfs:label>
    </owl:NamedIndividual>
    


    <!-- http://www.semanticweb.org/macoda/ontologies/PMOEA#BipolarReferencePoint -->

    <owl:NamedIndividual rdf:about="http://www.semanticweb.org/macoda/ontologies/PMOEA#BipolarReferencePoint">
        <rdf:type rdf:resource="http://www.semanticweb.org/macoda/ontologies/PMOEA#ReferencePoint"/>
        <rdfs:comment>positive and negative reference points indicating the most and least preferred solution</rdfs:comment>
        <rdfs:label xml:lang="en">BipolarReferencePoint</rdfs:label>
    </owl:NamedIndividual>
    


    <!-- http://www.semanticweb.org/macoda/ontologies/PMOEA#PicktheBestandWorst -->

    <owl:NamedIndividual rdf:about="http://www.semanticweb.org/macoda/ontologies/PMOEA#PicktheBestandWorst">
        <rdf:type rdf:resource="http://www.semanticweb.org/macoda/ontologies/PMOEA#SampleRanks"/>
        <rdfs:label xml:lang="en">PicktheBestandWorst</rdfs:label>
    </owl:NamedIndividual>
    


    <!-- http://www.semanticweb.org/macoda/ontologies/PMOEA#LZ09_F6 -->

    <owl:NamedIndividual rdf:about="http://www.semanticweb.org/macoda/ontologies/PMOEA#LZ09_F6">
        <rdf:type rdf:resource="http://www.semanticweb.org/macoda/ontologies/PMOEA#Academic_Problem"/>
        <PMOEA:isContinuousProblem rdf:datatype="http://www.w3.org/2001/XMLSchema#boolean">true</PMOEA:isContinuousProblem>
        <PMOEA:ObjectiveNumber rdf:datatype="http://www.w3.org/2001/XMLSchema#integer">3</PMOEA:ObjectiveNumber>
        <rdfs:label xml:lang="en">LZ09_F6</rdfs:label>
    </owl:NamedIndividual>
    


    <!-- http://www.semanticweb.org/macoda/ontologies/PMOEA#Piotr_Zielniewicz -->

    <owl:NamedIndividual rdf:about="http://www.semanticweb.org/macoda/ontologies/PMOEA#Piotr_Zielniewicz">
        <rdf:type rdf:resource="http://www.semanticweb.org/macoda/ontologies/PMOEA#Researcher"/>
        <rdfs:label xml:lang="en">Piotr Zielniewicz</rdfs:label>
    </owl:NamedIndividual>
    


    <!-- http://www.semanticweb.org/macoda/ontologies/PMOEA#Ian_C_Parmee -->

    <owl:NamedIndividual rdf:about="http://www.semanticweb.org/macoda/ontologies/PMOEA#Ian_C_Parmee">
        <rdf:type rdf:resource="http://www.semanticweb.org/macoda/ontologies/PMOEA#Researcher"/>
        <rdfs:label xml:lang="en">Ian C. Parmee</rdfs:label>
    </owl:NamedIndividual>
    


    <!-- http://www.semanticweb.org/macoda/ontologies/PMOEA#Karthik_Sindhya -->

    <owl:NamedIndividual rdf:about="http://www.semanticweb.org/macoda/ontologies/PMOEA#Karthik_Sindhya">
        <rdf:type rdf:resource="http://www.semanticweb.org/macoda/ontologies/PMOEA#Researcher"/>
        <rdfs:label xml:lang="en">Karthik Sindhya</rdfs:label>
    </owl:NamedIndividual>
    


    <!-- http://www.semanticweb.org/macoda/ontologies/PMOEA#POGA -->

    <owl:NamedIndividual rdf:about="http://www.semanticweb.org/macoda/ontologies/PMOEA#POGA">
        <rdf:type rdf:resource="http://www.semanticweb.org/macoda/ontologies/PMOEA#PMOEA"/>
        <PMOEA:hasInteractionTime rdf:resource="http://www.semanticweb.org/macoda/ontologies/PMOEA#a-priori"/>
        <PMOEA:hasPreferenceIntegration rdf:resource="http://www.semanticweb.org/macoda/ontologies/PMOEA#FitnessSetting"/>
        <PMOEA:canSolve rdf:resource="http://www.semanticweb.org/macoda/ontologies/PMOEA#DTLZ3_8"/>
        <PMOEA:canSolve rdf:resource="http://www.semanticweb.org/macoda/ontologies/PMOEA#DTLZ6_8"/>
        <PMOEA:canSolve rdf:resource="http://www.semanticweb.org/macoda/ontologies/PMOEA#DTLZ5_8"/>
        <PMOEA:canSolve rdf:resource="http://www.semanticweb.org/macoda/ontologies/PMOEA#DTLZ7_8"/>
        <PMOEA:canSolve rdf:resource="http://www.semanticweb.org/macoda/ontologies/PMOEA#DTLZ1_4"/>
        <PMOEA:canSolve rdf:resource="http://www.semanticweb.org/macoda/ontologies/PMOEA#DTLZ1_8"/>
        <PMOEA:canSolve rdf:resource="http://www.semanticweb.org/macoda/ontologies/PMOEA#DTLZ4_8"/>
        <PMOEA:canSolve rdf:resource="http://www.semanticweb.org/macoda/ontologies/PMOEA#DTLZ2_8"/>
        <PMOEA:hasResultInfluence rdf:resource="http://www.semanticweb.org/macoda/ontologies/PMOEA#SetOfSolutions"/>
        <PMOEA:hasAuthor rdf:resource="http://www.semanticweb.org/macoda/ontologies/PMOEA#Dragan_A_Savic"/>
        <PMOEA:hasAuthor rdf:resource="http://www.semanticweb.org/macoda/ontologies/PMOEA#Francesco_di_Pierro"/>
        <PMOEA:hasAuthor rdf:resource="http://www.semanticweb.org/macoda/ontologies/PMOEA#Soon-Thiam_Khu"/>
        <PMOEA:hasSearchAlgorithm rdf:resource="http://www.semanticweb.org/macoda/ontologies/PMOEA#NSGA-II"/>
        <PMOEA:hasDevelopingYear rdf:datatype="http://www.w3.org/2001/XMLSchema#integer">2007</PMOEA:hasDevelopingYear>
        <PMOEA:ParetoDominancePreservation rdf:datatype="http://www.w3.org/2001/XMLSchema#boolean">true</PMOEA:ParetoDominancePreservation>
        <PMOEA:hasReference>Di Pierro, Francesco, Soon-Thiam Khu, and Dragan A. Savic. &quot;An investigation on preference order ranking scheme for multiobjective evolutionary optimization.&quot; Evolutionary Computation, IEEE Transactions on 11.1 (2007): 17-45.</PMOEA:hasReference>
        <rdfs:comment>A ranking procedure that exploits the definition of preference ordering (PO) is proposed, along with two strategies that make different use of the conditions of efficiency provided, and it is compared with a more traditional Pareto dominance-based ranking scheme within the framework of NSGA-II</rdfs:comment>
        <rdfs:label xml:lang="en">POGA</rdfs:label>
    </owl:NamedIndividual>
    


    <!-- http://www.semanticweb.org/macoda/ontologies/PMOEA#WFG4_6 -->

    <owl:NamedIndividual rdf:about="http://www.semanticweb.org/macoda/ontologies/PMOEA#WFG4_6">
        <rdf:type rdf:resource="http://www.semanticweb.org/macoda/ontologies/PMOEA#WFG"/>
        <PMOEA:OWLDataProperty_61d3cd95_fde4_4c1b_af08_1eaf73473aea rdf:datatype="http://www.w3.org/2001/XMLSchema#boolean">true</PMOEA:OWLDataProperty_61d3cd95_fde4_4c1b_af08_1eaf73473aea>
        <PMOEA:isContinuousProblem rdf:datatype="http://www.w3.org/2001/XMLSchema#boolean">true</PMOEA:isContinuousProblem>
        <PMOEA:ObjectiveNumber rdf:datatype="http://www.w3.org/2001/XMLSchema#integer">6</PMOEA:ObjectiveNumber>
        <PMOEA:isManyObjectiveProblem rdf:datatype="http://www.w3.org/2001/XMLSchema#boolean">true</PMOEA:isManyObjectiveProblem>
        <rdfs:label xml:lang="en">WFG4_6</rdfs:label>
    </owl:NamedIndividual>
    


    <!-- http://www.semanticweb.org/macoda/ontologies/PMOEA#WFG2_7 -->

    <owl:NamedIndividual rdf:about="http://www.semanticweb.org/macoda/ontologies/PMOEA#WFG2_7">
        <rdf:type rdf:resource="http://www.semanticweb.org/macoda/ontologies/PMOEA#WFG"/>
        <PMOEA:isContinuousProblem rdf:datatype="http://www.w3.org/2001/XMLSchema#boolean">true</PMOEA:isContinuousProblem>
        <PMOEA:ObjectiveNumber rdf:datatype="http://www.w3.org/2001/XMLSchema#integer">7</PMOEA:ObjectiveNumber>
        <PMOEA:isManyObjectiveProblem rdf:datatype="http://www.w3.org/2001/XMLSchema#boolean">true</PMOEA:isManyObjectiveProblem>
        <rdfs:label xml:lang="en">WFG2_7</rdfs:label>
    </owl:NamedIndividual>
    


    <!-- http://www.semanticweb.org/macoda/ontologies/PMOEA#W_HypE -->

    <owl:NamedIndividual rdf:about="http://www.semanticweb.org/macoda/ontologies/PMOEA#W_HypE">
        <rdf:type rdf:resource="http://www.semanticweb.org/macoda/ontologies/PMOEA#PMOEA"/>
        <PMOEA:hasPreferenceModel rdf:resource="http://www.semanticweb.org/macoda/ontologies/PMOEA#ObjectiveSpaceWeightDistribution"/>
        <PMOEA:hasPreferenceInformationFromDM rdf:resource="http://www.semanticweb.org/macoda/ontologies/PMOEA#ExponentialFunctionPreferOneObjective"/>
        <PMOEA:hasPreferenceInformationFromDM rdf:resource="http://www.semanticweb.org/macoda/ontologies/PMOEA#GaussianFunctionPreferOneRP"/>
        <PMOEA:hasPreferenceInformationFromDM rdf:resource="http://www.semanticweb.org/macoda/ontologies/PMOEA#UniformDistributionPreferRegion"/>
        <PMOEA:hasPreferenceInformationFromDM rdf:resource="http://www.semanticweb.org/macoda/ontologies/PMOEA#Dirac-typeFunction"/>
        <PMOEA:hasInteractionTime rdf:resource="http://www.semanticweb.org/macoda/ontologies/PMOEA#a-priori"/>
        <PMOEA:hasPreferenceIntegration rdf:resource="http://www.semanticweb.org/macoda/ontologies/PMOEA#HypervolumeIndicator"/>
        <PMOEA:canSolve rdf:resource="http://www.semanticweb.org/macoda/ontologies/PMOEA#Knapsack_2"/>
        <PMOEA:canSolve rdf:resource="http://www.semanticweb.org/macoda/ontologies/PMOEA#DTLZ2_7"/>
        <PMOEA:canSolve rdf:resource="http://www.semanticweb.org/macoda/ontologies/PMOEA#DTLZ2_3"/>
        <PMOEA:canSolve rdf:resource="http://www.semanticweb.org/macoda/ontologies/PMOEA#ZDT1"/>
        <PMOEA:hasResultInfluence rdf:resource="http://www.semanticweb.org/macoda/ontologies/PMOEA#BiasedDistribution"/>
        <PMOEA:hasAuthor rdf:resource="http://www.semanticweb.org/macoda/ontologies/PMOEA#Johannes Bader"/>
        <PMOEA:hasAuthor rdf:resource="http://www.semanticweb.org/macoda/ontologies/PMOEA#Lothar_Thiele"/>
        <PMOEA:hasAuthor rdf:resource="http://www.semanticweb.org/macoda/ontologies/PMOEA#Dimo_Brockhoff"/>
        <PMOEA:hasAuthor rdf:resource="http://www.semanticweb.org/macoda/ontologies/PMOEA#Eckart_Zitzler"/>
        <PMOEA:isExtensionOf rdf:resource="http://www.semanticweb.org/macoda/ontologies/PMOEA#W_HypE"/>
        <PMOEA:hasSearchAlgorithm rdf:resource="http://www.semanticweb.org/macoda/ontologies/PMOEA#HypE"/>
        <PMOEA:hasImplementationLanguage rdf:resource="http://www.semanticweb.org/macoda/ontologies/PMOEA#Matlab"/>
        <PMOEA:hasDevelopingYear rdf:datatype="http://www.w3.org/2001/XMLSchema#integer">2013</PMOEA:hasDevelopingYear>
        <PMOEA:MultipleRegionOfInterest rdf:datatype="http://www.w3.org/2001/XMLSchema#boolean">true</PMOEA:MultipleRegionOfInterest>
        <PMOEA:SpreadControl rdf:datatype="http://www.w3.org/2001/XMLSchema#boolean">true</PMOEA:SpreadControl>
        <PMOEA:hasReference>Brockhoff, D., et al. (2013). &quot;Directed Multiobjective Optimization Based on the Weighted Hypervolume Indicator.&quot; Journal of Multi-Criteria Decision Analysis 20(5-6): 291-317</PMOEA:hasReference>
        <rdfs:comment>The present paper contains the necessary theoretical foundations and corresponding algorithms to (i) select appropriate weight functions, to (ii) transform user preferences into weight functions and to (iii) efficiently evaluate the weighted hypervolume indicator through Monte Carlo sampling. The algorithm W-HypE, which implements the previous concepts, is introduced, and the effectiveness of the search, directed towards the user&apos;s preferred solutions, is shown using an extensive set of experiments including the necessary statistical performance assessment.</rdfs:comment>
        <rdfs:label xml:lang="en">W_HypE</rdfs:label>
    </owl:NamedIndividual>
    


    <!-- http://www.semanticweb.org/macoda/ontologies/PMOEA#Knapsack_2 -->

    <owl:NamedIndividual rdf:about="http://www.semanticweb.org/macoda/ontologies/PMOEA#Knapsack_2">
        <rdf:type rdf:resource="http://www.semanticweb.org/macoda/ontologies/PMOEA#Knapsack"/>
        <PMOEA:isDiscreteProblem rdf:datatype="http://www.w3.org/2001/XMLSchema#boolean">true</PMOEA:isDiscreteProblem>
        <PMOEA:OWLDataProperty_61d3cd95_fde4_4c1b_af08_1eaf73473aea rdf:datatype="http://www.w3.org/2001/XMLSchema#boolean">false</PMOEA:OWLDataProperty_61d3cd95_fde4_4c1b_af08_1eaf73473aea>
        <PMOEA:isContinuousProblem rdf:datatype="http://www.w3.org/2001/XMLSchema#boolean">false</PMOEA:isContinuousProblem>
        <PMOEA:ObjectiveNumber rdf:datatype="http://www.w3.org/2001/XMLSchema#integer">2</PMOEA:ObjectiveNumber>
        <PMOEA:isManyObjectiveProblem rdf:datatype="http://www.w3.org/2001/XMLSchema#boolean">false</PMOEA:isManyObjectiveProblem>
        <rdfs:label xml:lang="en">Knapsack_2</rdfs:label>
    </owl:NamedIndividual>
    


    <!-- http://www.semanticweb.org/macoda/ontologies/PMOEA#IBEA -->

    <owl:NamedIndividual rdf:about="http://www.semanticweb.org/macoda/ontologies/PMOEA#IBEA">
        <rdf:type rdf:resource="http://www.semanticweb.org/macoda/ontologies/PMOEA#Indicator_based"/>
        <rdfs:label xml:lang="en">IBEA</rdfs:label>
    </owl:NamedIndividual>
    


    <!-- http://www.semanticweb.org/macoda/ontologies/PMOEA#PolyhedralCone-dominance -->

    <owl:NamedIndividual rdf:about="http://www.semanticweb.org/macoda/ontologies/PMOEA#PolyhedralCone-dominance">
        <rdf:type rdf:resource="http://www.semanticweb.org/macoda/ontologies/PMOEA#DominanceRelation"/>
        <rdfs:comment>The cone-based dominance in PI-EMO-PC, if for both solutions Pi(f1,...fM)&gt;0 for all i, or  Pi(f1,...fM)&lt;0 for at least one i, then two points are compared based on usual dominance principle. If one solution has  Pi(f1,...fM)&gt;0 for all i, the other has Pi(f1,...fM)&lt;0 for at least one i, then the former dominates the latter.</rdfs:comment>
        <rdfs:label xml:lang="en">PolyhedralCone-dominance</rdfs:label>
    </owl:NamedIndividual>
    


    <!-- http://www.semanticweb.org/macoda/ontologies/PMOEA#Deb1999 -->

    <owl:NamedIndividual rdf:about="http://www.semanticweb.org/macoda/ontologies/PMOEA#Deb1999">
        <rdf:type rdf:resource="http://www.semanticweb.org/macoda/ontologies/PMOEA#Academic_Problem"/>
        <PMOEA:isContinuousProblem rdf:datatype="http://www.w3.org/2001/XMLSchema#boolean">true</PMOEA:isContinuousProblem>
        <PMOEA:ObjectiveNumber rdf:datatype="http://www.w3.org/2001/XMLSchema#integer">2</PMOEA:ObjectiveNumber>
        <rdfs:comment>Deb, K. (1999). Evolutionary algorithms for multi-criterion optimization in engineering design. In
Miettinen. Evolutionary Algorithms in Engineering and Computer science: Recent Advances in
Genetic Algorithms, Evolution Strategies, Evolutionary Programming, Genetic Programming, and
Industrial Applications, Wiley, New York, 135-161.</rdfs:comment>
        <rdfs:label xml:lang="en">Deb1999</rdfs:label>
    </owl:NamedIndividual>
    


    <!-- http://www.semanticweb.org/macoda/ontologies/PMOEA#Matlab -->

    <owl:NamedIndividual rdf:about="http://www.semanticweb.org/macoda/ontologies/PMOEA#Matlab">
        <rdf:type rdf:resource="http://www.semanticweb.org/macoda/ontologies/PMOEA#ProgrammingLanguage"/>
        <rdfs:label xml:lang="en">Matlab</rdfs:label>
    </owl:NamedIndividual>
    


    <!-- http://www.semanticweb.org/macoda/ontologies/PMOEA#Andre_Deutz -->

    <owl:NamedIndividual rdf:about="http://www.semanticweb.org/macoda/ontologies/PMOEA#Andre_Deutz">
        <rdf:type rdf:resource="http://www.semanticweb.org/macoda/ontologies/PMOEA#Researcher"/>
        <rdfs:label xml:lang="en">Andre_Deutz</rdfs:label>
    </owl:NamedIndividual>
    


    <!-- http://www.semanticweb.org/macoda/ontologies/PMOEA#DTLZ9_5 -->

    <owl:NamedIndividual rdf:about="http://www.semanticweb.org/macoda/ontologies/PMOEA#DTLZ9_5">
        <rdf:type rdf:resource="http://www.semanticweb.org/macoda/ontologies/PMOEA#DTLZ"/>
        <PMOEA:isContinuousProblem rdf:datatype="http://www.w3.org/2001/XMLSchema#boolean">true</PMOEA:isContinuousProblem>
        <PMOEA:ObjectiveNumber rdf:datatype="http://www.w3.org/2001/XMLSchema#integer">5</PMOEA:ObjectiveNumber>
        <PMOEA:isManyObjectiveProblem rdf:datatype="http://www.w3.org/2001/XMLSchema#boolean">true</PMOEA:isManyObjectiveProblem>
        <rdfs:label xml:lang="en">DTLZ9_5</rdfs:label>
    </owl:NamedIndividual>
    


    <!-- http://www.semanticweb.org/macoda/ontologies/PMOEA#parametersInDF -->

    <owl:NamedIndividual rdf:about="http://www.semanticweb.org/macoda/ontologies/PMOEA#parametersInDF">
        <rdf:type rdf:resource="http://www.semanticweb.org/macoda/ontologies/PMOEA#DesirabilityFunction"/>
        <rdfs:label xml:lang="en">parametersInDF</rdfs:label>
    </owl:NamedIndividual>
    


    <!-- http://www.semanticweb.org/macoda/ontologies/PMOEA#AspirationSet -->

    <owl:NamedIndividual rdf:about="http://www.semanticweb.org/macoda/ontologies/PMOEA#AspirationSet">
        <rdf:type rdf:resource="http://www.semanticweb.org/macoda/ontologies/PMOEA#ReferencePoint"/>
        <rdfs:comment>a set of aspiration points, used in AS-EMOA</rdfs:comment>
        <rdfs:label xml:lang="en">AspirationSet</rdfs:label>
    </owl:NamedIndividual>
    


    <!-- http://www.semanticweb.org/macoda/ontologies/PMOEA#MOPSO -->

    <owl:NamedIndividual rdf:about="http://www.semanticweb.org/macoda/ontologies/PMOEA#MOPSO">
        <rdf:type rdf:resource="http://www.semanticweb.org/macoda/ontologies/PMOEA#PSO_based"/>
        <rdfs:label xml:lang="en">MOPSO</rdfs:label>
    </owl:NamedIndividual>
    


    <!-- http://www.semanticweb.org/macoda/ontologies/PMOEA#TEHVI -->

    <owl:NamedIndividual rdf:about="http://www.semanticweb.org/macoda/ontologies/PMOEA#TEHVI">
        <rdf:type rdf:resource="http://www.semanticweb.org/macoda/ontologies/PMOEA#PMOEA"/>
        <PMOEA:hasPreferenceModel rdf:resource="http://www.semanticweb.org/macoda/ontologies/PMOEA#PreferenceRegionModel"/>
        <PMOEA:hasPreferenceInformationFromDM rdf:resource="http://www.semanticweb.org/macoda/ontologies/PMOEA#RectangleRegion"/>
        <PMOEA:hasInteractionTime rdf:resource="http://www.semanticweb.org/macoda/ontologies/PMOEA#progressive"/>
        <PMOEA:hasPreferenceIntegration rdf:resource="http://www.semanticweb.org/macoda/ontologies/PMOEA#HypervolumeIndicator"/>
        <PMOEA:canSolve rdf:resource="http://www.semanticweb.org/macoda/ontologies/PMOEA#ZDT2"/>
        <PMOEA:canSolve rdf:resource="http://www.semanticweb.org/macoda/ontologies/PMOEA#GSP_2"/>
        <PMOEA:canSolve rdf:resource="http://www.semanticweb.org/macoda/ontologies/PMOEA#ZDT1"/>
        <PMOEA:hasResultInfluence rdf:resource="http://www.semanticweb.org/macoda/ontologies/PMOEA#BoundedRegion"/>
        <PMOEA:hasAuthor rdf:resource="http://www.semanticweb.org/macoda/ontologies/PMOEA#Andre_Deutz"/>
        <PMOEA:hasAuthor rdf:resource="http://www.semanticweb.org/macoda/ontologies/PMOEA#Kaifeng_Yang"/>
        <PMOEA:hasAuthor rdf:resource="http://www.semanticweb.org/macoda/ontologies/PMOEA#Thomas_Baeck"/>
        <PMOEA:hasAuthor rdf:resource="http://www.semanticweb.org/macoda/ontologies/PMOEA#Michael_Emmerich"/>
        <PMOEA:hasAuthor rdf:resource="http://www.semanticweb.org/macoda/ontologies/PMOEA#Longmei_Li"/>
        <PMOEA:hasSearchAlgorithm rdf:resource="http://www.semanticweb.org/macoda/ontologies/PMOEA#EHVI-EGO"/>
        <PMOEA:hasImplementationLanguage rdf:resource="http://www.semanticweb.org/macoda/ontologies/PMOEA#Matlab"/>
        <PMOEA:hasDevelopingYear rdf:datatype="http://www.w3.org/2001/XMLSchema#integer">2016</PMOEA:hasDevelopingYear>
        <rdfs:comment>In this paper, a method for effectively approximating a preferred Pareto front, based on multiobjective efficient global optimization (EGO), is introduced. EGO uses Gaussian processes (or Kriging) to build a model of the objective function and uses truncated expected hypervolume improvement (TEHVI) as an infill criterion, which takes predictive mean, variance and preference region in the objective space into consideration. Compared to expected hypervolume improvement (EHVI), the probability density function in TEHVI follows a truncated normal distribution. This paper proposes a TEHVI method that makes it possible to set a region of interest on the Pareto front and focus search effectively on this preferred region.</rdfs:comment>
        <rdfs:label xml:lang="en">TEHVI</rdfs:label>
    </owl:NamedIndividual>
    


    <!-- http://www.semanticweb.org/macoda/ontologies/PMOEA#MDEPSO-RP -->

    <owl:NamedIndividual rdf:about="http://www.semanticweb.org/macoda/ontologies/PMOEA#MDEPSO-RP">
        <rdf:type rdf:resource="http://www.semanticweb.org/macoda/ontologies/PMOEA#PMOEA"/>
        <PMOEA:hasPreferenceModel rdf:resource="http://www.semanticweb.org/macoda/ontologies/PMOEA#TchebycheffASF"/>
        <PMOEA:hasPreferenceInformationFromDM rdf:resource="http://www.semanticweb.org/macoda/ontologies/PMOEA#ReferencePoint"/>
        <PMOEA:hasInteractionTime rdf:resource="http://www.semanticweb.org/macoda/ontologies/PMOEA#a-priori"/>
        <PMOEA:hasPreferenceIntegration rdf:resource="http://www.semanticweb.org/macoda/ontologies/PMOEA#LeaderParticleSelection"/>
        <PMOEA:hasPreferenceIntegration rdf:resource="http://www.semanticweb.org/macoda/ontologies/PMOEA#PersonalBestUpdate"/>
        <PMOEA:hasPreferenceIntegration rdf:resource="http://www.semanticweb.org/macoda/ontologies/PMOEA#ParticleSelection"/>
        <PMOEA:canSolve rdf:resource="http://www.semanticweb.org/macoda/ontologies/PMOEA#ZDT6"/>
        <PMOEA:canSolve rdf:resource="http://www.semanticweb.org/macoda/ontologies/PMOEA#ZDT4"/>
        <PMOEA:canSolve rdf:resource="http://www.semanticweb.org/macoda/ontologies/PMOEA#DTLZ1_3"/>
        <PMOEA:canSolve rdf:resource="http://www.semanticweb.org/macoda/ontologies/PMOEA#DTLZ1_10"/>
        <PMOEA:canSolve rdf:resource="http://www.semanticweb.org/macoda/ontologies/PMOEA#WFG4_2"/>
        <PMOEA:hasResultInfluence rdf:resource="http://www.semanticweb.org/macoda/ontologies/PMOEA#BoundedRegion"/>
        <PMOEA:hasAuthor rdf:resource="http://www.semanticweb.org/macoda/ontologies/PMOEA#Upali_K_Wickramasinghe"/>
        <PMOEA:hasAuthor rdf:resource="http://www.semanticweb.org/macoda/ontologies/PMOEA#Xiaodong_Li"/>
        <PMOEA:hasDevelopingYear rdf:datatype="http://www.w3.org/2001/XMLSchema#integer">2009</PMOEA:hasDevelopingYear>
        <PMOEA:MultipleRegionOfInterest rdf:datatype="http://www.w3.org/2001/XMLSchema#boolean">true</PMOEA:MultipleRegionOfInterest>
        <PMOEA:SpreadControl rdf:datatype="http://www.w3.org/2001/XMLSchema#boolean">true</PMOEA:SpreadControl>
        <PMOEA:hasReference>Wickramasinghe U K, Li X. Using a distance metric to guide PSO algorithms for many-objective optimization[C]//Proceedings of the 11th Annual conference on Genetic and evolutionary computation. ACM, 2009: 667-674.</PMOEA:hasReference>
        <rdfs:comment>Multi-objective Differential Evolution and PSO with Reference point</rdfs:comment>
        <rdfs:label xml:lang="en">MDEPSO-RP</rdfs:label>
    </owl:NamedIndividual>
    


    <!-- http://www.semanticweb.org/macoda/ontologies/PMOEA#FuzzyIntegral -->

    <owl:NamedIndividual rdf:about="http://www.semanticweb.org/macoda/ontologies/PMOEA#FuzzyIntegral">
        <rdf:type rdf:resource="http://www.semanticweb.org/macoda/ontologies/PMOEA#FuzzyLogic"/>
        <rdfs:comment>weighted average of evidence,Sugeno fuzzy integral or Choquet fuzzy integral</rdfs:comment>
        <rdfs:label xml:lang="en">FuzzyIntegral</rdfs:label>
    </owl:NamedIndividual>
    


    <!-- http://www.semanticweb.org/macoda/ontologies/PMOEA#Pradyumn_Kumar_Shukla -->

    <owl:NamedIndividual rdf:about="http://www.semanticweb.org/macoda/ontologies/PMOEA#Pradyumn_Kumar_Shukla">
        <rdf:type rdf:resource="http://www.semanticweb.org/macoda/ontologies/PMOEA#Researcher"/>
        <rdfs:label xml:lang="en">Pradyumn Kumar Shukla</rdfs:label>
    </owl:NamedIndividual>
    


    <!-- http://www.semanticweb.org/macoda/ontologies/PMOEA#Qiang_Zhang -->

    <owl:NamedIndividual rdf:about="http://www.semanticweb.org/macoda/ontologies/PMOEA#Qiang_Zhang">
        <rdf:type rdf:resource="http://www.semanticweb.org/macoda/ontologies/PMOEA#Researcher"/>
        <rdfs:label xml:lang="en">Qiang Zhang</rdfs:label>
    </owl:NamedIndividual>
    


    <!-- http://www.semanticweb.org/macoda/ontologies/PMOEA#GaussianFunctionPreferOneRP -->

    <owl:NamedIndividual rdf:about="http://www.semanticweb.org/macoda/ontologies/PMOEA#GaussianFunctionPreferOneRP">
        <rdf:type rdf:resource="http://www.semanticweb.org/macoda/ontologies/PMOEA#DistributionFunctionInObjectiveSpace"/>
        <rdfs:label xml:lang="en">GaussianFunctionPreferOneRP</rdfs:label>
    </owl:NamedIndividual>
    


    <!-- http://www.semanticweb.org/macoda/ontologies/PMOEA#PyGMO -->

    <owl:NamedIndividual rdf:about="http://www.semanticweb.org/macoda/ontologies/PMOEA#PyGMO">
        <rdf:type rdf:resource="http://www.semanticweb.org/macoda/ontologies/PMOEA#ImplementationLibrary"/>
        <rdfs:comment>A Python platform to perform parallel computations of optimisation tasks (global and local) via the asynchronous generalized island model. State of the art optimization algorithms are included. A common interface is provided to other optimization frameworks/algorithms such as NLOPT, SciPy, SNOPT, IPOPT, GSL</rdfs:comment>
        <rdfs:label xml:lang="en">PyGMO</rdfs:label>
    </owl:NamedIndividual>
    


    <!-- http://www.semanticweb.org/macoda/ontologies/PMOEA#WeightedDominance -->

    <owl:NamedIndividual rdf:about="http://www.semanticweb.org/macoda/ontologies/PMOEA#WeightedDominance">
        <rdf:type rdf:resource="http://www.semanticweb.org/macoda/ontologies/PMOEA#DominanceRelation"/>
        <PMOEA:hasReference>Use of preferences for GA-based multi-objective optimization, in GECCO-99: Proceedings of the Genetic and Evolutionary Computation Conference, W. Banzhaf and J. Daida, Eds. San Mateo, CA: Morgan Kaufmann, July 1999, pp.
15041509.</PMOEA:hasReference>
        <rdfs:label xml:lang="en">WeightedDominance</rdfs:label>
    </owl:NamedIndividual>
    


    <!-- http://www.semanticweb.org/macoda/ontologies/PMOEA#PolyhedralCone -->

    <owl:NamedIndividual rdf:about="http://www.semanticweb.org/macoda/ontologies/PMOEA#PolyhedralCone">
        <rdf:type rdf:resource="http://www.semanticweb.org/macoda/ontologies/PMOEA#PolyhedralConeBased"/>
        <rdfs:comment>In PI-EMO-PC, at an instance of a DM call,  members need to be selected to create M different hyperplanes which form the sides of the polyhedral cone. The decision maker is asked to choose the best solution from the archive set and the end points (M in number) of the non-dominated front in the parent population are selected as other members. Through every end point to best point form a hyperplane, then M planes in total. Now, The M planes together form a polyhedral cone with the best member from the archive as the vertex. Solutions inside the cone are preferred to solutions outside</rdfs:comment>
        <rdfs:label xml:lang="en">PolyhedralCone</rdfs:label>
    </owl:NamedIndividual>
    


    <!-- http://www.semanticweb.org/macoda/ontologies/PMOEA#F1 -->

    <owl:NamedIndividual rdf:about="http://www.semanticweb.org/macoda/ontologies/PMOEA#F1">
        <rdf:type rdf:resource="http://www.semanticweb.org/macoda/ontologies/PMOEA#Academic_Problem"/>
        <PMOEA:isContinuousProblem rdf:datatype="http://www.w3.org/2001/XMLSchema#boolean">true</PMOEA:isContinuousProblem>
        <PMOEA:ObjectiveNumber rdf:datatype="http://www.w3.org/2001/XMLSchema#integer">2</PMOEA:ObjectiveNumber>
        <rdfs:comment>Y. Jin, M. Olhofer, and B. Sendhoff. Evolutionaynamic
weighted aggregation: Why does it work and how? In
L. Spector, E. Goodman, A. Wu, W.B. Langdon, H.-
M. Voigt, M. Gen, S. Sen, M. DOrigo, S. Pezeshk,
M. Garzon, and E. Burke, editors, Proceedings of Ge-
netic and Evolutionary Computation Conference, pages
10421049, San Francisco, CA, 2001</rdfs:comment>
        <rdfs:label xml:lang="en">F1</rdfs:label>
    </owl:NamedIndividual>
    


    <!-- http://www.semanticweb.org/macoda/ontologies/PMOEA#mco -->

    <owl:NamedIndividual rdf:about="http://www.semanticweb.org/macoda/ontologies/PMOEA#mco">
        <rdf:type rdf:resource="http://www.semanticweb.org/macoda/ontologies/PMOEA#ImplementationLibrary"/>
        <rdfs:comment>Functions for multiple criteria optimization using genetic algorithms and related test problems. Contains an implementation of the NSGA-II.</rdfs:comment>
        <rdfs:label xml:lang="en">mco</rdfs:label>
    </owl:NamedIndividual>
    


    <!-- http://www.semanticweb.org/macoda/ontologies/PMOEA#Olaf_Mersmann -->

    <owl:NamedIndividual rdf:about="http://www.semanticweb.org/macoda/ontologies/PMOEA#Olaf_Mersmann">
        <rdf:type rdf:resource="http://www.semanticweb.org/macoda/ontologies/PMOEA#Researcher"/>
        <rdfs:label xml:lang="en">Olaf Mersmann</rdfs:label>
    </owl:NamedIndividual>
    


    <!-- http://www.semanticweb.org/macoda/ontologies/PMOEA#Roberto_Battiti -->

    <owl:NamedIndividual rdf:about="http://www.semanticweb.org/macoda/ontologies/PMOEA#Roberto_Battiti">
        <rdf:type rdf:resource="http://www.semanticweb.org/macoda/ontologies/PMOEA#Researcher"/>
        <rdfs:label xml:lang="en">Roberto Battiti</rdfs:label>
    </owl:NamedIndividual>
    


    <!-- http://www.semanticweb.org/macoda/ontologies/PMOEA#DO2DK -->

    <owl:NamedIndividual rdf:about="http://www.semanticweb.org/macoda/ontologies/PMOEA#DO2DK">
        <rdf:type rdf:resource="http://www.semanticweb.org/macoda/ontologies/PMOEA#Academic_Problem"/>
        <PMOEA:isContinuousProblem rdf:datatype="http://www.w3.org/2001/XMLSchema#boolean">true</PMOEA:isContinuousProblem>
        <PMOEA:ObjectiveNumber rdf:datatype="http://www.w3.org/2001/XMLSchema#integer">2</PMOEA:ObjectiveNumber>
        <PMOEA:hasReference>Branke, J., Deb, K., Dierolf, H., and Osswald, M. Finding
knees in multi-objective optimization. In Proceedings of the
Parallel Problem Solving from Nature, LNCS, 3242, 2004,
722731.</PMOEA:hasReference>
        <rdfs:comment>DO2DK is a minimization problem with n decision variables (we use n = 30) and settable parameters K and s corresponding to the knees number and the extent of the skew in the Pareto front respectively</rdfs:comment>
        <rdfs:label xml:lang="en">DO2DK</rdfs:label>
    </owl:NamedIndividual>
    


    <!-- http://www.semanticweb.org/macoda/ontologies/PMOEA#Salvatore_Greco
 -->

    <owl:NamedIndividual rdf:about="http://www.semanticweb.org/macoda/ontologies/PMOEA#Salvatore_Greco
">
        <rdf:type rdf:resource="http://www.semanticweb.org/macoda/ontologies/PMOEA#Researcher"/>
        <rdfs:label xml:lang="en">Salvatore Greco</rdfs:label>
    </owl:NamedIndividual>
    


    <!-- http://www.semanticweb.org/macoda/ontologies/PMOEA#DesirabilityIndexbasedSelection -->

    <owl:NamedIndividual rdf:about="http://www.semanticweb.org/macoda/ontologies/PMOEA#DesirabilityIndexbasedSelection">
        <rdf:type rdf:resource="http://www.semanticweb.org/macoda/ontologies/PMOEA#SelectionCriterion"/>
        <rdfs:comment>DI-based selection is performed as a second level non-dominated sorting in order to reduce the number of active individuals to the population size . In DI-EMOA</rdfs:comment>
        <rdfs:label xml:lang="en">DesirabilityIndexbasedSelection</rdfs:label>
    </owl:NamedIndividual>
    


    <!-- http://www.semanticweb.org/macoda/ontologies/PMOEA#G-MOEA -->

    <owl:NamedIndividual rdf:about="http://www.semanticweb.org/macoda/ontologies/PMOEA#G-MOEA">
        <rdf:type rdf:resource="http://www.semanticweb.org/macoda/ontologies/PMOEA#PMOEA"/>
        <PMOEA:hasPreferenceInformationFromDM rdf:resource="http://www.semanticweb.org/macoda/ontologies/PMOEA#MaximumAndMinimumTrade-offs"/>
        <PMOEA:hasInteractionTime rdf:resource="http://www.semanticweb.org/macoda/ontologies/PMOEA#a-priori"/>
        <PMOEA:hasPreferenceIntegration rdf:resource="http://www.semanticweb.org/macoda/ontologies/PMOEA#trade-off_basedDomonance"/>
        <PMOEA:canSolve rdf:resource="http://www.semanticweb.org/macoda/ontologies/PMOEA#Schaffers_f2_Function"/>
        <PMOEA:canSolve rdf:resource="http://www.semanticweb.org/macoda/ontologies/PMOEA#ZDT1"/>
        <PMOEA:hasResultInfluence rdf:resource="http://www.semanticweb.org/macoda/ontologies/PMOEA#BoundedRegion"/>
        <PMOEA:hasAuthor rdf:resource="http://www.semanticweb.org/macoda/ontologies/PMOEA#T_Kaupler"/>
        <PMOEA:hasAuthor rdf:resource="http://www.semanticweb.org/macoda/ontologies/PMOEA#H_Schmeck"/>
        <PMOEA:hasAuthor rdf:resource="http://www.semanticweb.org/macoda/ontologies/PMOEA#Juergen_Branke"/>
        <PMOEA:hasSearchAlgorithm rdf:resource="http://www.semanticweb.org/macoda/ontologies/PMOEA#GeneralMOEA"/>
        <PMOEA:hasDevelopingYear rdf:datatype="http://www.w3.org/2001/XMLSchema#integer">2001</PMOEA:hasDevelopingYear>
        <PMOEA:ParetoDominancePreservation rdf:datatype="http://www.w3.org/2001/XMLSchema#boolean">true</PMOEA:ParetoDominancePreservation>
        <PMOEA:hasReference>Branke, J., T. Kauler and H. Schmeck (2001). &quot;Guidance in evolutionary multi-objective optimization.&quot; Advances in Engineering Software 32(6): 499-507.</PMOEA:hasReference>
        <rdfs:comment>DM is allowed to specify preferences in the form of maximally acceptable trade-offs like one unit improvement in objective i is worth at most aji units in objective j. The basic idea is to modify
the dominance criterion accordingly, so that it reflects the specified maximally acceptable trade-offs</rdfs:comment>
        <rdfs:label xml:lang="en">G-MOEA</rdfs:label>
    </owl:NamedIndividual>
    


    <!-- http://www.semanticweb.org/macoda/ontologies/PMOEA#Java -->

    <owl:NamedIndividual rdf:about="http://www.semanticweb.org/macoda/ontologies/PMOEA#Java">
        <rdf:type rdf:resource="http://www.semanticweb.org/macoda/ontologies/PMOEA#ProgrammingLanguage"/>
        <rdfs:label xml:lang="en">Java</rdfs:label>
    </owl:NamedIndividual>
    


    <!-- http://www.semanticweb.org/macoda/ontologies/PMOEA#Tong_Heng_Lee -->

    <owl:NamedIndividual rdf:about="http://www.semanticweb.org/macoda/ontologies/PMOEA#Tong_Heng_Lee">
        <rdf:type rdf:resource="http://www.semanticweb.org/macoda/ontologies/PMOEA#Researcher"/>
        <rdfs:label xml:lang="en">Tong Heng Lee</rdfs:label>
    </owl:NamedIndividual>
    


    <!-- http://www.semanticweb.org/macoda/ontologies/PMOEA#Johannes_Kruisselbrink -->

    <owl:NamedIndividual rdf:about="http://www.semanticweb.org/macoda/ontologies/PMOEA#Johannes_Kruisselbrink">
        <rdf:type rdf:resource="http://www.semanticweb.org/macoda/ontologies/PMOEA#Researcher"/>
        <rdfs:label xml:lang="en">Johannes Kruisselbrink</rdfs:label>
    </owl:NamedIndividual>
    


    <!-- http://www.semanticweb.org/macoda/ontologies/PMOEA#DTLZ2_2 -->

    <owl:NamedIndividual rdf:about="http://www.semanticweb.org/macoda/ontologies/PMOEA#DTLZ2_2">
        <rdf:type rdf:resource="http://www.semanticweb.org/macoda/ontologies/PMOEA#DTLZ"/>
        <PMOEA:OWLDataProperty_61d3cd95_fde4_4c1b_af08_1eaf73473aea rdf:datatype="http://www.w3.org/2001/XMLSchema#boolean">false</PMOEA:OWLDataProperty_61d3cd95_fde4_4c1b_af08_1eaf73473aea>
        <PMOEA:isContinuousProblem rdf:datatype="http://www.w3.org/2001/XMLSchema#boolean">true</PMOEA:isContinuousProblem>
        <PMOEA:ObjectiveNumber rdf:datatype="http://www.w3.org/2001/XMLSchema#integer">2</PMOEA:ObjectiveNumber>
        <PMOEA:isManyObjectiveProblem rdf:datatype="http://www.w3.org/2001/XMLSchema#boolean">false</PMOEA:isManyObjectiveProblem>
        <rdfs:label xml:lang="en">DTLZ2_2</rdfs:label>
    </owl:NamedIndividual>
    


    <!-- http://www.semanticweb.org/macoda/ontologies/PMOEA#Fang_Liu -->

    <owl:NamedIndividual rdf:about="http://www.semanticweb.org/macoda/ontologies/PMOEA#Fang_Liu">
        <rdf:type rdf:resource="http://www.semanticweb.org/macoda/ontologies/PMOEA#Researcher"/>
        <rdfs:label xml:lang="en">Fang Liu</rdfs:label>
    </owl:NamedIndividual>
    


    <!-- http://www.semanticweb.org/macoda/ontologies/PMOEA#CarSideImpactProblem -->

    <owl:NamedIndividual rdf:about="http://www.semanticweb.org/macoda/ontologies/PMOEA#CarSideImpactProblem">
        <rdf:type rdf:resource="http://www.semanticweb.org/macoda/ontologies/PMOEA#Realworld_Problem"/>
        <PMOEA:isContinuousProblem rdf:datatype="http://www.w3.org/2001/XMLSchema#boolean">true</PMOEA:isContinuousProblem>
        <PMOEA:ObjectiveNumber rdf:datatype="http://www.w3.org/2001/XMLSchema#integer">3</PMOEA:ObjectiveNumber>
        <PMOEA:hasReference>K. Deb and A. Kumar. Interactive evolutionary multi-objective
optimization and decision-making using reference direction method.
Technical Report KanGAL report number 2007001, Kanpur Genetic
Algorithms Laboratory, Department of Mechanical engineering, Indian
Institue of Technology Kanpur, India, 2007</PMOEA:hasReference>
        <rdfs:label xml:lang="en">CarSideImpactProblem</rdfs:label>
    </owl:NamedIndividual>
    


    <!-- http://www.semanticweb.org/macoda/ontologies/PMOEA#emoa -->

    <owl:NamedIndividual rdf:about="http://www.semanticweb.org/macoda/ontologies/PMOEA#emoa">
        <rdf:type rdf:resource="http://www.semanticweb.org/macoda/ontologies/PMOEA#ImplementationLibrary"/>
        <rdfs:comment>Collection of building blocks for the design and analysis of evolutionary multiobjective optimization algorithms</rdfs:comment>
        <rdfs:label xml:lang="en">emoa</rdfs:label>
    </owl:NamedIndividual>
    


    <!-- http://www.semanticweb.org/macoda/ontologies/PMOEA#PreferenceConvexCone -->

    <owl:NamedIndividual rdf:about="http://www.semanticweb.org/macoda/ontologies/PMOEA#PreferenceConvexCone">
        <rdf:type rdf:resource="http://www.semanticweb.org/macoda/ontologies/PMOEA#PolyhedralConeBased"/>
        <rdfs:comment>Preference convex cone , originally proposed  by Korhonen, Pekka, Wallenius, Jyrki, Zionts, Stanley, 1984. Solving the discrete multiple criteria problem using convex cones. Management Science 30, 13361345.Use of the DM&apos;s pairwise judgments to generate certain convex polyhedral cones that can eliminate inferior solutions</rdfs:comment>
        <rdfs:label xml:lang="en">PreferenceConvexCone</rdfs:label>
    </owl:NamedIndividual>
    


    <!-- http://www.semanticweb.org/macoda/ontologies/PMOEA#Salvatore_Corrente -->

    <owl:NamedIndividual rdf:about="http://www.semanticweb.org/macoda/ontologies/PMOEA#Salvatore_Corrente">
        <rdf:type rdf:resource="http://www.semanticweb.org/macoda/ontologies/PMOEA#Researcher"/>
        <rdfs:label xml:lang="en">Salvatore Corrente</rdfs:label>
    </owl:NamedIndividual>
    


    <!-- http://www.semanticweb.org/macoda/ontologies/PMOEA#DTLZ1_5 -->

    <owl:NamedIndividual rdf:about="http://www.semanticweb.org/macoda/ontologies/PMOEA#DTLZ1_5">
        <rdf:type rdf:resource="http://www.semanticweb.org/macoda/ontologies/PMOEA#DTLZ"/>
        <PMOEA:OWLDataProperty_61d3cd95_fde4_4c1b_af08_1eaf73473aea rdf:datatype="http://www.w3.org/2001/XMLSchema#boolean">true</PMOEA:OWLDataProperty_61d3cd95_fde4_4c1b_af08_1eaf73473aea>
        <PMOEA:isContinuousProblem rdf:datatype="http://www.w3.org/2001/XMLSchema#boolean">true</PMOEA:isContinuousProblem>
        <PMOEA:ObjectiveNumber rdf:datatype="http://www.w3.org/2001/XMLSchema#integer">5</PMOEA:ObjectiveNumber>
        <PMOEA:isManyObjectiveProblem rdf:datatype="http://www.w3.org/2001/XMLSchema#boolean">true</PMOEA:isManyObjectiveProblem>
        <rdfs:label xml:lang="en">DTLZ1_5</rdfs:label>
    </owl:NamedIndividual>
    


    <!-- http://www.semanticweb.org/macoda/ontologies/PMOEA#Abhishek_Kumar -->

    <owl:NamedIndividual rdf:about="http://www.semanticweb.org/macoda/ontologies/PMOEA#Abhishek_Kumar">
        <rdf:type rdf:resource="http://www.semanticweb.org/macoda/ontologies/PMOEA#Researcher"/>
        <rdfs:label xml:lang="en">Abhishek Kumar</rdfs:label>
    </owl:NamedIndividual>
    


    <!-- http://www.semanticweb.org/macoda/ontologies/PMOEA#Pedro_2 -->

    <owl:NamedIndividual rdf:about="http://www.semanticweb.org/macoda/ontologies/PMOEA#Pedro_2">
        <rdf:type rdf:resource="http://www.semanticweb.org/macoda/ontologies/PMOEA#Academic_Problem"/>
        <PMOEA:isContinuousProblem rdf:datatype="http://www.w3.org/2001/XMLSchema#boolean">true</PMOEA:isContinuousProblem>
        <PMOEA:ObjectiveNumber rdf:datatype="http://www.w3.org/2001/XMLSchema#integer">2</PMOEA:ObjectiveNumber>
        <rdfs:label xml:lang="en">Pedro_2</rdfs:label>
    </owl:NamedIndividual>
    


    <!-- http://www.semanticweb.org/macoda/ontologies/PMOEA#Yushi_Wu -->

    <owl:NamedIndividual rdf:about="http://www.semanticweb.org/macoda/ontologies/PMOEA#Yushi_Wu">
        <rdf:type rdf:resource="http://www.semanticweb.org/macoda/ontologies/PMOEA#Researcher"/>
        <rdfs:label xml:lang="en">Yushi Wu</rdfs:label>
    </owl:NamedIndividual>
    


    <!-- http://www.semanticweb.org/macoda/ontologies/PMOEA#GeneralMOEA -->

    <owl:NamedIndividual rdf:about="http://www.semanticweb.org/macoda/ontologies/PMOEA#GeneralMOEA">
        <rdf:type rdf:resource="http://www.semanticweb.org/macoda/ontologies/PMOEA#DiversityVSConvergence_based"/>
        <rdfs:comment>general MOEA based on diversity and convergence</rdfs:comment>
        <rdfs:label xml:lang="en">GeneralMOEA</rdfs:label>
    </owl:NamedIndividual>
    


    <!-- http://www.semanticweb.org/macoda/ontologies/PMOEA#R -->

    <owl:NamedIndividual rdf:about="http://www.semanticweb.org/macoda/ontologies/PMOEA#R">
        <rdf:type rdf:resource="http://www.semanticweb.org/macoda/ontologies/PMOEA#ProgrammingLanguage"/>
        <rdfs:label xml:lang="en">R</rdfs:label>
    </owl:NamedIndividual>
    


    <!-- http://www.semanticweb.org/macoda/ontologies/PMOEA#SpanningTree_3 -->

    <owl:NamedIndividual rdf:about="http://www.semanticweb.org/macoda/ontologies/PMOEA#SpanningTree_3">
        <rdf:type rdf:resource="http://www.semanticweb.org/macoda/ontologies/PMOEA#Academic_Problem"/>
        <PMOEA:isDiscreteProblem rdf:datatype="http://www.w3.org/2001/XMLSchema#boolean">true</PMOEA:isDiscreteProblem>
        <PMOEA:ObjectiveNumber rdf:datatype="http://www.w3.org/2001/XMLSchema#integer">3</PMOEA:ObjectiveNumber>
        <rdfs:label xml:lang="en">SpanningTree_3</rdfs:label>
    </owl:NamedIndividual>
    


    <!-- http://www.semanticweb.org/macoda/ontologies/PMOEA#Sanaz_Mostaghim -->

    <owl:NamedIndividual rdf:about="http://www.semanticweb.org/macoda/ontologies/PMOEA#Sanaz_Mostaghim">
        <rdf:type rdf:resource="http://www.semanticweb.org/macoda/ontologies/PMOEA#Researcher"/>
        <rdfs:label xml:lang="en">Sanaz Mostaghim</rdfs:label>
    </owl:NamedIndividual>
    


    <!-- http://www.semanticweb.org/macoda/ontologies/PMOEA#HarringtonsDF -->

    <owl:NamedIndividual rdf:about="http://www.semanticweb.org/macoda/ontologies/PMOEA#HarringtonsDF">
        <rdf:type rdf:resource="http://www.semanticweb.org/macoda/ontologies/PMOEA#DesirabilityFunction"/>
        <rdfs:label xml:lang="en">HarringtonsDF</rdfs:label>
    </owl:NamedIndividual>
    


    <!-- http://www.semanticweb.org/macoda/ontologies/PMOEA#SPAMO -->

    <owl:NamedIndividual rdf:about="http://www.semanticweb.org/macoda/ontologies/PMOEA#SPAMO">
        <rdf:type rdf:resource="http://www.semanticweb.org/macoda/ontologies/PMOEA#Indicator_based"/>
        <rdfs:label xml:lang="en">SPAMO</rdfs:label>
        <rdfs:label>Set Preference Algorithm for Multiobjective Optimization, in SPAM, like standard hill climber with two mutation operators, considering quality indicator</rdfs:label>
    </owl:NamedIndividual>
    


    <!-- http://www.semanticweb.org/macoda/ontologies/PMOEA#ZDT5 -->

    <owl:NamedIndividual rdf:about="http://www.semanticweb.org/macoda/ontologies/PMOEA#ZDT5">
        <rdf:type rdf:resource="http://www.semanticweb.org/macoda/ontologies/PMOEA#ZDT"/>
        <PMOEA:isDiscreteProblem rdf:datatype="http://www.w3.org/2001/XMLSchema#boolean">true</PMOEA:isDiscreteProblem>
        <PMOEA:ObjectiveNumber rdf:datatype="http://www.w3.org/2001/XMLSchema#integer">2</PMOEA:ObjectiveNumber>
        <rdfs:label xml:lang="en">ZDT5</rdfs:label>
    </owl:NamedIndividual>
    


    <!-- http://www.semanticweb.org/macoda/ontologies/PMOEA#MQEA -->

    <owl:NamedIndividual rdf:about="http://www.semanticweb.org/macoda/ontologies/PMOEA#MQEA">
        <rdf:type rdf:resource="http://www.semanticweb.org/macoda/ontologies/PMOEA#Probabilistic_based"/>
        <PMOEA:hasReference>Kim J H, Han J H, Kim Y H, et al. Preference-based solution selection algorithm for evolutionary multiobjective optimization[J]. Evolutionary Computation, IEEE Transactions on, 2012, 16(1): 20-34.</PMOEA:hasReference>
        <rdfs:comment>multiobjective quantum-inspired evolutionary algorithm</rdfs:comment>
        <rdfs:label xml:lang="en">MQEA</rdfs:label>
    </owl:NamedIndividual>
    


    <!-- http://www.semanticweb.org/macoda/ontologies/PMOEA#ChoquetIntegral -->

    <owl:NamedIndividual rdf:about="http://www.semanticweb.org/macoda/ontologies/PMOEA#ChoquetIntegral">
        <rdf:type rdf:resource="http://www.semanticweb.org/macoda/ontologies/PMOEA#ChoquetIntegral"/>
        <rdfs:label xml:lang="en">ChoquetIntegral</rdfs:label>
    </owl:NamedIndividual>
    


    <!-- http://www.semanticweb.org/macoda/ontologies/PMOEA#prTDEA -->

    <owl:NamedIndividual rdf:about="http://www.semanticweb.org/macoda/ontologies/PMOEA#prTDEA">
        <rdf:type rdf:resource="http://www.semanticweb.org/macoda/ontologies/PMOEA#PMOEA"/>
        <PMOEA:hasPreferenceModel rdf:resource="http://www.semanticweb.org/macoda/ontologies/PMOEA#PreferenceRegionModel"/>
        <PMOEA:hasPreferenceInformationFromDM rdf:resource="http://www.semanticweb.org/macoda/ontologies/PMOEA#RegionDefinedByTchebycheffWeightSet"/>
        <PMOEA:hasInteractionTime rdf:resource="http://www.semanticweb.org/macoda/ontologies/PMOEA#a-priori"/>
        <PMOEA:hasPreferenceIntegration rdf:resource="http://www.semanticweb.org/macoda/ontologies/PMOEA#TerritorySize"/>
        <PMOEA:canSolve rdf:resource="http://www.semanticweb.org/macoda/ontologies/PMOEA#DTLZ1_5"/>
        <PMOEA:canSolve rdf:resource="http://www.semanticweb.org/macoda/ontologies/PMOEA#DTLZ2_5"/>
        <PMOEA:canSolve rdf:resource="http://www.semanticweb.org/macoda/ontologies/PMOEA#ZDT4"/>
        <PMOEA:canSolve rdf:resource="http://www.semanticweb.org/macoda/ontologies/PMOEA#DTLZ1_3"/>
        <PMOEA:canSolve rdf:resource="http://www.semanticweb.org/macoda/ontologies/PMOEA#DTLZ2_3"/>
        <PMOEA:hasResultInfluence rdf:resource="http://www.semanticweb.org/macoda/ontologies/PMOEA#BiasedDistribution"/>
        <PMOEA:hasAuthor rdf:resource="http://www.semanticweb.org/macoda/ontologies/PMOEA#Murat_Koeksalan"/>
        <PMOEA:useLibrary rdf:resource="http://www.semanticweb.org/macoda/ontologies/PMOEA#KanGAL"/>
        <PMOEA:hasSearchAlgorithm rdf:resource="http://www.semanticweb.org/macoda/ontologies/PMOEA#TDEA"/>
        <PMOEA:hasImplementationLanguage rdf:resource="http://www.semanticweb.org/macoda/ontologies/PMOEA#C++"/>
        <PMOEA:hasDevelopingYear rdf:datatype="http://www.w3.org/2001/XMLSchema#integer">2010</PMOEA:hasDevelopingYear>
        <PMOEA:SpreadControl rdf:datatype="http://www.w3.org/2001/XMLSchema#boolean">true</PMOEA:SpreadControl>
        <PMOEA:ParetoDominancePreservation rdf:datatype="http://www.w3.org/2001/XMLSchema#boolean">true</PMOEA:ParetoDominancePreservation>
        <PMOEA:hasReference>Karahan, . and M. Kksalan (2010). &quot;A territory defining multiobjective evolutionary algorithms and preference incorporation.&quot; Evolutionary Computation, IEEE Transactions on 14(4): 636-664</PMOEA:hasReference>
        <rdfs:comment>We have developed a steady-state elitist evolutionary algorithm to approximate the Pareto-optimal frontiers of multiobjective decision making problems. The algorithms define a territory around each individual to prevent crowding in any region. This maintains diversity while facilitating the fast execution of the algorithm.Based on TDEA, the authors developed an a priori approach, named prTDEA, in which the DM specifies his/her preferred region by a weight set. Solutions in the preferred region and non-interesting region are then assigned different territories such that more solutions are obtained in the preferred region(s).</rdfs:comment>
        <rdfs:label xml:lang="en">prTDEA</rdfs:label>
    </owl:NamedIndividual>
    


    <!-- http://www.semanticweb.org/macoda/ontologies/PMOEA#MDEPSO-LBS -->

    <owl:NamedIndividual rdf:about="http://www.semanticweb.org/macoda/ontologies/PMOEA#MDEPSO-LBS">
        <rdf:type rdf:resource="http://www.semanticweb.org/macoda/ontologies/PMOEA#PMOEA"/>
        <PMOEA:hasPreferenceModel rdf:resource="http://www.semanticweb.org/macoda/ontologies/PMOEA#LightBeamSearch"/>
        <PMOEA:hasPreferenceInformationFromDM rdf:resource="http://www.semanticweb.org/macoda/ontologies/PMOEA#LBSParameters"/>
        <PMOEA:hasInteractionTime rdf:resource="http://www.semanticweb.org/macoda/ontologies/PMOEA#a-priori"/>
        <PMOEA:hasPreferenceIntegration rdf:resource="http://www.semanticweb.org/macoda/ontologies/PMOEA#LeaderParticleSelection"/>
        <PMOEA:hasPreferenceIntegration rdf:resource="http://www.semanticweb.org/macoda/ontologies/PMOEA#PersonalBestUpdate"/>
        <PMOEA:hasPreferenceIntegration rdf:resource="http://www.semanticweb.org/macoda/ontologies/PMOEA#ParticleSelection"/>
        <PMOEA:canSolve rdf:resource="http://www.semanticweb.org/macoda/ontologies/PMOEA#DTLZ3_3"/>
        <PMOEA:canSolve rdf:resource="http://www.semanticweb.org/macoda/ontologies/PMOEA#WFG2_2"/>
        <PMOEA:canSolve rdf:resource="http://www.semanticweb.org/macoda/ontologies/PMOEA#DTLZ3_10"/>
        <PMOEA:canSolve rdf:resource="http://www.semanticweb.org/macoda/ontologies/PMOEA#WFG4_2"/>
        <PMOEA:hasResultInfluence rdf:resource="http://www.semanticweb.org/macoda/ontologies/PMOEA#BoundedRegion"/>
        <PMOEA:hasAuthor rdf:resource="http://www.semanticweb.org/macoda/ontologies/PMOEA#Upali_K_Wickramasinghe"/>
        <PMOEA:hasAuthor rdf:resource="http://www.semanticweb.org/macoda/ontologies/PMOEA#Xiaodong_Li"/>
        <PMOEA:hasDevelopingYear rdf:datatype="http://www.w3.org/2001/XMLSchema#integer">2009</PMOEA:hasDevelopingYear>
        <PMOEA:MultipleRegionOfInterest rdf:datatype="http://www.w3.org/2001/XMLSchema#boolean">true</PMOEA:MultipleRegionOfInterest>
        <PMOEA:SpreadControl rdf:datatype="http://www.w3.org/2001/XMLSchema#boolean">true</PMOEA:SpreadControl>
        <PMOEA:hasReference>Wickramasinghe U K, Li X. Using a distance metric to guide PSO algorithms for many-objective optimization[C]//Proceedings of the 11th Annual conference on Genetic and evolutionary computation. ACM, 2009: 667-674.</PMOEA:hasReference>
        <rdfs:comment>Multi-objective Differential Evolution and PSO with Light Beam Search</rdfs:comment>
        <rdfs:label xml:lang="en">MDEPSO-LBS</rdfs:label>
    </owl:NamedIndividual>
    


    <!-- http://www.semanticweb.org/macoda/ontologies/PMOEA#Knapsack_4 -->

    <owl:NamedIndividual rdf:about="http://www.semanticweb.org/macoda/ontologies/PMOEA#Knapsack_4">
        <rdf:type rdf:resource="http://www.semanticweb.org/macoda/ontologies/PMOEA#Knapsack"/>
        <PMOEA:isDiscreteProblem rdf:datatype="http://www.w3.org/2001/XMLSchema#boolean">true</PMOEA:isDiscreteProblem>
        <PMOEA:ObjectiveNumber rdf:datatype="http://www.w3.org/2001/XMLSchema#integer">4</PMOEA:ObjectiveNumber>
        <PMOEA:isManyObjectiveProblem rdf:datatype="http://www.w3.org/2001/XMLSchema#boolean">true</PMOEA:isManyObjectiveProblem>
        <rdfs:label xml:lang="en">Knapsack_4</rdfs:label>
    </owl:NamedIndividual>
    


    <!-- http://www.semanticweb.org/macoda/ontologies/PMOEA#TimesofDMcalls -->

    <owl:NamedIndividual rdf:about="http://www.semanticweb.org/macoda/ontologies/PMOEA#TimesofDMcalls">
        <rdf:type rdf:resource="http://www.semanticweb.org/macoda/ontologies/PMOEA#BudgetofDMcalls"/>
        <rdfs:label xml:lang="en">TimesofDMcalls</rdfs:label>
        <rdfs:label>times that the DM wants to evaluate the solutions in the searching process</rdfs:label>
    </owl:NamedIndividual>
    


    <!-- http://www.semanticweb.org/macoda/ontologies/PMOEA#DTLZ6_8 -->

    <owl:NamedIndividual rdf:about="http://www.semanticweb.org/macoda/ontologies/PMOEA#DTLZ6_8">
        <rdf:type rdf:resource="http://www.semanticweb.org/macoda/ontologies/PMOEA#DTLZ"/>
        <PMOEA:isContinuousProblem rdf:datatype="http://www.w3.org/2001/XMLSchema#boolean">true</PMOEA:isContinuousProblem>
        <PMOEA:ObjectiveNumber rdf:datatype="http://www.w3.org/2001/XMLSchema#integer">8</PMOEA:ObjectiveNumber>
        <PMOEA:isManyObjectiveProblem rdf:datatype="http://www.w3.org/2001/XMLSchema#boolean">true</PMOEA:isManyObjectiveProblem>
        <rdfs:label xml:lang="en">DTLZ6_8</rdfs:label>
    </owl:NamedIndividual>
    


    <!-- http://www.semanticweb.org/macoda/ontologies/PMOEA#FP-EMO -->

    <owl:NamedIndividual rdf:about="http://www.semanticweb.org/macoda/ontologies/PMOEA#FP-EMO">
        <rdf:type rdf:resource="http://www.semanticweb.org/macoda/ontologies/PMOEA#PMOEA"/>
        <PMOEA:hasPreferenceModel rdf:resource="http://www.semanticweb.org/macoda/ontologies/PMOEA#FuzzyPreferenceRelationOnObjectives"/>
        <PMOEA:hasPreferenceInformationFromDM rdf:resource="http://www.semanticweb.org/macoda/ontologies/PMOEA#linguisticComparisonOnObjectives"/>
        <PMOEA:hasInteractionTime rdf:resource="http://www.semanticweb.org/macoda/ontologies/PMOEA#a-priori"/>
        <PMOEA:hasPreferenceIntegration rdf:resource="http://www.semanticweb.org/macoda/ontologies/PMOEA#WeightedAggregation"/>
        <PMOEA:canSolve rdf:resource="http://www.semanticweb.org/macoda/ontologies/PMOEA#F1"/>
        <PMOEA:canSolve rdf:resource="http://www.semanticweb.org/macoda/ontologies/PMOEA#F2"/>
        <PMOEA:canSolve rdf:resource="http://www.semanticweb.org/macoda/ontologies/PMOEA#F3"/>
        <PMOEA:hasResultInfluence rdf:resource="http://www.semanticweb.org/macoda/ontologies/PMOEA#BiasedDistribution"/>
        <PMOEA:hasAuthor rdf:resource="http://www.semanticweb.org/macoda/ontologies/PMOEA#Bernhard_Sendhoff"/>
        <PMOEA:hasAuthor rdf:resource="http://www.semanticweb.org/macoda/ontologies/PMOEA#Yaochu_Jin"/>
        <PMOEA:hasDevelopingYear rdf:datatype="http://www.w3.org/2001/XMLSchema#integer">2002</PMOEA:hasDevelopingYear>
        <PMOEA:ParetoDominancePreservation rdf:datatype="http://www.w3.org/2001/XMLSchema#boolean">false</PMOEA:ParetoDominancePreservation>
        <PMOEA:hasReference>Jin, Y. and B. Sendhoff (2002). Incorporation Of Fuzzy Preferences Into Evolutionary Multiobjective Optimization. GECCO</PMOEA:hasReference>
        <rdfs:comment>This method  converts  fuzzy preferences into interval-based weights where each weight indicates the importance of the relative objective. This approach converts the MOP into a SOP by weighted aggregation, but varies the weights dynamically during the run within the relevant boundaries</rdfs:comment>
        <rdfs:label xml:lang="en">FP-EMO</rdfs:label>
    </owl:NamedIndividual>
    


    <!-- http://www.semanticweb.org/macoda/ontologies/PMOEA#Licheng_Jiao -->

    <owl:NamedIndividual rdf:about="http://www.semanticweb.org/macoda/ontologies/PMOEA#Licheng_Jiao">
        <rdf:type rdf:resource="http://www.semanticweb.org/macoda/ontologies/PMOEA#Researcher"/>
        <rdfs:label xml:lang="en">Licheng Jiao</rdfs:label>
    </owl:NamedIndividual>
    


    <!-- http://www.semanticweb.org/macoda/ontologies/PMOEA#iEMOA-QCVF -->

    <owl:NamedIndividual rdf:about="http://www.semanticweb.org/macoda/ontologies/PMOEA#iEMOA-QCVF">
        <rdf:type rdf:resource="http://www.semanticweb.org/macoda/ontologies/PMOEA#PMOEA"/>
        <PMOEA:hasPreferenceModel rdf:resource="http://www.semanticweb.org/macoda/ontologies/PMOEA#PreferenceConvexCone"/>
        <PMOEA:hasPreferenceModel rdf:resource="http://www.semanticweb.org/macoda/ontologies/PMOEA#QuasiConcaveUtilityFunction"/>
        <PMOEA:hasPreferenceInformationFromDM rdf:resource="http://www.semanticweb.org/macoda/ontologies/PMOEA#PicktheBestandWorst"/>
        <PMOEA:hasInteractionTime rdf:resource="http://www.semanticweb.org/macoda/ontologies/PMOEA#progressive"/>
        <PMOEA:hasPreferenceIntegration rdf:resource="http://www.semanticweb.org/macoda/ontologies/PMOEA#PreferencebasedSelection"/>
        <PMOEA:hasPreferenceIntegration rdf:resource="http://www.semanticweb.org/macoda/ontologies/PMOEA#FrontSorting"/>
        <PMOEA:canSolve rdf:resource="http://www.semanticweb.org/macoda/ontologies/PMOEA#Knapsack_2"/>
        <PMOEA:canSolve rdf:resource="http://www.semanticweb.org/macoda/ontologies/PMOEA#Knapsack_4"/>
        <PMOEA:canSolve rdf:resource="http://www.semanticweb.org/macoda/ontologies/PMOEA#Knapsack_3"/>
        <PMOEA:hasResultInfluence rdf:resource="http://www.semanticweb.org/macoda/ontologies/PMOEA#OneSolution"/>
        <PMOEA:hasAuthor rdf:resource="http://www.semanticweb.org/macoda/ontologies/PMOEA#Murat_Koeksalan"/>
        <PMOEA:hasAuthor rdf:resource="http://www.semanticweb.org/macoda/ontologies/PMOEA#John_W_Fowler"/>
        <PMOEA:hasAuthor rdf:resource="http://www.semanticweb.org/macoda/ontologies/PMOEA#Esma_S_Gel"/>
        <PMOEA:hasAuthor rdf:resource="http://www.semanticweb.org/macoda/ontologies/PMOEA#Jyrki_Wallenius"/>
        <PMOEA:hasAuthor rdf:resource="http://www.semanticweb.org/macoda/ontologies/PMOEA#Jon_L_Marquis"/>
        <PMOEA:hasAuthor rdf:resource="http://www.semanticweb.org/macoda/ontologies/PMOEA#Pekka_J._Korhonen"/>
        <PMOEA:useLibrary rdf:resource="http://www.semanticweb.org/macoda/ontologies/PMOEA#GAlib"/>
        <PMOEA:hasSearchAlgorithm rdf:resource="http://www.semanticweb.org/macoda/ontologies/PMOEA#GeneralMOEA"/>
        <PMOEA:hasDevelopingYear rdf:datatype="http://www.w3.org/2001/XMLSchema#integer">2010</PMOEA:hasDevelopingYear>
        <PMOEA:ParetoDominancePreservation rdf:datatype="http://www.w3.org/2001/XMLSchema#boolean">true</PMOEA:ParetoDominancePreservation>
        <PMOEA:hasReference>Fowler, J. W., E. S. Gel, M. M. Kksalan, P. Korhonen, J. L. Marquis and J. Wallenius (2010). &quot;Interactive evolutionary multi-objective optimization for quasi-concave preference functions.&quot; European Journal of Operational Research 206(2): 417-425</PMOEA:hasReference>
        <rdfs:comment>We present a new hybrid approach to interactive evolutionary multi-objective optimization that uses a partial preference order to act as the fitness function in a customized genetic algorithm. We periodically send solutions to the decision maker (DM) for her evaluation and use the resulting preference information to form preference cones consisting of inferior solutions. The cones allow us to implicitly rank solutions that the DM has not considered. This technique avoids assuming an exact form for the preference function, but does assume that the preference function is quasi-concave.</rdfs:comment>
        <rdfs:label xml:lang="en">iEMOA-QCVF</rdfs:label>
    </owl:NamedIndividual>
    


    <!-- http://www.semanticweb.org/macoda/ontologies/PMOEA#WFG1_3 -->

    <owl:NamedIndividual rdf:about="http://www.semanticweb.org/macoda/ontologies/PMOEA#WFG1_3">
        <rdf:type rdf:resource="http://www.semanticweb.org/macoda/ontologies/PMOEA#WFG"/>
        <PMOEA:isContinuousProblem rdf:datatype="http://www.w3.org/2001/XMLSchema#boolean">true</PMOEA:isContinuousProblem>
        <PMOEA:ObjectiveNumber rdf:datatype="http://www.w3.org/2001/XMLSchema#integer">3</PMOEA:ObjectiveNumber>
        <rdfs:label xml:lang="en">WFG1_3</rdfs:label>
    </owl:NamedIndividual>
    


    <!-- http://www.semanticweb.org/macoda/ontologies/PMOEA#a-priori -->

    <owl:NamedIndividual rdf:about="http://www.semanticweb.org/macoda/ontologies/PMOEA#a-priori">
        <rdf:type rdf:resource="http://www.semanticweb.org/macoda/ontologies/PMOEA#a-priori"/>
        <rdfs:label xml:lang="en">a-priori</rdfs:label>
    </owl:NamedIndividual>
    


    <!-- http://www.semanticweb.org/macoda/ontologies/PMOEA#Ricardo_H_C_Takahashi -->

    <owl:NamedIndividual rdf:about="http://www.semanticweb.org/macoda/ontologies/PMOEA#Ricardo_H_C_Takahashi">
        <rdf:type rdf:resource="http://www.semanticweb.org/macoda/ontologies/PMOEA#Researcher"/>
        <rdfs:label xml:lang="en">Ricardo H.C. Takahashi</rdfs:label>
    </owl:NamedIndividual>
    


    <!-- http://www.semanticweb.org/macoda/ontologies/PMOEA#IEO-SOL -->

    <owl:NamedIndividual rdf:about="http://www.semanticweb.org/macoda/ontologies/PMOEA#IEO-SOL">
        <rdf:type rdf:resource="http://www.semanticweb.org/macoda/ontologies/PMOEA#PMOEA"/>
        <PMOEA:hasAuthor rdf:resource="http://www.semanticweb.org/macoda/ontologies/PMOEA#Jan_Braun"/>
        <PMOEA:hasAuthor rdf:resource="http://www.semanticweb.org/macoda/ontologies/PMOEA#Hans-Georg"/>
        <PMOEA:hasAuthor rdf:resource="http://www.semanticweb.org/macoda/ontologies/PMOEA#Johannes_Krettek"/>
        <PMOEA:hasAuthor rdf:resource="http://www.semanticweb.org/macoda/ontologies/PMOEA#Thomas_Ewald"/>
        <PMOEA:hasDevelopingYear rdf:datatype="http://www.w3.org/2001/XMLSchema#integer">2009</PMOEA:hasDevelopingYear>
        <PMOEA:hasReference>Krettek, Johannes, et al. &quot;Interactive evolutionary multiobjective optimization for hydraulic valve controller parameters.&quot; 2009 IEEE/ASME International Conference on Advanced Intelligent Mechatronics. IEEE, 2009.</PMOEA:hasReference>
        <rdfs:comment>This paper proposes a novel approach of interactive evolutionary multiobjective optimization combine  with an instance based supervised online learning scheme for user preferences.</rdfs:comment>
        <rdfs:label xml:lang="en">IEO-SOL</rdfs:label>
    </owl:NamedIndividual>
    


    <!-- http://www.semanticweb.org/macoda/ontologies/PMOEA#deap -->

    <owl:NamedIndividual rdf:about="http://www.semanticweb.org/macoda/ontologies/PMOEA#deap">
        <rdf:type rdf:resource="http://www.semanticweb.org/macoda/ontologies/PMOEA#ImplementationLibrary"/>
        <rdfs:comment>An evolutionary computation framework for rapid prototyping and testing of ideas. It includes a genetic algorithm with a variety of solution representations, genetic programing (including automatically defined functions), evolution strategies (including CMA-ES), multi-objective optimization (NSGA-II, SPEA-II), co-evolution of multiple populations, parallelization of evaluations and a benchmarks module with common test functions.</rdfs:comment>
        <rdfs:label xml:lang="en">deap</rdfs:label>
    </owl:NamedIndividual>
    


    <!-- http://www.semanticweb.org/macoda/ontologies/PMOEA#R2_EMOA -->

    <owl:NamedIndividual rdf:about="http://www.semanticweb.org/macoda/ontologies/PMOEA#R2_EMOA">
        <rdf:type rdf:resource="http://www.semanticweb.org/macoda/ontologies/PMOEA#Indicator_based"/>
        <rdfs:comment>The proposed R2-EMOA implements a steady state strategy based on the contribution
to the unary R2-indicator,use nondominated sorting first, then eliminate the solution in the worst front with smallest R2-indicator contribution</rdfs:comment>
        <rdfs:label xml:lang="en">R2_EMOA</rdfs:label>
    </owl:NamedIndividual>
    


    <!-- http://www.semanticweb.org/macoda/ontologies/PMOEA#Murat_Koeksalan -->

    <owl:NamedIndividual rdf:about="http://www.semanticweb.org/macoda/ontologies/PMOEA#Murat_Koeksalan">
        <rdf:type rdf:resource="http://www.semanticweb.org/macoda/ontologies/PMOEA#Researcher"/>
        <rdfs:label xml:lang="en">Murat Koeksalan</rdfs:label>
    </owl:NamedIndividual>
    


    <!-- http://www.semanticweb.org/macoda/ontologies/PMOEA#Ramasubramanian_Sathikannan -->

    <owl:NamedIndividual rdf:about="http://www.semanticweb.org/macoda/ontologies/PMOEA#Ramasubramanian_Sathikannan">
        <rdf:type rdf:resource="http://www.semanticweb.org/macoda/ontologies/PMOEA#Researcher"/>
        <rdfs:label xml:lang="en">Ramasubramanian Sathikannan</rdfs:label>
    </owl:NamedIndividual>
    


    <!-- http://www.semanticweb.org/macoda/ontologies/PMOEA#Rui_Wang -->

    <owl:NamedIndividual rdf:about="http://www.semanticweb.org/macoda/ontologies/PMOEA#Rui_Wang">
        <rdf:type rdf:resource="http://www.semanticweb.org/macoda/ontologies/PMOEA#Researcher"/>
        <rdfs:label xml:lang="en">Rui Wang</rdfs:label>
    </owl:NamedIndividual>
    


    <!-- http://www.semanticweb.org/macoda/ontologies/PMOEA#PI-EMO-PCs -->

    <owl:NamedIndividual rdf:about="http://www.semanticweb.org/macoda/ontologies/PMOEA#PI-EMO-PCs">
        <rdf:type rdf:resource="http://www.semanticweb.org/macoda/ontologies/PMOEA#PMOEA"/>
        <PMOEA:hasPreferenceModel rdf:resource="http://www.semanticweb.org/macoda/ontologies/PMOEA#PolyhedralCone"/>
        <PMOEA:hasPreferenceInformationFromDM rdf:resource="http://www.semanticweb.org/macoda/ontologies/PMOEA#TimesofDMcalls"/>
        <PMOEA:hasPreferenceInformationFromDM rdf:resource="http://www.semanticweb.org/macoda/ontologies/PMOEA#PickTheBest"/>
        <PMOEA:hasInteractionTime rdf:resource="http://www.semanticweb.org/macoda/ontologies/PMOEA#progressive"/>
        <PMOEA:hasPreferenceIntegration rdf:resource="http://www.semanticweb.org/macoda/ontologies/PMOEA#PolyhedralCone-dominance"/>
        <PMOEA:hasPreferenceIntegration rdf:resource="http://www.semanticweb.org/macoda/ontologies/PMOEA#LocalSearch-basedTerminationCriterion"/>
        <PMOEA:canSolve rdf:resource="http://www.semanticweb.org/macoda/ontologies/PMOEA#DTLZ9_5"/>
        <PMOEA:canSolve rdf:resource="http://www.semanticweb.org/macoda/ontologies/PMOEA#DTLZ2_5"/>
        <PMOEA:canSolve rdf:resource="http://www.semanticweb.org/macoda/ontologies/PMOEA#DTLZ2_3"/>
        <PMOEA:canSolve rdf:resource="http://www.semanticweb.org/macoda/ontologies/PMOEA#DTLZ8_3"/>
        <PMOEA:canSolve rdf:resource="http://www.semanticweb.org/macoda/ontologies/PMOEA#DTLZ9_3"/>
        <PMOEA:canSolve rdf:resource="http://www.semanticweb.org/macoda/ontologies/PMOEA#ZDT1"/>
        <PMOEA:hasResultInfluence rdf:resource="http://www.semanticweb.org/macoda/ontologies/PMOEA#OneSolution"/>
        <PMOEA:hasAuthor rdf:resource="http://www.semanticweb.org/macoda/ontologies/PMOEA#Ankur_Sinha"/>
        <PMOEA:hasAuthor rdf:resource="http://www.semanticweb.org/macoda/ontologies/PMOEA#Jyrki_Wallenius"/>
        <PMOEA:hasAuthor rdf:resource="http://www.semanticweb.org/macoda/ontologies/PMOEA#Kalyanmoy_Deb"/>
        <PMOEA:hasAuthor rdf:resource="http://www.semanticweb.org/macoda/ontologies/PMOEA#Pekka_J._Korhonen"/>
        <PMOEA:isExtensionOf rdf:resource="http://www.semanticweb.org/macoda/ontologies/PMOEA#PI-EMO-PC"/>
        <PMOEA:hasSearchAlgorithm rdf:resource="http://www.semanticweb.org/macoda/ontologies/PMOEA#NSGA-II"/>
        <PMOEA:hasDevelopingYear rdf:datatype="http://www.w3.org/2001/XMLSchema#integer">2014</PMOEA:hasDevelopingYear>
        <PMOEA:ParetoDominancePreservation rdf:datatype="http://www.w3.org/2001/XMLSchema#boolean">true</PMOEA:ParetoDominancePreservation>
        <PMOEA:hasReference>Sinha, A., P. Korhonen, J. Wallenius and K. Deb (2014). &quot;An interactive evolutionary multi-objective optimization algorithm with a limited number of decision maker calls.&quot; European Journal of Operational Research 233(3): 674-688</PMOEA:hasReference>
        <rdfs:comment>PI-EMO-PC with a limited budget of decision maker calls,  also tested on PI-EMO-VF.</rdfs:comment>
        <rdfs:label xml:lang="en">PI-EMO-PCs</rdfs:label>
    </owl:NamedIndividual>
    


    <!-- http://www.semanticweb.org/macoda/ontologies/PMOEA#Amos_H_C_Ng -->

    <owl:NamedIndividual rdf:about="http://www.semanticweb.org/macoda/ontologies/PMOEA#Amos_H_C_Ng">
        <rdf:type rdf:resource="http://www.semanticweb.org/macoda/ontologies/PMOEA#Researcher"/>
        <rdfs:label xml:lang="en">Amos H.C. Ng</rdfs:label>
    </owl:NamedIndividual>
    


    <!-- http://www.semanticweb.org/macoda/ontologies/PMOEA#Liping_Wang -->

    <owl:NamedIndividual rdf:about="http://www.semanticweb.org/macoda/ontologies/PMOEA#Liping_Wang">
        <rdf:type rdf:resource="http://www.semanticweb.org/macoda/ontologies/PMOEA#Researcher"/>
        <rdfs:label xml:lang="en">Liping Wang</rdfs:label>
    </owl:NamedIndividual>
    


    <!-- http://www.semanticweb.org/macoda/ontologies/PMOEA#DTLZ5_2 -->

    <owl:NamedIndividual rdf:about="http://www.semanticweb.org/macoda/ontologies/PMOEA#DTLZ5_2">
        <rdf:type rdf:resource="http://www.semanticweb.org/macoda/ontologies/PMOEA#DTLZ"/>
        <PMOEA:isContinuousProblem rdf:datatype="http://www.w3.org/2001/XMLSchema#boolean">true</PMOEA:isContinuousProblem>
        <PMOEA:ObjectiveNumber rdf:datatype="http://www.w3.org/2001/XMLSchema#integer">2</PMOEA:ObjectiveNumber>
        <rdfs:label xml:lang="en">DTLZ5_2</rdfs:label>
    </owl:NamedIndividual>
    


    <!-- http://www.semanticweb.org/macoda/ontologies/PMOEA#Souhila_Kaci -->

    <owl:NamedIndividual rdf:about="http://www.semanticweb.org/macoda/ontologies/PMOEA#Souhila_Kaci">
        <rdf:type rdf:resource="http://www.semanticweb.org/macoda/ontologies/PMOEA#Researcher"/>
        <rdfs:label xml:lang="en">Souhila Kaci</rdfs:label>
    </owl:NamedIndividual>
    


    <!-- http://www.semanticweb.org/macoda/ontologies/PMOEA#LinearProgramming -->

    <owl:NamedIndividual rdf:about="http://www.semanticweb.org/macoda/ontologies/PMOEA#LinearProgramming">
        <rdf:type rdf:resource="http://www.semanticweb.org/macoda/ontologies/PMOEA#LinearProgramming"/>
        <rdfs:label xml:lang="en">LinearProgramming</rdfs:label>
    </owl:NamedIndividual>
    


    <!-- http://www.semanticweb.org/macoda/ontologies/PMOEA#Slim_Bechikh -->

    <owl:NamedIndividual rdf:about="http://www.semanticweb.org/macoda/ontologies/PMOEA#Slim_Bechikh">
        <rdf:type rdf:resource="http://www.semanticweb.org/macoda/ontologies/PMOEA#Researcher"/>
        <rdfs:label xml:lang="en">Slim Bechikh</rdfs:label>
    </owl:NamedIndividual>
    


    <!-- http://www.semanticweb.org/macoda/ontologies/PMOEA#Knapsack_10 -->

    <owl:NamedIndividual rdf:about="http://www.semanticweb.org/macoda/ontologies/PMOEA#Knapsack_10">
        <rdf:type rdf:resource="http://www.semanticweb.org/macoda/ontologies/PMOEA#Knapsack"/>
        <PMOEA:isDiscreteProblem rdf:datatype="http://www.w3.org/2001/XMLSchema#boolean">true</PMOEA:isDiscreteProblem>
        <PMOEA:ObjectiveNumber rdf:datatype="http://www.w3.org/2001/XMLSchema#integer">10</PMOEA:ObjectiveNumber>
        <PMOEA:isManyObjectiveProblem rdf:datatype="http://www.w3.org/2001/XMLSchema#boolean">true</PMOEA:isManyObjectiveProblem>
        <rdfs:label xml:lang="en">Knapsack_10</rdfs:label>
    </owl:NamedIndividual>
    


    <!-- http://www.semanticweb.org/macoda/ontologies/PMOEA#Christian_Hirsch -->

    <owl:NamedIndividual rdf:about="http://www.semanticweb.org/macoda/ontologies/PMOEA#Christian_Hirsch">
        <rdf:type rdf:resource="http://www.semanticweb.org/macoda/ontologies/PMOEA#Researcher"/>
        <rdfs:label xml:lang="en">Christian Hirsch</rdfs:label>
    </owl:NamedIndividual>
    


    <!-- http://www.semanticweb.org/macoda/ontologies/PMOEA#I-MODE -->

    <owl:NamedIndividual rdf:about="http://www.semanticweb.org/macoda/ontologies/PMOEA#I-MODE">
        <rdf:type rdf:resource="http://www.semanticweb.org/macoda/ontologies/PMOEA#PMOEA"/>
        <PMOEA:canSolve rdf:resource="http://www.semanticweb.org/macoda/ontologies/PMOEA#WeldedBeamDesign"/>
        <PMOEA:hasResultInfluence rdf:resource="http://www.semanticweb.org/macoda/ontologies/PMOEA#OneSolution"/>
        <PMOEA:hasDevelopingYear rdf:datatype="http://www.w3.org/2001/XMLSchema#integer">2007</PMOEA:hasDevelopingYear>
        <PMOEA:hasReference>Deb, K. and S. Chaudhuri (2007). &quot;I-MODE: an interactive multi-objective optimization and decision-making using evolutionary methods.&quot; Lecture Notes in Computer Science 4403: 788-802</PMOEA:hasReference>
        <rdfs:comment>I-MODE is an interactive decision support system that implements an interactive procedure built over a number of existing EMO and classical decision making methods.The DM has options to use several tools for generation of potentially Pareto-optimal solutions concentrated in the desired regions. For example, he/she may use weighted sum approach, utility function based approach, Chebycheff function approach or trade-off information.The preference information is then used by an EMO to generate new solutions in the most interesting regions. G-MOEA and  R-NSGA-II are included.</rdfs:comment>
        <rdfs:label xml:lang="en">I-MODE</rdfs:label>
    </owl:NamedIndividual>
    


    <!-- http://www.semanticweb.org/macoda/ontologies/PMOEA#PISA -->

    <owl:NamedIndividual rdf:about="http://www.semanticweb.org/macoda/ontologies/PMOEA#PISA">
        <rdf:type rdf:resource="http://www.semanticweb.org/macoda/ontologies/PMOEA#ImplementationLibrary"/>
        <rdfs:comment>PISA is a text-based interface for search algorithms. It splits an optimization process into two modules. One module contains all parts specific to the optimization problem (e.g., evaluation of solutions, problem representation, variation of solutions). The other module contains the parts which are independent of the optimization problem (mainly the selection process). These two modules are implemented as separate programs which communicate through text files.
PISA is a library of ready-to-go modules, namely optimization problems (test and benchmark problems), selection modules (evolutionary multi-objective optimizers) and modules for performance assessment.</rdfs:comment>
        <rdfs:label xml:lang="en">PISA</rdfs:label>
    </owl:NamedIndividual>
    


    <!-- http://www.semanticweb.org/macoda/ontologies/PMOEA#progressive -->

    <owl:NamedIndividual rdf:about="http://www.semanticweb.org/macoda/ontologies/PMOEA#progressive">
        <rdf:type rdf:resource="http://www.semanticweb.org/macoda/ontologies/PMOEA#progressive"/>
        <rdfs:label xml:lang="en">progressive</rdfs:label>
    </owl:NamedIndividual>
    


    <!-- http://www.semanticweb.org/macoda/ontologies/PMOEA#Heike_Trautmann -->

    <owl:NamedIndividual rdf:about="http://www.semanticweb.org/macoda/ontologies/PMOEA#Heike_Trautmann">
        <rdf:type rdf:resource="http://www.semanticweb.org/macoda/ontologies/PMOEA#Researcher"/>
        <rdfs:label xml:lang="en">Heike Trautmann</rdfs:label>
    </owl:NamedIndividual>
    


    <!-- http://www.semanticweb.org/macoda/ontologies/PMOEA#S-ZDT2 -->

    <owl:NamedIndividual rdf:about="http://www.semanticweb.org/macoda/ontologies/PMOEA#S-ZDT2">
        <rdf:type rdf:resource="http://www.semanticweb.org/macoda/ontologies/PMOEA#Academic_Problem"/>
        <PMOEA:isContinuousProblem rdf:datatype="http://www.w3.org/2001/XMLSchema#boolean">true</PMOEA:isContinuousProblem>
        <PMOEA:ObjectiveNumber rdf:datatype="http://www.w3.org/2001/XMLSchema#integer">2</PMOEA:ObjectiveNumber>
        <rdfs:label xml:lang="en">S-ZDT2</rdfs:label>
    </owl:NamedIndividual>
    


    <!-- http://www.semanticweb.org/macoda/ontologies/PMOEA#DTLZ5_8 -->

    <owl:NamedIndividual rdf:about="http://www.semanticweb.org/macoda/ontologies/PMOEA#DTLZ5_8">
        <rdf:type rdf:resource="http://www.semanticweb.org/macoda/ontologies/PMOEA#DTLZ"/>
        <PMOEA:isContinuousProblem rdf:datatype="http://www.w3.org/2001/XMLSchema#boolean">true</PMOEA:isContinuousProblem>
        <PMOEA:ObjectiveNumber rdf:datatype="http://www.w3.org/2001/XMLSchema#integer">8</PMOEA:ObjectiveNumber>
        <PMOEA:isManyObjectiveProblem rdf:datatype="http://www.w3.org/2001/XMLSchema#boolean">true</PMOEA:isManyObjectiveProblem>
        <rdfs:label xml:lang="en">DTLZ5_8</rdfs:label>
    </owl:NamedIndividual>
    


    <!-- http://www.semanticweb.org/macoda/ontologies/PMOEA#BiasedDistribution -->

    <owl:NamedIndividual rdf:about="http://www.semanticweb.org/macoda/ontologies/PMOEA#BiasedDistribution">
        <rdf:type rdf:resource="http://www.semanticweb.org/macoda/ontologies/PMOEA#BiasedDistribution"/>
        <rdfs:label xml:lang="en">BiasedDistribution</rdfs:label>
    </owl:NamedIndividual>
    


    <!-- http://www.semanticweb.org/macoda/ontologies/PMOEA#Jorn_Mehnen -->

    <owl:NamedIndividual rdf:about="http://www.semanticweb.org/macoda/ontologies/PMOEA#Jorn_Mehnen">
        <rdf:type rdf:resource="http://www.semanticweb.org/macoda/ontologies/PMOEA#Researcher"/>
        <rdfs:label xml:lang="en">Jrn Mehnen</rdfs:label>
    </owl:NamedIndividual>
    


    <!-- http://www.semanticweb.org/macoda/ontologies/PMOEA#jMetal -->

    <owl:NamedIndividual rdf:about="http://www.semanticweb.org/macoda/ontologies/PMOEA#jMetal">
        <rdf:type rdf:resource="http://www.semanticweb.org/macoda/ontologies/PMOEA#ImplementationLibrary"/>
        <rdfs:comment>An object-oriented Java-based framework for multi-objective optimization with metaheuristics. It offers a variety of single- and multi-objective algoritms (including their parallel implementations), variable representations, test problems and quality indicators</rdfs:comment>
        <rdfs:label xml:lang="en">jMetal</rdfs:label>
    </owl:NamedIndividual>
    


    <!-- http://www.semanticweb.org/macoda/ontologies/PMOEA#TKR-NSGA-II -->

    <owl:NamedIndividual rdf:about="http://www.semanticweb.org/macoda/ontologies/PMOEA#TKR-NSGA-II">
        <rdf:type rdf:resource="http://www.semanticweb.org/macoda/ontologies/PMOEA#PMOEA"/>
        <PMOEA:hasPreferenceModel rdf:resource="http://www.semanticweb.org/macoda/ontologies/PMOEA#Knee-point"/>
        <PMOEA:hasInteractionTime rdf:resource="http://www.semanticweb.org/macoda/ontologies/PMOEA#a-priori"/>
        <PMOEA:hasInteractionTime rdf:resource="http://www.semanticweb.org/macoda/ontologies/PMOEA#progressive"/>
        <PMOEA:hasPreferenceIntegration rdf:resource="http://www.semanticweb.org/macoda/ontologies/PMOEA#CrowdingDistance"/>
        <PMOEA:canSolve rdf:resource="http://www.semanticweb.org/macoda/ontologies/PMOEA#DO2DK"/>
        <PMOEA:canSolve rdf:resource="http://www.semanticweb.org/macoda/ontologies/PMOEA#DEB2DK"/>
        <PMOEA:canSolve rdf:resource="http://www.semanticweb.org/macoda/ontologies/PMOEA#DEB3DK"/>
        <PMOEA:hasResultInfluence rdf:resource="http://www.semanticweb.org/macoda/ontologies/PMOEA#BiasedDistribution"/>
        <PMOEA:hasAuthor rdf:resource="http://www.semanticweb.org/macoda/ontologies/PMOEA#Slim_Bechikh"/>
        <PMOEA:hasAuthor rdf:resource="http://www.semanticweb.org/macoda/ontologies/PMOEA#Lamjed_Ben_Said,"/>
        <PMOEA:isExtensionOf rdf:resource="http://www.semanticweb.org/macoda/ontologies/PMOEA#KR-NSGA-II"/>
        <PMOEA:hasSearchAlgorithm rdf:resource="http://www.semanticweb.org/macoda/ontologies/PMOEA#NSGA-II"/>
        <PMOEA:hasImplementationLanguage rdf:resource="http://www.semanticweb.org/macoda/ontologies/PMOEA#Matlab"/>
        <PMOEA:MultipleRegionOfInterest rdf:datatype="http://www.w3.org/2001/XMLSchema#boolean">true</PMOEA:MultipleRegionOfInterest>
        <PMOEA:SpreadControl rdf:datatype="http://www.w3.org/2001/XMLSchema#boolean">true</PMOEA:SpreadControl>
        <PMOEA:ParetoDominancePreservation rdf:datatype="http://www.w3.org/2001/XMLSchema#boolean">true</PMOEA:ParetoDominancePreservation>
        <PMOEA:hasReference>Bechikh, Slim, Lamjed Ben Said, and Khaled Ghdira. &quot;Searching for knee regions of the Pareto front using mobile reference points.&quot; Soft Computing 15.9 (2011): 1807-1823.</PMOEA:hasReference>
        <rdfs:comment>The failure of KR-NSGA-II in discovering the true extreme solutions engenders the loss a potential knee solutions or the discovery of spurious ones. In order to avoid such problematic, we modified the knee point characterisation in KR-NSGA-II. In fact, instead of the distance to the extreme line, we used a recently proposed trade-off worth metric</rdfs:comment>
        <rdfs:label xml:lang="en">TKR-NSGA-II</rdfs:label>
    </owl:NamedIndividual>
    


    <!-- http://www.semanticweb.org/macoda/ontologies/PMOEA#Bi-objectivePortfolioOptimization -->

    <owl:NamedIndividual rdf:about="http://www.semanticweb.org/macoda/ontologies/PMOEA#Bi-objectivePortfolioOptimization">
        <rdf:type rdf:resource="http://www.semanticweb.org/macoda/ontologies/PMOEA#Realworld_Problem"/>
        <PMOEA:hasReference>K. Deb, R. E. Steuer, R. Tewari, and Ra. Tewari, Bi-objective portfolio optimization using a customized hybrid NSGA-II procedure, In Proceedings of the international conference on Evolutionary Multi-criterion Optimization (EMO11), pp. 358373,
LNCS, Springer, 2011.</PMOEA:hasReference>
        <rdfs:comment>there are two conflicting objectives: (1) minimize the Portfolio risk and (2) maximize the expected Portfolio return.</rdfs:comment>
        <rdfs:label xml:lang="en">Bi-objectivePortfolioOptimization</rdfs:label>
    </owl:NamedIndividual>
    


    <!-- http://www.semanticweb.org/macoda/ontologies/PMOEA#Bernhard_Sendhoff -->

    <owl:NamedIndividual rdf:about="http://www.semanticweb.org/macoda/ontologies/PMOEA#Bernhard_Sendhoff">
        <rdf:type rdf:resource="http://www.semanticweb.org/macoda/ontologies/PMOEA#Researcher"/>
        <rdfs:label xml:lang="en">Bernhard Sendhoff</rdfs:label>
    </owl:NamedIndividual>
    


    <!-- http://www.semanticweb.org/macoda/ontologies/PMOEA#iTDEA -->

    <owl:NamedIndividual rdf:about="http://www.semanticweb.org/macoda/ontologies/PMOEA#iTDEA">
        <rdf:type rdf:resource="http://www.semanticweb.org/macoda/ontologies/PMOEA#PMOEA"/>
        <PMOEA:hasPreferenceModel rdf:resource="http://www.semanticweb.org/macoda/ontologies/PMOEA#PreferenceRegionModel"/>
        <PMOEA:hasPreferenceInformationFromDM rdf:resource="http://www.semanticweb.org/macoda/ontologies/PMOEA#PickTheBest"/>
        <PMOEA:hasInteractionTime rdf:resource="http://www.semanticweb.org/macoda/ontologies/PMOEA#progressive"/>
        <PMOEA:hasPreferenceIntegration rdf:resource="http://www.semanticweb.org/macoda/ontologies/PMOEA#TerritorySize"/>
        <PMOEA:isInteractiveVersionOf rdf:resource="http://www.semanticweb.org/macoda/ontologies/PMOEA#prTDEA"/>
        <PMOEA:canSolve rdf:resource="http://www.semanticweb.org/macoda/ontologies/PMOEA#ZDT4"/>
        <PMOEA:canSolve rdf:resource="http://www.semanticweb.org/macoda/ontologies/PMOEA#DTLZ1_3"/>
        <PMOEA:canSolve rdf:resource="http://www.semanticweb.org/macoda/ontologies/PMOEA#DTLZ2_3"/>
        <PMOEA:hasResultInfluence rdf:resource="http://www.semanticweb.org/macoda/ontologies/PMOEA#BiasedDistribution"/>
        <PMOEA:hasAuthor rdf:resource="http://www.semanticweb.org/macoda/ontologies/PMOEA#Murat_Koeksalan"/>
        <PMOEA:hasAuthor rdf:resource="http://www.semanticweb.org/macoda/ontologies/PMOEA#Ibrahim_Karahan"/>
        <PMOEA:hasSearchAlgorithm rdf:resource="http://www.semanticweb.org/macoda/ontologies/PMOEA#TDEA"/>
        <PMOEA:hasImplementationLanguage rdf:resource="http://www.semanticweb.org/macoda/ontologies/PMOEA#C++"/>
        <PMOEA:hasDevelopingYear rdf:datatype="http://www.w3.org/2001/XMLSchema#integer">2010</PMOEA:hasDevelopingYear>
        <PMOEA:MultipleRegionOfInterest rdf:datatype="http://www.w3.org/2001/XMLSchema#boolean">false</PMOEA:MultipleRegionOfInterest>
        <PMOEA:SpreadControl rdf:datatype="http://www.w3.org/2001/XMLSchema#boolean">true</PMOEA:SpreadControl>
        <PMOEA:ParetoDominancePreservation rdf:datatype="http://www.w3.org/2001/XMLSchema#boolean">true</PMOEA:ParetoDominancePreservation>
        <PMOEA:hasReference>Kksalan, M. and I. Karahan (2010). &quot;An interactive territory defining evolutionary algorithm: iTDEA.&quot; Evolutionary Computation, IEEE Transactions on 14(5): 702-722</PMOEA:hasReference>
        <rdfs:comment>We create a territory around each solution where no other solutions are allowed. We define smaller territories around the preferred solutions in order to obtain denser coverage of these regions. At each interaction, the algorithm asks the DM to choose his/her best solution among a set of representative solutions to guide the search toward the neighborhood of the selected solution. The algorithm aims to converge to a final preferred region of the DM</rdfs:comment>
        <rdfs:label xml:lang="en">iTDEA</rdfs:label>
    </owl:NamedIndividual>
    


    <!-- http://www.semanticweb.org/macoda/ontologies/PMOEA#SpanningTree_4 -->

    <owl:NamedIndividual rdf:about="http://www.semanticweb.org/macoda/ontologies/PMOEA#SpanningTree_4">
        <rdf:type rdf:resource="http://www.semanticweb.org/macoda/ontologies/PMOEA#Academic_Problem"/>
        <PMOEA:isDiscreteProblem rdf:datatype="http://www.w3.org/2001/XMLSchema#boolean">true</PMOEA:isDiscreteProblem>
        <PMOEA:ObjectiveNumber rdf:datatype="http://www.w3.org/2001/XMLSchema#integer">4</PMOEA:ObjectiveNumber>
        <PMOEA:isManyObjectiveProblem rdf:datatype="http://www.w3.org/2001/XMLSchema#boolean">true</PMOEA:isManyObjectiveProblem>
        <rdfs:label xml:lang="en">SpanningTree_4</rdfs:label>
    </owl:NamedIndividual>
    


    <!-- http://www.semanticweb.org/macoda/ontologies/PMOEA#WFG1_2 -->

    <owl:NamedIndividual rdf:about="http://www.semanticweb.org/macoda/ontologies/PMOEA#WFG1_2">
        <rdf:type rdf:resource="http://www.semanticweb.org/macoda/ontologies/PMOEA#WFG"/>
        <PMOEA:isContinuousProblem rdf:datatype="http://www.w3.org/2001/XMLSchema#boolean">true</PMOEA:isContinuousProblem>
        <PMOEA:ObjectiveNumber rdf:datatype="http://www.w3.org/2001/XMLSchema#integer">2</PMOEA:ObjectiveNumber>
        <rdfs:label xml:lang="en">WFG1_2</rdfs:label>
    </owl:NamedIndividual>
    


    <!-- http://www.semanticweb.org/macoda/ontologies/PMOEA#SetPreference -->

    <owl:NamedIndividual rdf:about="http://www.semanticweb.org/macoda/ontologies/PMOEA#SetPreference">
        <rdf:type rdf:resource="http://www.semanticweb.org/macoda/ontologies/PMOEA#SetPreference"/>
        <rdfs:comment>In SPAM, set preference can be combinations of epsilon indicator and Hypervolume indicator, R2 indicator and Hypervolume , etc.</rdfs:comment>
        <rdfs:label xml:lang="en">SetPreference</rdfs:label>
    </owl:NamedIndividual>
    


    <!-- http://www.semanticweb.org/macoda/ontologies/PMOEA#Boris_Naujoks -->

    <owl:NamedIndividual rdf:about="http://www.semanticweb.org/macoda/ontologies/PMOEA#Boris_Naujoks">
        <rdf:type rdf:resource="http://www.semanticweb.org/macoda/ontologies/PMOEA#Researcher"/>
        <rdfs:label xml:lang="en">Boris Naujoks</rdfs:label>
    </owl:NamedIndividual>
    


    <!-- http://www.semanticweb.org/macoda/ontologies/PMOEA#DRSA-EMO-PCT -->

    <owl:NamedIndividual rdf:about="http://www.semanticweb.org/macoda/ontologies/PMOEA#DRSA-EMO-PCT">
        <rdf:type rdf:resource="http://www.semanticweb.org/macoda/ontologies/PMOEA#PMOEA"/>
        <PMOEA:hasPreferenceModel rdf:resource="http://www.semanticweb.org/macoda/ontologies/PMOEA#DRSA"/>
        <PMOEA:hasPreferenceInformationFromDM rdf:resource="http://www.semanticweb.org/macoda/ontologies/PMOEA#PairwiseComparison"/>
        <PMOEA:hasInteractionTime rdf:resource="http://www.semanticweb.org/macoda/ontologies/PMOEA#progressive"/>
        <PMOEA:hasPreferenceIntegration rdf:resource="http://www.semanticweb.org/macoda/ontologies/PMOEA#FrontSorting"/>
        <PMOEA:hasResultInfluence rdf:resource="http://www.semanticweb.org/macoda/ontologies/PMOEA#SetOfSolutions"/>
        <PMOEA:hasAuthor rdf:resource="http://www.semanticweb.org/macoda/ontologies/PMOEA#Salvatore_Greco
"/>
        <PMOEA:hasAuthor rdf:resource="http://www.semanticweb.org/macoda/ontologies/PMOEA#Benedetto_Matarazzo"/>
        <PMOEA:hasAuthor rdf:resource="http://www.semanticweb.org/macoda/ontologies/PMOEA#Roman_Sowinski"/>
        <PMOEA:hasSearchAlgorithm rdf:resource="http://www.semanticweb.org/macoda/ontologies/PMOEA#NSGA-II"/>
        <PMOEA:hasDevelopingYear rdf:datatype="http://www.w3.org/2001/XMLSchema#integer">2010</PMOEA:hasDevelopingYear>
        <PMOEA:hasReference>Greco, S., B. Matarazzo and R. Slowinski (2010). Interactive evolutionary multiobjective optimization using dominance-based rough set approach. Evolutionary Computation (CEC), 2010 IEEE Congress on, IEEE</PMOEA:hasReference>
        <rdfs:comment>Different with DRSA-EMO only by PrefrenceInformationFromDM, it&apos;s pairwise comparison in DRSA-EMO-PCT</rdfs:comment>
        <rdfs:label xml:lang="en">DRSA-EMO-PCT</rdfs:label>
    </owl:NamedIndividual>
    


    <!-- http://www.semanticweb.org/macoda/ontologies/PMOEA#GoalFulfilmentDominance -->

    <owl:NamedIndividual rdf:about="http://www.semanticweb.org/macoda/ontologies/PMOEA#GoalFulfilmentDominance">
        <rdf:type rdf:resource="http://www.semanticweb.org/macoda/ontologies/PMOEA#DominanceRelation"/>
        <rdfs:comment>dominance in PMOGA:  when deciding whether a solution x is preferable to a solution y or not, first, only the objectives in which solution x does not satisfy the goal are considered, and x is preferred to y if it dominates y on these objectives. If x is equal to y in all these objectives, or if x satisfies the goal in all objectives, x is preferred over y either if y does not fulfill some of the objectives fulfilled by x, or if x dominates y on the objectives fulfilled by x</rdfs:comment>
        <rdfs:label xml:lang="en">GoalFulfilmentDominance</rdfs:label>
    </owl:NamedIndividual>
    


    <!-- http://www.semanticweb.org/macoda/ontologies/PMOEA#John_W_Fowler -->

    <owl:NamedIndividual rdf:about="http://www.semanticweb.org/macoda/ontologies/PMOEA#John_W_Fowler">
        <rdf:type rdf:resource="http://www.semanticweb.org/macoda/ontologies/PMOEA#Researcher"/>
        <rdfs:label xml:lang="en">John W. Fowler</rdfs:label>
    </owl:NamedIndividual>
    


    <!-- http://www.semanticweb.org/macoda/ontologies/PMOEA#DistributeCreditsToObjectives -->

    <owl:NamedIndividual rdf:about="http://www.semanticweb.org/macoda/ontologies/PMOEA#DistributeCreditsToObjectives">
        <rdf:type rdf:resource="http://www.semanticweb.org/macoda/ontologies/PMOEA#ObjectiveComparison"/>
        <rdfs:comment>distribute 100 credits to objectives according to their importance</rdfs:comment>
        <rdfs:label xml:lang="en">DistributeCreditsToObjectives</rdfs:label>
    </owl:NamedIndividual>
    


    <!-- http://www.semanticweb.org/macoda/ontologies/PMOEA#GSP_3 -->

    <owl:NamedIndividual rdf:about="http://www.semanticweb.org/macoda/ontologies/PMOEA#GSP_3">
        <rdf:type rdf:resource="http://www.semanticweb.org/macoda/ontologies/PMOEA#Academic_Problem"/>
        <PMOEA:isContinuousProblem rdf:datatype="http://www.w3.org/2001/XMLSchema#boolean">true</PMOEA:isContinuousProblem>
        <PMOEA:ObjectiveNumber rdf:datatype="http://www.w3.org/2001/XMLSchema#integer">3</PMOEA:ObjectiveNumber>
        <PMOEA:hasReference>Emmerich, M.T.M., Deutz, A.H.: Test Problems Based on Lame Superspheres.
In: Obayashi, S., Deb, K., Poloni, C., Hiroyasu, T., Murata, T. (eds.) EMO 2007.
LNCS, vol. 4403, pp. 922936. Springer, Heidelberg (2007)</PMOEA:hasReference>
        <rdfs:label xml:lang="en">GSP_3</rdfs:label>
    </owl:NamedIndividual>
    


    <!-- http://www.semanticweb.org/macoda/ontologies/PMOEA#NumberofSolutions -->

    <owl:NamedIndividual rdf:about="http://www.semanticweb.org/macoda/ontologies/PMOEA#NumberofSolutions">
        <rdf:type rdf:resource="http://www.semanticweb.org/macoda/ontologies/PMOEA#BudgetofDMcalls"/>
        <rdfs:comment>the number of solutions DM can evaluate at the DM call</rdfs:comment>
        <rdfs:label xml:lang="en">NumberofSolutions</rdfs:label>
    </owl:NamedIndividual>
    


    <!-- http://www.semanticweb.org/macoda/ontologies/PMOEA#Upali_K_Wickramasinghe -->

    <owl:NamedIndividual rdf:about="http://www.semanticweb.org/macoda/ontologies/PMOEA#Upali_K_Wickramasinghe">
        <rdf:type rdf:resource="http://www.semanticweb.org/macoda/ontologies/PMOEA#Researcher"/>
        <rdfs:label xml:lang="en">Upali K Wickramasinghe</rdfs:label>
    </owl:NamedIndividual>
    


    <!-- http://www.semanticweb.org/macoda/ontologies/PMOEA#GroupDMPoints -->

    <owl:NamedIndividual rdf:about="http://www.semanticweb.org/macoda/ontologies/PMOEA#GroupDMPoints">
        <rdf:type rdf:resource="http://www.semanticweb.org/macoda/ontologies/PMOEA#GroupDecisionMaking"/>
        <rdf:type rdf:resource="http://www.semanticweb.org/macoda/ontologies/PMOEA#ReferencePoint"/>
        <rdfs:comment>reference points and the acceptable deviation quantity for every DM in group decision making, weights of DM.</rdfs:comment>
        <rdfs:label xml:lang="en">GroupDMPoints</rdfs:label>
    </owl:NamedIndividual>
    


    <!-- http://www.semanticweb.org/macoda/ontologies/PMOEA#SequentialQuadraticProgramming -->

    <owl:NamedIndividual rdf:about="http://www.semanticweb.org/macoda/ontologies/PMOEA#SequentialQuadraticProgramming">
        <rdf:type rdf:resource="http://www.semanticweb.org/macoda/ontologies/PMOEA#QuadraticProgramming"/>
        <rdfs:label xml:lang="en">SequentialQuadraticProgramming</rdfs:label>
    </owl:NamedIndividual>
    


    <!-- http://www.semanticweb.org/macoda/ontologies/PMOEA#WFG3_2 -->

    <owl:NamedIndividual rdf:about="http://www.semanticweb.org/macoda/ontologies/PMOEA#WFG3_2">
        <rdf:type rdf:resource="http://www.semanticweb.org/macoda/ontologies/PMOEA#WFG"/>
        <PMOEA:isContinuousProblem rdf:datatype="http://www.w3.org/2001/XMLSchema#boolean">true</PMOEA:isContinuousProblem>
        <PMOEA:ObjectiveNumber rdf:datatype="http://www.w3.org/2001/XMLSchema#integer">2</PMOEA:ObjectiveNumber>
        <rdfs:label xml:lang="en">WFG3_2</rdfs:label>
    </owl:NamedIndividual>
    


    <!-- http://www.semanticweb.org/macoda/ontologies/PMOEA#T_Kaupler -->

    <owl:NamedIndividual rdf:about="http://www.semanticweb.org/macoda/ontologies/PMOEA#T_Kaupler">
        <rdf:type rdf:resource="http://www.semanticweb.org/macoda/ontologies/PMOEA#Researcher"/>
        <rdfs:label xml:lang="en">T.Kaupler</rdfs:label>
    </owl:NamedIndividual>
    


    <!-- http://www.semanticweb.org/macoda/ontologies/PMOEA#PMOGA -->

    <owl:NamedIndividual rdf:about="http://www.semanticweb.org/macoda/ontologies/PMOEA#PMOGA">
        <rdf:type rdf:resource="http://www.semanticweb.org/macoda/ontologies/PMOEA#PMOEA"/>
        <PMOEA:hasPreferenceModel rdf:resource="http://www.semanticweb.org/macoda/ontologies/PMOEA#PreferencePoint"/>
        <PMOEA:hasPreferenceInformationFromDM rdf:resource="http://www.semanticweb.org/macoda/ontologies/PMOEA#ReferencePoint"/>
        <PMOEA:hasInteractionTime rdf:resource="http://www.semanticweb.org/macoda/ontologies/PMOEA#a-priori"/>
        <PMOEA:hasInteractionTime rdf:resource="http://www.semanticweb.org/macoda/ontologies/PMOEA#progressive"/>
        <PMOEA:hasPreferenceIntegration rdf:resource="http://www.semanticweb.org/macoda/ontologies/PMOEA#GoalFulfilmentDominance"/>
        <PMOEA:canSolve rdf:resource="http://www.semanticweb.org/macoda/ontologies/PMOEA#PegasusGasTurbinEngineOptimization"/>
        <PMOEA:hasResultInfluence rdf:resource="http://www.semanticweb.org/macoda/ontologies/PMOEA#BoundedRegion"/>
        <PMOEA:hasAuthor rdf:resource="http://www.semanticweb.org/macoda/ontologies/PMOEA#Peter_J_Fleming"/>
        <PMOEA:hasAuthor rdf:resource="http://www.semanticweb.org/macoda/ontologies/PMOEA#Carlos_M_Fonseca"/>
        <PMOEA:hasSearchAlgorithm rdf:resource="http://www.semanticweb.org/macoda/ontologies/PMOEA#MOGA"/>
        <PMOEA:hasImplementationLanguage rdf:resource="http://www.semanticweb.org/macoda/ontologies/PMOEA#Matlab"/>
        <PMOEA:hasDevelopingYear rdf:datatype="http://www.w3.org/2001/XMLSchema#integer">1993</PMOEA:hasDevelopingYear>
        <PMOEA:ParetoDominancePreservation rdf:datatype="http://www.w3.org/2001/XMLSchema#boolean">true</PMOEA:ParetoDominancePreservation>
        <PMOEA:hasReference>Fonseca, C. M. and P. J. Fleming (1993). Genetic Algorithms for Multiobjective Optimization: FormulationDiscussion and Generalization. ICGA, Citeseer</PMOEA:hasReference>
        <rdfs:comment>the earliest EMO algorithm incorporating preferences was proposed in this paper, they proposed to introduce preferences by ranking the population according to the goals specified by the DM. The idea behind this approach is to give a higher priority to the objectives for which the goals are not fulfilled in order to improve them and push the search towards the region of interest of the Pareto optimal front</rdfs:comment>
        <rdfs:label xml:lang="en">PMOGA</rdfs:label>
    </owl:NamedIndividual>
    


    <!-- http://www.semanticweb.org/macoda/ontologies/PMOEA#SPEA2 -->

    <owl:NamedIndividual rdf:about="http://www.semanticweb.org/macoda/ontologies/PMOEA#SPEA2">
        <rdf:type rdf:resource="http://www.semanticweb.org/macoda/ontologies/PMOEA#DiversityVSConvergence_based"/>
        <rdfs:label xml:lang="en">SPEA2</rdfs:label>
    </owl:NamedIndividual>
    


    <!-- http://www.semanticweb.org/macoda/ontologies/PMOEA#ValueFunction-dominance -->

    <owl:NamedIndividual rdf:about="http://www.semanticweb.org/macoda/ontologies/PMOEA#ValueFunction-dominance">
        <rdf:type rdf:resource="http://www.semanticweb.org/macoda/ontologies/PMOEA#DominanceRelation"/>
        <rdfs:comment>a new  dominance that consiedrs VF values in PI-EMO-VF, All individuals with an estimated value (according to the approximated value function) better than the solution ranked second by the DM are assumed to dominate all the solutions with an estimated value worse than the solution ranked second. If both solutions lie either above or below the estimated indifference curves of the value function through the second best individual, they are compared based on the usual Pareto dominance.</rdfs:comment>
        <rdfs:label xml:lang="en">ValueFunction-dominance</rdfs:label>
    </owl:NamedIndividual>
    


    <!-- http://www.semanticweb.org/macoda/ontologies/PMOEA#SR-NSGA-II -->

    <owl:NamedIndividual rdf:about="http://www.semanticweb.org/macoda/ontologies/PMOEA#SR-NSGA-II">
        <rdf:type rdf:resource="http://www.semanticweb.org/macoda/ontologies/PMOEA#PMOEA"/>
        <PMOEA:hasPreferenceModel rdf:resource="http://www.semanticweb.org/macoda/ontologies/PMOEA#STOM-ASF"/>
        <PMOEA:hasPreferenceModel rdf:resource="http://www.semanticweb.org/macoda/ontologies/PMOEA#GUESS-ASF"/>
        <PMOEA:hasPreferenceModel rdf:resource="http://www.semanticweb.org/macoda/ontologies/PMOEA#basicASF"/>
        <PMOEA:hasPreferenceModel rdf:resource="http://www.semanticweb.org/macoda/ontologies/PMOEA#PreferencePoint"/>
        <PMOEA:hasPreferenceInformationFromDM rdf:resource="http://www.semanticweb.org/macoda/ontologies/PMOEA#ReferencePoint"/>
        <PMOEA:hasInteractionTime rdf:resource="http://www.semanticweb.org/macoda/ontologies/PMOEA#a-priori"/>
        <PMOEA:hasPreferenceIntegration rdf:resource="http://www.semanticweb.org/macoda/ontologies/PMOEA#CrowdingDistance"/>
        <PMOEA:canSolve rdf:resource="http://www.semanticweb.org/macoda/ontologies/PMOEA#DTLZ3_3"/>
        <PMOEA:canSolve rdf:resource="http://www.semanticweb.org/macoda/ontologies/PMOEA#DTLZ5_3"/>
        <PMOEA:canSolve rdf:resource="http://www.semanticweb.org/macoda/ontologies/PMOEA#DTLZ6_3"/>
        <PMOEA:canSolve rdf:resource="http://www.semanticweb.org/macoda/ontologies/PMOEA#ZDT2"/>
        <PMOEA:canSolve rdf:resource="http://www.semanticweb.org/macoda/ontologies/PMOEA#DTLZ4_3"/>
        <PMOEA:canSolve rdf:resource="http://www.semanticweb.org/macoda/ontologies/PMOEA#ZDT6"/>
        <PMOEA:canSolve rdf:resource="http://www.semanticweb.org/macoda/ontologies/PMOEA#ZDT4"/>
        <PMOEA:canSolve rdf:resource="http://www.semanticweb.org/macoda/ontologies/PMOEA#DTLZ1_3"/>
        <PMOEA:canSolve rdf:resource="http://www.semanticweb.org/macoda/ontologies/PMOEA#ZDT3"/>
        <PMOEA:canSolve rdf:resource="http://www.semanticweb.org/macoda/ontologies/PMOEA#DTLZ2_3"/>
        <PMOEA:canSolve rdf:resource="http://www.semanticweb.org/macoda/ontologies/PMOEA#ZDT1"/>
        <PMOEA:hasResultInfluence rdf:resource="http://www.semanticweb.org/macoda/ontologies/PMOEA#SetOfSolutions"/>
        <PMOEA:hasAuthor rdf:resource="http://www.semanticweb.org/macoda/ontologies/PMOEA#Ernestas_Filatovas"/>
        <PMOEA:hasAuthor rdf:resource="http://www.semanticweb.org/macoda/ontologies/PMOEA#Olga_Kurasova"/>
        <PMOEA:isExtensionOf rdf:resource="http://www.semanticweb.org/macoda/ontologies/PMOEA#R-NSGA-II"/>
        <PMOEA:hasSearchAlgorithm rdf:resource="http://www.semanticweb.org/macoda/ontologies/PMOEA#NSGA-II"/>
        <PMOEA:hasDevelopingYear rdf:datatype="http://www.w3.org/2001/XMLSchema#integer">2015</PMOEA:hasDevelopingYear>
        <PMOEA:SpreadControl rdf:datatype="http://www.w3.org/2001/XMLSchema#boolean">true</PMOEA:SpreadControl>
        <PMOEA:ParetoDominancePreservation rdf:datatype="http://www.w3.org/2001/XMLSchema#boolean">true</PMOEA:ParetoDominancePreservation>
        <PMOEA:hasReference>Filatovas, Ernestas, Olga Kurasova, and Karthik Sindhya. &quot;Synchronous R-NSGA-II: an extended preference-based evolutionary algorithm for multi-objective optimization.&quot; Informatica 26.1 (2015): 33-50.</PMOEA:hasReference>
        <rdfs:comment>In this paper, we propose a new evolutionary preference-based algorithm where several scalarizing functions are used simultaneously. Concepts from the interactive reference point method  synchronous NIMBUS (Miettinen and Makela, 2006)  are borrowed and combined with the R-NSGA-II algorithm</rdfs:comment>
        <rdfs:label xml:lang="en">SR-NSGA-II</rdfs:label>
    </owl:NamedIndividual>
    


    <!-- http://www.semanticweb.org/macoda/ontologies/PMOEA#WFG4_8 -->

    <owl:NamedIndividual rdf:about="http://www.semanticweb.org/macoda/ontologies/PMOEA#WFG4_8">
        <rdf:type rdf:resource="http://www.semanticweb.org/macoda/ontologies/PMOEA#WFG"/>
        <PMOEA:OWLDataProperty_61d3cd95_fde4_4c1b_af08_1eaf73473aea rdf:datatype="http://www.w3.org/2001/XMLSchema#boolean">true</PMOEA:OWLDataProperty_61d3cd95_fde4_4c1b_af08_1eaf73473aea>
        <PMOEA:isContinuousProblem rdf:datatype="http://www.w3.org/2001/XMLSchema#boolean">true</PMOEA:isContinuousProblem>
        <PMOEA:ObjectiveNumber rdf:datatype="http://www.w3.org/2001/XMLSchema#integer">8</PMOEA:ObjectiveNumber>
        <PMOEA:isManyObjectiveProblem rdf:datatype="http://www.w3.org/2001/XMLSchema#boolean">true</PMOEA:isManyObjectiveProblem>
        <rdfs:label xml:lang="en">WFG4_8</rdfs:label>
    </owl:NamedIndividual>
    


    <!-- http://www.semanticweb.org/macoda/ontologies/PMOEA#FitnessSetting -->

    <owl:NamedIndividual rdf:about="http://www.semanticweb.org/macoda/ontologies/PMOEA#FitnessSetting">
        <rdf:type rdf:resource="http://www.semanticweb.org/macoda/ontologies/PMOEA#Fitness"/>
        <rdfs:comment>The way to set fitness for each solution, apart from the original objectives.</rdfs:comment>
        <rdfs:label xml:lang="en">FitnessSetting</rdfs:label>
    </owl:NamedIndividual>
    


    <!-- http://www.semanticweb.org/macoda/ontologies/PMOEA#CurvaturebasedCone -->

    <owl:NamedIndividual rdf:about="http://www.semanticweb.org/macoda/ontologies/PMOEA#CurvaturebasedCone">
        <rdf:type rdf:resource="http://www.semanticweb.org/macoda/ontologies/PMOEA#PolyhedralConeBased"/>
        <rdfs:comment>In many real-world MOPs from engineering design and financial applications, it is common to impose additional restrictions on the Pareto-optimal set,  like trade-offs limits, or additional properties/ axioms (like fairness or equitability). Consolidating these additional requirements with the axioms of Pareto-ordering gives a preference model ,proper Pareto optimality</rdfs:comment>
        <rdfs:label xml:lang="en">CurvaturebasedCone</rdfs:label>
    </owl:NamedIndividual>
    


    <!-- http://www.semanticweb.org/macoda/ontologies/PMOEA#FuzzyMeasure -->

    <owl:NamedIndividual rdf:about="http://www.semanticweb.org/macoda/ontologies/PMOEA#FuzzyMeasure">
        <rdf:type rdf:resource="http://www.semanticweb.org/macoda/ontologies/PMOEA#FuzzyLogic"/>
        <rdfs:comment>A fuzzy measure  defined on (x),f(x)) is a set function g : f(x)  [0, 1] satisfying Boundary condition and Monotonicity and classified as belief measure, plausibility measure, probability measure, etc.</rdfs:comment>
        <rdfs:label xml:lang="en">FuzzyMeasure</rdfs:label>
    </owl:NamedIndividual>
    


    <!-- http://www.semanticweb.org/macoda/ontologies/PMOEA#DF-MOPSO -->

    <owl:NamedIndividual rdf:about="http://www.semanticweb.org/macoda/ontologies/PMOEA#DF-MOPSO">
        <rdf:type rdf:resource="http://www.semanticweb.org/macoda/ontologies/PMOEA#PMOEA"/>
        <PMOEA:hasPreferenceModel rdf:resource="http://www.semanticweb.org/macoda/ontologies/PMOEA#HarringtonsDF"/>
        <PMOEA:hasPreferenceInformationFromDM rdf:resource="http://www.semanticweb.org/macoda/ontologies/PMOEA#parametersInDF"/>
        <PMOEA:hasInteractionTime rdf:resource="http://www.semanticweb.org/macoda/ontologies/PMOEA#a-priori"/>
        <PMOEA:hasPreferenceIntegration rdf:resource="http://www.semanticweb.org/macoda/ontologies/PMOEA#LeaderParticleSelection"/>
        <PMOEA:hasPreferenceIntegration rdf:resource="http://www.semanticweb.org/macoda/ontologies/PMOEA#ObjectiveTransformation"/>
        <PMOEA:canSolve rdf:resource="http://www.semanticweb.org/macoda/ontologies/PMOEA#S-ZDT2"/>
        <PMOEA:canSolve rdf:resource="http://www.semanticweb.org/macoda/ontologies/PMOEA#S-ZDT1"/>
        <PMOEA:canSolve rdf:resource="http://www.semanticweb.org/macoda/ontologies/PMOEA#FF"/>
        <PMOEA:hasAuthor rdf:resource="http://www.semanticweb.org/macoda/ontologies/PMOEA#Olaf_Mersmann"/>
        <PMOEA:hasAuthor rdf:resource="http://www.semanticweb.org/macoda/ontologies/PMOEA#Sanaz_Mostaghim"/>
        <PMOEA:hasAuthor rdf:resource="http://www.semanticweb.org/macoda/ontologies/PMOEA#Heike_Trautmann"/>
        <PMOEA:hasSearchAlgorithm rdf:resource="http://www.semanticweb.org/macoda/ontologies/PMOEA#MOPSO"/>
        <PMOEA:hasDevelopingYear rdf:datatype="http://www.w3.org/2001/XMLSchema#integer">2010</PMOEA:hasDevelopingYear>
        <PMOEA:hasReference>Mostaghim, S., H. Trautmann and O. Mersmann (2010). Preference-based multi-objective particle swarm optimization using desirabilities. Parallel Problem Solving from Nature, PPSN XI, Springer: 101-110</PMOEA:hasReference>
        <rdfs:comment>We transform the objective functions to the Harringtons one sided DF functions. Hence, from this point the DF-MOPSO algorithm optimizes the converted functions meaning (1) the definition of domination changes to the transformed functions, (2) the selection of personal best solutions is based on the transformed objective values and (3) the solution with the largest DI value is selected as the only global best for the population.</rdfs:comment>
        <rdfs:label xml:lang="en">DF-MOPSO</rdfs:label>
    </owl:NamedIndividual>
    


    <!-- http://www.semanticweb.org/macoda/ontologies/PMOEA#C -->

    <owl:NamedIndividual rdf:about="http://www.semanticweb.org/macoda/ontologies/PMOEA#C">
        <rdf:type rdf:resource="http://www.semanticweb.org/macoda/ontologies/PMOEA#ProgrammingLanguage"/>
        <rdfs:label xml:lang="en">C</rdfs:label>
    </owl:NamedIndividual>
    


    <!-- http://www.semanticweb.org/macoda/ontologies/PMOEA#Dragan_A_Savic -->

    <owl:NamedIndividual rdf:about="http://www.semanticweb.org/macoda/ontologies/PMOEA#Dragan_A_Savic">
        <rdf:type rdf:resource="http://www.semanticweb.org/macoda/ontologies/PMOEA#Researcher"/>
        <rdfs:label xml:lang="en">Dragan A. Savic</rdfs:label>
    </owl:NamedIndividual>
    


    <!-- http://www.semanticweb.org/macoda/ontologies/PMOEA#Kay_Chen_Tan -->

    <owl:NamedIndividual rdf:about="http://www.semanticweb.org/macoda/ontologies/PMOEA#Kay_Chen_Tan">
        <rdf:type rdf:resource="http://www.semanticweb.org/macoda/ontologies/PMOEA#Researcher"/>
        <rdfs:label xml:lang="en">Kay Chen Tan</rdfs:label>
    </owl:NamedIndividual>
    


    <!-- http://www.semanticweb.org/macoda/ontologies/PMOEA#Gunter_Ridolph -->

    <owl:NamedIndividual rdf:about="http://www.semanticweb.org/macoda/ontologies/PMOEA#Gunter_Ridolph">
        <rdf:type rdf:resource="http://www.semanticweb.org/macoda/ontologies/PMOEA#Researcher"/>
        <rdfs:label xml:lang="en">Gunter Ridolph</rdfs:label>
    </owl:NamedIndividual>
    


    <!-- http://www.semanticweb.org/macoda/ontologies/PMOEA#DTLZ6_4 -->

    <owl:NamedIndividual rdf:about="http://www.semanticweb.org/macoda/ontologies/PMOEA#DTLZ6_4">
        <rdf:type rdf:resource="http://www.semanticweb.org/macoda/ontologies/PMOEA#DTLZ"/>
        <PMOEA:isContinuousProblem rdf:datatype="http://www.w3.org/2001/XMLSchema#boolean">true</PMOEA:isContinuousProblem>
        <PMOEA:ObjectiveNumber rdf:datatype="http://www.w3.org/2001/XMLSchema#integer">4</PMOEA:ObjectiveNumber>
        <PMOEA:isManyObjectiveProblem rdf:datatype="http://www.w3.org/2001/XMLSchema#boolean">true</PMOEA:isManyObjectiveProblem>
        <rdfs:label xml:lang="en">DTLZ6_4</rdfs:label>
    </owl:NamedIndividual>
    


    <!-- http://www.semanticweb.org/macoda/ontologies/PMOEA#ZDT2 -->

    <owl:NamedIndividual rdf:about="http://www.semanticweb.org/macoda/ontologies/PMOEA#ZDT2">
        <rdf:type rdf:resource="http://www.semanticweb.org/macoda/ontologies/PMOEA#ZDT"/>
        <PMOEA:isContinuousProblem rdf:datatype="http://www.w3.org/2001/XMLSchema#boolean">true</PMOEA:isContinuousProblem>
        <PMOEA:ObjectiveNumber rdf:datatype="http://www.w3.org/2001/XMLSchema#integer">2</PMOEA:ObjectiveNumber>
        <rdfs:label xml:lang="en">ZDT2</rdfs:label>
    </owl:NamedIndividual>
    


    <!-- http://www.semanticweb.org/macoda/ontologies/PMOEA#PairwiseComparisonMatrix -->

    <owl:NamedIndividual rdf:about="http://www.semanticweb.org/macoda/ontologies/PMOEA#PairwiseComparisonMatrix">
        <rdf:type rdf:resource="http://www.semanticweb.org/macoda/ontologies/PMOEA#ObjectiveComparison"/>
        <rdfs:comment>The pairwise comparison matrix of criteria, which represents preference degrees between criteria, is defined as [pij] ,wherepij represents the preference degree between i-th criterion and j-th criterion,For example, if p12 is 5, it means f1 is five times more preferred to f2.</rdfs:comment>
        <rdfs:label xml:lang="en">PairwiseComparisonMatrix</rdfs:label>
    </owl:NamedIndividual>
    


    <!-- http://www.semanticweb.org/macoda/ontologies/PMOEA#iMOEA/D -->

    <owl:NamedIndividual rdf:about="http://www.semanticweb.org/macoda/ontologies/PMOEA#iMOEA/D">
        <rdf:type rdf:resource="http://www.semanticweb.org/macoda/ontologies/PMOEA#PMOEA"/>
        <PMOEA:hasPreferenceModel rdf:resource="http://www.semanticweb.org/macoda/ontologies/PMOEA#TchebycheffASF"/>
        <PMOEA:hasPreferenceInformationFromDM rdf:resource="http://www.semanticweb.org/macoda/ontologies/PMOEA#PickTheBest"/>
        <PMOEA:hasInteractionTime rdf:resource="http://www.semanticweb.org/macoda/ontologies/PMOEA#progressive"/>
        <PMOEA:hasPreferenceIntegration rdf:resource="http://www.semanticweb.org/macoda/ontologies/PMOEA#WeightsInASF"/>
        <PMOEA:canSolve rdf:resource="http://www.semanticweb.org/macoda/ontologies/PMOEA#ZDT2"/>
        <PMOEA:canSolve rdf:resource="http://www.semanticweb.org/macoda/ontologies/PMOEA#DTLZ1_3"/>
        <PMOEA:canSolve rdf:resource="http://www.semanticweb.org/macoda/ontologies/PMOEA#DTLZ2_3"/>
        <PMOEA:canSolve rdf:resource="http://www.semanticweb.org/macoda/ontologies/PMOEA#ZDT1"/>
        <PMOEA:canSolve rdf:resource="http://www.semanticweb.org/macoda/ontologies/PMOEA#WeldedBeamDesign"/>
        <PMOEA:hasResultInfluence rdf:resource="http://www.semanticweb.org/macoda/ontologies/PMOEA#BoundedRegion"/>
        <PMOEA:hasAuthor rdf:resource="http://www.semanticweb.org/macoda/ontologies/PMOEA#Maoguo_Gong"/>
        <PMOEA:hasAuthor rdf:resource="http://www.semanticweb.org/macoda/ontologies/PMOEA#Fang_Liu"/>
        <PMOEA:hasAuthor rdf:resource="http://www.semanticweb.org/macoda/ontologies/PMOEA#Licheng_Jiao"/>
        <PMOEA:hasAuthor rdf:resource="http://www.semanticweb.org/macoda/ontologies/PMOEA#Qingfu_Zhang"/>
        <PMOEA:hasAuthor rdf:resource="http://www.semanticweb.org/macoda/ontologies/PMOEA#Wei_Zhang"/>
        <PMOEA:hasSearchAlgorithm rdf:resource="http://www.semanticweb.org/macoda/ontologies/PMOEA#MOEA-D"/>
        <PMOEA:hasDevelopingYear rdf:datatype="http://www.w3.org/2001/XMLSchema#integer">2011</PMOEA:hasDevelopingYear>
        <PMOEA:hasReference>Gong, M., F. Liu, W. Zhang, L. Jiao and Q. Zhang (2011). Interactive MOEA/D for multi-objective decision making. Proceedings of the 13th annual conference on Genetic and evolutionary computation, ACM</PMOEA:hasReference>
        <rdfs:comment>an interactive version of the well-known MOEA/D method [25], where a set of solutions is shown to the DM at intermediate generations, who must choose one of them. Then, the search is guided to the  neighbourhood of the selected solution by relocating the weight vectors which determine the search directions</rdfs:comment>
        <rdfs:label xml:lang="en">iMOEA/D</rdfs:label>
    </owl:NamedIndividual>
    


    <!-- http://www.semanticweb.org/macoda/ontologies/PMOEA#GeneralUtilityFunction -->

    <owl:NamedIndividual rdf:about="http://www.semanticweb.org/macoda/ontologies/PMOEA#GeneralUtilityFunction">
        <rdf:type rdf:resource="http://www.semanticweb.org/macoda/ontologies/PMOEA#UtilityFunction"/>
        <rdfs:label xml:lang="en">GeneralUtilityFunction</rdfs:label>
    </owl:NamedIndividual>
    


    <!-- http://www.semanticweb.org/macoda/ontologies/PMOEA#DTLZ3_7 -->

    <owl:NamedIndividual rdf:about="http://www.semanticweb.org/macoda/ontologies/PMOEA#DTLZ3_7">
        <rdf:type rdf:resource="http://www.semanticweb.org/macoda/ontologies/PMOEA#DTLZ"/>
        <PMOEA:OWLDataProperty_61d3cd95_fde4_4c1b_af08_1eaf73473aea rdf:datatype="http://www.w3.org/2001/XMLSchema#boolean">true</PMOEA:OWLDataProperty_61d3cd95_fde4_4c1b_af08_1eaf73473aea>
        <PMOEA:isContinuousProblem rdf:datatype="http://www.w3.org/2001/XMLSchema#boolean">true</PMOEA:isContinuousProblem>
        <PMOEA:ObjectiveNumber rdf:datatype="http://www.w3.org/2001/XMLSchema#integer">7</PMOEA:ObjectiveNumber>
        <PMOEA:isManyObjectiveProblem rdf:datatype="http://www.w3.org/2001/XMLSchema#boolean">true</PMOEA:isManyObjectiveProblem>
        <rdfs:label xml:lang="en">DTLZ3_7</rdfs:label>
    </owl:NamedIndividual>
    


    <!-- http://www.semanticweb.org/macoda/ontologies/PMOEA#ParatemtersInR2Indicator -->

    <owl:NamedIndividual rdf:about="http://www.semanticweb.org/macoda/ontologies/PMOEA#ParatemtersInR2Indicator">
        <rdf:type rdf:resource="http://www.semanticweb.org/macoda/ontologies/PMOEA#Indicator"/>
        <rdfs:comment>position of reference point, restriction of the weight space, density of weight vector can be used to articulate preference</rdfs:comment>
        <rdfs:label xml:lang="en">ParatemtersInR2Indicator</rdfs:label>
    </owl:NamedIndividual>
    


    <!-- http://www.semanticweb.org/macoda/ontologies/PMOEA#W_IBEA -->

    <owl:NamedIndividual rdf:about="http://www.semanticweb.org/macoda/ontologies/PMOEA#W_IBEA">
        <rdf:type rdf:resource="http://www.semanticweb.org/macoda/ontologies/PMOEA#PMOEA"/>
        <PMOEA:hasPreferenceModel rdf:resource="http://www.semanticweb.org/macoda/ontologies/PMOEA#ObjectiveSpaceWeightDistribution"/>
        <PMOEA:hasPreferenceInformationFromDM rdf:resource="http://www.semanticweb.org/macoda/ontologies/PMOEA#ExponentialFunctionPreferOneObjective"/>
        <PMOEA:hasPreferenceInformationFromDM rdf:resource="http://www.semanticweb.org/macoda/ontologies/PMOEA#Ridge-likeFunctionPreferOneReferencePoint"/>
        <PMOEA:hasPreferenceInformationFromDM rdf:resource="http://www.semanticweb.org/macoda/ontologies/PMOEA#ExponentialFunctionPreferExtremalSolutions"/>
        <PMOEA:hasInteractionTime rdf:resource="http://www.semanticweb.org/macoda/ontologies/PMOEA#a-priori"/>
        <PMOEA:hasPreferenceIntegration rdf:resource="http://www.semanticweb.org/macoda/ontologies/PMOEA#HypervolumeIndicator"/>
        <PMOEA:canSolve rdf:resource="http://www.semanticweb.org/macoda/ontologies/PMOEA#ZDT6"/>
        <PMOEA:canSolve rdf:resource="http://www.semanticweb.org/macoda/ontologies/PMOEA#ZDT3"/>
        <PMOEA:canSolve rdf:resource="http://www.semanticweb.org/macoda/ontologies/PMOEA#ZDT1"/>
        <PMOEA:hasResultInfluence rdf:resource="http://www.semanticweb.org/macoda/ontologies/PMOEA#BiasedDistribution"/>
        <PMOEA:hasAuthor rdf:resource="http://www.semanticweb.org/macoda/ontologies/PMOEA#Lothar_Thiele"/>
        <PMOEA:hasAuthor rdf:resource="http://www.semanticweb.org/macoda/ontologies/PMOEA#Dimo_Brockhoff"/>
        <PMOEA:hasAuthor rdf:resource="http://www.semanticweb.org/macoda/ontologies/PMOEA#Eckart_Zitzler"/>
        <PMOEA:hasSearchAlgorithm rdf:resource="http://www.semanticweb.org/macoda/ontologies/PMOEA#IBEA"/>
        <PMOEA:hasDevelopingYear rdf:datatype="http://www.w3.org/2001/XMLSchema#integer">2007</PMOEA:hasDevelopingYear>
        <PMOEA:MultipleRegionOfInterest rdf:datatype="http://www.w3.org/2001/XMLSchema#boolean">false</PMOEA:MultipleRegionOfInterest>
        <PMOEA:SpreadControl rdf:datatype="http://www.w3.org/2001/XMLSchema#boolean">false</PMOEA:SpreadControl>
        <PMOEA:ParetoDominancePreservation rdf:datatype="http://www.w3.org/2001/XMLSchema#boolean">true</PMOEA:ParetoDominancePreservation>
        <PMOEA:hasReference>Zitzler, E., D. Brockhoff and L. Thiele (2007). The hypervolume indicator revisited: On the design of Pareto-compliant indicators via weighted integration. Evolutionary multi-criterion optimization, Springer</PMOEA:hasReference>
        <rdfs:comment>The key contributions are:  A generalized definition of the hypervolume indicator using attainment functions that can be used for any type of dominance relation; A weighted-integration approach to directly manipulate and control the influence of certain regions in the objective space for the hypervolume indicator;  Three new example set measures for biobjective problems that provide the same sensitivity as the hypervolume indicator, but represent different types of preference information: (i) the preference of extreme solutions, (ii) the preference of predefined reference points, and (iii) bias towards one of the objectives</rdfs:comment>
        <rdfs:label xml:lang="en">W_IBEA</rdfs:label>
    </owl:NamedIndividual>
    


    <!-- http://www.semanticweb.org/macoda/ontologies/PMOEA#ObjectivePriorityVector -->

    <owl:NamedIndividual rdf:about="http://www.semanticweb.org/macoda/ontologies/PMOEA#ObjectivePriorityVector">
        <rdf:type rdf:resource="http://www.semanticweb.org/macoda/ontologies/PMOEA#ObjectiveComparison"/>
        <rdfs:comment>the settings of Pf = [1, 1, 2, 2]  for a 4-objective optimization problem indicate that the first and second objective components are given top priority to be minimized, as much as possible, before considering minimization of the third and fourth objective components</rdfs:comment>
        <rdfs:label xml:lang="en">ObjectivePriorityVector</rdfs:label>
    </owl:NamedIndividual>
    


    <!-- http://www.semanticweb.org/macoda/ontologies/PMOEA#TDEA -->

    <owl:NamedIndividual rdf:about="http://www.semanticweb.org/macoda/ontologies/PMOEA#TDEA">
        <rdf:type rdf:resource="http://www.semanticweb.org/macoda/ontologies/PMOEA#DiversityVSConvergence_based"/>
        <rdfs:comment>This algorithm maintains two populations. A regular population which may contain both dominated and nondominated individuals and an archive population which contains only nondominated individuals.  In each generation, a single offspring is created than elvaluated whether it can replace solutions in the two populations. A territory of size  is defined around the archive individual closest to the offspring. A nondominated offspring is only accepted if it does not violate this territory. This territory defining property maintains the diversity of the archive population.</rdfs:comment>
        <rdfs:label xml:lang="en">TDEA</rdfs:label>
    </owl:NamedIndividual>
    


    <!-- http://www.semanticweb.org/macoda/ontologies/PMOEA#BinhProblem -->

    <owl:NamedIndividual rdf:about="http://www.semanticweb.org/macoda/ontologies/PMOEA#BinhProblem">
        <rdf:type rdf:resource="http://www.semanticweb.org/macoda/ontologies/PMOEA#Academic_Problem"/>
        <PMOEA:isContinuousProblem rdf:datatype="http://www.w3.org/2001/XMLSchema#boolean">true</PMOEA:isContinuousProblem>
        <PMOEA:ObjectiveNumber rdf:datatype="http://www.w3.org/2001/XMLSchema#integer">2</PMOEA:ObjectiveNumber>
        <rdfs:label xml:lang="en">BinhProblem</rdfs:label>
    </owl:NamedIndividual>
    


    <!-- http://www.semanticweb.org/macoda/ontologies/PMOEA#DTLZ2_5 -->

    <owl:NamedIndividual rdf:about="http://www.semanticweb.org/macoda/ontologies/PMOEA#DTLZ2_5">
        <rdf:type rdf:resource="http://www.semanticweb.org/macoda/ontologies/PMOEA#DTLZ"/>
        <PMOEA:isContinuousProblem rdf:datatype="http://www.w3.org/2001/XMLSchema#boolean">true</PMOEA:isContinuousProblem>
        <PMOEA:ObjectiveNumber rdf:datatype="http://www.w3.org/2001/XMLSchema#integer">5</PMOEA:ObjectiveNumber>
        <PMOEA:isManyObjectiveProblem rdf:datatype="http://www.w3.org/2001/XMLSchema#boolean">true</PMOEA:isManyObjectiveProblem>
        <rdfs:label xml:lang="en">DTLZ2_5</rdfs:label>
    </owl:NamedIndividual>
    


    <!-- http://www.semanticweb.org/macoda/ontologies/PMOEA#Peter_J_Fleming -->

    <owl:NamedIndividual rdf:about="http://www.semanticweb.org/macoda/ontologies/PMOEA#Peter_J_Fleming">
        <rdf:type rdf:resource="http://www.semanticweb.org/macoda/ontologies/PMOEA#Researcher"/>
        <rdfs:label xml:lang="en">Peter J. Fleming</rdfs:label>
    </owl:NamedIndividual>
    


    <!-- http://www.semanticweb.org/macoda/ontologies/PMOEA#Ji-Hyeong_Han -->

    <owl:NamedIndividual rdf:about="http://www.semanticweb.org/macoda/ontologies/PMOEA#Ji-Hyeong_Han">
        <rdf:type rdf:resource="http://www.semanticweb.org/macoda/ontologies/PMOEA#Researcher"/>
        <rdfs:label xml:lang="en">Ji-Hyeong Han</rdfs:label>
    </owl:NamedIndividual>
    


    <!-- http://www.semanticweb.org/macoda/ontologies/PMOEA#PickTheBest -->

    <owl:NamedIndividual rdf:about="http://www.semanticweb.org/macoda/ontologies/PMOEA#PickTheBest">
        <rdf:type rdf:resource="http://www.semanticweb.org/macoda/ontologies/PMOEA#SampleRanks"/>
        <rdfs:label xml:lang="en">PickTheBest</rdfs:label>
    </owl:NamedIndividual>
    


    <!-- http://www.semanticweb.org/macoda/ontologies/PMOEA#Selcen_Phelps -->

    <owl:NamedIndividual rdf:about="http://www.semanticweb.org/macoda/ontologies/PMOEA#Selcen_Phelps">
        <rdf:type rdf:resource="http://www.semanticweb.org/macoda/ontologies/PMOEA#Researcher"/>
        <rdfs:label xml:lang="en">Selcen Phelps</rdfs:label>
    </owl:NamedIndividual>
    


    <!-- http://www.semanticweb.org/macoda/ontologies/PMOEA#INSPM -->

    <owl:NamedIndividual rdf:about="http://www.semanticweb.org/macoda/ontologies/PMOEA#INSPM">
        <rdf:type rdf:resource="http://www.semanticweb.org/macoda/ontologies/PMOEA#PMOEA"/>
        <PMOEA:hasInteractionTime rdf:resource="http://www.semanticweb.org/macoda/ontologies/PMOEA#progressive"/>
        <PMOEA:hasDevelopingYear rdf:datatype="http://www.w3.org/2001/XMLSchema#integer">2014</PMOEA:hasDevelopingYear>
        <PMOEA:hasReference>Pedro, Luciana R., and Ricardo HC Takahashi. &quot;INSPM: An interactive evolutionary multi-objective algorithm with preference model.&quot; Information Sciences 268 (2014): 202-219.</PMOEA:hasReference>
        <rdfs:comment>a Radial Basis Function (RBF) network is employed to construct a function which represents the DMs utility function using ordinal information only, extracted from queries to the DM. The INSPM algorithm calls the DMs preference model via a Dynamic Crowding Distance (DCD) density control method which provides the mechanism for increasing the sampling in the preferred regions and for decreasing it in non-preferred regions which allows a fine-tunning control of the Pareto-optimal front sampling density</rdfs:comment>
        <rdfs:label xml:lang="en">INSPM</rdfs:label>
    </owl:NamedIndividual>
    


    <!-- http://www.semanticweb.org/macoda/ontologies/PMOEA#DTLZ4_3 -->

    <owl:NamedIndividual rdf:about="http://www.semanticweb.org/macoda/ontologies/PMOEA#DTLZ4_3">
        <rdf:type rdf:resource="http://www.semanticweb.org/macoda/ontologies/PMOEA#DTLZ"/>
        <PMOEA:isContinuousProblem rdf:datatype="http://www.w3.org/2001/XMLSchema#boolean">true</PMOEA:isContinuousProblem>
        <PMOEA:ObjectiveNumber rdf:datatype="http://www.w3.org/2001/XMLSchema#integer">3</PMOEA:ObjectiveNumber>
        <rdfs:label xml:lang="en">DTLZ4_3</rdfs:label>
    </owl:NamedIndividual>
    


    <!-- http://www.semanticweb.org/macoda/ontologies/PMOEA#Benedetto_Matarazzo -->

    <owl:NamedIndividual rdf:about="http://www.semanticweb.org/macoda/ontologies/PMOEA#Benedetto_Matarazzo">
        <rdf:type rdf:resource="http://www.semanticweb.org/macoda/ontologies/PMOEA#Researcher"/>
        <rdfs:label xml:lang="en">Benedetto Matarazzo</rdfs:label>
    </owl:NamedIndividual>
    


    <!-- http://www.semanticweb.org/macoda/ontologies/PMOEA#MatingSelection -->

    <owl:NamedIndividual rdf:about="http://www.semanticweb.org/macoda/ontologies/PMOEA#MatingSelection">
        <rdf:type rdf:resource="http://www.semanticweb.org/macoda/ontologies/PMOEA#SelectionCriterion"/>
        <rdfs:comment>a binary tournament selection strategy using three tournament strategies, namely, dominance comparison, knee point criterion, and a weighted distance, in KnEA</rdfs:comment>
        <rdfs:label xml:lang="en">MatingSelection</rdfs:label>
    </owl:NamedIndividual>
    


    <!-- http://www.semanticweb.org/macoda/ontologies/PMOEA#DTLZ7_8 -->

    <owl:NamedIndividual rdf:about="http://www.semanticweb.org/macoda/ontologies/PMOEA#DTLZ7_8">
        <rdf:type rdf:resource="http://www.semanticweb.org/macoda/ontologies/PMOEA#DTLZ"/>
        <PMOEA:isContinuousProblem rdf:datatype="http://www.w3.org/2001/XMLSchema#boolean">true</PMOEA:isContinuousProblem>
        <PMOEA:ObjectiveNumber rdf:datatype="http://www.w3.org/2001/XMLSchema#integer">8</PMOEA:ObjectiveNumber>
        <PMOEA:isManyObjectiveProblem rdf:datatype="http://www.w3.org/2001/XMLSchema#boolean">true</PMOEA:isManyObjectiveProblem>
        <rdfs:label xml:lang="en">DTLZ7_8</rdfs:label>
    </owl:NamedIndividual>
    


    <!-- http://www.semanticweb.org/macoda/ontologies/PMOEA#KnEA -->

    <owl:NamedIndividual rdf:about="http://www.semanticweb.org/macoda/ontologies/PMOEA#KnEA">
        <rdf:type rdf:resource="http://www.semanticweb.org/macoda/ontologies/PMOEA#PMOEA"/>
        <PMOEA:hasPreferenceModel rdf:resource="http://www.semanticweb.org/macoda/ontologies/PMOEA#Knee-point"/>
        <PMOEA:hasInteractionTime rdf:resource="http://www.semanticweb.org/macoda/ontologies/PMOEA#a-priori"/>
        <PMOEA:hasPreferenceIntegration rdf:resource="http://www.semanticweb.org/macoda/ontologies/PMOEA#MatingSelection"/>
        <PMOEA:canSolve rdf:resource="http://www.semanticweb.org/macoda/ontologies/PMOEA#DTLZ3_4"/>
        <PMOEA:canSolve rdf:resource="http://www.semanticweb.org/macoda/ontologies/PMOEA#DTLZ3_6"/>
        <PMOEA:canSolve rdf:resource="http://www.semanticweb.org/macoda/ontologies/PMOEA#DTLZ5_4"/>
        <PMOEA:canSolve rdf:resource="http://www.semanticweb.org/macoda/ontologies/PMOEA#DTLZ5_6"/>
        <PMOEA:canSolve rdf:resource="http://www.semanticweb.org/macoda/ontologies/PMOEA#DTLZ3_8"/>
        <PMOEA:canSolve rdf:resource="http://www.semanticweb.org/macoda/ontologies/PMOEA#DTLZ5_2"/>
        <PMOEA:canSolve rdf:resource="http://www.semanticweb.org/macoda/ontologies/PMOEA#DTLZ5_8"/>
        <PMOEA:canSolve rdf:resource="http://www.semanticweb.org/macoda/ontologies/PMOEA#WFG1_2"/>
        <PMOEA:canSolve rdf:resource="http://www.semanticweb.org/macoda/ontologies/PMOEA#WFG4_8"/>
        <PMOEA:canSolve rdf:resource="http://www.semanticweb.org/macoda/ontologies/PMOEA#DTLZ6_4"/>
        <PMOEA:canSolve rdf:resource="http://www.semanticweb.org/macoda/ontologies/PMOEA#DTLZ7_8"/>
        <PMOEA:canSolve rdf:resource="http://www.semanticweb.org/macoda/ontologies/PMOEA#DTLZ6_10"/>
        <PMOEA:canSolve rdf:resource="http://www.semanticweb.org/macoda/ontologies/PMOEA#DTLZ5_10"/>
        <PMOEA:canSolve rdf:resource="http://www.semanticweb.org/macoda/ontologies/PMOEA#DTLZ7_4"/>
        <PMOEA:canSolve rdf:resource="http://www.semanticweb.org/macoda/ontologies/PMOEA#DTLZ1_4"/>
        <PMOEA:canSolve rdf:resource="http://www.semanticweb.org/macoda/ontologies/PMOEA#DTLZ1_6"/>
        <PMOEA:canSolve rdf:resource="http://www.semanticweb.org/macoda/ontologies/PMOEA#DTLZ1_2"/>
        <PMOEA:canSolve rdf:resource="http://www.semanticweb.org/macoda/ontologies/PMOEA#DTLZ3_10"/>
        <PMOEA:canSolve rdf:resource="http://www.semanticweb.org/macoda/ontologies/PMOEA#DTLZ7_6"/>
        <PMOEA:canSolve rdf:resource="http://www.semanticweb.org/macoda/ontologies/PMOEA#DTLZ1_8"/>
        <PMOEA:canSolve rdf:resource="http://www.semanticweb.org/macoda/ontologies/PMOEA#DTLZ6_6"/>
        <PMOEA:canSolve rdf:resource="http://www.semanticweb.org/macoda/ontologies/PMOEA#WFG9_10"/>
        <PMOEA:canSolve rdf:resource="http://www.semanticweb.org/macoda/ontologies/PMOEA#DTLZ1_10"/>
        <PMOEA:canSolve rdf:resource="http://www.semanticweb.org/macoda/ontologies/PMOEA#DTLZ3_2"/>
        <PMOEA:canSolve rdf:resource="http://www.semanticweb.org/macoda/ontologies/PMOEA#DTLZ7_2"/>
        <PMOEA:canSolve rdf:resource="http://www.semanticweb.org/macoda/ontologies/PMOEA#DTLZ7_10"/>
        <PMOEA:hasResultInfluence rdf:resource="http://www.semanticweb.org/macoda/ontologies/PMOEA#SetOfSolutions"/>
        <PMOEA:hasSearchAlgorithm rdf:resource="http://www.semanticweb.org/macoda/ontologies/PMOEA#NSGA-II"/>
        <PMOEA:hasDevelopingYear rdf:datatype="http://www.w3.org/2001/XMLSchema#integer">2015</PMOEA:hasDevelopingYear>
        <PMOEA:ParetoDominancePreservation rdf:datatype="http://www.w3.org/2001/XMLSchema#boolean">true</PMOEA:ParetoDominancePreservation>
        <PMOEA:hasReference>Zhang, Xingyi, Ye Tian, and Yaochu Jin. &quot;A Knee Point-Driven Evolutionary Algorithm for Many-Objective Optimization.&quot; Evolutionary Computation, IEEE Transactions on 19.6 (2015): 761-776.</PMOEA:hasReference>
        <rdfs:comment>The importance of knee points and knee regions has long been recognized in evolutionary multiobjective optimization. Nevertheless, the use of knee points to improve the search ability of MOEAs, especially for solving MaOPs, has not been reported so far. In this paper, we hypothesize that the search ability of MOEAs for solving MaOPs can be significantly enhanced by giving preferences to the knee points among nondominated solutions</rdfs:comment>
        <rdfs:label xml:lang="en">KnEA</rdfs:label>
    </owl:NamedIndividual>
    


    <!-- http://www.semanticweb.org/macoda/ontologies/PMOEA#Ridge-likeFunctionPreferOneReferencePoint -->

    <owl:NamedIndividual rdf:about="http://www.semanticweb.org/macoda/ontologies/PMOEA#Ridge-likeFunctionPreferOneReferencePoint">
        <rdf:type rdf:resource="http://www.semanticweb.org/macoda/ontologies/PMOEA#DistributionFunctionInObjectiveSpace"/>
        <rdfs:label xml:lang="en">Ridge-likeFunctionPreferOneReferencePoint</rdfs:label>
    </owl:NamedIndividual>
    


    <!-- http://www.semanticweb.org/macoda/ontologies/PMOEA#Trent_Kroeger -->

    <owl:NamedIndividual rdf:about="http://www.semanticweb.org/macoda/ontologies/PMOEA#Trent_Kroeger">
        <rdf:type rdf:resource="http://www.semanticweb.org/macoda/ontologies/PMOEA#Researcher"/>
        <rdfs:label xml:lang="en">Trent Kroeger</rdfs:label>
    </owl:NamedIndividual>
    


    <!-- http://www.semanticweb.org/macoda/ontologies/PMOEA#ComparativePreferenceStatements -->

    <owl:NamedIndividual rdf:about="http://www.semanticweb.org/macoda/ontologies/PMOEA#ComparativePreferenceStatements">
        <rdf:type rdf:resource="http://www.semanticweb.org/macoda/ontologies/PMOEA#ObjectiveComparison"/>
        <rdfs:comment>prefer f1&lt;0.3 to f2&lt;0.6</rdfs:comment>
        <rdfs:label xml:lang="en">ComparativePreferenceStatements</rdfs:label>
    </owl:NamedIndividual>
    


    <!-- http://www.semanticweb.org/macoda/ontologies/PMOEA#Kaifeng_Yang -->

    <owl:NamedIndividual rdf:about="http://www.semanticweb.org/macoda/ontologies/PMOEA#Kaifeng_Yang">
        <rdf:type rdf:resource="http://www.semanticweb.org/macoda/ontologies/PMOEA#Researcher"/>
        <rdfs:label xml:lang="en">Kaifeng Yang</rdfs:label>
    </owl:NamedIndividual>
    


    <!-- http://www.semanticweb.org/macoda/ontologies/PMOEA#RectangleRegion -->

    <owl:NamedIndividual rdf:about="http://www.semanticweb.org/macoda/ontologies/PMOEA#RectangleRegion">
        <rdf:type rdf:resource="http://www.semanticweb.org/macoda/ontologies/PMOEA#PreferenceRegion"/>
        <rdfs:comment>DM should offer boundary of each objective, which defines a rectangle in 2D objective space</rdfs:comment>
        <rdfs:label xml:lang="en">RectangleRegion</rdfs:label>
    </owl:NamedIndividual>
    


    <!-- http://www.semanticweb.org/macoda/ontologies/PMOEA#RegionDefinedByTchebycheffWeightSet -->

    <owl:NamedIndividual rdf:about="http://www.semanticweb.org/macoda/ontologies/PMOEA#RegionDefinedByTchebycheffWeightSet">
        <rdf:type rdf:resource="http://www.semanticweb.org/macoda/ontologies/PMOEA#PreferenceRegion"/>
        <rdfs:comment>The favorable weights  of individual s are a set of weights that minimizes its weighted Tchebycheff distance from the ideal point. We define a preferred region RP by a set of Tchebycheff weights WP . Then, we say that an individual s is in RP if its weights, ws, is in WP</rdfs:comment>
        <rdfs:label xml:lang="en">RegionDefinedByTchebycheffWeightSet</rdfs:label>
    </owl:NamedIndividual>
    


    <!-- http://www.semanticweb.org/macoda/ontologies/PMOEA#weights -->

    <owl:NamedIndividual rdf:about="http://www.semanticweb.org/macoda/ontologies/PMOEA#weights">
        <rdf:type rdf:resource="http://www.semanticweb.org/macoda/ontologies/PMOEA#ObjectiveComparison"/>
        <rdfs:comment>weights indicating the importance of different objectives, sum of which is 1</rdfs:comment>
        <rdfs:label xml:lang="en">weights</rdfs:label>
    </owl:NamedIndividual>
    


    <!-- http://www.semanticweb.org/macoda/ontologies/PMOEA#DTLZ6_2 -->

    <owl:NamedIndividual rdf:about="http://www.semanticweb.org/macoda/ontologies/PMOEA#DTLZ6_2">
        <rdf:type rdf:resource="http://www.semanticweb.org/macoda/ontologies/PMOEA#DTLZ"/>
        <PMOEA:isContinuousProblem rdf:datatype="http://www.w3.org/2001/XMLSchema#boolean">true</PMOEA:isContinuousProblem>
        <PMOEA:ObjectiveNumber rdf:datatype="http://www.w3.org/2001/XMLSchema#integer">2</PMOEA:ObjectiveNumber>
        <rdfs:label xml:lang="en">DTLZ6_2</rdfs:label>
    </owl:NamedIndividual>
    


    <!-- http://www.semanticweb.org/macoda/ontologies/PMOEA#DEB2DK -->

    <owl:NamedIndividual rdf:about="http://www.semanticweb.org/macoda/ontologies/PMOEA#DEB2DK">
        <rdf:type rdf:resource="http://www.semanticweb.org/macoda/ontologies/PMOEA#Academic_Problem"/>
        <PMOEA:isContinuousProblem rdf:datatype="http://www.w3.org/2001/XMLSchema#boolean">true</PMOEA:isContinuousProblem>
        <PMOEA:ObjectiveNumber rdf:datatype="http://www.w3.org/2001/XMLSchema#integer">2</PMOEA:ObjectiveNumber>
        <PMOEA:hasReference>Branke, J., Deb, K., Dierolf, H., and Osswald, M. Finding
knees in multi-objective optimization. In Proceedings of the
Parallel Problem Solving from Nature, LNCS, 3242, 2004,
722731.</PMOEA:hasReference>
        <rdfs:comment>This problem has n decision variables (we use n = 30) and only one settable parameter K indicating the knees number</rdfs:comment>
        <rdfs:label xml:lang="en">DEB2DK</rdfs:label>
    </owl:NamedIndividual>
    


    <!-- http://www.semanticweb.org/macoda/ontologies/PMOEA#Ernestas_Filatovas -->

    <owl:NamedIndividual rdf:about="http://www.semanticweb.org/macoda/ontologies/PMOEA#Ernestas_Filatovas">
        <rdf:type rdf:resource="http://www.semanticweb.org/macoda/ontologies/PMOEA#Researcher"/>
        <rdfs:label xml:lang="en">Ernestas Filatovas</rdfs:label>
    </owl:NamedIndividual>
    


    <!-- http://www.semanticweb.org/macoda/ontologies/PMOEA#DTLZ2_4 -->

    <owl:NamedIndividual rdf:about="http://www.semanticweb.org/macoda/ontologies/PMOEA#DTLZ2_4">
        <rdf:type rdf:resource="http://www.semanticweb.org/macoda/ontologies/PMOEA#DTLZ"/>
        <PMOEA:isContinuousProblem rdf:datatype="http://www.w3.org/2001/XMLSchema#boolean">true</PMOEA:isContinuousProblem>
        <PMOEA:ObjectiveNumber rdf:datatype="http://www.w3.org/2001/XMLSchema#integer">4</PMOEA:ObjectiveNumber>
        <PMOEA:isManyObjectiveProblem rdf:datatype="http://www.w3.org/2001/XMLSchema#boolean">true</PMOEA:isManyObjectiveProblem>
        <rdfs:label xml:lang="en">DTLZ2_4</rdfs:label>
    </owl:NamedIndividual>
    


    <!-- http://www.semanticweb.org/macoda/ontologies/PMOEA#Olga_Kurasova -->

    <owl:NamedIndividual rdf:about="http://www.semanticweb.org/macoda/ontologies/PMOEA#Olga_Kurasova">
        <rdf:type rdf:resource="http://www.semanticweb.org/macoda/ontologies/PMOEA#Researcher"/>
        <rdfs:label xml:lang="en">Olga Kurasova</rdfs:label>
    </owl:NamedIndividual>
    


    <!-- http://www.semanticweb.org/macoda/ontologies/PMOEA#Qingfu_Zhang -->

    <owl:NamedIndividual rdf:about="http://www.semanticweb.org/macoda/ontologies/PMOEA#Qingfu_Zhang">
        <rdf:type rdf:resource="http://www.semanticweb.org/macoda/ontologies/PMOEA#Researcher"/>
        <rdfs:label xml:lang="en">Qingfu Zhang</rdfs:label>
    </owl:NamedIndividual>
    


    <!-- http://www.semanticweb.org/macoda/ontologies/PMOEA#trade-off_basedDomonance -->

    <owl:NamedIndividual rdf:about="http://www.semanticweb.org/macoda/ontologies/PMOEA#trade-off_basedDomonance">
        <rdf:type rdf:resource="http://www.semanticweb.org/macoda/ontologies/PMOEA#DominanceRelation"/>
        <rdfs:comment>A solution x is now preferred to a non-dominated solution y if the gain in the objective where y is better does not outweigh the loss in the other objective</rdfs:comment>
        <rdfs:label xml:lang="en">trade-off_basedDomonance</rdfs:label>
    </owl:NamedIndividual>
    


    <!-- http://www.semanticweb.org/macoda/ontologies/PMOEA#DF-SMS-EMOA -->

    <owl:NamedIndividual rdf:about="http://www.semanticweb.org/macoda/ontologies/PMOEA#DF-SMS-EMOA">
        <rdf:type rdf:resource="http://www.semanticweb.org/macoda/ontologies/PMOEA#PMOEA"/>
        <PMOEA:hasPreferenceModel rdf:resource="http://www.semanticweb.org/macoda/ontologies/PMOEA#HarringtonsDF"/>
        <PMOEA:hasPreferenceInformationFromDM rdf:resource="http://www.semanticweb.org/macoda/ontologies/PMOEA#parametersInDF"/>
        <PMOEA:hasInteractionTime rdf:resource="http://www.semanticweb.org/macoda/ontologies/PMOEA#a-priori"/>
        <PMOEA:hasPreferenceIntegration rdf:resource="http://www.semanticweb.org/macoda/ontologies/PMOEA#ObjectiveTransformation"/>
        <PMOEA:canSolve rdf:resource="http://www.semanticweb.org/macoda/ontologies/PMOEA#ZDT2"/>
        <PMOEA:canSolve rdf:resource="http://www.semanticweb.org/macoda/ontologies/PMOEA#ZDT3"/>
        <PMOEA:canSolve rdf:resource="http://www.semanticweb.org/macoda/ontologies/PMOEA#TurningOptimizationProblem"/>
        <PMOEA:canSolve rdf:resource="http://www.semanticweb.org/macoda/ontologies/PMOEA#ZDT1"/>
        <PMOEA:hasResultInfluence rdf:resource="http://www.semanticweb.org/macoda/ontologies/PMOEA#BoundedRegion"/>
        <PMOEA:hasAuthor rdf:resource="http://www.semanticweb.org/macoda/ontologies/PMOEA#Heike_Trautmann"/>
        <PMOEA:hasAuthor rdf:resource="http://www.semanticweb.org/macoda/ontologies/PMOEA#Tobias_Wagner"/>
        <PMOEA:hasAuthor rdf:resource="http://www.semanticweb.org/macoda/ontologies/PMOEA#Dirk_Biermann"/>
        <PMOEA:hasSearchAlgorithm rdf:resource="http://www.semanticweb.org/macoda/ontologies/PMOEA#SMS-EMOA"/>
        <PMOEA:hasImplementationLanguage rdf:resource="http://www.semanticweb.org/macoda/ontologies/PMOEA#Matlab"/>
        <PMOEA:hasDevelopingYear rdf:datatype="http://www.w3.org/2001/XMLSchema#integer">2010</PMOEA:hasDevelopingYear>
        <PMOEA:MultipleRegionOfInterest rdf:datatype="http://www.w3.org/2001/XMLSchema#boolean">true</PMOEA:MultipleRegionOfInterest>
        <PMOEA:ParetoDominancePreservation rdf:datatype="http://www.w3.org/2001/XMLSchema#boolean">true</PMOEA:ParetoDominancePreservation>
        <PMOEA:hasReference>Wagner, T. and H. Trautmann (2010). &quot;Integration of Preferences in Hypervolume-Based Multiobjective Evolutionary Algorithms by Means of Desirability Functions.&quot; Evolutionary Computation, IEEE Transactions on 14(5): 688-701</PMOEA:hasReference>
        <rdfs:comment>Instead of the original objectives, desirability functions (DFs) of the objectives are optimized, which express the preferences of the decision maker. The original problem formulation and the optimization algorithm do not have to be modified. We propose the integration of DFs into the S-metric selection evolutionary multiobjective algorithm. The transformation ensures the meaning
of the hypervolumes internally computed.</rdfs:comment>
        <rdfs:label xml:lang="en">DF-SMS-EMOA</rdfs:label>
    </owl:NamedIndividual>
    


    <!-- http://www.semanticweb.org/macoda/ontologies/PMOEA#AveragedHausdorffDistance -->

    <owl:NamedIndividual rdf:about="http://www.semanticweb.org/macoda/ontologies/PMOEA#AveragedHausdorffDistance">
        <rdf:type rdf:resource="http://www.semanticweb.org/macoda/ontologies/PMOEA#SetQualityIndicator"/>
        <rdfs:comment>averaged Hausdorff distance is used as measure between two sets</rdfs:comment>
        <rdfs:label xml:lang="en">AveragedHausdorffDistance</rdfs:label>
    </owl:NamedIndividual>
    


    <!-- http://www.semanticweb.org/macoda/ontologies/PMOEA#EHVI-EGO -->

    <owl:NamedIndividual rdf:about="http://www.semanticweb.org/macoda/ontologies/PMOEA#EHVI-EGO">
        <rdf:type rdf:resource="http://www.semanticweb.org/macoda/ontologies/PMOEA#Indicator_based"/>
        <rdfs:label xml:lang="en">EHVI-EGO</rdfs:label>
    </owl:NamedIndividual>
    


    <!-- http://www.semanticweb.org/macoda/ontologies/PMOEA#Eik_Fun_Khor -->

    <owl:NamedIndividual rdf:about="http://www.semanticweb.org/macoda/ontologies/PMOEA#Eik_Fun_Khor">
        <rdf:type rdf:resource="http://www.semanticweb.org/macoda/ontologies/PMOEA#Researcher"/>
        <rdfs:label xml:lang="en">Eik Fun Khor</rdfs:label>
    </owl:NamedIndividual>
    


    <!-- http://www.semanticweb.org/macoda/ontologies/PMOEA#iW_HypE -->

    <owl:NamedIndividual rdf:about="http://www.semanticweb.org/macoda/ontologies/PMOEA#iW_HypE">
        <rdf:type rdf:resource="http://www.semanticweb.org/macoda/ontologies/PMOEA#PMOEA"/>
        <PMOEA:hasPreferenceModel rdf:resource="http://www.semanticweb.org/macoda/ontologies/PMOEA#ObjectiveSpaceWeightDistribution"/>
        <PMOEA:hasPreferenceInformationFromDM rdf:resource="http://www.semanticweb.org/macoda/ontologies/PMOEA#PickTheBest"/>
        <PMOEA:hasPreferenceInformationFromDM rdf:resource="http://www.semanticweb.org/macoda/ontologies/PMOEA#ComparativePreferenceStatements"/>
        <PMOEA:hasInteractionTime rdf:resource="http://www.semanticweb.org/macoda/ontologies/PMOEA#progressive"/>
        <PMOEA:hasPreferenceIntegration rdf:resource="http://www.semanticweb.org/macoda/ontologies/PMOEA#HypervolumeIndicator"/>
        <PMOEA:isInteractiveVersionOf rdf:resource="http://www.semanticweb.org/macoda/ontologies/PMOEA#W_HypE"/>
        <PMOEA:hasComparison rdf:resource="http://www.semanticweb.org/macoda/ontologies/PMOEA#iTDEA"/>
        <PMOEA:canSolve rdf:resource="http://www.semanticweb.org/macoda/ontologies/PMOEA#DTLZ2_2"/>
        <PMOEA:canSolve rdf:resource="http://www.semanticweb.org/macoda/ontologies/PMOEA#DTLZ2_5"/>
        <PMOEA:canSolve rdf:resource="http://www.semanticweb.org/macoda/ontologies/PMOEA#ZDT4"/>
        <PMOEA:canSolve rdf:resource="http://www.semanticweb.org/macoda/ontologies/PMOEA#DTLZ1_3"/>
        <PMOEA:hasResultInfluence rdf:resource="http://www.semanticweb.org/macoda/ontologies/PMOEA#BiasedDistribution"/>
        <PMOEA:hasAuthor rdf:resource="http://www.semanticweb.org/macoda/ontologies/PMOEA#Souhila_Kaci"/>
        <PMOEA:hasAuthor rdf:resource="http://www.semanticweb.org/macoda/ontologies/PMOEA#Youssef_Hamadi"/>
        <PMOEA:hasAuthor rdf:resource="http://www.semanticweb.org/macoda/ontologies/PMOEA#Dimo_Brockhoff"/>
        <PMOEA:useLibrary rdf:resource="http://www.semanticweb.org/macoda/ontologies/PMOEA#PISA"/>
        <PMOEA:hasSearchAlgorithm rdf:resource="http://www.semanticweb.org/macoda/ontologies/PMOEA#HypE"/>
        <PMOEA:hasImplementationLanguage rdf:resource="http://www.semanticweb.org/macoda/ontologies/PMOEA#Java"/>
        <PMOEA:hasDevelopingYear rdf:datatype="http://www.w3.org/2001/XMLSchema#integer">2014</PMOEA:hasDevelopingYear>
        <PMOEA:SpreadControl rdf:datatype="http://www.w3.org/2001/XMLSchema#boolean">true</PMOEA:SpreadControl>
        <PMOEA:hasReference>Brockhoff, D., Y. Hamadi and S. Kaci (2014). Using comparative preference statements in hypervolume-based interactive multiobjective optimization. Learning and Intelligent Optimization, Springer: 121-136</PMOEA:hasReference>
        <rdfs:comment>interactive version of W_HypE, means of Gaussian weight functions used in the W-HypE algorithm are derived by information given by the DM ( pick themost preferred or comparative preference statements)</rdfs:comment>
        <rdfs:label xml:lang="en">iW_HypE</rdfs:label>
    </owl:NamedIndividual>
    


    <!-- http://www.semanticweb.org/macoda/ontologies/PMOEA#PaGMO -->

    <owl:NamedIndividual rdf:about="http://www.semanticweb.org/macoda/ontologies/PMOEA#PaGMO">
        <rdf:type rdf:resource="http://www.semanticweb.org/macoda/ontologies/PMOEA#ImplementationLibrary"/>
        <rdfs:comment>A C++ platform to perform parallel computations of optimisation tasks (global and local) via the asynchronous generalized island model. State of the art optimization algorithms are included. A common interface is provided to other optimization frameworks/algorithms such as NLOPT, SciPy, SNOPT, IPOPT, GSL</rdfs:comment>
        <rdfs:label xml:lang="en">PaGMO</rdfs:label>
    </owl:NamedIndividual>
    


    <!-- http://www.semanticweb.org/macoda/ontologies/PMOEA#Florian Siegmund -->

    <owl:NamedIndividual rdf:about="http://www.semanticweb.org/macoda/ontologies/PMOEA#Florian_Siegmund">
        <rdf:type rdf:resource="http://www.semanticweb.org/macoda/ontologies/PMOEA#Researcher"/>
        <rdfs:label xml:lang="en">Florian Siegmund</rdfs:label>
    </owl:NamedIndividual>
    


    <!-- http://www.semanticweb.org/macoda/ontologies/PMOEA#MaximumAndMinimumTrade-offs -->

    <owl:NamedIndividual rdf:about="http://www.semanticweb.org/macoda/ontologies/PMOEA#MaximumAndMinimumTrade-offs">
        <rdf:type rdf:resource="http://www.semanticweb.org/macoda/ontologies/PMOEA#Trade-off"/>
        <rdfs:label xml:lang="en">MaximumAndMinimumTrade-offs</rdfs:label>
    </owl:NamedIndividual>
    


    <!-- http://www.semanticweb.org/macoda/ontologies/PMOEA#CrowdingDistance -->

    <owl:NamedIndividual rdf:about="http://www.semanticweb.org/macoda/ontologies/PMOEA#CrowdingDistance">
        <rdf:type rdf:resource="http://www.semanticweb.org/macoda/ontologies/PMOEA#CrowdingDistance"/>
        <rdfs:comment>crowding distance, used as second selection criterion in NSGA-II, is replaced or modified to incorporate preference.</rdfs:comment>
        <rdfs:label xml:lang="en">CrowdingDistance</rdfs:label>
    </owl:NamedIndividual>
    


    <!-- http://www.semanticweb.org/macoda/ontologies/PMOEA#CHI-EMOA -->

    <owl:NamedIndividual rdf:about="http://www.semanticweb.org/macoda/ontologies/PMOEA#CHI-EMOA">
        <rdf:type rdf:resource="http://www.semanticweb.org/macoda/ontologies/PMOEA#PMOEA"/>
        <PMOEA:hasPreferenceModel rdf:resource="http://www.semanticweb.org/macoda/ontologies/PMOEA#CurvaturebasedCone"/>
        <PMOEA:hasPreferenceInformationFromDM rdf:resource="http://www.semanticweb.org/macoda/ontologies/PMOEA#MaximumAndMinimumTrade-offs"/>
        <PMOEA:hasInteractionTime rdf:resource="http://www.semanticweb.org/macoda/ontologies/PMOEA#a-priori"/>
        <PMOEA:hasPreferenceIntegration rdf:resource="http://www.semanticweb.org/macoda/ontologies/PMOEA#HypervolumeIndicator"/>
        <PMOEA:canSolve rdf:resource="http://www.semanticweb.org/macoda/ontologies/PMOEA#GSP_3"/>
        <PMOEA:canSolve rdf:resource="http://www.semanticweb.org/macoda/ontologies/PMOEA#GSP_2"/>
        <PMOEA:hasResultInfluence rdf:resource="http://www.semanticweb.org/macoda/ontologies/PMOEA#BiasedDistribution"/>
        <PMOEA:hasAuthor rdf:resource="http://www.semanticweb.org/macoda/ontologies/PMOEA#Andre_Deutz"/>
        <PMOEA:hasAuthor rdf:resource="http://www.semanticweb.org/macoda/ontologies/PMOEA#Pradyumn_Kumar_Shukla"/>
        <PMOEA:hasAuthor rdf:resource="http://www.semanticweb.org/macoda/ontologies/PMOEA#Johannes_Kruisselbrink"/>
        <PMOEA:hasAuthor rdf:resource="http://www.semanticweb.org/macoda/ontologies/PMOEA#Michael_Emmerich"/>
        <PMOEA:useLibrary rdf:resource="http://www.semanticweb.org/macoda/ontologies/PMOEA#RODEOlib"/>
        <PMOEA:hasSearchAlgorithm rdf:resource="http://www.semanticweb.org/macoda/ontologies/PMOEA#SMS-EMOA"/>
        <PMOEA:hasImplementationLanguage rdf:resource="http://www.semanticweb.org/macoda/ontologies/PMOEA#Matlab"/>
        <PMOEA:hasDevelopingYear rdf:datatype="http://www.w3.org/2001/XMLSchema#integer">2013</PMOEA:hasDevelopingYear>
        <PMOEA:hasReference>Emmerich, Michael, et al. &quot;Cone-based hypervolume indicators: Construction, properties, and efficient computation.&quot; Evolutionary Multi-Criterion Optimization. Springer Berlin Heidelberg, 2013.</PMOEA:hasReference>
        <rdfs:comment>The attention of this paper is mainly focused on a singly parametrized family of symmetrical, polyhedral cones. For these cones we show how to 1. construct the base vectors of a member given its angle-parameter 2. check cone dominance efficiently and compute the cone non-dominated subset of a finite set 3. compute the cone based hypervolume efficiently</rdfs:comment>
        <rdfs:label xml:lang="en">CHI-EMOA</rdfs:label>
    </owl:NamedIndividual>
    


    <!-- http://www.semanticweb.org/macoda/ontologies/PMOEA#W_NSGA-II -->

    <owl:NamedIndividual rdf:about="http://www.semanticweb.org/macoda/ontologies/PMOEA#W_NSGA-II">
        <rdf:type rdf:resource="http://www.semanticweb.org/macoda/ontologies/PMOEA#PMOEA"/>
        <PMOEA:hasPreferenceModel rdf:resource="http://www.semanticweb.org/macoda/ontologies/PMOEA#ObjectiveSpaceWeightDistribution"/>
        <PMOEA:hasPreferenceInformationFromDM rdf:resource="http://www.semanticweb.org/macoda/ontologies/PMOEA#ExponentialFunctionPreferOneObjective"/>
        <PMOEA:hasPreferenceInformationFromDM rdf:resource="http://www.semanticweb.org/macoda/ontologies/PMOEA#Ridge-likeFunctionPreferOneReferencePoint"/>
        <PMOEA:hasPreferenceInformationFromDM rdf:resource="http://www.semanticweb.org/macoda/ontologies/PMOEA#ExponentialFunctionPreferExtremalSolutions"/>
        <PMOEA:hasInteractionTime rdf:resource="http://www.semanticweb.org/macoda/ontologies/PMOEA#a-priori"/>
        <PMOEA:hasPreferenceIntegration rdf:resource="http://www.semanticweb.org/macoda/ontologies/PMOEA#CrowdingDistance"/>
        <PMOEA:canSolve rdf:resource="http://www.semanticweb.org/macoda/ontologies/PMOEA#WFG1_2"/>
        <PMOEA:canSolve rdf:resource="http://www.semanticweb.org/macoda/ontologies/PMOEA#WFG3_2"/>
        <PMOEA:canSolve rdf:resource="http://www.semanticweb.org/macoda/ontologies/PMOEA#ZDT2"/>
        <PMOEA:canSolve rdf:resource="http://www.semanticweb.org/macoda/ontologies/PMOEA#ZDT6"/>
        <PMOEA:canSolve rdf:resource="http://www.semanticweb.org/macoda/ontologies/PMOEA#ZDT4"/>
        <PMOEA:canSolve rdf:resource="http://www.semanticweb.org/macoda/ontologies/PMOEA#WFG2_2"/>
        <PMOEA:canSolve rdf:resource="http://www.semanticweb.org/macoda/ontologies/PMOEA#ZDT3"/>
        <PMOEA:canSolve rdf:resource="http://www.semanticweb.org/macoda/ontologies/PMOEA#WFG5_2"/>
        <PMOEA:canSolve rdf:resource="http://www.semanticweb.org/macoda/ontologies/PMOEA#WFG4_2"/>
        <PMOEA:canSolve rdf:resource="http://www.semanticweb.org/macoda/ontologies/PMOEA#ZDT1"/>
        <PMOEA:hasResultInfluence rdf:resource="http://www.semanticweb.org/macoda/ontologies/PMOEA#BiasedDistribution"/>
        <PMOEA:hasAuthor rdf:resource="http://www.semanticweb.org/macoda/ontologies/PMOEA#Trent_Kroeger"/>
        <PMOEA:hasAuthor rdf:resource="http://www.semanticweb.org/macoda/ontologies/PMOEA#Frank_Neumann"/>
        <PMOEA:hasAuthor rdf:resource="http://www.semanticweb.org/macoda/ontologies/PMOEA#Tobias_Friedrich"/>
        <PMOEA:hasSearchAlgorithm rdf:resource="http://www.semanticweb.org/macoda/ontologies/PMOEA#NSGA-II"/>
        <PMOEA:hasDevelopingYear rdf:datatype="http://www.w3.org/2001/XMLSchema#integer">2012</PMOEA:hasDevelopingYear>
        <PMOEA:ParetoDominancePreservation rdf:datatype="http://www.w3.org/2001/XMLSchema#boolean">true</PMOEA:ParetoDominancePreservation>
        <PMOEA:hasReference>Friedrich, T., T. Kroeger and F. Neumann (2012). &quot;Weighted preferences in evolutionary multi-objective optimization.&quot; International Journal of Machine Learning and Cybernetics 4(2): 139-148</PMOEA:hasReference>
        <rdfs:comment>In this paper, we present a neat and simple approach to use the preference information given by weightings on the objective space in classical algorithms such as NSGA-II and SPEA2. Furthermore, our algorithms are as efficient as the original implementation of NSGA-II and SPEA2 and do not have to deal with the expensive computations that hypervolume-based algorithms have to face.</rdfs:comment>
        <rdfs:label xml:lang="en">W_NSGA-II</rdfs:label>
    </owl:NamedIndividual>
    


    <!-- http://www.semanticweb.org/macoda/ontologies/PMOEA#ZDT6 -->

    <owl:NamedIndividual rdf:about="http://www.semanticweb.org/macoda/ontologies/PMOEA#ZDT6">
        <rdf:type rdf:resource="http://www.semanticweb.org/macoda/ontologies/PMOEA#ZDT"/>
        <PMOEA:isDiscreteProblem rdf:datatype="http://www.w3.org/2001/XMLSchema#boolean">false</PMOEA:isDiscreteProblem>
        <PMOEA:OWLDataProperty_61d3cd95_fde4_4c1b_af08_1eaf73473aea rdf:datatype="http://www.w3.org/2001/XMLSchema#boolean">true</PMOEA:OWLDataProperty_61d3cd95_fde4_4c1b_af08_1eaf73473aea>
        <PMOEA:isContinuousProblem rdf:datatype="http://www.w3.org/2001/XMLSchema#boolean">true</PMOEA:isContinuousProblem>
        <PMOEA:ObjectiveNumber rdf:datatype="http://www.w3.org/2001/XMLSchema#integer">2</PMOEA:ObjectiveNumber>
        <PMOEA:isManyObjectiveProblem rdf:datatype="http://www.w3.org/2001/XMLSchema#boolean">false</PMOEA:isManyObjectiveProblem>
        <rdfs:label xml:lang="en">ZDT6</rdfs:label>
    </owl:NamedIndividual>
    


    <!-- http://www.semanticweb.org/macoda/ontologies/PMOEA#ZDT4 -->

    <owl:NamedIndividual rdf:about="http://www.semanticweb.org/macoda/ontologies/PMOEA#ZDT4">
        <rdf:type rdf:resource="http://www.semanticweb.org/macoda/ontologies/PMOEA#ZDT"/>
        <PMOEA:OWLDataProperty_61d3cd95_fde4_4c1b_af08_1eaf73473aea rdf:datatype="http://www.w3.org/2001/XMLSchema#boolean">true</PMOEA:OWLDataProperty_61d3cd95_fde4_4c1b_af08_1eaf73473aea>
        <PMOEA:isContinuousProblem rdf:datatype="http://www.w3.org/2001/XMLSchema#boolean">true</PMOEA:isContinuousProblem>
        <PMOEA:ObjectiveNumber rdf:datatype="http://www.w3.org/2001/XMLSchema#integer">2</PMOEA:ObjectiveNumber>
        <PMOEA:isManyObjectiveProblem rdf:datatype="http://www.w3.org/2001/XMLSchema#boolean">false</PMOEA:isManyObjectiveProblem>
        <rdfs:label xml:lang="en">ZDT4</rdfs:label>
    </owl:NamedIndividual>
    


    <!-- http://www.semanticweb.org/macoda/ontologies/PMOEA#SearchRange -->

    <owl:NamedIndividual rdf:about="http://www.semanticweb.org/macoda/ontologies/PMOEA#SearchRange">
        <rdf:type rdf:resource="http://www.semanticweb.org/macoda/ontologies/PMOEA#ReferenceDirection"/>
        <rdfs:comment>angle from the reference point to control the range of the ROI, used in iPICEA-G</rdfs:comment>
        <rdfs:label xml:lang="en">SearchRange</rdfs:label>
    </owl:NamedIndividual>
    


    <!-- http://www.semanticweb.org/macoda/ontologies/PMOEA#RankSamples -->

    <owl:NamedIndividual rdf:about="http://www.semanticweb.org/macoda/ontologies/PMOEA#RankSamples">
        <rdf:type rdf:resource="http://www.semanticweb.org/macoda/ontologies/PMOEA#SampleRanks"/>
        <rdfs:comment>rank a set of solutions from best to worst</rdfs:comment>
        <rdfs:label xml:lang="en">RankSamples</rdfs:label>
    </owl:NamedIndividual>
    


    <!-- http://www.semanticweb.org/macoda/ontologies/PMOEA#DTLZ6_10 -->

    <owl:NamedIndividual rdf:about="http://www.semanticweb.org/macoda/ontologies/PMOEA#DTLZ6_10">
        <rdf:type rdf:resource="http://www.semanticweb.org/macoda/ontologies/PMOEA#DTLZ"/>
        <PMOEA:isContinuousProblem rdf:datatype="http://www.w3.org/2001/XMLSchema#boolean">true</PMOEA:isContinuousProblem>
        <PMOEA:ObjectiveNumber rdf:datatype="http://www.w3.org/2001/XMLSchema#integer">10</PMOEA:ObjectiveNumber>
        <PMOEA:isManyObjectiveProblem rdf:datatype="http://www.w3.org/2001/XMLSchema#boolean">true</PMOEA:isManyObjectiveProblem>
        <rdfs:label xml:lang="en">DTLZ6_10</rdfs:label>
    </owl:NamedIndividual>
    


    <!-- http://www.semanticweb.org/macoda/ontologies/PMOEA#DTLZ5_10 -->

    <owl:NamedIndividual rdf:about="http://www.semanticweb.org/macoda/ontologies/PMOEA#DTLZ5_10">
        <rdf:type rdf:resource="http://www.semanticweb.org/macoda/ontologies/PMOEA#DTLZ"/>
        <PMOEA:isContinuousProblem rdf:datatype="http://www.w3.org/2001/XMLSchema#boolean">true</PMOEA:isContinuousProblem>
        <PMOEA:ObjectiveNumber rdf:datatype="http://www.w3.org/2001/XMLSchema#integer">10</PMOEA:ObjectiveNumber>
        <PMOEA:isManyObjectiveProblem rdf:datatype="http://www.w3.org/2001/XMLSchema#boolean">true</PMOEA:isManyObjectiveProblem>
        <rdfs:label xml:lang="en">DTLZ5_10</rdfs:label>
    </owl:NamedIndividual>
    


    <!-- http://www.semanticweb.org/macoda/ontologies/PMOEA#Thomas_Baeck -->

    <owl:NamedIndividual rdf:about="http://www.semanticweb.org/macoda/ontologies/PMOEA#Thomas_Baeck">
        <rdf:type rdf:resource="http://www.semanticweb.org/macoda/ontologies/PMOEA#Researcher"/>
        <rdfs:label xml:lang="en">Thomas Baeck</rdfs:label>
    </owl:NamedIndividual>
    


    <!-- http://www.semanticweb.org/macoda/ontologies/PMOEA#DRSA-EMO -->

    <owl:NamedIndividual rdf:about="http://www.semanticweb.org/macoda/ontologies/PMOEA#DRSA-EMO">
        <rdf:type rdf:resource="http://www.semanticweb.org/macoda/ontologies/PMOEA#PMOEA"/>
        <PMOEA:hasPreferenceModel rdf:resource="http://www.semanticweb.org/macoda/ontologies/PMOEA#DRSA"/>
        <PMOEA:hasPreferenceInformationFromDM rdf:resource="http://www.semanticweb.org/macoda/ontologies/PMOEA#SortSampleIntoCategory"/>
        <PMOEA:hasInteractionTime rdf:resource="http://www.semanticweb.org/macoda/ontologies/PMOEA#progressive"/>
        <PMOEA:hasPreferenceIntegration rdf:resource="http://www.semanticweb.org/macoda/ontologies/PMOEA#FrontSorting"/>
        <PMOEA:hasResultInfluence rdf:resource="http://www.semanticweb.org/macoda/ontologies/PMOEA#OneSolution"/>
        <PMOEA:hasAuthor rdf:resource="http://www.semanticweb.org/macoda/ontologies/PMOEA#Salvatore_Greco
"/>
        <PMOEA:hasAuthor rdf:resource="http://www.semanticweb.org/macoda/ontologies/PMOEA#Benedetto_Matarazzo"/>
        <PMOEA:hasAuthor rdf:resource="http://www.semanticweb.org/macoda/ontologies/PMOEA#Roman_Sowinski"/>
        <PMOEA:hasSearchAlgorithm rdf:resource="http://www.semanticweb.org/macoda/ontologies/PMOEA#GeneralMOEA"/>
        <PMOEA:hasDevelopingYear rdf:datatype="http://www.w3.org/2001/XMLSchema#integer">2010</PMOEA:hasDevelopingYear>
        <PMOEA:hasReference>Greco, S., B. Matarazzo and R. Slowinski (2010). Interactive evolutionary multiobjective optimization using dominance-based rough set approach. Evolutionary Computation (CEC), 2010 IEEE Congress on, IEEE</PMOEA:hasReference>
        <rdfs:comment>We present basic ideas related to application of Dominance-based Rough Set Approach (DRSA) in interactive Evolutionary Multiobjective Optimization (EMO). In the proposed methodology, the preference information elicited by the decision maker in successive iterations consists in sorting some solutions in the current population into relatively good and others(DRSA-EMO) , or in comparing some pairs of solutions with respect to preference(DRSA-EMO-PCT). The if ..., then ... decision rules are then induced from this preference information and  used within EMO in order to focus on populations of solutions satisfying the preferences of the decision maker, speeding up convergence to the most preferred region of the Pareto-front</rdfs:comment>
        <rdfs:label xml:lang="en">DRSA-EMO</rdfs:label>
    </owl:NamedIndividual>
    


    <!-- http://www.semanticweb.org/macoda/ontologies/PMOEA#Michael_Emmerich -->

    <owl:NamedIndividual rdf:about="http://www.semanticweb.org/macoda/ontologies/PMOEA#Michael_Emmerich">
        <rdf:type rdf:resource="http://www.semanticweb.org/macoda/ontologies/PMOEA#Researcher"/>
        <rdfs:label xml:lang="en">Michael Emmerich</rdfs:label>
    </owl:NamedIndividual>
    


    <!-- http://www.semanticweb.org/macoda/ontologies/PMOEA#PIE -->

    <owl:NamedIndividual rdf:about="http://www.semanticweb.org/macoda/ontologies/PMOEA#PIE">
        <rdf:type rdf:resource="http://www.semanticweb.org/macoda/ontologies/PMOEA#PMOEA"/>
        <PMOEA:hasPreferenceModel rdf:resource="http://www.semanticweb.org/macoda/ontologies/PMOEA#WierzbickiASF"/>
        <PMOEA:hasPreferenceInformationFromDM rdf:resource="http://www.semanticweb.org/macoda/ontologies/PMOEA#DistributeCreditsToObjectives"/>
        <PMOEA:hasPreferenceInformationFromDM rdf:resource="http://www.semanticweb.org/macoda/ontologies/PMOEA#ReferencePoint"/>
        <PMOEA:hasPreferenceInformationFromDM rdf:resource="http://www.semanticweb.org/macoda/ontologies/PMOEA#SortSampleIntoCategory"/>
        <PMOEA:hasInteractionTime rdf:resource="http://www.semanticweb.org/macoda/ontologies/PMOEA#progressive"/>
        <PMOEA:hasPreferenceIntegration rdf:resource="http://www.semanticweb.org/macoda/ontologies/PMOEA#WeightsInASF"/>
        <PMOEA:canSolve rdf:resource="http://www.semanticweb.org/macoda/ontologies/PMOEA#PollutionMonitoringStationLocation"/>
        <PMOEA:hasResultInfluence rdf:resource="http://www.semanticweb.org/macoda/ontologies/PMOEA#OneSolution"/>
        <PMOEA:hasAuthor rdf:resource="http://www.semanticweb.org/macoda/ontologies/PMOEA#Ana_Beln_Ruiz"/>
        <PMOEA:hasAuthor rdf:resource="http://www.semanticweb.org/macoda/ontologies/PMOEA#Kaisa_Miettinen"/>
        <PMOEA:hasAuthor rdf:resource="http://www.semanticweb.org/macoda/ontologies/PMOEA#Karthik_Sindhya"/>
        <PMOEA:hasSearchAlgorithm rdf:resource="http://www.semanticweb.org/macoda/ontologies/PMOEA#SingleObjectiveEA"/>
        <PMOEA:hasDevelopingYear rdf:datatype="http://www.w3.org/2001/XMLSchema#integer">2011</PMOEA:hasDevelopingYear>
        <PMOEA:hasRemarks>EA in MCDM</PMOEA:hasRemarks>
        <PMOEA:ParetoDominancePreservation rdf:datatype="http://www.w3.org/2001/XMLSchema#boolean">true</PMOEA:ParetoDominancePreservation>
        <PMOEA:hasReference>Sindhya, K., A. B. Ruiz and K. Miettinen (2011). A preference based interactive evolutionary algorithm for multi-objective optimization: PIE. Evolutionary Multi-Criterion Optimization, Springer</PMOEA:hasReference>
        <rdfs:comment>Starting from an approximated nadir point, the PIE algorithm improves progressively the objective function values of a solution by finding a better solution at each iteration that improves the previous one. The decision maker decides from which solution, in which direction, and at what distance from the Pareto front to find the next solution. Thus, the PIE algorithm is guided interactively by the decision maker. A flexible approach is obtained with the use of archive sets to store all the solutions generated during an evolutionary algorithms run, as it allows the decision maker to freely navigate and inspect previous solutions if needed.</rdfs:comment>
        <rdfs:label xml:lang="en">PIE</rdfs:label>
    </owl:NamedIndividual>
    


    <!-- http://www.semanticweb.org/macoda/ontologies/PMOEA#Carlos_M_Fonseca -->

    <owl:NamedIndividual rdf:about="http://www.semanticweb.org/macoda/ontologies/PMOEA#Carlos_M_Fonseca">
        <rdf:type rdf:resource="http://www.semanticweb.org/macoda/ontologies/PMOEA#Researcher"/>
        <rdfs:label xml:lang="en">Carlos M.Fonseca</rdfs:label>
    </owl:NamedIndividual>
    


    <!-- http://www.semanticweb.org/macoda/ontologies/PMOEA#DRSA -->

    <owl:NamedIndividual rdf:about="http://www.semanticweb.org/macoda/ontologies/PMOEA#DRSA">
        <rdf:type rdf:resource="http://www.semanticweb.org/macoda/ontologies/PMOEA#DecisionRules"/>
        <rdfs:comment>Dominance-based Rough Set Approach (DRSA),DRSA is a methodology of multiple criteria decision analysis aiming at obtaining a representation of the DMs preferences in terms of easily understandable  if ..., then ... decision rules, on the basis of some exemplary decisions (past decisions or simulated decisions) given by the DM</rdfs:comment>
        <rdfs:label xml:lang="en">DRSA</rdfs:label>
    </owl:NamedIndividual>
    


    <!-- http://www.semanticweb.org/macoda/ontologies/PMOEA#WFG4_10 -->

    <owl:NamedIndividual rdf:about="http://www.semanticweb.org/macoda/ontologies/PMOEA#WFG4_10">
        <rdf:type rdf:resource="http://www.semanticweb.org/macoda/ontologies/PMOEA#WFG"/>
        <PMOEA:OWLDataProperty_61d3cd95_fde4_4c1b_af08_1eaf73473aea rdf:datatype="http://www.w3.org/2001/XMLSchema#boolean">true</PMOEA:OWLDataProperty_61d3cd95_fde4_4c1b_af08_1eaf73473aea>
        <PMOEA:isContinuousProblem rdf:datatype="http://www.w3.org/2001/XMLSchema#boolean">true</PMOEA:isContinuousProblem>
        <PMOEA:ObjectiveNumber rdf:datatype="http://www.w3.org/2001/XMLSchema#integer">10</PMOEA:ObjectiveNumber>
        <PMOEA:isManyObjectiveProblem rdf:datatype="http://www.w3.org/2001/XMLSchema#boolean">true</PMOEA:isManyObjectiveProblem>
        <rdfs:label xml:lang="en">WFG4_10</rdfs:label>
    </owl:NamedIndividual>
    


    <!-- http://www.semanticweb.org/macoda/ontologies/PMOEA#PreferencePointSet -->

    <owl:NamedIndividual rdf:about="http://www.semanticweb.org/macoda/ontologies/PMOEA#PreferencePointSet">
        <rdf:type rdf:resource="http://www.semanticweb.org/macoda/ontologies/PMOEA#PreferencePoint"/>
        <rdfs:label xml:lang="en">PreferencePointSet</rdfs:label>
    </owl:NamedIndividual>
    


    <!-- http://www.semanticweb.org/macoda/ontologies/PMOEA#Frank_Neumann -->

    <owl:NamedIndividual rdf:about="http://www.semanticweb.org/macoda/ontologies/PMOEA#Frank_Neumann">
        <rdf:type rdf:resource="http://www.semanticweb.org/macoda/ontologies/PMOEA#Researcher"/>
        <rdfs:label xml:lang="en">Frank Neumann</rdfs:label>
    </owl:NamedIndividual>
    


    <!-- http://www.semanticweb.org/macoda/ontologies/PMOEA#Gregorio_Toscano-Pulido -->

    <owl:NamedIndividual rdf:about="http://www.semanticweb.org/macoda/ontologies/PMOEA#Gregorio_Toscano-Pulido">
        <rdf:type rdf:resource="http://www.semanticweb.org/macoda/ontologies/PMOEA#Researcher"/>
        <rdfs:label xml:lang="en">Gregorio Toscano-Pulido</rdfs:label>
    </owl:NamedIndividual>
    


    <!-- http://www.semanticweb.org/macoda/ontologies/PMOEA#WFG4_4 -->

    <owl:NamedIndividual rdf:about="http://www.semanticweb.org/macoda/ontologies/PMOEA#WFG4_4">
        <rdf:type rdf:resource="http://www.semanticweb.org/macoda/ontologies/PMOEA#WFG"/>
        <PMOEA:OWLDataProperty_61d3cd95_fde4_4c1b_af08_1eaf73473aea rdf:datatype="http://www.w3.org/2001/XMLSchema#boolean">true</PMOEA:OWLDataProperty_61d3cd95_fde4_4c1b_af08_1eaf73473aea>
        <PMOEA:isContinuousProblem rdf:datatype="http://www.w3.org/2001/XMLSchema#boolean">true</PMOEA:isContinuousProblem>
        <PMOEA:ObjectiveNumber rdf:datatype="http://www.w3.org/2001/XMLSchema#integer">4</PMOEA:ObjectiveNumber>
        <PMOEA:isManyObjectiveProblem rdf:datatype="http://www.w3.org/2001/XMLSchema#boolean">true</PMOEA:isManyObjectiveProblem>
        <rdfs:label xml:lang="en">WFG4_4</rdfs:label>
    </owl:NamedIndividual>
    


    <!-- http://www.semanticweb.org/macoda/ontologies/PMOEA#DTLZ7_4 -->

    <owl:NamedIndividual rdf:about="http://www.semanticweb.org/macoda/ontologies/PMOEA#DTLZ7_4">
        <rdf:type rdf:resource="http://www.semanticweb.org/macoda/ontologies/PMOEA#DTLZ"/>
        <PMOEA:isContinuousProblem rdf:datatype="http://www.w3.org/2001/XMLSchema#boolean">true</PMOEA:isContinuousProblem>
        <PMOEA:ObjectiveNumber rdf:datatype="http://www.w3.org/2001/XMLSchema#integer">4</PMOEA:ObjectiveNumber>
        <PMOEA:isManyObjectiveProblem rdf:datatype="http://www.w3.org/2001/XMLSchema#boolean">true</PMOEA:isManyObjectiveProblem>
        <rdfs:label xml:lang="en">DTLZ7_4</rdfs:label>
    </owl:NamedIndividual>
    


    <!-- http://www.semanticweb.org/macoda/ontologies/PMOEA#Derringer-SuichDF -->

    <owl:NamedIndividual rdf:about="http://www.semanticweb.org/macoda/ontologies/PMOEA#Derringer-SuichDF">
        <rdf:type rdf:resource="http://www.semanticweb.org/macoda/ontologies/PMOEA#DesirabilityFunction"/>
        <rdfs:label xml:lang="en">Derringer-SuichDF</rdfs:label>
    </owl:NamedIndividual>
    


    <!-- http://www.semanticweb.org/macoda/ontologies/PMOEA#STOM-ASF -->

    <owl:NamedIndividual rdf:about="http://www.semanticweb.org/macoda/ontologies/PMOEA#STOM-ASF">
        <rdf:type rdf:resource="http://www.semanticweb.org/macoda/ontologies/PMOEA#AchievementScalarizingFunction"/>
        <PMOEA:hasReference>H. Nakayama, Y. Sawaragi, Satisficing trade-off method
for multiobjective programming, in: M. Grauer, A.P.
Wierzbicki (Eds.), Interactive Decision Analysis, Springer
Verlag, Berlin, 1984, pp. 113122</PMOEA:hasReference>
        <rdfs:comment>ASF used inSTOM method</rdfs:comment>
        <rdfs:label xml:lang="en">STOM-ASF</rdfs:label>
    </owl:NamedIndividual>
    


    <!-- http://www.semanticweb.org/macoda/ontologies/PMOEA#DF-NSGA-II -->

    <owl:NamedIndividual rdf:about="http://www.semanticweb.org/macoda/ontologies/PMOEA#DF-NSGA-II">
        <rdf:type rdf:resource="http://www.semanticweb.org/macoda/ontologies/PMOEA#PMOEA"/>
        <PMOEA:hasPreferenceModel rdf:resource="http://www.semanticweb.org/macoda/ontologies/PMOEA#HarringtonsDF"/>
        <PMOEA:hasPreferenceInformationFromDM rdf:resource="http://www.semanticweb.org/macoda/ontologies/PMOEA#parametersInDF"/>
        <PMOEA:hasInteractionTime rdf:resource="http://www.semanticweb.org/macoda/ontologies/PMOEA#a-priori"/>
        <PMOEA:hasPreferenceIntegration rdf:resource="http://www.semanticweb.org/macoda/ontologies/PMOEA#ObjectiveTransformation"/>
        <PMOEA:canSolve rdf:resource="http://www.semanticweb.org/macoda/ontologies/PMOEA#BinhProblem"/>
        <PMOEA:canSolve rdf:resource="http://www.semanticweb.org/macoda/ontologies/PMOEA#SingleCutTurningCostOptimization"/>
        <PMOEA:canSolve rdf:resource="http://www.semanticweb.org/macoda/ontologies/PMOEA#NoisyBinhProblem"/>
        <PMOEA:hasResultInfluence rdf:resource="http://www.semanticweb.org/macoda/ontologies/PMOEA#BoundedRegion"/>
        <PMOEA:hasAuthor rdf:resource="http://www.semanticweb.org/macoda/ontologies/PMOEA#Heike_Trautmann"/>
        <PMOEA:hasAuthor rdf:resource="http://www.semanticweb.org/macoda/ontologies/PMOEA#Jorn_Mehnen"/>
        <PMOEA:hasSearchAlgorithm rdf:resource="http://www.semanticweb.org/macoda/ontologies/PMOEA#NSGA-II"/>
        <PMOEA:hasImplementationLanguage rdf:resource="http://www.semanticweb.org/macoda/ontologies/PMOEA#Matlab"/>
        <PMOEA:hasDevelopingYear rdf:datatype="http://www.w3.org/2001/XMLSchema#integer">2009</PMOEA:hasDevelopingYear>
        <PMOEA:ParetoDominancePreservation rdf:datatype="http://www.w3.org/2001/XMLSchema#boolean">true</PMOEA:ParetoDominancePreservation>
        <PMOEA:hasReference>Trautmann, H. and J. Mehnen (2009). &quot;Preference-based Pareto optimization in certain and noisy environments.&quot; Engineering Optimization 41(1): 23-38</PMOEA:hasReference>
        <rdfs:comment>A set of Pareto-optimal solutions is determined via desirability functions of the objectives which reveal experts preferences regarding different objective regions. By applying the methods to the original and uncertain Binh problem and a noisy single cut turning cost optimization problem, these approaches prove to be very effective in focusing on different parts of the Pareto front of the original problem in both certain and noisy environments</rdfs:comment>
        <rdfs:label xml:lang="en">DF-NSGA-II</rdfs:label>
    </owl:NamedIndividual>
    


    <!-- http://www.semanticweb.org/macoda/ontologies/PMOEA#WFG9_4 -->

    <owl:NamedIndividual rdf:about="http://www.semanticweb.org/macoda/ontologies/PMOEA#WFG9_4">
        <rdf:type rdf:resource="http://www.semanticweb.org/macoda/ontologies/PMOEA#WFG"/>
        <PMOEA:OWLDataProperty_61d3cd95_fde4_4c1b_af08_1eaf73473aea rdf:datatype="http://www.w3.org/2001/XMLSchema#boolean">true</PMOEA:OWLDataProperty_61d3cd95_fde4_4c1b_af08_1eaf73473aea>
        <PMOEA:isContinuousProblem rdf:datatype="http://www.w3.org/2001/XMLSchema#boolean">true</PMOEA:isContinuousProblem>
        <PMOEA:ObjectiveNumber rdf:datatype="http://www.w3.org/2001/XMLSchema#integer">4</PMOEA:ObjectiveNumber>
        <PMOEA:isManyObjectiveProblem rdf:datatype="http://www.w3.org/2001/XMLSchema#boolean">true</PMOEA:isManyObjectiveProblem>
        <rdfs:label xml:lang="en">WFG9_4</rdfs:label>
    </owl:NamedIndividual>
    


    <!-- http://www.semanticweb.org/macoda/ontologies/PMOEA#Feiyue_Qiu -->

    <owl:NamedIndividual rdf:about="http://www.semanticweb.org/macoda/ontologies/PMOEA#Feiyue_Qiu">
        <rdf:type rdf:resource="http://www.semanticweb.org/macoda/ontologies/PMOEA#Researcher"/>
        <rdfs:label xml:lang="en">Feiyue Qiu</rdfs:label>
    </owl:NamedIndividual>
    


    <!-- http://www.semanticweb.org/macoda/ontologies/PMOEA#SetQualityIndicator -->

    <owl:NamedIndividual rdf:about="http://www.semanticweb.org/macoda/ontologies/PMOEA#SetQualityIndicator">
        <rdf:type rdf:resource="http://www.semanticweb.org/macoda/ontologies/PMOEA#SetQualityIndicator"/>
        <rdfs:label xml:lang="en">SetQualityIndicator</rdfs:label>
    </owl:NamedIndividual>
    


    <!-- http://www.semanticweb.org/macoda/ontologies/PMOEA#Johannes Bader -->

    <owl:NamedIndividual rdf:about="http://www.semanticweb.org/macoda/ontologies/PMOEA#Johannes Bader">
        <rdf:type rdf:resource="http://www.semanticweb.org/macoda/ontologies/PMOEA#Researcher"/>
        <rdfs:label xml:lang="en">Johannes Bader</rdfs:label>
    </owl:NamedIndividual>
    


    <!-- http://www.semanticweb.org/macoda/ontologies/PMOEA#Jianwei Wang -->

    <owl:NamedIndividual rdf:about="http://www.semanticweb.org/macoda/ontologies/PMOEA#Jianwei Wang">
        <rdf:type rdf:resource="http://www.semanticweb.org/macoda/ontologies/PMOEA#Researcher"/>
        <rdfs:label xml:lang="en">Jianwei Wang</rdfs:label>
    </owl:NamedIndividual>
    


    <!-- http://www.semanticweb.org/macoda/ontologies/PMOEA#EGCM -->

    <owl:NamedIndividual rdf:about="http://www.semanticweb.org/macoda/ontologies/PMOEA#EGCM">
        <rdf:type rdf:resource="http://www.semanticweb.org/macoda/ontologies/PMOEA#PMOEA"/>
        <PMOEA:hasPreferenceModel rdf:resource="http://www.semanticweb.org/macoda/ontologies/PMOEA#PreferencePoint"/>
        <PMOEA:hasPreferenceInformationFromDM rdf:resource="http://www.semanticweb.org/macoda/ontologies/PMOEA#ReferencePoint"/>
        <PMOEA:hasInteractionTime rdf:resource="http://www.semanticweb.org/macoda/ontologies/PMOEA#a-priori"/>
        <PMOEA:hasPreferenceIntegration rdf:resource="http://www.semanticweb.org/macoda/ontologies/PMOEA#constraints"/>
        <PMOEA:canSolve rdf:resource="http://www.semanticweb.org/macoda/ontologies/PMOEA#WFG1_3"/>
        <PMOEA:canSolve rdf:resource="http://www.semanticweb.org/macoda/ontologies/PMOEA#WFG1_2"/>
        <PMOEA:canSolve rdf:resource="http://www.semanticweb.org/macoda/ontologies/PMOEA#WFG2_2"/>
        <PMOEA:canSolve rdf:resource="http://www.semanticweb.org/macoda/ontologies/PMOEA#WFG1_5"/>
        <PMOEA:canSolve rdf:resource="http://www.semanticweb.org/macoda/ontologies/PMOEA#WFG2_10"/>
        <PMOEA:canSolve rdf:resource="http://www.semanticweb.org/macoda/ontologies/PMOEA#WFG1_10"/>
        <PMOEA:hasResultInfluence rdf:resource="http://www.semanticweb.org/macoda/ontologies/PMOEA#SetOfSolutions"/>
        <PMOEA:hasAuthor rdf:resource="http://www.semanticweb.org/macoda/ontologies/PMOEA#Carlos_Coello_Coello"/>
        <PMOEA:hasAuthor rdf:resource="http://www.semanticweb.org/macoda/ontologies/PMOEA#Gregorio_Toscano-Pulido"/>
        <PMOEA:hasAuthor rdf:resource="http://www.semanticweb.org/macoda/ontologies/PMOEA#Ricardo_Landa"/>
        <PMOEA:hasSearchAlgorithm rdf:resource="http://www.semanticweb.org/macoda/ontologies/PMOEA#DifferentialEvolution"/>
        <PMOEA:hasDevelopingYear rdf:datatype="http://www.w3.org/2001/XMLSchema#integer">2013</PMOEA:hasDevelopingYear>
        <PMOEA:hasReference>Landa, Ricardo, Carlos A. Coello Coello, and Gregorio Toscano-Pulido. &quot;Goal-constraint: Incorporating preferences through an evolutionary -constraint based method.&quot; 2013 IEEE Congress on Evolutionary Computation. IEEE, 2013.</PMOEA:hasReference>
        <rdfs:comment>In this work, we propose a hybrid of an epsilon -constraint like method and a single-objective evolutionary algorithm. The modification to the  epsilon-constraint is made to incorporate preferences, and simultaneously reduce the extension of the generated Pareto front.</rdfs:comment>
        <rdfs:label xml:lang="en">EGCM</rdfs:label>
    </owl:NamedIndividual>
    


    <!-- http://www.semanticweb.org/macoda/ontologies/PMOEA#LinearUtilityFunction -->

    <owl:NamedIndividual rdf:about="http://www.semanticweb.org/macoda/ontologies/PMOEA#LinearUtilityFunction">
        <rdf:type rdf:resource="http://www.semanticweb.org/macoda/ontologies/PMOEA#Linear"/>
        <rdfs:label xml:lang="en">LinearUtilityFunction</rdfs:label>
    </owl:NamedIndividual>
    


    <!-- http://www.semanticweb.org/macoda/ontologies/PMOEA#F2 -->

    <owl:NamedIndividual rdf:about="http://www.semanticweb.org/macoda/ontologies/PMOEA#F2">
        <rdf:type rdf:resource="http://www.semanticweb.org/macoda/ontologies/PMOEA#Academic_Problem"/>
        <PMOEA:isContinuousProblem rdf:datatype="http://www.w3.org/2001/XMLSchema#boolean">true</PMOEA:isContinuousProblem>
        <PMOEA:ObjectiveNumber rdf:datatype="http://www.w3.org/2001/XMLSchema#integer">2</PMOEA:ObjectiveNumber>
        <rdfs:comment>Y. Jin, M. Olhofer, and B. Sendhoff. Evolutionaynamic
weighted aggregation: Why does it work and how? In
L. Spector, E. Goodman, A. Wu, W.B. Langdon, H.-
M. Voigt, M. Gen, S. Sen, M. DOrigo, S. Pezeshk,
M. Garzon, and E. Burke, editors, Proceedings of Ge-
netic and Evolutionary Computation Conference, pages
10421049, San Francisco, CA, 2001</rdfs:comment>
        <rdfs:label xml:lang="en">F2</rdfs:label>
    </owl:NamedIndividual>
    


    <!-- http://www.semanticweb.org/macoda/ontologies/PMOEA#PMA -->

    <owl:NamedIndividual rdf:about="http://www.semanticweb.org/macoda/ontologies/PMOEA#PMA">
        <rdf:type rdf:resource="http://www.semanticweb.org/macoda/ontologies/PMOEA#Memetic"/>
        <rdfs:comment>Pareto memetic algorithm (PMA) is a hybrid multiple objective evolutionary algorithm. The main idea of the algorithm is to draw at random a weight vector in each iteration. The weight vector defines a scalarizing function. Two solutions, being very good on the scalarizing function are then recombined and a local heuristic is applied to the offspring</rdfs:comment>
        <rdfs:label xml:lang="en">PMA</rdfs:label>
    </owl:NamedIndividual>
    


    <!-- http://www.semanticweb.org/macoda/ontologies/PMOEA#g-dominance -->

    <owl:NamedIndividual rdf:about="http://www.semanticweb.org/macoda/ontologies/PMOEA#g-dominance">
        <rdf:type rdf:resource="http://www.semanticweb.org/macoda/ontologies/PMOEA#DominanceRelation"/>
        <rdfs:comment>In this relation, objective vectors satisfying all the aspiration values and objective vectors fulfilling none of them are preferred over objective vectors satisfying some of the aspiration levels.</rdfs:comment>
        <rdfs:label xml:lang="en">g-dominance</rdfs:label>
    </owl:NamedIndividual>
    


    <!-- http://www.semanticweb.org/macoda/ontologies/PMOEA#PI-EMO-PC -->

    <owl:NamedIndividual rdf:about="http://www.semanticweb.org/macoda/ontologies/PMOEA#PI-EMO-PC">
        <rdf:type rdf:resource="http://www.semanticweb.org/macoda/ontologies/PMOEA#PMOEA"/>
        <PMOEA:hasPreferenceModel rdf:resource="http://www.semanticweb.org/macoda/ontologies/PMOEA#PolyhedralCone"/>
        <PMOEA:hasPreferenceInformationFromDM rdf:resource="http://www.semanticweb.org/macoda/ontologies/PMOEA#PickTheBest"/>
        <PMOEA:hasInteractionTime rdf:resource="http://www.semanticweb.org/macoda/ontologies/PMOEA#progressive"/>
        <PMOEA:hasPreferenceIntegration rdf:resource="http://www.semanticweb.org/macoda/ontologies/PMOEA#PolyhedralCone-dominance"/>
        <PMOEA:hasPreferenceIntegration rdf:resource="http://www.semanticweb.org/macoda/ontologies/PMOEA#LocalSearch-basedTerminationCriterion"/>
        <PMOEA:canSolve rdf:resource="http://www.semanticweb.org/macoda/ontologies/PMOEA#DTLZ2_5"/>
        <PMOEA:canSolve rdf:resource="http://www.semanticweb.org/macoda/ontologies/PMOEA#DTLZ2_3"/>
        <PMOEA:canSolve rdf:resource="http://www.semanticweb.org/macoda/ontologies/PMOEA#ZDT1"/>
        <PMOEA:hasResultInfluence rdf:resource="http://www.semanticweb.org/macoda/ontologies/PMOEA#OneSolution"/>
        <PMOEA:hasAuthor rdf:resource="http://www.semanticweb.org/macoda/ontologies/PMOEA#Ankur_Sinha"/>
        <PMOEA:hasAuthor rdf:resource="http://www.semanticweb.org/macoda/ontologies/PMOEA#Jyrki_Wallenius"/>
        <PMOEA:hasAuthor rdf:resource="http://www.semanticweb.org/macoda/ontologies/PMOEA#Kalyanmoy_Deb"/>
        <PMOEA:hasAuthor rdf:resource="http://www.semanticweb.org/macoda/ontologies/PMOEA#Pekka_J._Korhonen"/>
        <PMOEA:hasSearchAlgorithm rdf:resource="http://www.semanticweb.org/macoda/ontologies/PMOEA#NSGA-II"/>
        <PMOEA:hasDevelopingYear rdf:datatype="http://www.w3.org/2001/XMLSchema#integer">2010</PMOEA:hasDevelopingYear>
        <PMOEA:ParetoDominancePreservation rdf:datatype="http://www.w3.org/2001/XMLSchema#boolean">true</PMOEA:ParetoDominancePreservation>
        <PMOEA:hasReference>Sinha, A., P. Korhonen, J. Wallenius and K. Deb (2010). An interactive evolutionary multi-objective optimization method based on polyhedral cones. Learning and Intelligent Optimization, Springer: 318-332</PMOEA:hasReference>
        <rdfs:comment>a polyhedral cone is used to construct the DM preference. The constructed polyhedral cone is then applied to modify the domination principle of an EMO and drives the search towards a preferred region</rdfs:comment>
        <rdfs:label xml:lang="en">PI-EMO-PC</rdfs:label>
    </owl:NamedIndividual>
    


    <!-- http://www.semanticweb.org/macoda/ontologies/PMOEA#NN-DM-iTDEA -->

    <owl:NamedIndividual rdf:about="http://www.semanticweb.org/macoda/ontologies/PMOEA#NN-DM-iTDEA">
        <rdf:type rdf:resource="http://www.semanticweb.org/macoda/ontologies/PMOEA#PMOEA"/>
        <PMOEA:hasPreferenceModel rdf:resource="http://www.semanticweb.org/macoda/ontologies/PMOEA#GeneralUtilityFunction"/>
        <PMOEA:hasPreferenceInformationFromDM rdf:resource="http://www.semanticweb.org/macoda/ontologies/PMOEA#PickTheBest"/>
        <PMOEA:hasInteractionTime rdf:resource="http://www.semanticweb.org/macoda/ontologies/PMOEA#progressive"/>
        <PMOEA:hasPreferenceIntegration rdf:resource="http://www.semanticweb.org/macoda/ontologies/PMOEA#TerritorySize"/>
        <PMOEA:hasLearningMethod rdf:resource="http://www.semanticweb.org/macoda/ontologies/PMOEA#ArtificialNeuralNetwork"/>
        <PMOEA:canSolve rdf:resource="http://www.semanticweb.org/macoda/ontologies/PMOEA#Pedro_2"/>
        <PMOEA:canSolve rdf:resource="http://www.semanticweb.org/macoda/ontologies/PMOEA#Pedro_3"/>
        <PMOEA:hasResultInfluence rdf:resource="http://www.semanticweb.org/macoda/ontologies/PMOEA#BiasedDistribution"/>
        <PMOEA:hasAuthor rdf:resource="http://www.semanticweb.org/macoda/ontologies/PMOEA#Ricardo_H_C_Takahashi"/>
        <PMOEA:hasAuthor rdf:resource="http://www.semanticweb.org/macoda/ontologies/PMOEA#Luciana_R_Pedro"/>
        <PMOEA:hasSearchAlgorithm rdf:resource="http://www.semanticweb.org/macoda/ontologies/PMOEA#TDEA"/>
        <PMOEA:hasDevelopingYear rdf:datatype="http://www.w3.org/2001/XMLSchema#integer">2013</PMOEA:hasDevelopingYear>
        <PMOEA:hasReference>Pedro, L. R. and R. H. Takahashi (2013). Decision-maker preference modeling in interactive multiobjective optimization. Evolutionary Multi-Criterion Optimization, Springer</PMOEA:hasReference>
        <rdfs:comment>This paper presents the results of the hybridization of the iTDEA with an enhanced version of NN-DM. Using the same amount of preference information required by the iTDEA, the NN-DM is able to construct a model for the DMs preferences, so that no more queries are required from the DM related to that specific region of the objective space. This model can now solve similar decision-making problems that comes from optimization problem leading to Pareto-optimal fronts in the same region of the space. Once this preference model is adjusted, it can be used inside the optimization process to guide the search without demanding more information from the DM.</rdfs:comment>
        <rdfs:label xml:lang="en">NN-DM-iTDEA</rdfs:label>
    </owl:NamedIndividual>
    


    <!-- http://www.semanticweb.org/macoda/ontologies/PMOEA#a-posteriori -->

    <owl:NamedIndividual rdf:about="http://www.semanticweb.org/macoda/ontologies/PMOEA#a-posteriori">
        <rdf:type rdf:resource="http://www.semanticweb.org/macoda/ontologies/PMOEA#a-posteriori"/>
        <rdfs:label xml:lang="en">a-posteriori</rdfs:label>
    </owl:NamedIndividual>
    


    <!-- http://www.semanticweb.org/macoda/ontologies/PMOEA#DTLZ1_3 -->

    <owl:NamedIndividual rdf:about="http://www.semanticweb.org/macoda/ontologies/PMOEA#DTLZ1_3">
        <rdf:type rdf:resource="http://www.semanticweb.org/macoda/ontologies/PMOEA#DTLZ"/>
        <PMOEA:OWLDataProperty_61d3cd95_fde4_4c1b_af08_1eaf73473aea rdf:datatype="http://www.w3.org/2001/XMLSchema#boolean">true</PMOEA:OWLDataProperty_61d3cd95_fde4_4c1b_af08_1eaf73473aea>
        <PMOEA:isContinuousProblem rdf:datatype="http://www.w3.org/2001/XMLSchema#boolean">true</PMOEA:isContinuousProblem>
        <PMOEA:ObjectiveNumber rdf:datatype="http://www.w3.org/2001/XMLSchema#integer">3</PMOEA:ObjectiveNumber>
        <rdfs:label xml:lang="en">DTLZ1_3</rdfs:label>
    </owl:NamedIndividual>
    


    <!-- http://www.semanticweb.org/macoda/ontologies/PMOEA#R2Indicator -->

    <owl:NamedIndividual rdf:about="http://www.semanticweb.org/macoda/ontologies/PMOEA#R2Indicator">
        <rdf:type rdf:resource="http://www.semanticweb.org/macoda/ontologies/PMOEA#SetQualityIndicator"/>
        <rdfs:label xml:lang="en">R2Indicator</rdfs:label>
    </owl:NamedIndividual>
    


    <!-- http://www.semanticweb.org/macoda/ontologies/PMOEA#PairwiseComparison -->

    <owl:NamedIndividual rdf:about="http://www.semanticweb.org/macoda/ontologies/PMOEA#PairwiseComparison">
        <rdf:type rdf:resource="http://www.semanticweb.org/macoda/ontologies/PMOEA#SolutionComparison"/>
        <rdfs:comment>The DM is expected to make pairwise comparison of a few pairs of reference alternatives</rdfs:comment>
        <rdfs:label xml:lang="en">PairwiseComparison</rdfs:label>
    </owl:NamedIndividual>
    


    <!-- http://www.semanticweb.org/macoda/ontologies/PMOEA#DI-MOEA -->

    <owl:NamedIndividual rdf:about="http://www.semanticweb.org/macoda/ontologies/PMOEA#DI-MOEA">
        <rdf:type rdf:resource="http://www.semanticweb.org/macoda/ontologies/PMOEA#PMOEA"/>
        <PMOEA:hasPreferenceModel rdf:resource="http://www.semanticweb.org/macoda/ontologies/PMOEA#HarringtonsDF"/>
        <PMOEA:hasPreferenceInformationFromDM rdf:resource="http://www.semanticweb.org/macoda/ontologies/PMOEA#parametersInDF"/>
        <PMOEA:hasInteractionTime rdf:resource="http://www.semanticweb.org/macoda/ontologies/PMOEA#a-priori"/>
        <PMOEA:hasPreferenceIntegration rdf:resource="http://www.semanticweb.org/macoda/ontologies/PMOEA#DesirabilityIndexbasedSelection"/>
        <PMOEA:hasComparison rdf:resource="http://www.semanticweb.org/macoda/ontologies/PMOEA#DF-SMS-EMOA"/>
        <PMOEA:hasComparison rdf:resource="http://www.semanticweb.org/macoda/ontologies/PMOEA#R-NSGA-II"/>
        <PMOEA:canSolve rdf:resource="http://www.semanticweb.org/macoda/ontologies/PMOEA#DTLZ1_5"/>
        <PMOEA:canSolve rdf:resource="http://www.semanticweb.org/macoda/ontologies/PMOEA#ZDT2"/>
        <PMOEA:canSolve rdf:resource="http://www.semanticweb.org/macoda/ontologies/PMOEA#DTLZ2_5"/>
        <PMOEA:canSolve rdf:resource="http://www.semanticweb.org/macoda/ontologies/PMOEA#DTLZ2_4"/>
        <PMOEA:canSolve rdf:resource="http://www.semanticweb.org/macoda/ontologies/PMOEA#ZDT4"/>
        <PMOEA:canSolve rdf:resource="http://www.semanticweb.org/macoda/ontologies/PMOEA#DTLZ1_3"/>
        <PMOEA:canSolve rdf:resource="http://www.semanticweb.org/macoda/ontologies/PMOEA#DTLZ1_4"/>
        <PMOEA:canSolve rdf:resource="http://www.semanticweb.org/macoda/ontologies/PMOEA#DTLZ2_3"/>
        <PMOEA:canSolve rdf:resource="http://www.semanticweb.org/macoda/ontologies/PMOEA#ZDT1"/>
        <PMOEA:hasResultInfluence rdf:resource="http://www.semanticweb.org/macoda/ontologies/PMOEA#BoundedRegion"/>
        <PMOEA:hasAuthor rdf:resource="http://www.semanticweb.org/macoda/ontologies/PMOEA#Heike_Trautmann"/>
        <PMOEA:hasAuthor rdf:resource="http://www.semanticweb.org/macoda/ontologies/PMOEA#Tobias_Wagner"/>
        <PMOEA:hasAuthor rdf:resource="http://www.semanticweb.org/macoda/ontologies/PMOEA#Dirk_Biermann"/>
        <PMOEA:hasAuthor rdf:resource="http://www.semanticweb.org/macoda/ontologies/PMOEA#Claus_Weihs"/>
        <PMOEA:useLibrary rdf:resource="http://www.semanticweb.org/macoda/ontologies/PMOEA#emoa"/>
        <PMOEA:hasSearchAlgorithm rdf:resource="http://www.semanticweb.org/macoda/ontologies/PMOEA#GeneralMOEA"/>
        <PMOEA:hasImplementationLanguage rdf:resource="http://www.semanticweb.org/macoda/ontologies/PMOEA#R"/>
        <PMOEA:hasDevelopingYear rdf:datatype="http://www.w3.org/2001/XMLSchema#integer">2013</PMOEA:hasDevelopingYear>
        <PMOEA:ParetoDominancePreservation rdf:datatype="http://www.w3.org/2001/XMLSchema#boolean">true</PMOEA:ParetoDominancePreservation>
        <PMOEA:hasReference>Trautmann, H., T. Wagner, D. Biermann and C. Weihs (2013). &quot;Indicator-based Selection in Evolutionary Multiobjective Optimization Algorithms Based On the Desirability Index.&quot; Journal of Multi-Criteria Decision Analysis 20(5-6): 319-337</PMOEA:hasReference>
        <rdfs:comment>In many-objective optimization, however, the computational complexity of the hypervolume can become a crucial part. Thus, an alternative to this approach(DF-SMS-EMOA) will be presented in this paper. The new algorithm operates in the untransformed objective space, but the desirability index (DI), that is, a DF-based scalarization, will be used as the second-level selection criterion in the non-dominated sorting.</rdfs:comment>
        <rdfs:label xml:lang="en">DI-MOEA</rdfs:label>
    </owl:NamedIndividual>
    


    <!-- http://www.semanticweb.org/macoda/ontologies/PMOEA#DTLZ1_4 -->

    <owl:NamedIndividual rdf:about="http://www.semanticweb.org/macoda/ontologies/PMOEA#DTLZ1_4">
        <rdf:type rdf:resource="http://www.semanticweb.org/macoda/ontologies/PMOEA#DTLZ"/>
        <PMOEA:OWLDataProperty_61d3cd95_fde4_4c1b_af08_1eaf73473aea rdf:datatype="http://www.w3.org/2001/XMLSchema#boolean">true</PMOEA:OWLDataProperty_61d3cd95_fde4_4c1b_af08_1eaf73473aea>
        <PMOEA:isContinuousProblem rdf:datatype="http://www.w3.org/2001/XMLSchema#boolean">true</PMOEA:isContinuousProblem>
        <PMOEA:ObjectiveNumber rdf:datatype="http://www.w3.org/2001/XMLSchema#integer">4</PMOEA:ObjectiveNumber>
        <PMOEA:isManyObjectiveProblem rdf:datatype="http://www.w3.org/2001/XMLSchema#boolean">true</PMOEA:isManyObjectiveProblem>
        <rdfs:label xml:lang="en">DTLZ1_4</rdfs:label>
    </owl:NamedIndividual>
    


    <!-- http://www.semanticweb.org/macoda/ontologies/PMOEA#Robin_C_Purshouse -->

    <owl:NamedIndividual rdf:about="http://www.semanticweb.org/macoda/ontologies/PMOEA#Robin_C_Purshouse">
        <rdf:type rdf:resource="http://www.semanticweb.org/macoda/ontologies/PMOEA#Researcher"/>
        <rdfs:label xml:lang="en">Robin C. Purshouse</rdfs:label>
    </owl:NamedIndividual>
    


    <!-- http://www.semanticweb.org/macoda/ontologies/PMOEA#BipolarPreferencePoint -->

    <owl:NamedIndividual rdf:about="http://www.semanticweb.org/macoda/ontologies/PMOEA#BipolarPreferencePoint">
        <rdf:type rdf:resource="http://www.semanticweb.org/macoda/ontologies/PMOEA#PreferencePoint"/>
        <rdfs:comment>DM wants to get solutions as close as to the positive reference point and as far as to the negative reference point</rdfs:comment>
        <rdfs:label xml:lang="en">BipolarPreferencePoint</rdfs:label>
    </owl:NamedIndividual>
    


    <!-- http://www.semanticweb.org/macoda/ontologies/PMOEA#DHI -->

    <owl:NamedIndividual rdf:about="http://www.semanticweb.org/macoda/ontologies/PMOEA#DHI">
        <rdf:type rdf:resource="http://www.semanticweb.org/macoda/ontologies/PMOEA#PMOEA"/>
        <PMOEA:hasPreferenceModel rdf:resource="http://www.semanticweb.org/macoda/ontologies/PMOEA#HarringtonsDF"/>
        <PMOEA:hasPreferenceModel rdf:resource="http://www.semanticweb.org/macoda/ontologies/PMOEA#Derringer-SuichDF"/>
        <PMOEA:hasPreferenceInformationFromDM rdf:resource="http://www.semanticweb.org/macoda/ontologies/PMOEA#parametersInDF"/>
        <PMOEA:hasInteractionTime rdf:resource="http://www.semanticweb.org/macoda/ontologies/PMOEA#a-priori"/>
        <PMOEA:hasPreferenceIntegration rdf:resource="http://www.semanticweb.org/macoda/ontologies/PMOEA#HypervolumeIndicator"/>
        <PMOEA:hasAuthor rdf:resource="http://www.semanticweb.org/macoda/ontologies/PMOEA#Andre_Deutz"/>
        <PMOEA:hasAuthor rdf:resource="http://www.semanticweb.org/macoda/ontologies/PMOEA#Michael_Emmerich"/>
        <PMOEA:hasAuthor rdf:resource="http://www.semanticweb.org/macoda/ontologies/PMOEA#Iryna_Yevseyeva"/>
        <PMOEA:hasDevelopingYear rdf:datatype="http://www.w3.org/2001/XMLSchema#integer">2014</PMOEA:hasDevelopingYear>
        <PMOEA:hasReference>Emmerich, M. T. M., A. H. Deutz and I. Yevseyeva (2014). &quot;On Reference Point Free Weighted Hypervolume Indicators based on Desirability Functions and their Probabilistic Interpretation.&quot; Procedia Technology 16: 532-541</PMOEA:hasReference>
        <rdfs:comment>This work presents a reference point free hypervolume indicator that uses a density that is derived from the users preferences expressed as desirability functions. This approach will bias the distribution of the approximation set towards a set that more densely samples highly desirable solutions of the objective space. It is shown that for a product type of aggregation the weighted hypervolume indicator is mathematically equivalent with an approach that computes the standard hypervolume indicator after transformation of the axes.It only propose a set indicator to incorporate preference, no searching algorithm involved.</rdfs:comment>
        <rdfs:label xml:lang="en">DHI</rdfs:label>
    </owl:NamedIndividual>
    


    <!-- http://www.semanticweb.org/macoda/ontologies/PMOEA#GoalVectors -->

    <owl:NamedIndividual rdf:about="http://www.semanticweb.org/macoda/ontologies/PMOEA#GoalVectors">
        <rdf:type rdf:resource="http://www.semanticweb.org/macoda/ontologies/PMOEA#ReferencePoint"/>
        <rdfs:comment>a set of aspiration points, used in PICEA-G.</rdfs:comment>
        <rdfs:label xml:lang="en">GoalVectors</rdfs:label>
    </owl:NamedIndividual>
    


    <!-- http://www.semanticweb.org/macoda/ontologies/PMOEA#ObjectiveSpaceWeightDistribution -->

    <owl:NamedIndividual rdf:about="http://www.semanticweb.org/macoda/ontologies/PMOEA#ObjectiveSpaceWeightDistribution">
        <rdf:type rdf:resource="http://www.semanticweb.org/macoda/ontologies/PMOEA#WeightFunctionInObjectiveSpace"/>
        <rdfs:label xml:lang="en">ObjectiveSpaceWeightDistribution</rdfs:label>
    </owl:NamedIndividual>
    


    <!-- http://www.semanticweb.org/macoda/ontologies/PMOEA#Lothar_Thiele -->

    <owl:NamedIndividual rdf:about="http://www.semanticweb.org/macoda/ontologies/PMOEA#Lothar_Thiele">
        <rdf:type rdf:resource="http://www.semanticweb.org/macoda/ontologies/PMOEA#Researcher"/>
        <rdfs:label xml:lang="en">Lothar Thiele</rdfs:label>
    </owl:NamedIndividual>
    


    <!-- http://www.semanticweb.org/macoda/ontologies/PMOEA#C++ -->

    <owl:NamedIndividual rdf:about="http://www.semanticweb.org/macoda/ontologies/PMOEA#C++">
        <rdf:type rdf:resource="http://www.semanticweb.org/macoda/ontologies/PMOEA#ProgrammingLanguage"/>
        <rdfs:label xml:lang="en">C++</rdfs:label>
    </owl:NamedIndividual>
    


    <!-- http://www.semanticweb.org/macoda/ontologies/PMOEA#H_Schmeck -->

    <owl:NamedIndividual rdf:about="http://www.semanticweb.org/macoda/ontologies/PMOEA#H_Schmeck">
        <rdf:type rdf:resource="http://www.semanticweb.org/macoda/ontologies/PMOEA#Researcher"/>
        <rdfs:label xml:lang="en">H.Schmeck</rdfs:label>
    </owl:NamedIndividual>
    


    <!-- http://www.semanticweb.org/macoda/ontologies/PMOEA#MQEA-PS -->

    <owl:NamedIndividual rdf:about="http://www.semanticweb.org/macoda/ontologies/PMOEA#MQEA-PS">
        <rdf:type rdf:resource="http://www.semanticweb.org/macoda/ontologies/PMOEA#PMOEA"/>
        <PMOEA:hasPreferenceModel rdf:resource="http://www.semanticweb.org/macoda/ontologies/PMOEA#FuzzyIntegral"/>
        <PMOEA:hasPreferenceModel rdf:resource="http://www.semanticweb.org/macoda/ontologies/PMOEA#FuzzyMeasure"/>
        <PMOEA:hasPreferenceInformationFromDM rdf:resource="http://www.semanticweb.org/macoda/ontologies/PMOEA#PairwiseComparisonMatrix"/>
        <PMOEA:hasInteractionTime rdf:resource="http://www.semanticweb.org/macoda/ontologies/PMOEA#a-priori"/>
        <PMOEA:hasPreferenceIntegration rdf:resource="http://www.semanticweb.org/macoda/ontologies/PMOEA#FrontSorting"/>
        <PMOEA:canSolve rdf:resource="http://www.semanticweb.org/macoda/ontologies/PMOEA#DTLZ3_7"/>
        <PMOEA:canSolve rdf:resource="http://www.semanticweb.org/macoda/ontologies/PMOEA#DTLZ7_7"/>
        <PMOEA:canSolve rdf:resource="http://www.semanticweb.org/macoda/ontologies/PMOEA#DTLZ1_7"/>
        <PMOEA:canSolve rdf:resource="http://www.semanticweb.org/macoda/ontologies/PMOEA#FuzzyPathPlannerOptimization"/>
        <PMOEA:canSolve rdf:resource="http://www.semanticweb.org/macoda/ontologies/PMOEA#DTLZ2_7"/>
        <PMOEA:canSolve rdf:resource="http://www.semanticweb.org/macoda/ontologies/PMOEA#DTLZ4_7"/>
        <PMOEA:hasResultInfluence rdf:resource="http://www.semanticweb.org/macoda/ontologies/PMOEA#OneSolution"/>
        <PMOEA:hasAuthor rdf:resource="http://www.semanticweb.org/macoda/ontologies/PMOEA#Ji-Hyeong_Han"/>
        <PMOEA:hasAuthor rdf:resource="http://www.semanticweb.org/macoda/ontologies/PMOEA#Ye-Hoon_Kim"/>
        <PMOEA:hasAuthor rdf:resource="http://www.semanticweb.org/macoda/ontologies/PMOEA#Eun-Soo_Kim"/>
        <PMOEA:hasAuthor rdf:resource="http://www.semanticweb.org/macoda/ontologies/PMOEA#Jong-Hwan_Kim"/>
        <PMOEA:hasAuthor rdf:resource="http://www.semanticweb.org/macoda/ontologies/PMOEA#Seung-Hwan_Choi"/>
        <PMOEA:hasSearchAlgorithm rdf:resource="http://www.semanticweb.org/macoda/ontologies/PMOEA#MQEA"/>
        <PMOEA:hasDevelopingYear rdf:datatype="http://www.w3.org/2001/XMLSchema#integer">2012</PMOEA:hasDevelopingYear>
        <PMOEA:ParetoDominancePreservation rdf:datatype="http://www.w3.org/2001/XMLSchema#boolean">true</PMOEA:ParetoDominancePreservation>
        <PMOEA:hasReference>Kim J H, Han J H, Kim Y H, et al. Preference-based solution selection algorithm for evolutionary multiobjective optimization[J]. Evolutionary Computation, IEEE Transactions on, 2012, 16(1): 20-34.</PMOEA:hasReference>
        <rdfs:comment>This paper proposes preference-based solution selection algorithm (PSSA) by which user can select a preferred one out of nondominated solutions obtained by any one of MOEAs. The PSSA, which is a kind of multiple criteria decision making (MCDM) algorithm, represents users preference to multiple objectives or criteria as a degree of consideration by fuzzy measure and globally evaluates obtained solutions by fuzzy integral. The PSSA is also  employed in each and every generation of evolutionary process to propose multi-objective quantum-inspired evolutionary algorithm with preference-based selection (MQEA-PS).</rdfs:comment>
        <rdfs:label xml:lang="en">MQEA-PS</rdfs:label>
    </owl:NamedIndividual>
    


    <!-- http://www.semanticweb.org/macoda/ontologies/PMOEA#Ankur_Sinha -->

    <owl:NamedIndividual rdf:about="http://www.semanticweb.org/macoda/ontologies/PMOEA#Ankur_Sinha">
        <rdf:type rdf:resource="http://www.semanticweb.org/macoda/ontologies/PMOEA#Researcher"/>
        <rdfs:label xml:lang="en">Ankur Sinha</rdfs:label>
    </owl:NamedIndividual>
    


    <!-- http://www.semanticweb.org/macoda/ontologies/PMOEA#Yaochu_Jin -->

    <owl:NamedIndividual rdf:about="http://www.semanticweb.org/macoda/ontologies/PMOEA#Yaochu_Jin">
        <rdf:type rdf:resource="http://www.semanticweb.org/macoda/ontologies/PMOEA#Researcher"/>
        <rdfs:label xml:lang="en">Yaochu Jin</rdfs:label>
    </owl:NamedIndividual>
    


    <!-- http://www.semanticweb.org/macoda/ontologies/PMOEA#WFG2_2 -->

    <owl:NamedIndividual rdf:about="http://www.semanticweb.org/macoda/ontologies/PMOEA#WFG2_2">
        <rdf:type rdf:resource="http://www.semanticweb.org/macoda/ontologies/PMOEA#WFG"/>
        <PMOEA:isContinuousProblem rdf:datatype="http://www.w3.org/2001/XMLSchema#boolean">true</PMOEA:isContinuousProblem>
        <PMOEA:ObjectiveNumber rdf:datatype="http://www.w3.org/2001/XMLSchema#integer">2</PMOEA:ObjectiveNumber>
        <rdfs:label xml:lang="en">WFG2_2</rdfs:label>
    </owl:NamedIndividual>
    


    <!-- http://www.semanticweb.org/macoda/ontologies/PMOEA#DTLZ7_7 -->

    <owl:NamedIndividual rdf:about="http://www.semanticweb.org/macoda/ontologies/PMOEA#DTLZ7_7">
        <rdf:type rdf:resource="http://www.semanticweb.org/macoda/ontologies/PMOEA#DTLZ"/>
        <PMOEA:isContinuousProblem rdf:datatype="http://www.w3.org/2001/XMLSchema#boolean">true</PMOEA:isContinuousProblem>
        <PMOEA:ObjectiveNumber rdf:datatype="http://www.w3.org/2001/XMLSchema#integer">7</PMOEA:ObjectiveNumber>
        <PMOEA:isManyObjectiveProblem rdf:datatype="http://www.w3.org/2001/XMLSchema#boolean">true</PMOEA:isManyObjectiveProblem>
        <rdfs:label xml:lang="en">DTLZ7_7</rdfs:label>
    </owl:NamedIndividual>
    


    <!-- http://www.semanticweb.org/macoda/ontologies/PMOEA#AS-EMOA -->

    <owl:NamedIndividual rdf:about="http://www.semanticweb.org/macoda/ontologies/PMOEA#AS-EMOA">
        <rdf:type rdf:resource="http://www.semanticweb.org/macoda/ontologies/PMOEA#Indicator_based"/>
        <rdfs:comment>Aspiration Set_based EMOA, using Averaged Hausdorff Distances as set quality indicator</rdfs:comment>
        <rdfs:label xml:lang="en">AS-EMOA</rdfs:label>
    </owl:NamedIndividual>
    


    <!-- http://www.semanticweb.org/macoda/ontologies/PMOEA#DTLZ1_6 -->

    <owl:NamedIndividual rdf:about="http://www.semanticweb.org/macoda/ontologies/PMOEA#DTLZ1_6">
        <rdf:type rdf:resource="http://www.semanticweb.org/macoda/ontologies/PMOEA#DTLZ"/>
        <PMOEA:OWLDataProperty_61d3cd95_fde4_4c1b_af08_1eaf73473aea rdf:datatype="http://www.w3.org/2001/XMLSchema#boolean">true</PMOEA:OWLDataProperty_61d3cd95_fde4_4c1b_af08_1eaf73473aea>
        <PMOEA:isContinuousProblem rdf:datatype="http://www.w3.org/2001/XMLSchema#boolean">true</PMOEA:isContinuousProblem>
        <PMOEA:ObjectiveNumber rdf:datatype="http://www.w3.org/2001/XMLSchema#integer">6</PMOEA:ObjectiveNumber>
        <PMOEA:isManyObjectiveProblem rdf:datatype="http://www.w3.org/2001/XMLSchema#boolean">true</PMOEA:isManyObjectiveProblem>
        <rdfs:label xml:lang="en">DTLZ1_6</rdfs:label>
    </owl:NamedIndividual>
    


    <!-- http://www.semanticweb.org/macoda/ontologies/PMOEA#AS_EMOA -->

    <owl:NamedIndividual rdf:about="http://www.semanticweb.org/macoda/ontologies/PMOEA#AS_EMOA">
        <rdf:type rdf:resource="http://www.semanticweb.org/macoda/ontologies/PMOEA#PMOEA"/>
        <PMOEA:hasPreferenceModel rdf:resource="http://www.semanticweb.org/macoda/ontologies/PMOEA#PreferencePointSet"/>
        <PMOEA:hasPreferenceInformationFromDM rdf:resource="http://www.semanticweb.org/macoda/ontologies/PMOEA#AspirationSet"/>
        <PMOEA:hasInteractionTime rdf:resource="http://www.semanticweb.org/macoda/ontologies/PMOEA#a-priori"/>
        <PMOEA:hasPreferenceIntegration rdf:resource="http://www.semanticweb.org/macoda/ontologies/PMOEA#AveragedHausdorffDistance"/>
        <PMOEA:canSolve rdf:resource="http://www.semanticweb.org/macoda/ontologies/PMOEA#DTLZ2_2"/>
        <PMOEA:canSolve rdf:resource="http://www.semanticweb.org/macoda/ontologies/PMOEA#SPHERE"/>
        <PMOEA:canSolve rdf:resource="http://www.semanticweb.org/macoda/ontologies/PMOEA#ZDT3"/>
        <PMOEA:canSolve rdf:resource="http://www.semanticweb.org/macoda/ontologies/PMOEA#DENT"/>
        <PMOEA:hasResultInfluence rdf:resource="http://www.semanticweb.org/macoda/ontologies/PMOEA#BoundedRegion"/>
        <PMOEA:hasAuthor rdf:resource="http://www.semanticweb.org/macoda/ontologies/PMOEA#Heike_Trautmann"/>
        <PMOEA:hasAuthor rdf:resource="http://www.semanticweb.org/macoda/ontologies/PMOEA#Gunter_Ridolph"/>
        <PMOEA:hasAuthor rdf:resource="http://www.semanticweb.org/macoda/ontologies/PMOEA#Christian_Grimme"/>
        <PMOEA:hasAuthor rdf:resource="http://www.semanticweb.org/macoda/ontologies/PMOEA#Oliver_Schutze"/>
        <PMOEA:hasSearchAlgorithm rdf:resource="http://www.semanticweb.org/macoda/ontologies/PMOEA#AS-EMOA"/>
        <PMOEA:hasDevelopingYear rdf:datatype="http://www.w3.org/2001/XMLSchema#integer">2014</PMOEA:hasDevelopingYear>
        <PMOEA:MultipleRegionOfInterest rdf:datatype="http://www.w3.org/2001/XMLSchema#boolean">true</PMOEA:MultipleRegionOfInterest>
        <PMOEA:hasReference>Pardalos, P. M., M. G. C. Resende, C. Vogiatzis and J. L. Walteros (2014). An Aspiration Set EMOA Based on Averaged Hausdorff Distances. LION 2014</PMOEA:hasReference>
        <rdfs:comment>We propose an evolutionary multiobjective algorithm that approximates multiple reference points (the aspiration set) in a single run using the concept of the averaged Hausdorff distance.</rdfs:comment>
        <rdfs:label xml:lang="en">AS_EMOA</rdfs:label>
    </owl:NamedIndividual>
    


    <!-- http://www.semanticweb.org/macoda/ontologies/PMOEA#Ki-Baek_Lee -->

    <owl:NamedIndividual rdf:about="http://www.semanticweb.org/macoda/ontologies/PMOEA#Ki-Baek_Lee">
        <rdf:type rdf:resource="http://www.semanticweb.org/macoda/ontologies/PMOEA#Researcher"/>
        <rdfs:label xml:lang="en">Ki-Baek Lee</rdfs:label>
    </owl:NamedIndividual>
    


    <!-- http://www.semanticweb.org/macoda/ontologies/PMOEA#WFG1_5 -->

    <owl:NamedIndividual rdf:about="http://www.semanticweb.org/macoda/ontologies/PMOEA#WFG1_5">
        <rdf:type rdf:resource="http://www.semanticweb.org/macoda/ontologies/PMOEA#WFG"/>
        <PMOEA:isContinuousProblem rdf:datatype="http://www.w3.org/2001/XMLSchema#boolean">true</PMOEA:isContinuousProblem>
        <PMOEA:ObjectiveNumber rdf:datatype="http://www.w3.org/2001/XMLSchema#integer">5</PMOEA:ObjectiveNumber>
        <PMOEA:isManyObjectiveProblem rdf:datatype="http://www.w3.org/2001/XMLSchema#boolean">true</PMOEA:isManyObjectiveProblem>
        <rdfs:label xml:lang="en">WFG1_5</rdfs:label>
    </owl:NamedIndividual>
    


    <!-- http://www.semanticweb.org/macoda/ontologies/PMOEA#FP -->

    <owl:NamedIndividual rdf:about="http://www.semanticweb.org/macoda/ontologies/PMOEA#FP">
        <rdf:type rdf:resource="http://www.semanticweb.org/macoda/ontologies/PMOEA#PMOEA"/>
        <PMOEA:hasPreferenceModel rdf:resource="http://www.semanticweb.org/macoda/ontologies/PMOEA#FuzzyPreferenceRelationOnObjectives"/>
        <PMOEA:hasPreferenceInformationFromDM rdf:resource="http://www.semanticweb.org/macoda/ontologies/PMOEA#linguisticComparisonOnObjectives"/>
        <PMOEA:hasPreferenceIntegration rdf:resource="http://www.semanticweb.org/macoda/ontologies/PMOEA#WeightedDominance"/>
        <PMOEA:hasPreferenceIntegration rdf:resource="http://www.semanticweb.org/macoda/ontologies/PMOEA#WeightedAggregation"/>
        <PMOEA:canSolve rdf:resource="http://www.semanticweb.org/macoda/ontologies/PMOEA#MiniCAPS"/>
        <PMOEA:hasResultInfluence rdf:resource="http://www.semanticweb.org/macoda/ontologies/PMOEA#BiasedDistribution"/>
        <PMOEA:hasResultInfluence rdf:resource="http://www.semanticweb.org/macoda/ontologies/PMOEA#OneSolution"/>
        <PMOEA:hasAuthor rdf:resource="http://www.semanticweb.org/macoda/ontologies/PMOEA#Ian_C_Parmee"/>
        <PMOEA:hasAuthor rdf:resource="http://www.semanticweb.org/macoda/ontologies/PMOEA#Dragan_Cvetkovic"/>
        <PMOEA:hasSearchAlgorithm rdf:resource="http://www.semanticweb.org/macoda/ontologies/PMOEA#SingleObjectiveEA"/>
        <PMOEA:hasSearchAlgorithm rdf:resource="http://www.semanticweb.org/macoda/ontologies/PMOEA#COGA"/>
        <PMOEA:hasDevelopingYear rdf:datatype="http://www.w3.org/2001/XMLSchema#integer">2002</PMOEA:hasDevelopingYear>
        <PMOEA:hasReference>Cvetkovic, D. &amp; Parmee, I. C. Preferences and their application in evolutionary multiobjective optimization IEEE Transactions on evolutionary computation, IEEE, 2002, 6, 42-57</PMOEA:hasReference>
        <rdfs:comment>The paper proposed a fuzzy preference that turns qualitative preference such as vastly more important, much more important into weights, then use the weights in sum-based method (single objective optimization), weighted Pareto optimization (new dominance relation is defined), weighted coevolutionary algorithm, dynamic constraint handling.</rdfs:comment>
        <rdfs:label xml:lang="en">FP</rdfs:label>
    </owl:NamedIndividual>
    


    <!-- http://www.semanticweb.org/macoda/ontologies/PMOEA#Std-EA -->

    <owl:NamedIndividual rdf:about="http://www.semanticweb.org/macoda/ontologies/PMOEA#Std-EA">
        <rdf:type rdf:resource="http://www.semanticweb.org/macoda/ontologies/PMOEA#PMOEA"/>
        <PMOEA:hasPreferenceModel rdf:resource="http://www.semanticweb.org/macoda/ontologies/PMOEA#IndexWithWeightedRanking"/>
        <PMOEA:hasPreferenceInformationFromDM rdf:resource="http://www.semanticweb.org/macoda/ontologies/PMOEA#weights"/>
        <PMOEA:hasInteractionTime rdf:resource="http://www.semanticweb.org/macoda/ontologies/PMOEA#a-priori"/>
        <PMOEA:hasPreferenceIntegration rdf:resource="http://www.semanticweb.org/macoda/ontologies/PMOEA#WeightedAggregation"/>
        <PMOEA:canSolve rdf:resource="http://www.semanticweb.org/macoda/ontologies/PMOEA#ReducerDesign"/>
        <PMOEA:hasResultInfluence rdf:resource="http://www.semanticweb.org/macoda/ontologies/PMOEA#OneSolution"/>
        <PMOEA:hasAuthor rdf:resource="http://www.semanticweb.org/macoda/ontologies/PMOEA#Qiang_Zhang"/>
        <PMOEA:hasAuthor rdf:resource="http://www.semanticweb.org/macoda/ontologies/PMOEA#Jianwei Wang"/>
        <PMOEA:hasSearchAlgorithm rdf:resource="http://www.semanticweb.org/macoda/ontologies/PMOEA#SingleObjectiveEA"/>
        <PMOEA:hasImplementationLanguage rdf:resource="http://www.semanticweb.org/macoda/ontologies/PMOEA#Matlab"/>
        <PMOEA:hasDevelopingYear rdf:datatype="http://www.w3.org/2001/XMLSchema#integer">2005</PMOEA:hasDevelopingYear>
        <PMOEA:hasReference>Wang, J.-W.; Zhang, Q.; Zhang, J.-M. &amp; Wei, X.-P. An approach to evolutionary multi-objective optimization algorithm with preference 2005 International Conference on Machine Learning and Cybernetics, 2005, 5, 2966-2970</PMOEA:hasReference>
        <rdfs:comment>a novel method of evolutionary multi-objective optimization algorithm with preference was proposed. It aims at solving multi-objective and multi-constraint problems, where the user incorporates his/her preferences about the objectives since the very start of the search process, by means of weights. It consists in considering the satisfaction of the constraints as a new objective, and using a multi-criteria decision aid method to rank the members of the EA population at each generation. Besides, adaptivity of the weights is applied in order to converge more easily towards the feasible domain</rdfs:comment>
        <rdfs:label xml:lang="en">Std-EA</rdfs:label>
    </owl:NamedIndividual>
    


    <!-- http://www.semanticweb.org/macoda/ontologies/PMOEA#Andrea_Passerini -->

    <owl:NamedIndividual rdf:about="http://www.semanticweb.org/macoda/ontologies/PMOEA#Andrea_Passerini">
        <rdf:type rdf:resource="http://www.semanticweb.org/macoda/ontologies/PMOEA#Researcher"/>
        <rdfs:label xml:lang="en">Andrea Passerini</rdfs:label>
    </owl:NamedIndividual>
    


    <!-- http://www.semanticweb.org/macoda/ontologies/PMOEA#Juergen_Branke -->

    <owl:NamedIndividual rdf:about="http://www.semanticweb.org/macoda/ontologies/PMOEA#Juergen_Branke">
        <rdf:type rdf:resource="http://www.semanticweb.org/macoda/ontologies/PMOEA#Researcher"/>
        <rdfs:label xml:lang="en">Juergen Branke</rdfs:label>
    </owl:NamedIndividual>
    


    <!-- http://www.semanticweb.org/macoda/ontologies/PMOEA#DTLZ1_7 -->

    <owl:NamedIndividual rdf:about="http://www.semanticweb.org/macoda/ontologies/PMOEA#DTLZ1_7">
        <rdf:type rdf:resource="http://www.semanticweb.org/macoda/ontologies/PMOEA#DTLZ"/>
        <PMOEA:OWLDataProperty_61d3cd95_fde4_4c1b_af08_1eaf73473aea rdf:datatype="http://www.w3.org/2001/XMLSchema#boolean">true</PMOEA:OWLDataProperty_61d3cd95_fde4_4c1b_af08_1eaf73473aea>
        <PMOEA:isContinuousProblem rdf:datatype="http://www.w3.org/2001/XMLSchema#boolean">true</PMOEA:isContinuousProblem>
        <PMOEA:ObjectiveNumber rdf:datatype="http://www.w3.org/2001/XMLSchema#integer">7</PMOEA:ObjectiveNumber>
        <PMOEA:isManyObjectiveProblem rdf:datatype="http://www.w3.org/2001/XMLSchema#boolean">true</PMOEA:isManyObjectiveProblem>
        <rdfs:label xml:lang="en">DTLZ1_7</rdfs:label>
    </owl:NamedIndividual>
    


    <!-- http://www.semanticweb.org/macoda/ontologies/PMOEA#Python -->

    <owl:NamedIndividual rdf:about="http://www.semanticweb.org/macoda/ontologies/PMOEA#Python">
        <rdf:type rdf:resource="http://www.semanticweb.org/macoda/ontologies/PMOEA#ProgrammingLanguage"/>
        <rdfs:label xml:lang="en">Python</rdfs:label>
    </owl:NamedIndividual>
    


    <!-- http://www.semanticweb.org/macoda/ontologies/PMOEA#PreferenceRegionModel -->

    <owl:NamedIndividual rdf:about="http://www.semanticweb.org/macoda/ontologies/PMOEA#PreferenceRegionModel">
        <rdf:type rdf:resource="http://www.semanticweb.org/macoda/ontologies/PMOEA#PreferenceRegion"/>
        <rdfs:comment>a region is specified by the DM and the goal is to find solutions in this region</rdfs:comment>
        <rdfs:label xml:lang="en">PreferenceRegionModel</rdfs:label>
    </owl:NamedIndividual>
    


    <!-- http://www.semanticweb.org/macoda/ontologies/PMOEA#WeightsInASF -->

    <owl:NamedIndividual rdf:about="http://www.semanticweb.org/macoda/ontologies/PMOEA#WeightsInASF">
        <rdf:type rdf:resource="http://www.semanticweb.org/macoda/ontologies/PMOEA#ASF"/>
        <rdfs:label xml:lang="en">WeightsInASF</rdfs:label>
    </owl:NamedIndividual>
    


    <!-- http://www.semanticweb.org/macoda/ontologies/PMOEA#GUESS-ASF -->

    <owl:NamedIndividual rdf:about="http://www.semanticweb.org/macoda/ontologies/PMOEA#GUESS-ASF">
        <rdf:type rdf:resource="http://www.semanticweb.org/macoda/ontologies/PMOEA#AchievementScalarizingFunction"/>
        <PMOEA:hasReference>J.T. Buchanan, A na ve approach for solving MCDM
problems: the GUESS method, Journal of the Operational
Research Society 48 (1997) 202206.</PMOEA:hasReference>
        <rdfs:comment>ASF used in GUESS method</rdfs:comment>
        <rdfs:label xml:lang="en">GUESS-ASF</rdfs:label>
    </owl:NamedIndividual>
    


    <!-- http://www.semanticweb.org/macoda/ontologies/PMOEA#Francesco_di_Pierro -->

    <owl:NamedIndividual rdf:about="http://www.semanticweb.org/macoda/ontologies/PMOEA#Francesco_di_Pierro">
        <rdf:type rdf:resource="http://www.semanticweb.org/macoda/ontologies/PMOEA#Researcher"/>
        <rdfs:label xml:lang="en">Francesco di Pierro</rdfs:label>
    </owl:NamedIndividual>
    


    <!-- http://www.semanticweb.org/macoda/ontologies/PMOEA#WeightedAggregation -->

    <owl:NamedIndividual rdf:about="http://www.semanticweb.org/macoda/ontologies/PMOEA#WeightedAggregation">
        <rdf:type rdf:resource="http://www.semanticweb.org/macoda/ontologies/PMOEA#Objectives"/>
        <rdfs:comment>transform multi-objective into single objective</rdfs:comment>
        <rdfs:label xml:lang="en">WeightedAggregation</rdfs:label>
    </owl:NamedIndividual>
    


    <!-- http://www.semanticweb.org/macoda/ontologies/PMOEA#Jan_Braun -->

    <owl:NamedIndividual rdf:about="http://www.semanticweb.org/macoda/ontologies/PMOEA#Jan_Braun">
        <rdf:type rdf:resource="http://www.semanticweb.org/macoda/ontologies/PMOEA#Researcher"/>
        <rdfs:label xml:lang="en">Jan Braun</rdfs:label>
    </owl:NamedIndividual>
    


    <!-- http://www.semanticweb.org/macoda/ontologies/PMOEA#PersonalBestUpdate -->

    <owl:NamedIndividual rdf:about="http://www.semanticweb.org/macoda/ontologies/PMOEA#PersonalBestUpdate">
        <rdf:type rdf:resource="http://www.semanticweb.org/macoda/ontologies/PMOEA#LeaderSelection"/>
        <rdfs:comment>in PSO</rdfs:comment>
        <rdfs:label xml:lang="en">PersonalBestUpdate</rdfs:label>
    </owl:NamedIndividual>
    


    <!-- http://www.semanticweb.org/macoda/ontologies/PMOEA#W_SPEA2 -->

    <owl:NamedIndividual rdf:about="http://www.semanticweb.org/macoda/ontologies/PMOEA#W_SPEA2">
        <rdf:type rdf:resource="http://www.semanticweb.org/macoda/ontologies/PMOEA#PMOEA"/>
        <PMOEA:hasPreferenceModel rdf:resource="http://www.semanticweb.org/macoda/ontologies/PMOEA#ObjectiveSpaceWeightDistribution"/>
        <PMOEA:hasPreferenceInformationFromDM rdf:resource="http://www.semanticweb.org/macoda/ontologies/PMOEA#ExponentialFunctionPreferOneObjective"/>
        <PMOEA:hasPreferenceInformationFromDM rdf:resource="http://www.semanticweb.org/macoda/ontologies/PMOEA#Ridge-likeFunctionPreferOneReferencePoint"/>
        <PMOEA:hasPreferenceInformationFromDM rdf:resource="http://www.semanticweb.org/macoda/ontologies/PMOEA#ExponentialFunctionPreferExtremalSolutions"/>
        <PMOEA:hasInteractionTime rdf:resource="http://www.semanticweb.org/macoda/ontologies/PMOEA#a-priori"/>
        <PMOEA:hasPreferenceIntegration rdf:resource="http://www.semanticweb.org/macoda/ontologies/PMOEA#FitnessSetting"/>
        <PMOEA:canSolve rdf:resource="http://www.semanticweb.org/macoda/ontologies/PMOEA#WFG1_2"/>
        <PMOEA:canSolve rdf:resource="http://www.semanticweb.org/macoda/ontologies/PMOEA#WFG3_2"/>
        <PMOEA:canSolve rdf:resource="http://www.semanticweb.org/macoda/ontologies/PMOEA#ZDT2"/>
        <PMOEA:canSolve rdf:resource="http://www.semanticweb.org/macoda/ontologies/PMOEA#ZDT6"/>
        <PMOEA:canSolve rdf:resource="http://www.semanticweb.org/macoda/ontologies/PMOEA#ZDT4"/>
        <PMOEA:canSolve rdf:resource="http://www.semanticweb.org/macoda/ontologies/PMOEA#WFG2_2"/>
        <PMOEA:canSolve rdf:resource="http://www.semanticweb.org/macoda/ontologies/PMOEA#ZDT3"/>
        <PMOEA:canSolve rdf:resource="http://www.semanticweb.org/macoda/ontologies/PMOEA#WFG5_2"/>
        <PMOEA:canSolve rdf:resource="http://www.semanticweb.org/macoda/ontologies/PMOEA#WFG4_2"/>
        <PMOEA:canSolve rdf:resource="http://www.semanticweb.org/macoda/ontologies/PMOEA#ZDT1"/>
        <PMOEA:hasResultInfluence rdf:resource="http://www.semanticweb.org/macoda/ontologies/PMOEA#BiasedDistribution"/>
        <PMOEA:hasAuthor rdf:resource="http://www.semanticweb.org/macoda/ontologies/PMOEA#Trent_Kroeger"/>
        <PMOEA:hasAuthor rdf:resource="http://www.semanticweb.org/macoda/ontologies/PMOEA#Frank_Neumann"/>
        <PMOEA:hasAuthor rdf:resource="http://www.semanticweb.org/macoda/ontologies/PMOEA#Tobias_Friedrich"/>
        <PMOEA:hasSearchAlgorithm rdf:resource="http://www.semanticweb.org/macoda/ontologies/PMOEA#SPEA2"/>
        <PMOEA:hasDevelopingYear rdf:datatype="http://www.w3.org/2001/XMLSchema#integer">2012</PMOEA:hasDevelopingYear>
        <PMOEA:ParetoDominancePreservation rdf:datatype="http://www.w3.org/2001/XMLSchema#boolean">true</PMOEA:ParetoDominancePreservation>
        <PMOEA:hasReference>Friedrich, T., T. Kroeger and F. Neumann (2012). &quot;Weighted preferences in evolutionary multi-objective optimization.&quot; International Journal of Machine Learning and Cybernetics 4(2): 139-148</PMOEA:hasReference>
        <rdfs:comment>In this paper, we present a neat and simple approach to use the preference information given by weightings on the objective space in classical algorithms such as NSGA-II and SPEA2. Furthermore, our algorithms are as efficient as the original implementation of NSGA-II and SPEA2 and do not have to deal with the expensive computations that hypervolume-based algorithms have to face.</rdfs:comment>
        <rdfs:label xml:lang="en">W_SPEA2</rdfs:label>
    </owl:NamedIndividual>
    


    <!-- http://www.semanticweb.org/macoda/ontologies/PMOEA#ReducerDesign -->

    <owl:NamedIndividual rdf:about="http://www.semanticweb.org/macoda/ontologies/PMOEA#ReducerDesign">
        <rdf:type rdf:resource="http://www.semanticweb.org/macoda/ontologies/PMOEA#Realworld_Problem"/>
        <PMOEA:isMixedInteger rdf:datatype="http://www.w3.org/2001/XMLSchema#boolean">true</PMOEA:isMixedInteger>
        <PMOEA:ObjectiveNumber rdf:datatype="http://www.w3.org/2001/XMLSchema#integer">3</PMOEA:ObjectiveNumber>
        <PMOEA:hasReference>Gao yugen, Wang guobiao, et.al. Optimization design based Genetic algorithm for helical gear reducer. Hoisting and conveying machinery, No.6, pp.47-49, June, 2003</PMOEA:hasReference>
        <rdfs:label xml:lang="en">ReducerDesign</rdfs:label>
    </owl:NamedIndividual>
    


    <!-- http://www.semanticweb.org/macoda/ontologies/PMOEA#DifferentialEvolution -->

    <owl:NamedIndividual rdf:about="http://www.semanticweb.org/macoda/ontologies/PMOEA#DifferentialEvolution">
        <rdf:type rdf:resource="http://www.semanticweb.org/macoda/ontologies/PMOEA#SOEA"/>
        <rdfs:label xml:lang="en">DifferentialEvolution</rdfs:label>
    </owl:NamedIndividual>
    


    <!-- http://www.semanticweb.org/macoda/ontologies/PMOEA#WFG9_2 -->

    <owl:NamedIndividual rdf:about="http://www.semanticweb.org/macoda/ontologies/PMOEA#WFG9_2">
        <rdf:type rdf:resource="http://www.semanticweb.org/macoda/ontologies/PMOEA#WFG"/>
        <PMOEA:OWLDataProperty_61d3cd95_fde4_4c1b_af08_1eaf73473aea rdf:datatype="http://www.w3.org/2001/XMLSchema#boolean">true</PMOEA:OWLDataProperty_61d3cd95_fde4_4c1b_af08_1eaf73473aea>
        <PMOEA:isContinuousProblem rdf:datatype="http://www.w3.org/2001/XMLSchema#boolean">true</PMOEA:isContinuousProblem>
        <PMOEA:ObjectiveNumber rdf:datatype="http://www.w3.org/2001/XMLSchema#integer">2</PMOEA:ObjectiveNumber>
        <rdfs:label xml:lang="en">WFG9_2</rdfs:label>
    </owl:NamedIndividual>
    


    <!-- http://www.semanticweb.org/macoda/ontologies/PMOEA#DTLZ1_2 -->

    <owl:NamedIndividual rdf:about="http://www.semanticweb.org/macoda/ontologies/PMOEA#DTLZ1_2">
        <rdf:type rdf:resource="http://www.semanticweb.org/macoda/ontologies/PMOEA#DTLZ"/>
        <PMOEA:OWLDataProperty_61d3cd95_fde4_4c1b_af08_1eaf73473aea rdf:datatype="http://www.w3.org/2001/XMLSchema#boolean">true</PMOEA:OWLDataProperty_61d3cd95_fde4_4c1b_af08_1eaf73473aea>
        <PMOEA:isContinuousProblem rdf:datatype="http://www.w3.org/2001/XMLSchema#boolean">true</PMOEA:isContinuousProblem>
        <PMOEA:ObjectiveNumber rdf:datatype="http://www.w3.org/2001/XMLSchema#integer">2</PMOEA:ObjectiveNumber>
        <rdfs:label xml:lang="en">DTLZ1_2</rdfs:label>
    </owl:NamedIndividual>
    


    <!-- http://www.semanticweb.org/macoda/ontologies/PMOEA#MDEPSO -->

    <owl:NamedIndividual rdf:about="http://www.semanticweb.org/macoda/ontologies/PMOEA#MDEPSO">
        <rdf:type rdf:resource="http://www.semanticweb.org/macoda/ontologies/PMOEA#PSO_based"/>
        <rdfs:comment>Multi-objective Differential Evolution and PSO (MDEPSO)</rdfs:comment>
        <rdfs:label xml:lang="en">MDEPSO</rdfs:label>
    </owl:NamedIndividual>
    


    <!-- http://www.semanticweb.org/macoda/ontologies/PMOEA#PreferencebasedSelection -->

    <owl:NamedIndividual rdf:about="http://www.semanticweb.org/macoda/ontologies/PMOEA#PreferencebasedSelection">
        <rdf:type rdf:resource="http://www.semanticweb.org/macoda/ontologies/PMOEA#SelectionCriterion"/>
        <rdfs:comment>In iEMOA-QCVF, selection probability is related to the index of the solution in the partially ordered population. Smaller index implies higher preference and more likely to be chosen.</rdfs:comment>
        <rdfs:label xml:lang="en">PreferencebasedSelection</rdfs:label>
    </owl:NamedIndividual>
    


    <!-- http://www.semanticweb.org/macoda/ontologies/PMOEA#PICEA-G -->

    <owl:NamedIndividual rdf:about="http://www.semanticweb.org/macoda/ontologies/PMOEA#PICEA-G">
        <rdf:type rdf:resource="http://www.semanticweb.org/macoda/ontologies/PMOEA#PMOEA"/>
        <PMOEA:hasPreferenceInformationFromDM rdf:resource="http://www.semanticweb.org/macoda/ontologies/PMOEA#GoalVectors"/>
        <PMOEA:hasInteractionTime rdf:resource="http://www.semanticweb.org/macoda/ontologies/PMOEA#a-posteriori"/>
        <PMOEA:hasPreferenceIntegration rdf:resource="http://www.semanticweb.org/macoda/ontologies/PMOEA#FitnessSetting"/>
        <PMOEA:hasInteractiveVersion rdf:resource="http://www.semanticweb.org/macoda/ontologies/PMOEA#iPICEA-G"/>
        <PMOEA:canSolve rdf:resource="http://www.semanticweb.org/macoda/ontologies/PMOEA#WFG2_7"/>
        <PMOEA:canSolve rdf:resource="http://www.semanticweb.org/macoda/ontologies/PMOEA#WFG2_2"/>
        <PMOEA:canSolve rdf:resource="http://www.semanticweb.org/macoda/ontologies/PMOEA#WFG2_10"/>
        <PMOEA:canSolve rdf:resource="http://www.semanticweb.org/macoda/ontologies/PMOEA#WFG2_4"/>
        <PMOEA:hasAuthor rdf:resource="http://www.semanticweb.org/macoda/ontologies/PMOEA#Rui_Wang"/>
        <PMOEA:hasAuthor rdf:resource="http://www.semanticweb.org/macoda/ontologies/PMOEA#Peter_J_Fleming"/>
        <PMOEA:hasAuthor rdf:resource="http://www.semanticweb.org/macoda/ontologies/PMOEA#Robin_C_Purshouse"/>
        <PMOEA:hasSearchAlgorithm rdf:resource="http://www.semanticweb.org/macoda/ontologies/PMOEA#PICEA"/>
        <PMOEA:hasDevelopingYear rdf:datatype="http://www.w3.org/2001/XMLSchema#integer">2013</PMOEA:hasDevelopingYear>
        <PMOEA:hasReference>Wang, R., R. C. Purshouse and P. J. Fleming (2013). &quot;Preference-inspired coevolutionary algorithms for many-objective optimization.&quot; Evolutionary Computation, IEEE Transactions on 17(4): 474-494</PMOEA:hasReference>
        <rdfs:comment>The concept of coevolving a family of decision-maker preferences together with a population of candidate solutions is studied here and demonstrated to have promising performance characteristics . After introducing the concept of the preference-inspired co-evolutionary algorithm (PICEA), a realization of this concept, PICEA-g, is systematically compared with four of the best-in-class MOEAs.</rdfs:comment>
        <rdfs:label xml:lang="en">PICEA-G</rdfs:label>
    </owl:NamedIndividual>
    


    <!-- http://www.semanticweb.org/macoda/ontologies/PMOEA#SPHERE -->

    <owl:NamedIndividual rdf:about="http://www.semanticweb.org/macoda/ontologies/PMOEA#SPHERE">
        <rdf:type rdf:resource="http://www.semanticweb.org/macoda/ontologies/PMOEA#Academic_Problem"/>
        <PMOEA:isContinuousProblem rdf:datatype="http://www.w3.org/2001/XMLSchema#boolean">true</PMOEA:isContinuousProblem>
        <PMOEA:ObjectiveNumber rdf:datatype="http://www.w3.org/2001/XMLSchema#integer">2</PMOEA:ObjectiveNumber>
        <rdfs:label xml:lang="en">SPHERE</rdfs:label>
    </owl:NamedIndividual>
    


    <!-- http://www.semanticweb.org/macoda/ontologies/PMOEA#Bo_Jiang -->

    <owl:NamedIndividual rdf:about="http://www.semanticweb.org/macoda/ontologies/PMOEA#Bo_Jiang">
        <rdf:type rdf:resource="http://www.semanticweb.org/macoda/ontologies/PMOEA#Researcher"/>
        <rdfs:label xml:lang="en">Bo Jiang</rdfs:label>
    </owl:NamedIndividual>
    


    <!-- http://www.semanticweb.org/macoda/ontologies/PMOEA#R2_MOEA -->

    <owl:NamedIndividual rdf:about="http://www.semanticweb.org/macoda/ontologies/PMOEA#R2_MOEA">
        <rdf:type rdf:resource="http://www.semanticweb.org/macoda/ontologies/PMOEA#PMOEA"/>
        <PMOEA:hasPreferenceModel rdf:resource="http://www.semanticweb.org/macoda/ontologies/PMOEA#TchebycheffASF"/>
        <PMOEA:hasPreferenceInformationFromDM rdf:resource="http://www.semanticweb.org/macoda/ontologies/PMOEA#ParatemtersInR2Indicator"/>
        <PMOEA:hasInteractionTime rdf:resource="http://www.semanticweb.org/macoda/ontologies/PMOEA#a-priori"/>
        <PMOEA:hasPreferenceIntegration rdf:resource="http://www.semanticweb.org/macoda/ontologies/PMOEA#R2Indicator"/>
        <PMOEA:canSolve rdf:resource="http://www.semanticweb.org/macoda/ontologies/PMOEA#DTLZ2_2"/>
        <PMOEA:canSolve rdf:resource="http://www.semanticweb.org/macoda/ontologies/PMOEA#DTLZ1_2"/>
        <PMOEA:canSolve rdf:resource="http://www.semanticweb.org/macoda/ontologies/PMOEA#ZDT1"/>
        <PMOEA:hasResultInfluence rdf:resource="http://www.semanticweb.org/macoda/ontologies/PMOEA#BiasedDistribution"/>
        <PMOEA:hasResultInfluence rdf:resource="http://www.semanticweb.org/macoda/ontologies/PMOEA#BoundedRegion"/>
        <PMOEA:hasAuthor rdf:resource="http://www.semanticweb.org/macoda/ontologies/PMOEA#Heike_Trautmann"/>
        <PMOEA:hasAuthor rdf:resource="http://www.semanticweb.org/macoda/ontologies/PMOEA#Tobias_Wagner"/>
        <PMOEA:hasAuthor rdf:resource="http://www.semanticweb.org/macoda/ontologies/PMOEA#Dimo_Brockhoff"/>
        <PMOEA:hasSearchAlgorithm rdf:resource="http://www.semanticweb.org/macoda/ontologies/PMOEA#R2_EMOA"/>
        <PMOEA:hasImplementationLanguage rdf:resource="http://www.semanticweb.org/macoda/ontologies/PMOEA#Matlab"/>
        <PMOEA:hasDevelopingYear rdf:datatype="http://www.w3.org/2001/XMLSchema#integer">2013</PMOEA:hasDevelopingYear>
        <PMOEA:MultipleRegionOfInterest rdf:datatype="http://www.w3.org/2001/XMLSchema#boolean">true</PMOEA:MultipleRegionOfInterest>
        <PMOEA:hasReference>Trautmann H, Wagner T, Brockhoff D. R2-EMOA: Focused multiobjective search using R2-indicator-based selection[M]//Learning and Intelligent Optimization. Springer Berlin Heidelberg, 2013: 70-74.</PMOEA:hasReference>
        <PMOEA:hasReference>Wagner, T., H. Trautmann and D. Brockhoff (2013). Preference articulation by means of the R2 indicator. Evolutionary Multi-Criterion Optimization, Springer</PMOEA:hasReference>
        <rdfs:comment>In this paper, three variants for integrating preferences into the R2 indicator were introduced. These variants exploit that the optimal -distributions for the R2-indicator are affected by moving the reference point, by restricting the weight space, as well as by skewing the weight vector distribution.Then in the second paper, An indicator-based evolutionary multiobjective optimization algorithm (EMOA) is introduced which incorporates the contribution to the unary R2-indicator as the secondary selection criterion</rdfs:comment>
        <rdfs:label xml:lang="en">R2_MOEA</rdfs:label>
    </owl:NamedIndividual>
    


    <!-- http://www.semanticweb.org/macoda/ontologies/PMOEA#Dunwei_Gong -->

    <owl:NamedIndividual rdf:about="http://www.semanticweb.org/macoda/ontologies/PMOEA#Dunwei_Gong">
        <rdf:type rdf:resource="http://www.semanticweb.org/macoda/ontologies/PMOEA#Researcher"/>
        <rdfs:label xml:lang="en">Dunwei Gong</rdfs:label>
    </owl:NamedIndividual>
    


    <!-- http://www.semanticweb.org/macoda/ontologies/PMOEA#Christian_Grimme -->

    <owl:NamedIndividual rdf:about="http://www.semanticweb.org/macoda/ontologies/PMOEA#Christian_Grimme">
        <rdf:type rdf:resource="http://www.semanticweb.org/macoda/ontologies/PMOEA#Researcher"/>
        <rdfs:label xml:lang="en">Christian Grimme</rdfs:label>
    </owl:NamedIndividual>
    


    <!-- http://www.semanticweb.org/macoda/ontologies/PMOEA#Roman_Sowinski -->

    <owl:NamedIndividual rdf:about="http://www.semanticweb.org/macoda/ontologies/PMOEA#Roman_Sowinski">
        <rdf:type rdf:resource="http://www.semanticweb.org/macoda/ontologies/PMOEA#Researcher"/>
        <rdfs:label xml:lang="en">Roman Sowiski</rdfs:label>
    </owl:NamedIndividual>
    


    <!-- http://www.semanticweb.org/macoda/ontologies/PMOEA#Hans-Georg -->

    <owl:NamedIndividual rdf:about="http://www.semanticweb.org/macoda/ontologies/PMOEA#Hans-Georg">
        <rdf:type rdf:resource="http://www.semanticweb.org/macoda/ontologies/PMOEA#Researcher"/>
        <rdfs:label xml:lang="en">Hans-Georg</rdfs:label>
    </owl:NamedIndividual>
    


    <!-- http://www.semanticweb.org/macoda/ontologies/PMOEA#PreferenceOrderingBasedonUtilityFunction -->

    <owl:NamedIndividual rdf:about="http://www.semanticweb.org/macoda/ontologies/PMOEA#PreferenceOrderingBasedonUtilityFunction">
        <rdf:type rdf:resource="http://www.semanticweb.org/macoda/ontologies/PMOEA#FrontSorting"/>
        <rdfs:comment>In BC-MOEA, a solution ranking procedure is 1) collecting the subset of non-dominated individuals in the population;2) sorting them according to the learned utility function;3) appending to the sorted set, the result of repeating the procedure on the remaining dominated individuals</rdfs:comment>
        <rdfs:label xml:lang="en">PreferenceOrderingBasedonUtilityFunction</rdfs:label>
    </owl:NamedIndividual>
    


    <!-- http://www.semanticweb.org/macoda/ontologies/PMOEA#Opt4J -->

    <owl:NamedIndividual rdf:about="http://www.semanticweb.org/macoda/ontologies/PMOEA#Opt4J">
        <rdf:type rdf:resource="http://www.semanticweb.org/macoda/ontologies/PMOEA#ImplementationLibrary"/>
        <rdfs:comment>Opt4J is an open source Java-based framework for evolutionary computation. It contains a set of (multi-objective) optimization algorithms such as evolutionary algorithms (including SPEA2 and NSGA2), differential evolution, particle swarm optimization, and simulated annealing. The benchmarks that are included comprise ZDT, DTLZ, WFG, and the knapsack problem.</rdfs:comment>
        <rdfs:label xml:lang="en">Opt4J</rdfs:label>
    </owl:NamedIndividual>
    


    <!-- http://www.semanticweb.org/macoda/ontologies/PMOEA#Esma_S_Gel -->

    <owl:NamedIndividual rdf:about="http://www.semanticweb.org/macoda/ontologies/PMOEA#Esma_S_Gel">
        <rdf:type rdf:resource="http://www.semanticweb.org/macoda/ontologies/PMOEA#Researcher"/>
        <rdfs:label xml:lang="en">Esma S. Gel</rdfs:label>
    </owl:NamedIndividual>
    


    <!-- http://www.semanticweb.org/macoda/ontologies/PMOEA#LocalSearch-basedTerminationCriterion -->

    <owl:NamedIndividual rdf:about="http://www.semanticweb.org/macoda/ontologies/PMOEA#LocalSearch-basedTerminationCriterion">
        <rdf:type rdf:resource="http://www.semanticweb.org/macoda/ontologies/PMOEA#TerminationCriterion"/>
        <rdfs:comment>In PI-EMO-PC and PI-EMO-VF, The authors additionally use the approximated value function or polyhedral cone to perform a local single-objective optimization starting with the solution ranked best by the DM. If this local improvement step is not able to improve the solutions value by at least a certain margin, it is concluded that the algorithm has found the most preferred solution and the optimization is stopped</rdfs:comment>
        <rdfs:label xml:lang="en">LocalSearch-basedTerminationCriterion</rdfs:label>
    </owl:NamedIndividual>
    


    <!-- http://www.semanticweb.org/macoda/ontologies/PMOEA#MOPSO-PS -->

    <owl:NamedIndividual rdf:about="http://www.semanticweb.org/macoda/ontologies/PMOEA#MOPSO-PS">
        <rdf:type rdf:resource="http://www.semanticweb.org/macoda/ontologies/PMOEA#PMOEA"/>
        <PMOEA:hasPreferenceModel rdf:resource="http://www.semanticweb.org/macoda/ontologies/PMOEA#FuzzyIntegral"/>
        <PMOEA:hasPreferenceModel rdf:resource="http://www.semanticweb.org/macoda/ontologies/PMOEA#FuzzyMeasure"/>
        <PMOEA:hasPreferenceInformationFromDM rdf:resource="http://www.semanticweb.org/macoda/ontologies/PMOEA#PairwiseComparisonMatrix"/>
        <PMOEA:hasInteractionTime rdf:resource="http://www.semanticweb.org/macoda/ontologies/PMOEA#a-priori"/>
        <PMOEA:hasPreferenceIntegration rdf:resource="http://www.semanticweb.org/macoda/ontologies/PMOEA#LeaderParticleSelection"/>
        <PMOEA:hasPreferenceIntegration rdf:resource="http://www.semanticweb.org/macoda/ontologies/PMOEA#FrontSorting"/>
        <PMOEA:canSolve rdf:resource="http://www.semanticweb.org/macoda/ontologies/PMOEA#DTLZ1_7"/>
        <PMOEA:canSolve rdf:resource="http://www.semanticweb.org/macoda/ontologies/PMOEA#DTLZ2_7"/>
        <PMOEA:hasResultInfluence rdf:resource="http://www.semanticweb.org/macoda/ontologies/PMOEA#BoundedRegion"/>
        <PMOEA:hasAuthor rdf:resource="http://www.semanticweb.org/macoda/ontologies/PMOEA#Ki-Baek_Lee"/>
        <PMOEA:hasAuthor rdf:resource="http://www.semanticweb.org/macoda/ontologies/PMOEA#Jong-Hwan_Kim"/>
        <PMOEA:hasSearchAlgorithm rdf:resource="http://www.semanticweb.org/macoda/ontologies/PMOEA#MOPSO"/>
        <PMOEA:hasDevelopingYear rdf:datatype="http://www.w3.org/2001/XMLSchema#integer">2011</PMOEA:hasDevelopingYear>
        <PMOEA:hasReference>Lee, K.-B. and J.-H. Kim (2011). Multi-objective particle swarm optimization with preference-based sorting. Evolutionary Computation (CEC), 2011 IEEE Congress on, IEEE</PMOEA:hasReference>
        <rdfs:comment>In this paper, multi-objective particle swarm optimization with preference-based sorting (MOPSO-PS) is proposed, where a global best position is randomly selected from the archive of nondominated solutions sorted by global evaluation considering users preferences for multiple objectives. The users preference is represented as a degree of consideration for the objectives by the fuzzy measures. The global evaluation of the solutions is carried out by the fuzzy integral of partial evaluation with respect to the fuzzy measures, where the partial evaluation of each solution is obtained as a normalized objective function value.</rdfs:comment>
        <rdfs:label xml:lang="en">MOPSO-PS</rdfs:label>
    </owl:NamedIndividual>
    


    <!-- http://www.semanticweb.org/macoda/ontologies/PMOEA#DTLZ3_10 -->

    <owl:NamedIndividual rdf:about="http://www.semanticweb.org/macoda/ontologies/PMOEA#DTLZ3_10">
        <rdf:type rdf:resource="http://www.semanticweb.org/macoda/ontologies/PMOEA#DTLZ"/>
        <PMOEA:OWLDataProperty_61d3cd95_fde4_4c1b_af08_1eaf73473aea rdf:datatype="http://www.w3.org/2001/XMLSchema#boolean">true</PMOEA:OWLDataProperty_61d3cd95_fde4_4c1b_af08_1eaf73473aea>
        <PMOEA:isContinuousProblem rdf:datatype="http://www.w3.org/2001/XMLSchema#boolean">true</PMOEA:isContinuousProblem>
        <PMOEA:ObjectiveNumber rdf:datatype="http://www.w3.org/2001/XMLSchema#integer">10</PMOEA:ObjectiveNumber>
        <PMOEA:isManyObjectiveProblem rdf:datatype="http://www.w3.org/2001/XMLSchema#boolean">true</PMOEA:isManyObjectiveProblem>
        <rdfs:label xml:lang="en">DTLZ3_10</rdfs:label>
    </owl:NamedIndividual>
    


    <!-- http://www.semanticweb.org/macoda/ontologies/PMOEA#GSP_2 -->

    <owl:NamedIndividual rdf:about="http://www.semanticweb.org/macoda/ontologies/PMOEA#GSP_2">
        <rdf:type rdf:resource="http://www.semanticweb.org/macoda/ontologies/PMOEA#Academic_Problem"/>
        <PMOEA:isContinuousProblem rdf:datatype="http://www.w3.org/2001/XMLSchema#boolean">true</PMOEA:isContinuousProblem>
        <PMOEA:ObjectiveNumber rdf:datatype="http://www.w3.org/2001/XMLSchema#integer">2</PMOEA:ObjectiveNumber>
        <PMOEA:hasReference>Emmerich, M.T.M., Deutz, A.H.: Test Problems Based on Lame Superspheres.
In: Obayashi, S., Deb, K., Poloni, C., Hiroyasu, T., Murata, T. (eds.) EMO 2007.
LNCS, vol. 4403, pp. 922936. Springer, Heidelberg (2007)</PMOEA:hasReference>
        <rdfs:label xml:lang="en">GSP_2</rdfs:label>
    </owl:NamedIndividual>
    


    <!-- http://www.semanticweb.org/macoda/ontologies/PMOEA#Tobias_Wagner -->

    <owl:NamedIndividual rdf:about="http://www.semanticweb.org/macoda/ontologies/PMOEA#Tobias_Wagner">
        <rdf:type rdf:resource="http://www.semanticweb.org/macoda/ontologies/PMOEA#Researcher"/>
        <rdfs:label xml:lang="en">Tobias Wagner</rdfs:label>
    </owl:NamedIndividual>
    


    <!-- http://www.semanticweb.org/macoda/ontologies/PMOEA#Jyrki_Wallenius -->

    <owl:NamedIndividual rdf:about="http://www.semanticweb.org/macoda/ontologies/PMOEA#Jyrki_Wallenius">
        <rdf:type rdf:resource="http://www.semanticweb.org/macoda/ontologies/PMOEA#Researcher"/>
        <rdfs:label xml:lang="en">Jyrki Wallenius</rdfs:label>
    </owl:NamedIndividual>
    


    <!-- http://www.semanticweb.org/macoda/ontologies/PMOEA#WFG2_10 -->

    <owl:NamedIndividual rdf:about="http://www.semanticweb.org/macoda/ontologies/PMOEA#WFG2_10">
        <rdf:type rdf:resource="http://www.semanticweb.org/macoda/ontologies/PMOEA#WFG"/>
        <PMOEA:isContinuousProblem rdf:datatype="http://www.w3.org/2001/XMLSchema#boolean">true</PMOEA:isContinuousProblem>
        <PMOEA:ObjectiveNumber rdf:datatype="http://www.w3.org/2001/XMLSchema#integer">10</PMOEA:ObjectiveNumber>
        <PMOEA:isManyObjectiveProblem rdf:datatype="http://www.w3.org/2001/XMLSchema#boolean">true</PMOEA:isManyObjectiveProblem>
        <rdfs:label xml:lang="en">WFG2_10</rdfs:label>
    </owl:NamedIndividual>
    


    <!-- http://www.semanticweb.org/macoda/ontologies/PMOEA#ER-NSGA-II -->

    <owl:NamedIndividual rdf:about="http://www.semanticweb.org/macoda/ontologies/PMOEA#ER-NSGA-II">
        <rdf:type rdf:resource="http://www.semanticweb.org/macoda/ontologies/PMOEA#PMOEA"/>
        <PMOEA:hasPreferenceModel rdf:resource="http://www.semanticweb.org/macoda/ontologies/PMOEA#PreferencePoint"/>
        <PMOEA:hasPreferenceInformationFromDM rdf:resource="http://www.semanticweb.org/macoda/ontologies/PMOEA#ReferencePoint"/>
        <PMOEA:hasInteractionTime rdf:resource="http://www.semanticweb.org/macoda/ontologies/PMOEA#a-priori"/>
        <PMOEA:hasPreferenceIntegration rdf:resource="http://www.semanticweb.org/macoda/ontologies/PMOEA#SelectionOfNSGAII"/>
        <PMOEA:canSolve rdf:resource="http://www.semanticweb.org/macoda/ontologies/PMOEA#ZDT1"/>
        <PMOEA:hasResultInfluence rdf:resource="http://www.semanticweb.org/macoda/ontologies/PMOEA#BoundedRegion"/>
        <PMOEA:hasAuthor rdf:resource="http://www.semanticweb.org/macoda/ontologies/PMOEA#Amos_H_C_Ng"/>
        <PMOEA:hasAuthor rdf:resource="http://www.semanticweb.org/macoda/ontologies/PMOEA#Florian Siegmund"/>
        <PMOEA:hasAuthor rdf:resource="http://www.semanticweb.org/macoda/ontologies/PMOEA#Kalyanmoy_Deb"/>
        <PMOEA:isExtensionOf rdf:resource="http://www.semanticweb.org/macoda/ontologies/PMOEA#R-NSGA-II"/>
        <PMOEA:hasSearchAlgorithm rdf:resource="http://www.semanticweb.org/macoda/ontologies/PMOEA#NSGA-II"/>
        <PMOEA:hasDevelopingYear rdf:datatype="http://www.w3.org/2001/XMLSchema#integer">2012</PMOEA:hasDevelopingYear>
        <PMOEA:SpreadControl rdf:datatype="http://www.w3.org/2001/XMLSchema#boolean">true</PMOEA:SpreadControl>
        <PMOEA:ParetoDominancePreservation rdf:datatype="http://www.w3.org/2001/XMLSchema#boolean">true</PMOEA:ParetoDominancePreservation>
        <PMOEA:hasReference>Siegmund, Florian, Amos HC Ng, and Kalyanmoy Deb. &quot;Finding a preferred diverse set of Pareto-optimal solutions for a limited number of function calls.&quot; 2012 IEEE Congress on Evolutionary Computation. IEEE, 2012.</PMOEA:hasReference>
        <rdfs:comment>In this paper, we propose an extension to R-NSGA-II that limits the Pareto-fitness to speed up the search for a limited number of function calls. It avoids to automatically select all solutions of the first front of the candidate set into the next population. In this way non-preferred Pareto-optimal solutions are not considered thereby accelerating the search process</rdfs:comment>
        <rdfs:label xml:lang="en">ER-NSGA-II</rdfs:label>
    </owl:NamedIndividual>
    


    <!-- http://www.semanticweb.org/macoda/ontologies/PMOEA#DTLZ7_6 -->

    <owl:NamedIndividual rdf:about="http://www.semanticweb.org/macoda/ontologies/PMOEA#DTLZ7_6">
        <rdf:type rdf:resource="http://www.semanticweb.org/macoda/ontologies/PMOEA#DTLZ"/>
        <PMOEA:isContinuousProblem rdf:datatype="http://www.w3.org/2001/XMLSchema#boolean">true</PMOEA:isContinuousProblem>
        <PMOEA:ObjectiveNumber rdf:datatype="http://www.w3.org/2001/XMLSchema#integer">7</PMOEA:ObjectiveNumber>
        <PMOEA:isManyObjectiveProblem rdf:datatype="http://www.w3.org/2001/XMLSchema#boolean">true</PMOEA:isManyObjectiveProblem>
        <rdfs:label xml:lang="en">DTLZ7_6</rdfs:label>
    </owl:NamedIndividual>
    


    <!-- http://www.semanticweb.org/macoda/ontologies/PMOEA#DTLZ1_8 -->

    <owl:NamedIndividual rdf:about="http://www.semanticweb.org/macoda/ontologies/PMOEA#DTLZ1_8">
        <rdf:type rdf:resource="http://www.semanticweb.org/macoda/ontologies/PMOEA#DTLZ"/>
        <PMOEA:OWLDataProperty_61d3cd95_fde4_4c1b_af08_1eaf73473aea rdf:datatype="http://www.w3.org/2001/XMLSchema#boolean">true</PMOEA:OWLDataProperty_61d3cd95_fde4_4c1b_af08_1eaf73473aea>
        <PMOEA:isContinuousProblem rdf:datatype="http://www.w3.org/2001/XMLSchema#boolean">true</PMOEA:isContinuousProblem>
        <PMOEA:ObjectiveNumber rdf:datatype="http://www.w3.org/2001/XMLSchema#integer">8</PMOEA:ObjectiveNumber>
        <PMOEA:isManyObjectiveProblem rdf:datatype="http://www.w3.org/2001/XMLSchema#boolean">true</PMOEA:isManyObjectiveProblem>
        <rdfs:label xml:lang="en">DTLZ1_8</rdfs:label>
    </owl:NamedIndividual>
    


    <!-- http://www.semanticweb.org/macoda/ontologies/PMOEA#MOGA -->

    <owl:NamedIndividual rdf:about="http://www.semanticweb.org/macoda/ontologies/PMOEA#MOGA">
        <rdf:type rdf:resource="http://www.semanticweb.org/macoda/ontologies/PMOEA#DiversityVSConvergence_based"/>
        <rdfs:label xml:lang="en">MOGA</rdfs:label>
    </owl:NamedIndividual>
    


    <!-- http://www.semanticweb.org/macoda/ontologies/PMOEA#Jing_Sun -->

    <owl:NamedIndividual rdf:about="http://www.semanticweb.org/macoda/ontologies/PMOEA#Jing_Sun">
        <rdf:type rdf:resource="http://www.semanticweb.org/macoda/ontologies/PMOEA#Researcher"/>
        <rdfs:label xml:lang="en">Jing Sun</rdfs:label>
    </owl:NamedIndividual>
    


    <!-- http://www.semanticweb.org/macoda/ontologies/PMOEA#NSGAIII -->

    <owl:NamedIndividual rdf:about="http://www.semanticweb.org/macoda/ontologies/PMOEA#NSGAIII">
        <rdf:type rdf:resource="http://www.semanticweb.org/macoda/ontologies/PMOEA#Decomposition_based"/>
        <rdfs:label xml:lang="en">NSGAIII</rdfs:label>
    </owl:NamedIndividual>
    


    <!-- http://www.semanticweb.org/macoda/ontologies/PMOEA#NEMO-I -->

    <owl:NamedIndividual rdf:about="http://www.semanticweb.org/macoda/ontologies/PMOEA#NEMO-I">
        <rdf:type rdf:resource="http://www.semanticweb.org/macoda/ontologies/PMOEA#PMOEA"/>
        <PMOEA:hasPreferenceModel rdf:resource="http://www.semanticweb.org/macoda/ontologies/PMOEA#AdditivePiecewiseLinear"/>
        <PMOEA:hasPreferenceModel rdf:resource="http://www.semanticweb.org/macoda/ontologies/PMOEA#GeneralAdditiveUtilityFunction"/>
        <PMOEA:hasPreferenceInformationFromDM rdf:resource="http://www.semanticweb.org/macoda/ontologies/PMOEA#PairwiseComparison"/>
        <PMOEA:hasInteractionTime rdf:resource="http://www.semanticweb.org/macoda/ontologies/PMOEA#progressive"/>
        <PMOEA:hasPreferenceIntegration rdf:resource="http://www.semanticweb.org/macoda/ontologies/PMOEA#CrowdingDistance"/>
        <PMOEA:hasPreferenceIntegration rdf:resource="http://www.semanticweb.org/macoda/ontologies/PMOEA#NecessaryPreferenceRelation"/>
        <PMOEA:hasLearningMethod rdf:resource="http://www.semanticweb.org/macoda/ontologies/PMOEA#RobustOrdinalRegression"/>
        <PMOEA:canSolve rdf:resource="http://www.semanticweb.org/macoda/ontologies/PMOEA#ZDT2"/>
        <PMOEA:canSolve rdf:resource="http://www.semanticweb.org/macoda/ontologies/PMOEA#ZDT1"/>
        <PMOEA:hasResultInfluence rdf:resource="http://www.semanticweb.org/macoda/ontologies/PMOEA#BiasedDistribution"/>
        <PMOEA:hasAuthor rdf:resource="http://www.semanticweb.org/macoda/ontologies/PMOEA#Piotr_Zielniewicz"/>
        <PMOEA:hasAuthor rdf:resource="http://www.semanticweb.org/macoda/ontologies/PMOEA#Salvatore_Greco
"/>
        <PMOEA:hasAuthor rdf:resource="http://www.semanticweb.org/macoda/ontologies/PMOEA#Juergen_Branke"/>
        <PMOEA:hasAuthor rdf:resource="http://www.semanticweb.org/macoda/ontologies/PMOEA#Roman_Sowinski"/>
        <PMOEA:hasSearchAlgorithm rdf:resource="http://www.semanticweb.org/macoda/ontologies/PMOEA#NSGA-II"/>
        <PMOEA:hasDevelopingYear rdf:datatype="http://www.w3.org/2001/XMLSchema#integer">2010</PMOEA:hasDevelopingYear>
        <PMOEA:ParetoDominancePreservation rdf:datatype="http://www.w3.org/2001/XMLSchema#boolean">true</PMOEA:ParetoDominancePreservation>
        <PMOEA:hasReference>Branke, J., S. Greco, R. Sowiski and P. Zielniewicz (2010). &quot;Interactive evolutionary multiobjective optimization driven by robust ordinal regression.&quot; Bulletin of the Polish Academy of Sciences: Technical Sciences 58(3): 347-358.</PMOEA:hasReference>
        <rdfs:comment>This paper presents the Necessary-preference-enhanced Evolutionary Multiobjective Optimizer (NEMO), which combines an evolutionary multiobjective optimization with robust ordinal regression (ROR) within an interactive procedure. In the course of NEMO, the decision maker is asked to express preferences by simply comparing some pairs of solutions in the current population. The whole set of additive value functions compatible with this preference information is used within a properly modified version of the evolutionary multiobjective optimization technique NSGA-II in order to focus the search towards solutions satisfying the preferences of the decision maker.</rdfs:comment>
        <rdfs:label xml:lang="en">NEMO-I</rdfs:label>
    </owl:NamedIndividual>
    


    <!-- http://www.semanticweb.org/macoda/ontologies/PMOEA#ObjectiveTransformation -->

    <owl:NamedIndividual rdf:about="http://www.semanticweb.org/macoda/ontologies/PMOEA#ObjectiveTransformation">
        <rdf:type rdf:resource="http://www.semanticweb.org/macoda/ontologies/PMOEA#Objectives"/>
        <rdfs:label xml:lang="en">ObjectiveTransformation</rdfs:label>
    </owl:NamedIndividual>
    


    <!-- http://www.semanticweb.org/macoda/ontologies/PMOEA#FuzzyPathPlannerOptimization -->

    <owl:NamedIndividual rdf:about="http://www.semanticweb.org/macoda/ontologies/PMOEA#FuzzyPathPlannerOptimization">
        <rdf:type rdf:resource="http://www.semanticweb.org/macoda/ontologies/PMOEA#Realworld_Problem"/>
        <PMOEA:isContinuousProblem rdf:datatype="http://www.w3.org/2001/XMLSchema#boolean">true</PMOEA:isContinuousProblem>
        <PMOEA:ObjectiveNumber rdf:datatype="http://www.w3.org/2001/XMLSchema#integer">3</PMOEA:ObjectiveNumber>
        <PMOEA:hasReference>Kim J H, Han J H, Kim Y H, et al. Preference-based solution selection algorithm for evolutionary multiobjective optimization[J]. Evolutionary Computation, IEEE Transactions on, 2012, 16(1): 20-34.</PMOEA:hasReference>
        <rdfs:comment>The fuzzy path planner generates a desired path from the current posture to the ball position</rdfs:comment>
        <rdfs:label xml:lang="en">FuzzyPathPlannerOptimization</rdfs:label>
    </owl:NamedIndividual>
    


    <!-- http://www.semanticweb.org/macoda/ontologies/PMOEA#Ye-Hoon_Kim -->

    <owl:NamedIndividual rdf:about="http://www.semanticweb.org/macoda/ontologies/PMOEA#Ye-Hoon_Kim">
        <rdf:type rdf:resource="http://www.semanticweb.org/macoda/ontologies/PMOEA#Researcher"/>
        <rdfs:label xml:lang="en">Ye-Hoon Kim</rdfs:label>
    </owl:NamedIndividual>
    


    <!-- http://www.semanticweb.org/macoda/ontologies/PMOEA#UniformDistributionPreferRegion -->

    <owl:NamedIndividual rdf:about="http://www.semanticweb.org/macoda/ontologies/PMOEA#UniformDistributionPreferRegion">
        <rdf:type rdf:resource="http://www.semanticweb.org/macoda/ontologies/PMOEA#DistributionFunctionInObjectiveSpace"/>
        <rdfs:label xml:lang="en">UniformDistributionPreferRegion</rdfs:label>
    </owl:NamedIndividual>
    


    <!-- http://www.semanticweb.org/macoda/ontologies/PMOEA#evoalgos -->

    <owl:NamedIndividual rdf:about="http://www.semanticweb.org/macoda/ontologies/PMOEA#evoalgos">
        <rdf:type rdf:resource="http://www.semanticweb.org/macoda/ontologies/PMOEA#ImplementationLibrary"/>
        <rdfs:comment>A package containing the S-metric selection evolutionary multi-objective optimization algorithm (SMS-EMOA). It currently works only on real-valued search spaces. Including other algorithms is planned for the future</rdfs:comment>
        <rdfs:label xml:lang="en">evoalgos</rdfs:label>
    </owl:NamedIndividual>
    


    <!-- http://www.semanticweb.org/macoda/ontologies/PMOEA#FrontSorting -->

    <owl:NamedIndividual rdf:about="http://www.semanticweb.org/macoda/ontologies/PMOEA#FrontSorting">
        <rdf:type rdf:resource="http://www.semanticweb.org/macoda/ontologies/PMOEA#FrontSorting"/>
        <rdfs:comment>The way to sort the population into different fronts</rdfs:comment>
        <rdfs:label xml:lang="en">FrontSorting</rdfs:label>
    </owl:NamedIndividual>
    


    <!-- http://www.semanticweb.org/macoda/ontologies/PMOEA#Soon-Thiam_Khu -->

    <owl:NamedIndividual rdf:about="http://www.semanticweb.org/macoda/ontologies/PMOEA#Soon-Thiam_Khu">
        <rdf:type rdf:resource="http://www.semanticweb.org/macoda/ontologies/PMOEA#Researcher"/>
        <rdfs:label xml:lang="en">Soon-Thiam Khu</rdfs:label>
    </owl:NamedIndividual>
    


    <!-- http://www.semanticweb.org/macoda/ontologies/PMOEA#DTLZ4_8 -->

    <owl:NamedIndividual rdf:about="http://www.semanticweb.org/macoda/ontologies/PMOEA#DTLZ4_8">
        <rdf:type rdf:resource="http://www.semanticweb.org/macoda/ontologies/PMOEA#DTLZ"/>
        <PMOEA:isContinuousProblem rdf:datatype="http://www.w3.org/2001/XMLSchema#boolean">true</PMOEA:isContinuousProblem>
        <PMOEA:ObjectiveNumber rdf:datatype="http://www.w3.org/2001/XMLSchema#integer">8</PMOEA:ObjectiveNumber>
        <PMOEA:isManyObjectiveProblem rdf:datatype="http://www.w3.org/2001/XMLSchema#boolean">true</PMOEA:isManyObjectiveProblem>
        <rdfs:label xml:lang="en">DTLZ4_8</rdfs:label>
    </owl:NamedIndividual>
    


    <!-- http://www.semanticweb.org/macoda/ontologies/PMOEA#Jon_L_Marquis -->

    <owl:NamedIndividual rdf:about="http://www.semanticweb.org/macoda/ontologies/PMOEA#Jon_L_Marquis">
        <rdf:type rdf:resource="http://www.semanticweb.org/macoda/ontologies/PMOEA#Researcher"/>
        <rdfs:label xml:lang="en">Jon L. Marquis</rdfs:label>
    </owl:NamedIndividual>
    


    <!-- http://www.semanticweb.org/macoda/ontologies/PMOEA#Goal-sequenceDomination -->

    <owl:NamedIndividual rdf:about="http://www.semanticweb.org/macoda/ontologies/PMOEA#Goal-sequenceDomination">
        <rdf:type rdf:resource="http://www.semanticweb.org/macoda/ontologies/PMOEA#DominanceRelation"/>
        <rdfs:comment>In the first stage, the ranking scheme prefers objective vectors fulfilling all criteria and ranks those vectors according to PMOGA dominance(GoalFulfilmentDominance). Among the remaining solutions, the objective vector u dominates the objective vector v if and only if u dominates v with respect to the criteria in which u does not fulfil the goal, or if |u-g|&lt;|v-g| (where |u-g| denotes the vector composed with the absolute values of the differences between the objectives values of the solution v and the goal g).</rdfs:comment>
        <rdfs:label xml:lang="en">Goal-sequenceDomination</rdfs:label>
    </owl:NamedIndividual>
    


    <!-- http://www.semanticweb.org/macoda/ontologies/PMOEA#FuzzyPreferenceRelationOnObjectives -->

    <owl:NamedIndividual rdf:about="http://www.semanticweb.org/macoda/ontologies/PMOEA#FuzzyPreferenceRelationOnObjectives">
        <rdf:type rdf:resource="http://www.semanticweb.org/macoda/ontologies/PMOEA#FuzzyLogic"/>
        <rdfs:comment>objective f2 is much more important than objective f1, f3 is more important than f2</rdfs:comment>
        <rdfs:label xml:lang="en">FuzzyPreferenceRelationOnObjectives</rdfs:label>
    </owl:NamedIndividual>
    


    <!-- http://www.semanticweb.org/macoda/ontologies/PMOEA#ExponentialFunctionPreferExtremalSolutions -->

    <owl:NamedIndividual rdf:about="http://www.semanticweb.org/macoda/ontologies/PMOEA#ExponentialFunctionPreferExtremalSolutions">
        <rdf:type rdf:resource="http://www.semanticweb.org/macoda/ontologies/PMOEA#DistributionFunctionInObjectiveSpace"/>
        <rdfs:label xml:lang="en">ExponentialFunctionPreferExtremalSolutions</rdfs:label>
    </owl:NamedIndividual>
    


    <!-- http://www.semanticweb.org/macoda/ontologies/PMOEA#DTLZ2_7 -->

    <owl:NamedIndividual rdf:about="http://www.semanticweb.org/macoda/ontologies/PMOEA#DTLZ2_7">
        <rdf:type rdf:resource="http://www.semanticweb.org/macoda/ontologies/PMOEA#DTLZ"/>
        <PMOEA:isDiscreteProblem rdf:datatype="http://www.w3.org/2001/XMLSchema#boolean">false</PMOEA:isDiscreteProblem>
        <PMOEA:OWLDataProperty_61d3cd95_fde4_4c1b_af08_1eaf73473aea rdf:datatype="http://www.w3.org/2001/XMLSchema#boolean">false</PMOEA:OWLDataProperty_61d3cd95_fde4_4c1b_af08_1eaf73473aea>
        <PMOEA:isContinuousProblem rdf:datatype="http://www.w3.org/2001/XMLSchema#boolean">true</PMOEA:isContinuousProblem>
        <PMOEA:ObjectiveNumber rdf:datatype="http://www.w3.org/2001/XMLSchema#integer">7</PMOEA:ObjectiveNumber>
        <PMOEA:isManyObjectiveProblem rdf:datatype="http://www.w3.org/2001/XMLSchema#boolean">true</PMOEA:isManyObjectiveProblem>
        <rdfs:label xml:lang="en">DTLZ2_7</rdfs:label>
    </owl:NamedIndividual>
    


    <!-- http://www.semanticweb.org/macoda/ontologies/PMOEA#ZDT3 -->

    <owl:NamedIndividual rdf:about="http://www.semanticweb.org/macoda/ontologies/PMOEA#ZDT3">
        <rdf:type rdf:resource="http://www.semanticweb.org/macoda/ontologies/PMOEA#ZDT"/>
        <PMOEA:isDiscreteProblem rdf:datatype="http://www.w3.org/2001/XMLSchema#boolean">false</PMOEA:isDiscreteProblem>
        <PMOEA:OWLDataProperty_61d3cd95_fde4_4c1b_af08_1eaf73473aea rdf:datatype="http://www.w3.org/2001/XMLSchema#boolean">false</PMOEA:OWLDataProperty_61d3cd95_fde4_4c1b_af08_1eaf73473aea>
        <PMOEA:isContinuousProblem rdf:datatype="http://www.w3.org/2001/XMLSchema#boolean">true</PMOEA:isContinuousProblem>
        <PMOEA:ObjectiveNumber rdf:datatype="http://www.w3.org/2001/XMLSchema#integer">2</PMOEA:ObjectiveNumber>
        <PMOEA:isManyObjectiveProblem rdf:datatype="http://www.w3.org/2001/XMLSchema#boolean">false</PMOEA:isManyObjectiveProblem>
        <rdfs:label xml:lang="en">ZDT3</rdfs:label>
    </owl:NamedIndividual>
    


    <!-- http://www.semanticweb.org/macoda/ontologies/PMOEA#WFG2_4 -->

    <owl:NamedIndividual rdf:about="http://www.semanticweb.org/macoda/ontologies/PMOEA#WFG2_4">
        <rdf:type rdf:resource="http://www.semanticweb.org/macoda/ontologies/PMOEA#WFG"/>
        <PMOEA:isContinuousProblem rdf:datatype="http://www.w3.org/2001/XMLSchema#boolean">true</PMOEA:isContinuousProblem>
        <PMOEA:ObjectiveNumber rdf:datatype="http://www.w3.org/2001/XMLSchema#integer">4</PMOEA:ObjectiveNumber>
        <PMOEA:isManyObjectiveProblem rdf:datatype="http://www.w3.org/2001/XMLSchema#boolean">true</PMOEA:isManyObjectiveProblem>
        <rdfs:label xml:lang="en">WFG2_4</rdfs:label>
    </owl:NamedIndividual>
    


    <!-- http://www.semanticweb.org/macoda/ontologies/PMOEA#Hartmut_Schmeck -->

    <owl:NamedIndividual rdf:about="http://www.semanticweb.org/macoda/ontologies/PMOEA#Hartmut_Schmeck">
        <rdf:type rdf:resource="http://www.semanticweb.org/macoda/ontologies/PMOEA#Researcher"/>
        <rdfs:label xml:lang="en">Hartmut Schmeck</rdfs:label>
    </owl:NamedIndividual>
    


    <!-- http://www.semanticweb.org/macoda/ontologies/PMOEA#Luciana_R_Pedro -->

    <owl:NamedIndividual rdf:about="http://www.semanticweb.org/macoda/ontologies/PMOEA#Luciana_R_Pedro">
        <rdf:type rdf:resource="http://www.semanticweb.org/macoda/ontologies/PMOEA#Researcher"/>
        <rdfs:label xml:lang="en">Luciana R. Pedro</rdfs:label>
    </owl:NamedIndividual>
    


    <!-- http://www.semanticweb.org/macoda/ontologies/PMOEA#IndexWithWeightedRanking -->

    <owl:NamedIndividual rdf:about="http://www.semanticweb.org/macoda/ontologies/PMOEA#IndexWithWeightedRanking">
        <rdf:type rdf:resource="http://www.semanticweb.org/macoda/ontologies/PMOEA#Ranking"/>
        <rdfs:comment>The prefernce index of solution a over solution b is defined as the weighted number of objectives that a is smaller then b, convert multi-objective to single objective by obtaining the solution with largest preference index.</rdfs:comment>
        <rdfs:label xml:lang="en">IndexWithWeightedRanking</rdfs:label>
    </owl:NamedIndividual>
    


    <!-- http://www.semanticweb.org/macoda/ontologies/PMOEA#Johannes_Krettek -->

    <owl:NamedIndividual rdf:about="http://www.semanticweb.org/macoda/ontologies/PMOEA#Johannes_Krettek">
        <rdf:type rdf:resource="http://www.semanticweb.org/macoda/ontologies/PMOEA#Researcher"/>
        <rdfs:label xml:lang="en">Johannes Krettek</rdfs:label>
    </owl:NamedIndividual>
    


    <!-- http://www.semanticweb.org/macoda/ontologies/PMOEA#WFG1_10 -->

    <owl:NamedIndividual rdf:about="http://www.semanticweb.org/macoda/ontologies/PMOEA#WFG1_10">
        <rdf:type rdf:resource="http://www.semanticweb.org/macoda/ontologies/PMOEA#WFG"/>
        <PMOEA:isContinuousProblem rdf:datatype="http://www.w3.org/2001/XMLSchema#boolean">true</PMOEA:isContinuousProblem>
        <PMOEA:ObjectiveNumber rdf:datatype="http://www.w3.org/2001/XMLSchema#integer">10</PMOEA:ObjectiveNumber>
        <PMOEA:isManyObjectiveProblem rdf:datatype="http://www.w3.org/2001/XMLSchema#boolean">true</PMOEA:isManyObjectiveProblem>
        <rdfs:label xml:lang="en">WFG1_10</rdfs:label>
    </owl:NamedIndividual>
    


    <!-- http://www.semanticweb.org/macoda/ontologies/PMOEA#Thomas_Ewald -->

    <owl:NamedIndividual rdf:about="http://www.semanticweb.org/macoda/ontologies/PMOEA#Thomas_Ewald">
        <rdf:type rdf:resource="http://www.semanticweb.org/macoda/ontologies/PMOEA#Researcher"/>
        <rdfs:label xml:lang="en">Thomas Ewald</rdfs:label>
    </owl:NamedIndividual>
    


    <!-- http://www.semanticweb.org/macoda/ontologies/PMOEA#ServoControlSystemDesign -->

    <owl:NamedIndividual rdf:about="http://www.semanticweb.org/macoda/ontologies/PMOEA#ServoControlSystemDesign">
        <rdf:type rdf:resource="http://www.semanticweb.org/macoda/ontologies/PMOEA#Realworld_Problem"/>
        <PMOEA:isContinuousProblem rdf:datatype="http://www.w3.org/2001/XMLSchema#boolean">true</PMOEA:isContinuousProblem>
        <PMOEA:ObjectiveNumber rdf:datatype="http://www.w3.org/2001/XMLSchema#integer">6</PMOEA:ObjectiveNumber>
        <PMOEA:isManyObjectiveProblem rdf:datatype="http://www.w3.org/2001/XMLSchema#boolean">true</PMOEA:isManyObjectiveProblem>
        <rdfs:label xml:lang="en">ServoControlSystemDesign</rdfs:label>
    </owl:NamedIndividual>
    


    <!-- http://www.semanticweb.org/macoda/ontologies/PMOEA#OneSolution -->

    <owl:NamedIndividual rdf:about="http://www.semanticweb.org/macoda/ontologies/PMOEA#OneSolution">
        <rdf:type rdf:resource="http://www.semanticweb.org/macoda/ontologies/PMOEA#OneSolution"/>
        <rdfs:label xml:lang="en">OneSolution</rdfs:label>
    </owl:NamedIndividual>
    


    <!-- http://www.semanticweb.org/macoda/ontologies/PMOEA#CBPM -->

    <owl:NamedIndividual rdf:about="http://www.semanticweb.org/macoda/ontologies/PMOEA#CBPM">
        <rdf:type rdf:resource="http://www.semanticweb.org/macoda/ontologies/PMOEA#PMOEA"/>
        <PMOEA:hasPreferenceModel rdf:resource="http://www.semanticweb.org/macoda/ontologies/PMOEA#CurvaturebasedCone"/>
        <PMOEA:hasPreferenceInformationFromDM rdf:resource="http://www.semanticweb.org/macoda/ontologies/PMOEA#MaximumAndMinimumTrade-offs"/>
        <PMOEA:hasInteractionTime rdf:resource="http://www.semanticweb.org/macoda/ontologies/PMOEA#a-priori"/>
        <PMOEA:hasPreferenceIntegration rdf:resource="http://www.semanticweb.org/macoda/ontologies/PMOEA#HypervolumeIndicator"/>
        <PMOEA:canSolve rdf:resource="http://www.semanticweb.org/macoda/ontologies/PMOEA#ZDT2"/>
        <PMOEA:canSolve rdf:resource="http://www.semanticweb.org/macoda/ontologies/PMOEA#ZDT3"/>
        <PMOEA:canSolve rdf:resource="http://www.semanticweb.org/macoda/ontologies/PMOEA#ZDT1"/>
        <PMOEA:hasResultInfluence rdf:resource="http://www.semanticweb.org/macoda/ontologies/PMOEA#BiasedDistribution"/>
        <PMOEA:hasAuthor rdf:resource="http://www.semanticweb.org/macoda/ontologies/PMOEA#Andre_Deutz"/>
        <PMOEA:hasAuthor rdf:resource="http://www.semanticweb.org/macoda/ontologies/PMOEA#Pradyumn_Kumar_Shukla"/>
        <PMOEA:hasAuthor rdf:resource="http://www.semanticweb.org/macoda/ontologies/PMOEA#Michael_Emmerich"/>
        <PMOEA:useLibrary rdf:resource="http://www.semanticweb.org/macoda/ontologies/PMOEA#jMetal"/>
        <PMOEA:hasSearchAlgorithm rdf:resource="http://www.semanticweb.org/macoda/ontologies/PMOEA#SMS-EMOA"/>
        <PMOEA:hasImplementationLanguage rdf:resource="http://www.semanticweb.org/macoda/ontologies/PMOEA#Java"/>
        <PMOEA:hasDevelopingYear rdf:datatype="http://www.w3.org/2001/XMLSchema#integer">2013</PMOEA:hasDevelopingYear>
        <PMOEA:hasReference>Shukla, P. K., M. Emmerich and A. Deutz (2013). A Theoretical Analysis of Curvature Based Preference Models. Evolutionary Multi-Criterion Optimization, Springer</PMOEA:hasReference>
        <rdfs:comment>In this paper,  we are interested in curvature/ slope based models where the preferred set depend upon the curvature of efficient front. This amounts to having a direct control on trade-offs among the objective functions. A related concept of cone-based hypervolume is also theoretically investigated in this paper.  Furthermore, we present two algorithms for finding solutions that are compatible with a given reference model.</rdfs:comment>
        <rdfs:label xml:lang="en">CBPM</rdfs:label>
    </owl:NamedIndividual>
    


    <!-- http://www.semanticweb.org/macoda/ontologies/PMOEA#ParetoConeDominance -->

    <owl:NamedIndividual rdf:about="http://www.semanticweb.org/macoda/ontologies/PMOEA#ParetoConeDominance">
        <rdf:type rdf:resource="http://www.semanticweb.org/macoda/ontologies/PMOEA#DominanceRelation"/>
        <rdfs:comment>The dominance used in iPICEA-g .A goal vector, gi is said to be Pareto cone-dominated by a candidate solution, f(si) if and only if the gi is within the search range of f(si).</rdfs:comment>
        <rdfs:label xml:lang="en">ParetoConeDominance</rdfs:label>
    </owl:NamedIndividual>
    


    <!-- http://www.semanticweb.org/macoda/ontologies/PMOEA#GPS-EA -->

    <owl:NamedIndividual rdf:about="http://www.semanticweb.org/macoda/ontologies/PMOEA#GPS-EA">
        <rdf:type rdf:resource="http://www.semanticweb.org/macoda/ontologies/PMOEA#PMOEA"/>
        <PMOEA:hasPreferenceModel rdf:resource="http://www.semanticweb.org/macoda/ontologies/PMOEA#PreferencePoint"/>
        <PMOEA:hasPreferenceInformationFromDM rdf:resource="http://www.semanticweb.org/macoda/ontologies/PMOEA#ObjectivePriorityVector"/>
        <PMOEA:hasPreferenceInformationFromDM rdf:resource="http://www.semanticweb.org/macoda/ontologies/PMOEA#ReferencePoint"/>
        <PMOEA:hasInteractionTime rdf:resource="http://www.semanticweb.org/macoda/ontologies/PMOEA#a-priori"/>
        <PMOEA:hasPreferenceIntegration rdf:resource="http://www.semanticweb.org/macoda/ontologies/PMOEA#Goal-sequenceDomination"/>
        <PMOEA:hasComparison rdf:resource="http://www.semanticweb.org/macoda/ontologies/PMOEA#PMOGA"/>
        <PMOEA:canSolve rdf:resource="http://www.semanticweb.org/macoda/ontologies/PMOEA#Fonseca_test"/>
        <PMOEA:canSolve rdf:resource="http://www.semanticweb.org/macoda/ontologies/PMOEA#Deb1999"/>
        <PMOEA:canSolve rdf:resource="http://www.semanticweb.org/macoda/ontologies/PMOEA#ServoControlSystemDesign"/>
        <PMOEA:hasResultInfluence rdf:resource="http://www.semanticweb.org/macoda/ontologies/PMOEA#BoundedRegion"/>
        <PMOEA:hasAuthor rdf:resource="http://www.semanticweb.org/macoda/ontologies/PMOEA#Tong_Heng_Lee"/>
        <PMOEA:hasAuthor rdf:resource="http://www.semanticweb.org/macoda/ontologies/PMOEA#Ramasubramanian_Sathikannan"/>
        <PMOEA:hasAuthor rdf:resource="http://www.semanticweb.org/macoda/ontologies/PMOEA#Kay_Chen_Tan"/>
        <PMOEA:hasAuthor rdf:resource="http://www.semanticweb.org/macoda/ontologies/PMOEA#Eik_Fun_Khor"/>
        <PMOEA:isExtensionOf rdf:resource="http://www.semanticweb.org/macoda/ontologies/PMOEA#PMOGA"/>
        <PMOEA:hasSearchAlgorithm rdf:resource="http://www.semanticweb.org/macoda/ontologies/PMOEA#GeneralMOEA"/>
        <PMOEA:hasImplementationLanguage rdf:resource="http://www.semanticweb.org/macoda/ontologies/PMOEA#Matlab"/>
        <PMOEA:hasDevelopingYear rdf:datatype="http://www.w3.org/2001/XMLSchema#integer">2003</PMOEA:hasDevelopingYear>
        <PMOEA:MultipleRegionOfInterest rdf:datatype="http://www.w3.org/2001/XMLSchema#boolean">true</PMOEA:MultipleRegionOfInterest>
        <PMOEA:hasReference>Tan, K. C., E. F. Khor, T. H. Lee and R. Sathikannan (2003). &quot;An evolutionary algorithm with advanced goal and priority specification for multi-objective optimization.&quot; Journal of Artificial Intelligence Research: 183-215</PMOEA:hasReference>
        <rdfs:comment>It extended PMOGA by introducing a new goal-sequence domination scheme to allow advanced specifications such as priorities and hard/soft constraints to be incorporated</rdfs:comment>
        <rdfs:label xml:lang="en">GPS-EA</rdfs:label>
    </owl:NamedIndividual>
    


    <!-- http://www.semanticweb.org/macoda/ontologies/PMOEA#Ibrahim_Karahan -->

    <owl:NamedIndividual rdf:about="http://www.semanticweb.org/macoda/ontologies/PMOEA#Ibrahim_Karahan">
        <rdf:type rdf:resource="http://www.semanticweb.org/macoda/ontologies/PMOEA#Researcher"/>
        <rdfs:label xml:lang="en">Ibrahim Karahan</rdfs:label>
    </owl:NamedIndividual>
    


    <!-- http://www.semanticweb.org/macoda/ontologies/PMOEA#ParticleSelection -->

    <owl:NamedIndividual rdf:about="http://www.semanticweb.org/macoda/ontologies/PMOEA#ParticleSelection">
        <rdf:type rdf:resource="http://www.semanticweb.org/macoda/ontologies/PMOEA#LeaderSelection"/>
        <rdfs:comment>The population of N particles at the beginning of the iteration is combined with the N updated particles to create a population of size 2N. This 2N population needs a selection  to obtain a population of size N closest to the preferred region.</rdfs:comment>
        <rdfs:label xml:lang="en">ParticleSelection</rdfs:label>
    </owl:NamedIndividual>
    


    <!-- http://www.semanticweb.org/macoda/ontologies/PMOEA#Dirk_Biermann -->

    <owl:NamedIndividual rdf:about="http://www.semanticweb.org/macoda/ontologies/PMOEA#Dirk_Biermann">
        <rdf:type rdf:resource="http://www.semanticweb.org/macoda/ontologies/PMOEA#Researcher"/>
        <rdfs:label xml:lang="en">Dirk Biermann</rdfs:label>
    </owl:NamedIndividual>
    


    <!-- http://www.semanticweb.org/macoda/ontologies/PMOEA#BCD_NSGA-II -->

    <owl:NamedIndividual rdf:about="http://www.semanticweb.org/macoda/ontologies/PMOEA#BCD_NSGA-II">
        <rdf:type rdf:resource="http://www.semanticweb.org/macoda/ontologies/PMOEA#PMOEA"/>
        <PMOEA:hasPreferenceModel rdf:resource="http://www.semanticweb.org/macoda/ontologies/PMOEA#LinearUtilityFunction"/>
        <PMOEA:hasPreferenceInformationFromDM rdf:resource="http://www.semanticweb.org/macoda/ontologies/PMOEA#ReferenceVectorFORIso-UtilityFunction"/>
        <PMOEA:hasInteractionTime rdf:resource="http://www.semanticweb.org/macoda/ontologies/PMOEA#a-priori"/>
        <PMOEA:hasPreferenceIntegration rdf:resource="http://www.semanticweb.org/macoda/ontologies/PMOEA#CrowdingDistance"/>
        <PMOEA:hasComparison rdf:resource="http://www.semanticweb.org/macoda/ontologies/PMOEA#G-MOEA"/>
        <PMOEA:canSolve rdf:resource="http://www.semanticweb.org/macoda/ontologies/PMOEA#ZDT2"/>
        <PMOEA:canSolve rdf:resource="http://www.semanticweb.org/macoda/ontologies/PMOEA#DTLZ4_3"/>
        <PMOEA:canSolve rdf:resource="http://www.semanticweb.org/macoda/ontologies/PMOEA#ZDT6"/>
        <PMOEA:canSolve rdf:resource="http://www.semanticweb.org/macoda/ontologies/PMOEA#DTLZ2_3"/>
        <PMOEA:canSolve rdf:resource="http://www.semanticweb.org/macoda/ontologies/PMOEA#ZDT1"/>
        <PMOEA:hasResultInfluence rdf:resource="http://www.semanticweb.org/macoda/ontologies/PMOEA#BiasedDistribution"/>
        <PMOEA:hasAuthor rdf:resource="http://www.semanticweb.org/macoda/ontologies/PMOEA#Juergen_Branke"/>
        <PMOEA:hasAuthor rdf:resource="http://www.semanticweb.org/macoda/ontologies/PMOEA#Kalyanmoy_Deb"/>
        <PMOEA:hasSearchAlgorithm rdf:resource="http://www.semanticweb.org/macoda/ontologies/PMOEA#NSGA-II"/>
        <PMOEA:hasDevelopingYear rdf:datatype="http://www.w3.org/2001/XMLSchema#integer">2003</PMOEA:hasDevelopingYear>
        <PMOEA:SpreadControl rdf:datatype="http://www.w3.org/2001/XMLSchema#boolean">true</PMOEA:SpreadControl>
        <PMOEA:ParetoDominancePreservation rdf:datatype="http://www.w3.org/2001/XMLSchema#boolean">true</PMOEA:ParetoDominancePreservation>
        <PMOEA:hasReference>Branke, J. and K. Deb (2005). Integrating user preferences into evolutionary multi-objective optimization. Knowledge incorporation in evolutionary computation, Springer: 461-477.</PMOEA:hasReference>
        <rdfs:comment>This approach aims to search for a set of solutions that are parallel to an iso-utility function defined by a specified reference direction. Specifically, a parameter is applied to control the range of ROI along the Pareto optimal front. This parameter is defined as the ratio of the real distances between neighboring solutions on the Pareto optimal front and the projected distance of the same solutions on a plane defined by a linear utility function</rdfs:comment>
        <rdfs:label xml:lang="en">BCD_NSGA-II</rdfs:label>
    </owl:NamedIndividual>
    


    <!-- http://www.semanticweb.org/macoda/ontologies/PMOEA#ecr -->

    <owl:NamedIndividual rdf:about="http://www.semanticweb.org/macoda/ontologies/PMOEA#ecr">
        <rdf:type rdf:resource="http://www.semanticweb.org/macoda/ontologies/PMOEA#ImplementationLibrary"/>
        <rdfs:comment>A framework for implementing single- and multi-objective evolutionary algorithms supporting several genotypes like real-valued vectors, binary strings and permutations. Different pre-defined building blocks in the form of evolutionary operators and many helper functions needed in evolutionary algorithms are provided. Etensions with new operators and solution representations are also possible.</rdfs:comment>
        <rdfs:label xml:lang="en">ecr</rdfs:label>
    </owl:NamedIndividual>
    


    <!-- http://www.semanticweb.org/macoda/ontologies/PMOEA#Youssef_Hamadi -->

    <owl:NamedIndividual rdf:about="http://www.semanticweb.org/macoda/ontologies/PMOEA#Youssef_Hamadi">
        <rdf:type rdf:resource="http://www.semanticweb.org/macoda/ontologies/PMOEA#Researcher"/>
        <rdfs:label xml:lang="en">Youssef Hamadi</rdfs:label>
    </owl:NamedIndividual>
    


    <!-- http://www.semanticweb.org/macoda/ontologies/PMOEA#Knapsack_3 -->

    <owl:NamedIndividual rdf:about="http://www.semanticweb.org/macoda/ontologies/PMOEA#Knapsack_3">
        <rdf:type rdf:resource="http://www.semanticweb.org/macoda/ontologies/PMOEA#Knapsack"/>
        <PMOEA:isDiscreteProblem rdf:datatype="http://www.w3.org/2001/XMLSchema#boolean">true</PMOEA:isDiscreteProblem>
        <PMOEA:ObjectiveNumber rdf:datatype="http://www.w3.org/2001/XMLSchema#integer">3</PMOEA:ObjectiveNumber>
        <rdfs:label xml:lang="en">Knapsack_3</rdfs:label>
    </owl:NamedIndividual>
    


    <!-- http://www.semanticweb.org/macoda/ontologies/PMOEA#DEB3DK -->

    <owl:NamedIndividual rdf:about="http://www.semanticweb.org/macoda/ontologies/PMOEA#DEB3DK">
        <rdf:type rdf:resource="http://www.semanticweb.org/macoda/ontologies/PMOEA#Academic_Problem"/>
        <PMOEA:isContinuousProblem rdf:datatype="http://www.w3.org/2001/XMLSchema#boolean">true</PMOEA:isContinuousProblem>
        <PMOEA:ObjectiveNumber rdf:datatype="http://www.w3.org/2001/XMLSchema#integer">3</PMOEA:ObjectiveNumber>
        <PMOEA:hasReference>Branke, J., Deb, K., Dierolf, H., and Osswald, M. Finding
knees in multi-objective optimization. In Proceedings of the
Parallel Problem Solving from Nature, LNCS, 3242, 2004,
722731.</PMOEA:hasReference>
        <rdfs:comment>three-objective knee-based test problems</rdfs:comment>
        <rdfs:label xml:lang="en">DEB3DK</rdfs:label>
    </owl:NamedIndividual>
    


    <!-- http://www.semanticweb.org/macoda/ontologies/PMOEA#SMS-EMOA -->

    <owl:NamedIndividual rdf:about="http://www.semanticweb.org/macoda/ontologies/PMOEA#SMS-EMOA">
        <rdf:type rdf:resource="http://www.semanticweb.org/macoda/ontologies/PMOEA#Indicator_based"/>
        <rdfs:label xml:lang="en">SMS-EMOA</rdfs:label>
    </owl:NamedIndividual>
    


    <!-- http://www.semanticweb.org/macoda/ontologies/PMOEA#Dragan_Cvetkovic -->

    <owl:NamedIndividual rdf:about="http://www.semanticweb.org/macoda/ontologies/PMOEA#Dragan_Cvetkovic">
        <rdf:type rdf:resource="http://www.semanticweb.org/macoda/ontologies/PMOEA#Researcher"/>
        <rdfs:label xml:lang="en">Dragan Cvetkovic</rdfs:label>
    </owl:NamedIndividual>
    


    <!-- http://www.semanticweb.org/macoda/ontologies/PMOEA#BoundedRegion -->

    <owl:NamedIndividual rdf:about="http://www.semanticweb.org/macoda/ontologies/PMOEA#BoundedRegion">
        <rdf:type rdf:resource="http://www.semanticweb.org/macoda/ontologies/PMOEA#BoundedRegion"/>
        <rdfs:label xml:lang="en">BoundedRegion</rdfs:label>
    </owl:NamedIndividual>
    


    <!-- http://www.semanticweb.org/macoda/ontologies/PMOEA#WFG5_2 -->

    <owl:NamedIndividual rdf:about="http://www.semanticweb.org/macoda/ontologies/PMOEA#WFG5_2">
        <rdf:type rdf:resource="http://www.semanticweb.org/macoda/ontologies/PMOEA#WFG"/>
        <PMOEA:isContinuousProblem rdf:datatype="http://www.w3.org/2001/XMLSchema#boolean">true</PMOEA:isContinuousProblem>
        <PMOEA:ObjectiveNumber rdf:datatype="http://www.w3.org/2001/XMLSchema#integer">2</PMOEA:ObjectiveNumber>
        <rdfs:label xml:lang="en">WFG5_2</rdfs:label>
    </owl:NamedIndividual>
    


    <!-- http://www.semanticweb.org/macoda/ontologies/PMOEA#DTLZ2_3 -->

    <owl:NamedIndividual rdf:about="http://www.semanticweb.org/macoda/ontologies/PMOEA#DTLZ2_3">
        <rdf:type rdf:resource="http://www.semanticweb.org/macoda/ontologies/PMOEA#DTLZ"/>
        <PMOEA:isDiscreteProblem rdf:datatype="http://www.w3.org/2001/XMLSchema#boolean">false</PMOEA:isDiscreteProblem>
        <PMOEA:OWLDataProperty_61d3cd95_fde4_4c1b_af08_1eaf73473aea rdf:datatype="http://www.w3.org/2001/XMLSchema#boolean">false</PMOEA:OWLDataProperty_61d3cd95_fde4_4c1b_af08_1eaf73473aea>
        <PMOEA:isContinuousProblem rdf:datatype="http://www.w3.org/2001/XMLSchema#boolean">true</PMOEA:isContinuousProblem>
        <PMOEA:ObjectiveNumber rdf:datatype="http://www.w3.org/2001/XMLSchema#integer">3</PMOEA:ObjectiveNumber>
        <PMOEA:isManyObjectiveProblem rdf:datatype="http://www.w3.org/2001/XMLSchema#boolean">false</PMOEA:isManyObjectiveProblem>
        <rdfs:label xml:lang="en">DTLZ2_3</rdfs:label>
    </owl:NamedIndividual>
    


    <!-- http://www.semanticweb.org/macoda/ontologies/PMOEA#pNSGA-II -->

    <owl:NamedIndividual rdf:about="http://www.semanticweb.org/macoda/ontologies/PMOEA#pNSGA-II">
        <rdf:type rdf:resource="http://www.semanticweb.org/macoda/ontologies/PMOEA#PMOEA"/>
        <PMOEA:hasPreferenceInformationFromDM rdf:resource="http://www.semanticweb.org/macoda/ontologies/PMOEA#M-ProperParetoOptimal"/>
        <PMOEA:hasInteractionTime rdf:resource="http://www.semanticweb.org/macoda/ontologies/PMOEA#a-priori"/>
        <PMOEA:hasPreferenceIntegration rdf:resource="http://www.semanticweb.org/macoda/ontologies/PMOEA#FrontSorting"/>
        <PMOEA:canSolve rdf:resource="http://www.semanticweb.org/macoda/ontologies/PMOEA#ZDT5"/>
        <PMOEA:canSolve rdf:resource="http://www.semanticweb.org/macoda/ontologies/PMOEA#WFG1_3"/>
        <PMOEA:canSolve rdf:resource="http://www.semanticweb.org/macoda/ontologies/PMOEA#S-ZDT2"/>
        <PMOEA:canSolve rdf:resource="http://www.semanticweb.org/macoda/ontologies/PMOEA#WFG1_2"/>
        <PMOEA:canSolve rdf:resource="http://www.semanticweb.org/macoda/ontologies/PMOEA#DTLZ4_3"/>
        <PMOEA:canSolve rdf:resource="http://www.semanticweb.org/macoda/ontologies/PMOEA#ZDT6"/>
        <PMOEA:canSolve rdf:resource="http://www.semanticweb.org/macoda/ontologies/PMOEA#ZDT4"/>
        <PMOEA:canSolve rdf:resource="http://www.semanticweb.org/macoda/ontologies/PMOEA#ZDT3"/>
        <PMOEA:canSolve rdf:resource="http://www.semanticweb.org/macoda/ontologies/PMOEA#S-ZDT1"/>
        <PMOEA:hasResultInfluence rdf:resource="http://www.semanticweb.org/macoda/ontologies/PMOEA#BoundedRegion"/>
        <PMOEA:hasAuthor rdf:resource="http://www.semanticweb.org/macoda/ontologies/PMOEA#Pradyumn_Kumar_Shukla"/>
        <PMOEA:hasAuthor rdf:resource="http://www.semanticweb.org/macoda/ontologies/PMOEA#Christian_Hirsch"/>
        <PMOEA:hasAuthor rdf:resource="http://www.semanticweb.org/macoda/ontologies/PMOEA#Hartmut_Schmeck"/>
        <PMOEA:useLibrary rdf:resource="http://www.semanticweb.org/macoda/ontologies/PMOEA#jMetal"/>
        <PMOEA:hasSearchAlgorithm rdf:resource="http://www.semanticweb.org/macoda/ontologies/PMOEA#NSGA-II"/>
        <PMOEA:hasImplementationLanguage rdf:resource="http://www.semanticweb.org/macoda/ontologies/PMOEA#Java"/>
        <PMOEA:hasDevelopingYear rdf:datatype="http://www.w3.org/2001/XMLSchema#integer">2010</PMOEA:hasDevelopingYear>
        <PMOEA:hasReference>Shukla, P. K., C. Hirsch and H. Schmeck (2010). A framework for incorporating trade-off information using multi-objective evolutionary algorithms. Parallel Problem Solving from Nature, PPSN XI, Springer: 131-140</PMOEA:hasReference>
        <rdfs:comment>In the standard NSGA-II, the parent population Pt and the offspring population Qt are combined and non-dominated fronts F1,...,Fr of this combined population are found. We do the same in pNSGA-II,  however from F1 (best non-dominated set), we additionally find a set F0 which satisfies the trade-off in Definition 4, considering the entire population. So we have one additional (preferred) front. Members of F0 are assigned a rank of 0 (better than 1, the rank of F1, as we consider minimization in tournament selection).</rdfs:comment>
        <rdfs:label xml:lang="en">pNSGA-II</rdfs:label>
    </owl:NamedIndividual>
    


    <!-- http://www.semanticweb.org/macoda/ontologies/PMOEA#DTLZ6_6 -->

    <owl:NamedIndividual rdf:about="http://www.semanticweb.org/macoda/ontologies/PMOEA#DTLZ6_6">
        <rdf:type rdf:resource="http://www.semanticweb.org/macoda/ontologies/PMOEA#DTLZ"/>
        <PMOEA:isContinuousProblem rdf:datatype="http://www.w3.org/2001/XMLSchema#boolean">true</PMOEA:isContinuousProblem>
        <PMOEA:ObjectiveNumber rdf:datatype="http://www.w3.org/2001/XMLSchema#integer">6</PMOEA:ObjectiveNumber>
        <PMOEA:isManyObjectiveProblem rdf:datatype="http://www.w3.org/2001/XMLSchema#boolean">true</PMOEA:isManyObjectiveProblem>
        <rdfs:label xml:lang="en">DTLZ6_6</rdfs:label>
    </owl:NamedIndividual>
    


    <!-- http://www.semanticweb.org/macoda/ontologies/PMOEA#MOEAFramework -->

    <owl:NamedIndividual rdf:about="http://www.semanticweb.org/macoda/ontologies/PMOEA#MOEAFramework">
        <rdf:type rdf:resource="http://www.semanticweb.org/macoda/ontologies/PMOEA#ImplementationLibrary"/>
        <rdfs:comment>The MOEA Framework is a free and open source Java library for developing and experimenting with multiobjective evolutionary algorithms (MOEAs) and other general-purpose multiobjective optimization algorithms. The MOEA Framework supports genetic algorithms, differential evolution, particle swarm optimization, genetic programming, grammatical evolution, and more. A number of algorithms are provided out-of-the-box, including NSGA-II, NSGA-III, -MOEA, GDE3, PAES, PESA2, SPEA2, IBEA, SMS-EMOA, SMPSO, OMOPSO, CMA-ES, and MOEA/D. In addition, the MOEA Framework provides the tools necessary to rapidly design, develop, execute and statistically test optimization algorithms.</rdfs:comment>
        <rdfs:label xml:lang="en">MOEAFramework</rdfs:label>
    </owl:NamedIndividual>
    


    <!-- http://www.semanticweb.org/macoda/ontologies/PMOEA#iPICEA-G -->

    <owl:NamedIndividual rdf:about="http://www.semanticweb.org/macoda/ontologies/PMOEA#iPICEA-G">
        <rdf:type rdf:resource="http://www.semanticweb.org/macoda/ontologies/PMOEA#PMOEA"/>
        <PMOEA:hasPreferenceModel rdf:resource="http://www.semanticweb.org/macoda/ontologies/PMOEA#PreferencePoint"/>
        <PMOEA:hasPreferenceInformationFromDM rdf:resource="http://www.semanticweb.org/macoda/ontologies/PMOEA#SearchRange"/>
        <PMOEA:hasPreferenceInformationFromDM rdf:resource="http://www.semanticweb.org/macoda/ontologies/PMOEA#SearchDirection"/>
        <PMOEA:hasPreferenceInformationFromDM rdf:resource="http://www.semanticweb.org/macoda/ontologies/PMOEA#BrushingPreferenceRegionInObjectiveSpace"/>
        <PMOEA:hasPreferenceInformationFromDM rdf:resource="http://www.semanticweb.org/macoda/ontologies/PMOEA#ReferencePoint"/>
        <PMOEA:hasInteractionTime rdf:resource="http://www.semanticweb.org/macoda/ontologies/PMOEA#a-priori"/>
        <PMOEA:hasInteractionTime rdf:resource="http://www.semanticweb.org/macoda/ontologies/PMOEA#progressive"/>
        <PMOEA:hasPreferenceIntegration rdf:resource="http://www.semanticweb.org/macoda/ontologies/PMOEA#ParetoConeDominance"/>
        <PMOEA:canSolve rdf:resource="http://www.semanticweb.org/macoda/ontologies/PMOEA#DTLZ2_2"/>
        <PMOEA:canSolve rdf:resource="http://www.semanticweb.org/macoda/ontologies/PMOEA#ZDT2"/>
        <PMOEA:canSolve rdf:resource="http://www.semanticweb.org/macoda/ontologies/PMOEA#DTLZ2_4"/>
        <PMOEA:canSolve rdf:resource="http://www.semanticweb.org/macoda/ontologies/PMOEA#ZDT1"/>
        <PMOEA:hasResultInfluence rdf:resource="http://www.semanticweb.org/macoda/ontologies/PMOEA#BoundedRegion"/>
        <PMOEA:hasAuthor rdf:resource="http://www.semanticweb.org/macoda/ontologies/PMOEA#Rui_Wang"/>
        <PMOEA:hasAuthor rdf:resource="http://www.semanticweb.org/macoda/ontologies/PMOEA#Peter_J_Fleming"/>
        <PMOEA:hasAuthor rdf:resource="http://www.semanticweb.org/macoda/ontologies/PMOEA#Robin_C_Purshouse"/>
        <PMOEA:hasSearchAlgorithm rdf:resource="http://www.semanticweb.org/macoda/ontologies/PMOEA#PICEA"/>
        <PMOEA:hasDevelopingYear rdf:datatype="http://www.w3.org/2001/XMLSchema#integer">2013</PMOEA:hasDevelopingYear>
        <PMOEA:MultipleRegionOfInterest rdf:datatype="http://www.w3.org/2001/XMLSchema#boolean">true</PMOEA:MultipleRegionOfInterest>
        <PMOEA:SpreadControl rdf:datatype="http://www.w3.org/2001/XMLSchema#boolean">true</PMOEA:SpreadControl>
        <PMOEA:hasReference>Wang, R., R. C. Purshouse and P. J. Fleming (2013). Whatever Works Best for You-A New Method for a Priori and Progressive Multi-objective Optimisation. Evolutionary Multi-Criterion Optimization, Springer</PMOEA:hasReference>
        <rdfs:comment>in some cases it is easier for the DM to express the preferences by weights and in some cases by aspiration levels. The most flexible approach would be to develop a unified approach which enables the DM to articulate both types of the preferences. In this paper, we describe such a unified approach. Three parameters: reference point (R), weight (W) and search range () are introduced. Then a new interactive evolutionary multiobjective optimization and decision-making algorithm, iPICEA-g, is proposed that incorporates the unified approach within the existing algorithm PICEA-g</rdfs:comment>
        <rdfs:label xml:lang="en">iPICEA-G</rdfs:label>
    </owl:NamedIndividual>
    


    <!-- http://www.semanticweb.org/macoda/ontologies/PMOEA#PICEA -->

    <owl:NamedIndividual rdf:about="http://www.semanticweb.org/macoda/ontologies/PMOEA#PICEA">
        <rdf:type rdf:resource="http://www.semanticweb.org/macoda/ontologies/PMOEA#Coevolution_based"/>
        <rdfs:comment>A population of candidate solutions and preference sets, S and G, of fixed size, N and NGoal, are evolved for a fixed number of generations maxGen. In each generation t, parents S(t) are subjected to (representation appropriate) genetic variation operators to produce N offspring
Sc(t). Simultaneously, NGoal new preference sets Gc(t), are randomly regenerated based on the initial bounds. S(t) and Sc(t), and G(t) and Gc(t), are then pooled, respectively, and the combined populations are sorted according to the fitness. Truncation selection is applied to select the best N solutions as new parent population S(t+1), and NGoal solutions as new
preference population G(t + 1).</rdfs:comment>
        <rdfs:label xml:lang="en">PICEA</rdfs:label>
    </owl:NamedIndividual>
    


    <!-- http://www.semanticweb.org/macoda/ontologies/PMOEA#SetOfSolutions -->

    <owl:NamedIndividual rdf:about="http://www.semanticweb.org/macoda/ontologies/PMOEA#SetOfSolutions">
        <rdf:type rdf:resource="http://www.semanticweb.org/macoda/ontologies/PMOEA#SetOfSolutions"/>
        <rdfs:label xml:lang="en">SetOfSolutions</rdfs:label>
    </owl:NamedIndividual>
    


    <!-- http://www.semanticweb.org/macoda/ontologies/PMOEA#Oliver_Schutze -->

    <owl:NamedIndividual rdf:about="http://www.semanticweb.org/macoda/ontologies/PMOEA#Oliver_Schutze">
        <rdf:type rdf:resource="http://www.semanticweb.org/macoda/ontologies/PMOEA#Researcher"/>
        <rdfs:label xml:lang="en">Oliver Schutze</rdfs:label>
    </owl:NamedIndividual>
    


    <!-- http://www.semanticweb.org/macoda/ontologies/PMOEA#RobustOrdinalRegression -->

    <owl:NamedIndividual rdf:about="http://www.semanticweb.org/macoda/ontologies/PMOEA#RobustOrdinalRegression">
        <rdf:type rdf:resource="http://www.semanticweb.org/macoda/ontologies/PMOEA#OrdinalRegression"/>
        <rdfs:label xml:lang="en">RobustOrdinalRegression</rdfs:label>
    </owl:NamedIndividual>
    


    <!-- http://www.semanticweb.org/macoda/ontologies/PMOEA#SingleCutTurningCostOptimization -->

    <owl:NamedIndividual rdf:about="http://www.semanticweb.org/macoda/ontologies/PMOEA#SingleCutTurningCostOptimization">
        <rdf:type rdf:resource="http://www.semanticweb.org/macoda/ontologies/PMOEA#Realworld_Problem"/>
        <PMOEA:isNoisy rdf:datatype="http://www.w3.org/2001/XMLSchema#boolean">true</PMOEA:isNoisy>
        <PMOEA:isContinuousProblem rdf:datatype="http://www.w3.org/2001/XMLSchema#boolean">true</PMOEA:isContinuousProblem>
        <PMOEA:ObjectiveNumber rdf:datatype="http://www.w3.org/2001/XMLSchema#integer">2</PMOEA:ObjectiveNumber>
        <rdfs:label xml:lang="en">SingleCutTurningCostOptimization</rdfs:label>
    </owl:NamedIndividual>
    


    <!-- http://www.semanticweb.org/macoda/ontologies/PMOEA#QuasiConcaveUtilityFunction -->

    <owl:NamedIndividual rdf:about="http://www.semanticweb.org/macoda/ontologies/PMOEA#QuasiConcaveUtilityFunction">
        <rdf:type rdf:resource="http://www.semanticweb.org/macoda/ontologies/PMOEA#QuasiConcave"/>
        <rdfs:label xml:lang="en">QuasiConcaveUtilityFunction</rdfs:label>
    </owl:NamedIndividual>
    


    <!-- http://www.semanticweb.org/macoda/ontologies/PMOEA#ParentSelection -->

    <owl:NamedIndividual rdf:about="http://www.semanticweb.org/macoda/ontologies/PMOEA#ParentSelection">
        <rdf:type rdf:resource="http://www.semanticweb.org/macoda/ontologies/PMOEA#SelectionCriterion"/>
        <rdfs:comment>How to select part of population as parents to generate new offspring</rdfs:comment>
        <rdfs:label xml:lang="en">ParentSelection</rdfs:label>
    </owl:NamedIndividual>
    


    <!-- http://www.semanticweb.org/macoda/ontologies/PMOEA#S-ZDT1 -->

    <owl:NamedIndividual rdf:about="http://www.semanticweb.org/macoda/ontologies/PMOEA#S-ZDT1">
        <rdf:type rdf:resource="http://www.semanticweb.org/macoda/ontologies/PMOEA#Academic_Problem"/>
        <PMOEA:isContinuousProblem rdf:datatype="http://www.w3.org/2001/XMLSchema#boolean">true</PMOEA:isContinuousProblem>
        <PMOEA:ObjectiveNumber rdf:datatype="http://www.w3.org/2001/XMLSchema#integer">2</PMOEA:ObjectiveNumber>
        <rdfs:label xml:lang="en">S-ZDT1</rdfs:label>
    </owl:NamedIndividual>
    


    <!-- http://www.semanticweb.org/macoda/ontologies/PMOEA#MOGLS -->

    <owl:NamedIndividual rdf:about="http://www.semanticweb.org/macoda/ontologies/PMOEA#MOGLS">
        <rdf:type rdf:resource="http://www.semanticweb.org/macoda/ontologies/PMOEA#Memetic"/>
        <rdfs:label xml:lang="en">MOGLS</rdfs:label>
    </owl:NamedIndividual>
    


    <!-- http://www.semanticweb.org/macoda/ontologies/PMOEA#Pedro_3 -->

    <owl:NamedIndividual rdf:about="http://www.semanticweb.org/macoda/ontologies/PMOEA#Pedro_3">
        <rdf:type rdf:resource="http://www.semanticweb.org/macoda/ontologies/PMOEA#Academic_Problem"/>
        <PMOEA:isContinuousProblem rdf:datatype="http://www.w3.org/2001/XMLSchema#boolean">true</PMOEA:isContinuousProblem>
        <PMOEA:ObjectiveNumber rdf:datatype="http://www.w3.org/2001/XMLSchema#integer">3</PMOEA:ObjectiveNumber>
        <rdfs:label xml:lang="en">Pedro_3</rdfs:label>
    </owl:NamedIndividual>
    


    <!-- http://www.semanticweb.org/macoda/ontologies/PMOEA#StrictlyIncreasingPolynomialValueFunction -->

    <owl:NamedIndividual rdf:about="http://www.semanticweb.org/macoda/ontologies/PMOEA#StrictlyIncreasingPolynomialValueFunction">
        <rdf:type rdf:resource="http://www.semanticweb.org/macoda/ontologies/PMOEA#Polynomial"/>
        <rdfs:label xml:lang="en">StrictlyIncreasingPolynomialValueFunction</rdfs:label>
    </owl:NamedIndividual>
    


    <!-- http://www.semanticweb.org/macoda/ontologies/PMOEA#Claus_Weihs -->

    <owl:NamedIndividual rdf:about="http://www.semanticweb.org/macoda/ontologies/PMOEA#Claus_Weihs">
        <rdf:type rdf:resource="http://www.semanticweb.org/macoda/ontologies/PMOEA#Researcher"/>
        <rdfs:label xml:lang="en">Claus Weihs</rdfs:label>
    </owl:NamedIndividual>
    


    <!-- http://www.semanticweb.org/macoda/ontologies/PMOEA#HypervolumeIndicator -->

    <owl:NamedIndividual rdf:about="http://www.semanticweb.org/macoda/ontologies/PMOEA#HypervolumeIndicator">
        <rdf:type rdf:resource="http://www.semanticweb.org/macoda/ontologies/PMOEA#SetQualityIndicator"/>
        <rdfs:label xml:lang="en">HypervolumeIndicator</rdfs:label>
    </owl:NamedIndividual>
    


    <!-- http://www.semanticweb.org/macoda/ontologies/PMOEA#SamplePartialOrder -->

    <owl:NamedIndividual rdf:about="http://www.semanticweb.org/macoda/ontologies/PMOEA#SamplePartialOrder">
        <rdf:type rdf:resource="http://www.semanticweb.org/macoda/ontologies/PMOEA#SampleRanks"/>
        <rdfs:comment>give partial order of some solutions in the reference set</rdfs:comment>
        <rdfs:label xml:lang="en">SamplePartialOrder</rdfs:label>
    </owl:NamedIndividual>
    


    <!-- http://www.semanticweb.org/macoda/ontologies/PMOEA#SearchDirection -->

    <owl:NamedIndividual rdf:about="http://www.semanticweb.org/macoda/ontologies/PMOEA#SearchDirection">
        <rdf:type rdf:resource="http://www.semanticweb.org/macoda/ontologies/PMOEA#ReferenceDirection"/>
        <rdfs:comment>weights to introduce the DMs bias toward some objectives,objective f1 is twice as important as f2 then W = [0.67, 0.33],used in iPICEA-g</rdfs:comment>
        <rdfs:label xml:lang="en">SearchDirection</rdfs:label>
    </owl:NamedIndividual>
    


    <!-- http://www.semanticweb.org/macoda/ontologies/PMOEA#W-NSS-GPA -->

    <owl:NamedIndividual rdf:about="http://www.semanticweb.org/macoda/ontologies/PMOEA#W-NSS-GPA">
        <rdf:type rdf:resource="http://www.semanticweb.org/macoda/ontologies/PMOEA#PMOEA"/>
        <PMOEA:hasPreferenceModel rdf:resource="http://www.semanticweb.org/macoda/ontologies/PMOEA#WeightedEuclideanDistanceASF"/>
        <PMOEA:hasPreferenceInformationFromDM rdf:resource="http://www.semanticweb.org/macoda/ontologies/PMOEA#GroupDMPoints"/>
        <PMOEA:hasInteractionTime rdf:resource="http://www.semanticweb.org/macoda/ontologies/PMOEA#a-priori"/>
        <PMOEA:hasPreferenceIntegration rdf:resource="http://www.semanticweb.org/macoda/ontologies/PMOEA#r-Dominance"/>
        <PMOEA:canSolve rdf:resource="http://www.semanticweb.org/macoda/ontologies/PMOEA#Bi-objectivePortfolioOptimization"/>
        <PMOEA:canSolve rdf:resource="http://www.semanticweb.org/macoda/ontologies/PMOEA#DTLZ2_4"/>
        <PMOEA:hasResultInfluence rdf:resource="http://www.semanticweb.org/macoda/ontologies/PMOEA#BoundedRegion"/>
        <PMOEA:hasAuthor rdf:resource="http://www.semanticweb.org/macoda/ontologies/PMOEA#Khaled_Ghdira"/>
        <PMOEA:hasAuthor rdf:resource="http://www.semanticweb.org/macoda/ontologies/PMOEA#Slim_Bechikh"/>
        <PMOEA:hasAuthor rdf:resource="http://www.semanticweb.org/macoda/ontologies/PMOEA#Lamjed_Ben_Said,"/>
        <PMOEA:hasSearchAlgorithm rdf:resource="http://www.semanticweb.org/macoda/ontologies/PMOEA#NSGA-II"/>
        <PMOEA:hasImplementationLanguage rdf:resource="http://www.semanticweb.org/macoda/ontologies/PMOEA#Java"/>
        <PMOEA:hasDevelopingYear rdf:datatype="http://www.w3.org/2001/XMLSchema#integer">2013</PMOEA:hasDevelopingYear>
        <PMOEA:SpreadControl rdf:datatype="http://www.w3.org/2001/XMLSchema#boolean">true</PMOEA:SpreadControl>
        <PMOEA:ParetoDominancePreservation rdf:datatype="http://www.w3.org/2001/XMLSchema#boolean">true</PMOEA:ParetoDominancePreservation>
        <PMOEA:hasReference>Bechikh S, Said L B, Ghdira K. Group preferencebased evolutionary multi-objective optimization with nonequally important decision makers: Application to the portfolio selection problem[J]. International Journal of Computer Information Systems and Industrial Management Applications, 2013, 5(278-288): 71.</PMOEA:hasReference>
        <rdfs:comment>Weighted Negotiation Support System for Group Preference Aggregation.W-NSS-GPA takes as inputs the DMs preferences modelled as reference points and the DMs hierarchy levels modelled by weights. Then, it provides as output a single Social Reference Point (SRP) that corresponds to an aggregation of all DMs preferences. By running the preference-based EMOA(r-NSGA-II) with this SRP, we obtain a social ROI corresponding to aggregated DMs preferences.</rdfs:comment>
        <rdfs:label xml:lang="en">W-NSS-GPA</rdfs:label>
    </owl:NamedIndividual>
    


    <!-- http://www.semanticweb.org/macoda/ontologies/PMOEA#ReferenceDirection -->

    <owl:NamedIndividual rdf:about="http://www.semanticweb.org/macoda/ontologies/PMOEA#ReferenceDirection">
        <rdf:type rdf:resource="http://www.semanticweb.org/macoda/ontologies/PMOEA#ReferenceDirection"/>
        <rdfs:comment>DM gives one start point and an end point, the difference of them defines a direction, proposed originally by Korhonen and Laakso 1986</rdfs:comment>
        <rdfs:label xml:lang="en">ReferenceDirection</rdfs:label>
    </owl:NamedIndividual>
    


    <!-- http://www.semanticweb.org/macoda/ontologies/PMOEA#WFG9_10 -->

    <owl:NamedIndividual rdf:about="http://www.semanticweb.org/macoda/ontologies/PMOEA#WFG9_10">
        <rdf:type rdf:resource="http://www.semanticweb.org/macoda/ontologies/PMOEA#WFG"/>
        <PMOEA:OWLDataProperty_61d3cd95_fde4_4c1b_af08_1eaf73473aea rdf:datatype="http://www.w3.org/2001/XMLSchema#boolean">true</PMOEA:OWLDataProperty_61d3cd95_fde4_4c1b_af08_1eaf73473aea>
        <PMOEA:isContinuousProblem rdf:datatype="http://www.w3.org/2001/XMLSchema#boolean">true</PMOEA:isContinuousProblem>
        <PMOEA:ObjectiveNumber rdf:datatype="http://www.w3.org/2001/XMLSchema#integer">10</PMOEA:ObjectiveNumber>
        <PMOEA:isManyObjectiveProblem rdf:datatype="http://www.w3.org/2001/XMLSchema#boolean">true</PMOEA:isManyObjectiveProblem>
        <rdfs:label xml:lang="en">WFG9_10</rdfs:label>
    </owl:NamedIndividual>
    


    <!-- http://www.semanticweb.org/macoda/ontologies/PMOEA#2p-NSGA-II -->

    <owl:NamedIndividual rdf:about="http://www.semanticweb.org/macoda/ontologies/PMOEA#2p-NSGA-II">
        <rdf:type rdf:resource="http://www.semanticweb.org/macoda/ontologies/PMOEA#PMOEA"/>
        <PMOEA:hasPreferenceModel rdf:resource="http://www.semanticweb.org/macoda/ontologies/PMOEA#BipolarPreferencePoint"/>
        <PMOEA:hasPreferenceInformationFromDM rdf:resource="http://www.semanticweb.org/macoda/ontologies/PMOEA#BipolarReferencePoint"/>
        <PMOEA:hasInteractionTime rdf:resource="http://www.semanticweb.org/macoda/ontologies/PMOEA#a-priori"/>
        <PMOEA:hasPreferenceIntegration rdf:resource="http://www.semanticweb.org/macoda/ontologies/PMOEA#CrowdingDistance"/>
        <PMOEA:canSolve rdf:resource="http://www.semanticweb.org/macoda/ontologies/PMOEA#DTLZ2_10"/>
        <PMOEA:canSolve rdf:resource="http://www.semanticweb.org/macoda/ontologies/PMOEA#ZDT2"/>
        <PMOEA:canSolve rdf:resource="http://www.semanticweb.org/macoda/ontologies/PMOEA#DTLZ2_5"/>
        <PMOEA:canSolve rdf:resource="http://www.semanticweb.org/macoda/ontologies/PMOEA#ZDT3"/>
        <PMOEA:canSolve rdf:resource="http://www.semanticweb.org/macoda/ontologies/PMOEA#DTLZ2_3"/>
        <PMOEA:canSolve rdf:resource="http://www.semanticweb.org/macoda/ontologies/PMOEA#ZDT1"/>
        <PMOEA:canSolve rdf:resource="http://www.semanticweb.org/macoda/ontologies/PMOEA#DTLZ2_15"/>
        <PMOEA:hasResultInfluence rdf:resource="http://www.semanticweb.org/macoda/ontologies/PMOEA#BiasedDistribution"/>
        <PMOEA:hasAuthor rdf:resource="http://www.semanticweb.org/macoda/ontologies/PMOEA#Yushi_Wu"/>
        <PMOEA:hasAuthor rdf:resource="http://www.semanticweb.org/macoda/ontologies/PMOEA#Liping_Wang"/>
        <PMOEA:hasAuthor rdf:resource="http://www.semanticweb.org/macoda/ontologies/PMOEA#Feiyue_Qiu"/>
        <PMOEA:hasAuthor rdf:resource="http://www.semanticweb.org/macoda/ontologies/PMOEA#Bo_Jiang"/>
        <PMOEA:isExtensionOf rdf:resource="http://www.semanticweb.org/macoda/ontologies/PMOEA#g-NSGA-II"/>
        <PMOEA:hasSearchAlgorithm rdf:resource="http://www.semanticweb.org/macoda/ontologies/PMOEA#NSGA-II"/>
        <PMOEA:hasImplementationLanguage rdf:resource="http://www.semanticweb.org/macoda/ontologies/PMOEA#Matlab"/>
        <PMOEA:hasDevelopingYear rdf:datatype="http://www.w3.org/2001/XMLSchema#integer">2012</PMOEA:hasDevelopingYear>
        <PMOEA:MultipleRegionOfInterest rdf:datatype="http://www.w3.org/2001/XMLSchema#boolean">true</PMOEA:MultipleRegionOfInterest>
        <PMOEA:SpreadControl rdf:datatype="http://www.w3.org/2001/XMLSchema#boolean">true</PMOEA:SpreadControl>
        <PMOEA:hasReference>Fei-yue, Q.; Yu-shi, W.; Li-ping, W. &amp; Bo, J. Bipolar preferences dominance based evolutionary algorithm for many-objective optimization 2012 IEEE Congress on Evolutionary Computation, 2012, 1-8</PMOEA:hasReference>
        <rdfs:comment>The DM may have positive preference and negative preference simultaneously for some practical problems; it is insufficient to articulate the DMs preferences when using only one reference point. Besides, g-dominance adds the dominance relation of solutions between preference area and non-preference area only, for the solutions belong to the same area, it still adopts Pareto dominance. When solving many-objective problem, it faces the same trouble with Pareto dominance. To solve the problem mentioned above, this paper proposes a scheme of bipolar preferences dominance, which brings in the concept of bipolar preferences based on g-dominance. The preference dominance relation of g-dominance is adopted to promote the efficiency of Pareto sorting, the non-dominated solutions similarities are compared to increase the proportion of solutions comparability.</rdfs:comment>
        <rdfs:label xml:lang="en">2p-NSGA-II</rdfs:label>
    </owl:NamedIndividual>
    


    <!-- http://www.semanticweb.org/macoda/ontologies/PMOEA#Xinfang_Ji -->

    <owl:NamedIndividual rdf:about="http://www.semanticweb.org/macoda/ontologies/PMOEA#Xinfang_Ji">
        <rdf:type rdf:resource="http://www.semanticweb.org/macoda/ontologies/PMOEA#Researcher"/>
        <rdfs:label xml:lang="en">Xinfang Ji</rdfs:label>
    </owl:NamedIndividual>
    


    <!-- http://www.semanticweb.org/macoda/ontologies/PMOEA#AdditivePiecewiseLinear -->

    <owl:NamedIndividual rdf:about="http://www.semanticweb.org/macoda/ontologies/PMOEA#AdditivePiecewiseLinear">
        <rdf:type rdf:resource="http://www.semanticweb.org/macoda/ontologies/PMOEA#AdditivePiecewiseLinear"/>
        <rdfs:label xml:lang="en">AdditivePiecewiseLinear</rdfs:label>
    </owl:NamedIndividual>
    


    <!-- http://www.semanticweb.org/macoda/ontologies/PMOEA#LBSParameters -->

    <owl:NamedIndividual rdf:about="http://www.semanticweb.org/macoda/ontologies/PMOEA#LBSParameters">
        <rdf:type rdf:resource="http://www.semanticweb.org/macoda/ontologies/PMOEA#ReferenceDirection"/>
        <rdfs:comment>Parameters in Light Beam Search, including Aspiration Point (AP), Reservation Point (RP), from them a direction is defined. Threshold values in outranking relation to find neighbours of middle point is also needed.</rdfs:comment>
        <rdfs:label xml:lang="en">LBSParameters</rdfs:label>
    </owl:NamedIndividual>
    


    <!-- http://www.semanticweb.org/macoda/ontologies/PMOEA#Iryna_Yevseyeva -->

    <owl:NamedIndividual rdf:about="http://www.semanticweb.org/macoda/ontologies/PMOEA#Iryna_Yevseyeva">
        <rdf:type rdf:resource="http://www.semanticweb.org/macoda/ontologies/PMOEA#Researcher"/>
        <rdfs:label xml:lang="en">Iryna Yevseyeva</rdfs:label>
    </owl:NamedIndividual>
    


    <!-- http://www.semanticweb.org/macoda/ontologies/PMOEA#ArtificialNeuralNetwork -->

    <owl:NamedIndividual rdf:about="http://www.semanticweb.org/macoda/ontologies/PMOEA#ArtificialNeuralNetwork">
        <rdf:type rdf:resource="http://www.semanticweb.org/macoda/ontologies/PMOEA#NeuralNetwork"/>
        <rdfs:label xml:lang="en">ArtificialNeuralNetwork</rdfs:label>
    </owl:NamedIndividual>
    


    <!-- http://www.semanticweb.org/macoda/ontologies/PMOEA#M-ProperParetoOptimal -->

    <owl:NamedIndividual rdf:about="http://www.semanticweb.org/macoda/ontologies/PMOEA#M-ProperParetoOptimal">
        <rdf:type rdf:resource="http://www.semanticweb.org/macoda/ontologies/PMOEA#Trade-off"/>
        <rdfs:comment>value M to define M-proper Pareto-optimality</rdfs:comment>
        <rdfs:label xml:lang="en">M-ProperParetoOptimal</rdfs:label>
    </owl:NamedIndividual>
    


    <!-- http://www.semanticweb.org/macoda/ontologies/PMOEA#Dimo_Brockhoff -->

    <owl:NamedIndividual rdf:about="http://www.semanticweb.org/macoda/ontologies/PMOEA#Dimo_Brockhoff">
        <rdf:type rdf:resource="http://www.semanticweb.org/macoda/ontologies/PMOEA#Researcher"/>
        <rdfs:label xml:lang="en">Dimo Brockhoff</rdfs:label>
    </owl:NamedIndividual>
    


    <!-- http://www.semanticweb.org/macoda/ontologies/PMOEA#BC-EMOA -->

    <owl:NamedIndividual rdf:about="http://www.semanticweb.org/macoda/ontologies/PMOEA#BC-EMOA">
        <rdf:type rdf:resource="http://www.semanticweb.org/macoda/ontologies/PMOEA#PMOEA"/>
        <PMOEA:hasPreferenceModel rdf:resource="http://www.semanticweb.org/macoda/ontologies/PMOEA#GeneralUtilityFunction"/>
        <PMOEA:hasPreferenceInformationFromDM rdf:resource="http://www.semanticweb.org/macoda/ontologies/PMOEA#RankSamples"/>
        <PMOEA:hasPreferenceIntegration rdf:resource="http://www.semanticweb.org/macoda/ontologies/PMOEA#PreferenceOrderingBasedonUtilityFunction"/>
        <PMOEA:hasLearningMethod rdf:resource="http://www.semanticweb.org/macoda/ontologies/PMOEA#SupportVectorRanking"/>
        <PMOEA:canSolve rdf:resource="http://www.semanticweb.org/macoda/ontologies/PMOEA#Knapsack_4"/>
        <PMOEA:canSolve rdf:resource="http://www.semanticweb.org/macoda/ontologies/PMOEA#DTLZ6_8"/>
        <PMOEA:canSolve rdf:resource="http://www.semanticweb.org/macoda/ontologies/PMOEA#Knapsack_10"/>
        <PMOEA:canSolve rdf:resource="http://www.semanticweb.org/macoda/ontologies/PMOEA#DTLZ6_4"/>
        <PMOEA:canSolve rdf:resource="http://www.semanticweb.org/macoda/ontologies/PMOEA#DTLZ7_8"/>
        <PMOEA:canSolve rdf:resource="http://www.semanticweb.org/macoda/ontologies/PMOEA#DTLZ6_10"/>
        <PMOEA:canSolve rdf:resource="http://www.semanticweb.org/macoda/ontologies/PMOEA#DTLZ7_4"/>
        <PMOEA:canSolve rdf:resource="http://www.semanticweb.org/macoda/ontologies/PMOEA#DTLZ1_4"/>
        <PMOEA:canSolve rdf:resource="http://www.semanticweb.org/macoda/ontologies/PMOEA#DTLZ1_8"/>
        <PMOEA:canSolve rdf:resource="http://www.semanticweb.org/macoda/ontologies/PMOEA#DTLZ1_10"/>
        <PMOEA:canSolve rdf:resource="http://www.semanticweb.org/macoda/ontologies/PMOEA#Knapsack_8"/>
        <PMOEA:canSolve rdf:resource="http://www.semanticweb.org/macoda/ontologies/PMOEA#DTLZ7_10"/>
        <PMOEA:hasResultInfluence rdf:resource="http://www.semanticweb.org/macoda/ontologies/PMOEA#BoundedRegion"/>
        <PMOEA:hasAuthor rdf:resource="http://www.semanticweb.org/macoda/ontologies/PMOEA#Roberto_Battiti"/>
        <PMOEA:hasAuthor rdf:resource="http://www.semanticweb.org/macoda/ontologies/PMOEA#Andrea_Passerini"/>
        <PMOEA:useLibrary rdf:resource="http://www.semanticweb.org/macoda/ontologies/PMOEA#KanGAL"/>
        <PMOEA:hasSearchAlgorithm rdf:resource="http://www.semanticweb.org/macoda/ontologies/PMOEA#NSGA-II"/>
        <PMOEA:hasImplementationLanguage rdf:resource="http://www.semanticweb.org/macoda/ontologies/PMOEA#C"/>
        <PMOEA:hasDevelopingYear rdf:datatype="http://www.w3.org/2001/XMLSchema#integer">2010</PMOEA:hasDevelopingYear>
        <PMOEA:ParetoDominancePreservation rdf:datatype="http://www.w3.org/2001/XMLSchema#boolean">true</PMOEA:ParetoDominancePreservation>
        <PMOEA:hasReference>Battiti, R. and A. Passerini (2010). &quot;Braincomputer evolutionary multiobjective optimization: a genetic algorithm adapting to the decision maker.&quot; Evolutionary Computation, IEEE Transactions on 14(5): 671-687</PMOEA:hasReference>
        <rdfs:comment>Periodically, the DM is presented with a set of solutions and asked to (at least partially) rank them. This information is then used to train the SVM, with cross validation employed to select an appropriate kernel. The ordering of the new population and the selection criterion of the binary tournament selection operator are performed based on the actual utility function value..</rdfs:comment>
        <rdfs:label xml:lang="en">BC-EMOA</rdfs:label>
    </owl:NamedIndividual>
    


    <!-- http://www.semanticweb.org/macoda/ontologies/PMOEA#DTLZ1_10 -->

    <owl:NamedIndividual rdf:about="http://www.semanticweb.org/macoda/ontologies/PMOEA#DTLZ1_10">
        <rdf:type rdf:resource="http://www.semanticweb.org/macoda/ontologies/PMOEA#DTLZ"/>
        <PMOEA:OWLDataProperty_61d3cd95_fde4_4c1b_af08_1eaf73473aea rdf:datatype="http://www.w3.org/2001/XMLSchema#boolean">true</PMOEA:OWLDataProperty_61d3cd95_fde4_4c1b_af08_1eaf73473aea>
        <PMOEA:isContinuousProblem rdf:datatype="http://www.w3.org/2001/XMLSchema#boolean">true</PMOEA:isContinuousProblem>
        <PMOEA:ObjectiveNumber rdf:datatype="http://www.w3.org/2001/XMLSchema#integer">10</PMOEA:ObjectiveNumber>
        <PMOEA:isManyObjectiveProblem rdf:datatype="http://www.w3.org/2001/XMLSchema#boolean">true</PMOEA:isManyObjectiveProblem>
        <rdfs:label xml:lang="en">DTLZ1_10</rdfs:label>
    </owl:NamedIndividual>
    


    <!-- http://www.semanticweb.org/macoda/ontologies/PMOEA#RD-NSGA-II -->

    <owl:NamedIndividual rdf:about="http://www.semanticweb.org/macoda/ontologies/PMOEA#RD-NSGA-II">
        <rdf:type rdf:resource="http://www.semanticweb.org/macoda/ontologies/PMOEA#PMOEA"/>
        <PMOEA:hasPreferenceModel rdf:resource="http://www.semanticweb.org/macoda/ontologies/PMOEA#TchebycheffASF"/>
        <PMOEA:hasPreferenceInformationFromDM rdf:resource="http://www.semanticweb.org/macoda/ontologies/PMOEA#ReferenceDirection"/>
        <PMOEA:hasInteractionTime rdf:resource="http://www.semanticweb.org/macoda/ontologies/PMOEA#progressive"/>
        <PMOEA:hasPreferenceIntegration rdf:resource="http://www.semanticweb.org/macoda/ontologies/PMOEA#FrontSorting"/>
        <PMOEA:canSolve rdf:resource="http://www.semanticweb.org/macoda/ontologies/PMOEA#DTLZ2_10"/>
        <PMOEA:canSolve rdf:resource="http://www.semanticweb.org/macoda/ontologies/PMOEA#CarSideImpactProblem"/>
        <PMOEA:canSolve rdf:resource="http://www.semanticweb.org/macoda/ontologies/PMOEA#ZDT2"/>
        <PMOEA:canSolve rdf:resource="http://www.semanticweb.org/macoda/ontologies/PMOEA#DTLZ2_5"/>
        <PMOEA:canSolve rdf:resource="http://www.semanticweb.org/macoda/ontologies/PMOEA#DTLZ2_3"/>
        <PMOEA:canSolve rdf:resource="http://www.semanticweb.org/macoda/ontologies/PMOEA#ZDT1"/>
        <PMOEA:hasResultInfluence rdf:resource="http://www.semanticweb.org/macoda/ontologies/PMOEA#OneSolution"/>
        <PMOEA:hasAuthor rdf:resource="http://www.semanticweb.org/macoda/ontologies/PMOEA#Abhishek_Kumar"/>
        <PMOEA:hasAuthor rdf:resource="http://www.semanticweb.org/macoda/ontologies/PMOEA#Kalyanmoy_Deb"/>
        <PMOEA:hasSearchAlgorithm rdf:resource="http://www.semanticweb.org/macoda/ontologies/PMOEA#NSGA-II"/>
        <PMOEA:hasDevelopingYear rdf:datatype="http://www.w3.org/2001/XMLSchema#integer">2007</PMOEA:hasDevelopingYear>
        <PMOEA:hasRemarks>EMO in MCDM</PMOEA:hasRemarks>
        <PMOEA:MultipleRegionOfInterest rdf:datatype="http://www.w3.org/2001/XMLSchema#boolean">true</PMOEA:MultipleRegionOfInterest>
        <PMOEA:SpreadControl rdf:datatype="http://www.w3.org/2001/XMLSchema#boolean">true</PMOEA:SpreadControl>
        <PMOEA:ParetoDominancePreservation rdf:datatype="http://www.w3.org/2001/XMLSchema#boolean">true</PMOEA:ParetoDominancePreservation>
        <PMOEA:hasReference>Deb, K. and A. Kumar (2007). Interactive evolutionary multi-objective optimization and decision-making using reference direction method. Proceedings of the 9th annual conference on Genetic and evolutionary computation, ACM</PMOEA:hasReference>
        <rdfs:comment>An evolutionary multi-objective optimization (EMO) can be introduced to achieve a set of efficient solutions of the reference direction procedure simultaneously.</rdfs:comment>
        <rdfs:label xml:lang="en">RD-NSGA-II</rdfs:label>
    </owl:NamedIndividual>
    


    <!-- http://www.semanticweb.org/macoda/ontologies/PMOEA#KanGAL -->

    <owl:NamedIndividual rdf:about="http://www.semanticweb.org/macoda/ontologies/PMOEA#KanGAL">
        <rdf:type rdf:resource="http://www.semanticweb.org/macoda/ontologies/PMOEA#ImplementationLibrary"/>
        <rdfs:comment>library by Kanpur Genetic Algorithms Laboratory (KanGAL), Indian Institute of Technology Kanpur dedicated to pursuing research and industrial collaboration in the areas of genetic algorithms, fuzzy logic controllers, bioinformatics and neural networks. Fundamental research and application to engineering problems are primary focus of KanGAL.</rdfs:comment>
        <rdfs:label xml:lang="en">KanGAL</rdfs:label>
    </owl:NamedIndividual>
    


    <!-- http://www.semanticweb.org/macoda/ontologies/PMOEA#SingleObjectiveEA -->

    <owl:NamedIndividual rdf:about="http://www.semanticweb.org/macoda/ontologies/PMOEA#SingleObjectiveEA">
        <rdf:type rdf:resource="http://www.semanticweb.org/macoda/ontologies/PMOEA#SOEA"/>
        <rdfs:label xml:lang="en">SingleObjectiveEA</rdfs:label>
    </owl:NamedIndividual>
    


    <!-- http://www.semanticweb.org/macoda/ontologies/PMOEA#LZ09_F1 -->

    <owl:NamedIndividual rdf:about="http://www.semanticweb.org/macoda/ontologies/PMOEA#LZ09_F1">
        <rdf:type rdf:resource="http://www.semanticweb.org/macoda/ontologies/PMOEA#Academic_Problem"/>
        <PMOEA:isContinuousProblem rdf:datatype="http://www.w3.org/2001/XMLSchema#boolean">true</PMOEA:isContinuousProblem>
        <PMOEA:ObjectiveNumber rdf:datatype="http://www.w3.org/2001/XMLSchema#integer">2</PMOEA:ObjectiveNumber>
        <rdfs:label xml:lang="en">LZ09_F1</rdfs:label>
    </owl:NamedIndividual>
    


    <!-- http://www.semanticweb.org/macoda/ontologies/PMOEA#FF -->

    <owl:NamedIndividual rdf:about="http://www.semanticweb.org/macoda/ontologies/PMOEA#FF">
        <rdf:type rdf:resource="http://www.semanticweb.org/macoda/ontologies/PMOEA#Academic_Problem"/>
        <PMOEA:isContinuousProblem rdf:datatype="http://www.w3.org/2001/XMLSchema#boolean">true</PMOEA:isContinuousProblem>
        <PMOEA:ObjectiveNumber rdf:datatype="http://www.w3.org/2001/XMLSchema#integer">2</PMOEA:ObjectiveNumber>
        <rdfs:comment>Fonseca, C.M., Fleming, J.: An overview of evolutionary algorithms in multiobjective
optimization. Evolutionary Computation 3(1), 116 (1995)</rdfs:comment>
        <rdfs:label xml:lang="en">FF</rdfs:label>
    </owl:NamedIndividual>
    


    <!-- http://www.semanticweb.org/macoda/ontologies/PMOEA#DTLZ8_3 -->

    <owl:NamedIndividual rdf:about="http://www.semanticweb.org/macoda/ontologies/PMOEA#DTLZ8_3">
        <rdf:type rdf:resource="http://www.semanticweb.org/macoda/ontologies/PMOEA#DTLZ"/>
        <PMOEA:isContinuousProblem rdf:datatype="http://www.w3.org/2001/XMLSchema#boolean">true</PMOEA:isContinuousProblem>
        <PMOEA:ObjectiveNumber rdf:datatype="http://www.w3.org/2001/XMLSchema#integer">3</PMOEA:ObjectiveNumber>
        <rdfs:label xml:lang="en">DTLZ8_3</rdfs:label>
    </owl:NamedIndividual>
    


    <!-- http://www.semanticweb.org/macoda/ontologies/PMOEA#NoisyBinhProblem -->

    <owl:NamedIndividual rdf:about="http://www.semanticweb.org/macoda/ontologies/PMOEA#NoisyBinhProblem">
        <rdf:type rdf:resource="http://www.semanticweb.org/macoda/ontologies/PMOEA#Academic_Problem"/>
        <PMOEA:isNoisy rdf:datatype="http://www.w3.org/2001/XMLSchema#boolean">true</PMOEA:isNoisy>
        <PMOEA:isContinuousProblem rdf:datatype="http://www.w3.org/2001/XMLSchema#boolean">true</PMOEA:isContinuousProblem>
        <PMOEA:ObjectiveNumber rdf:datatype="http://www.w3.org/2001/XMLSchema#integer">2</PMOEA:ObjectiveNumber>
        <rdfs:label xml:lang="en">NoisyBinhProblem</rdfs:label>
    </owl:NamedIndividual>
    


    <!-- http://www.semanticweb.org/macoda/ontologies/PMOEA#DTLZ9_3 -->

    <owl:NamedIndividual rdf:about="http://www.semanticweb.org/macoda/ontologies/PMOEA#DTLZ9_3">
        <rdf:type rdf:resource="http://www.semanticweb.org/macoda/ontologies/PMOEA#DTLZ"/>
        <rdfs:label xml:lang="en">DTLZ9_3</rdfs:label>
    </owl:NamedIndividual>
    


    <!-- http://www.semanticweb.org/macoda/ontologies/PMOEA#GAlib -->

    <owl:NamedIndividual rdf:about="http://www.semanticweb.org/macoda/ontologies/PMOEA#GAlib">
        <rdf:type rdf:resource="http://www.semanticweb.org/macoda/ontologies/PMOEA#ImplementationLibrary"/>
        <rdfs:comment>GAlib is a set of C++ genetic algorithm objects. The library includes tools for using genetic algorithms to do optimization in any C++ program</rdfs:comment>
        <rdfs:label xml:lang="en">GAlib</rdfs:label>
    </owl:NamedIndividual>
    


    <!-- http://www.semanticweb.org/macoda/ontologies/PMOEA#DTLZ4_7 -->

    <owl:NamedIndividual rdf:about="http://www.semanticweb.org/macoda/ontologies/PMOEA#DTLZ4_7">
        <rdf:type rdf:resource="http://www.semanticweb.org/macoda/ontologies/PMOEA#DTLZ"/>
        <PMOEA:isContinuousProblem rdf:datatype="http://www.w3.org/2001/XMLSchema#boolean">true</PMOEA:isContinuousProblem>
        <PMOEA:ObjectiveNumber rdf:datatype="http://www.w3.org/2001/XMLSchema#integer">7</PMOEA:ObjectiveNumber>
        <PMOEA:isManyObjectiveProblem rdf:datatype="http://www.w3.org/2001/XMLSchema#boolean">true</PMOEA:isManyObjectiveProblem>
        <rdfs:label xml:lang="en">DTLZ4_7</rdfs:label>
    </owl:NamedIndividual>
    


    <!-- http://www.semanticweb.org/macoda/ontologies/PMOEA#TerritorySize -->

    <owl:NamedIndividual rdf:about="http://www.semanticweb.org/macoda/ontologies/PMOEA#TerritorySize">
        <rdf:type rdf:resource="http://www.semanticweb.org/macoda/ontologies/PMOEA#TerritorySize"/>
        <rdfs:comment>Territory size around each archive individual, in TDEA</rdfs:comment>
        <rdfs:label xml:lang="en">TerritorySize</rdfs:label>
    </owl:NamedIndividual>
    


    <!-- http://www.semanticweb.org/macoda/ontologies/PMOEA#Ruben_Saborido -->

    <owl:NamedIndividual rdf:about="http://www.semanticweb.org/macoda/ontologies/PMOEA#Ruben_Saborido">
        <rdf:type rdf:resource="http://www.semanticweb.org/macoda/ontologies/PMOEA#Researcher"/>
        <rdfs:label xml:lang="en">Rubn Saborido</rdfs:label>
    </owl:NamedIndividual>
    


    <!-- http://www.semanticweb.org/macoda/ontologies/PMOEA#PISA -->

    <owl:NamedIndividual rdf:about="http://www.semanticweb.org/macoda/ontologies/PMOEA#PISA">
        <rdfs:comment>PISA is a text-based interface for search algorithms. It splits an optimization process into two modules. One module contains all parts specific to the optimization problem (e.g., evaluation of solutions, problem representation, variation of solutions). The other module contains the parts which are independent of the optimization problem (mainly the selection process). These two modules are implemented as separate programs which communicate through text files.
PISA is a library of ready-to-go modules, namely optimization problems (test and benchmark problems), selection modules (evolutionary multi-objective optimizers) and modules for performance assessment.</rdfs:comment>
        <rdfs:label xml:lang="en">PISA</rdfs:label>
    </owl:NamedIndividual>
    


    <!-- http://www.semanticweb.org/macoda/ontologies/PMOEA#NEMO-0 -->

    <owl:NamedIndividual rdf:about="http://www.semanticweb.org/macoda/ontologies/PMOEA#NEMO-0">
        <rdf:type rdf:resource="http://www.semanticweb.org/macoda/ontologies/PMOEA#PMOEA"/>
        <PMOEA:hasPreferenceModel rdf:resource="http://www.semanticweb.org/macoda/ontologies/PMOEA#GeneralAdditiveUtilityFunction"/>
        <PMOEA:hasPreferenceInformationFromDM rdf:resource="http://www.semanticweb.org/macoda/ontologies/PMOEA#PairwiseComparison"/>
        <PMOEA:hasInteractionTime rdf:resource="http://www.semanticweb.org/macoda/ontologies/PMOEA#progressive"/>
        <PMOEA:hasPreferenceIntegration rdf:resource="http://www.semanticweb.org/macoda/ontologies/PMOEA#CrowdingDistance"/>
        <PMOEA:hasLearningMethod rdf:resource="http://www.semanticweb.org/macoda/ontologies/PMOEA#LinearProgramming"/>
        <PMOEA:canSolve rdf:resource="http://www.semanticweb.org/macoda/ontologies/PMOEA#DTLZ2_4"/>
        <PMOEA:canSolve rdf:resource="http://www.semanticweb.org/macoda/ontologies/PMOEA#ZDT4"/>
        <PMOEA:canSolve rdf:resource="http://www.semanticweb.org/macoda/ontologies/PMOEA#WFG1_5"/>
        <PMOEA:canSolve rdf:resource="http://www.semanticweb.org/macoda/ontologies/PMOEA#DTLZ2_3"/>
        <PMOEA:canSolve rdf:resource="http://www.semanticweb.org/macoda/ontologies/PMOEA#ZDT1"/>
        <PMOEA:hasResultInfluence rdf:resource="http://www.semanticweb.org/macoda/ontologies/PMOEA#BiasedDistribution"/>
        <PMOEA:hasAuthor rdf:resource="http://www.semanticweb.org/macoda/ontologies/PMOEA#Piotr_Zielniewicz"/>
        <PMOEA:hasAuthor rdf:resource="http://www.semanticweb.org/macoda/ontologies/PMOEA#Salvatore_Greco
"/>
        <PMOEA:hasAuthor rdf:resource="http://www.semanticweb.org/macoda/ontologies/PMOEA#Juergen_Branke"/>
        <PMOEA:hasAuthor rdf:resource="http://www.semanticweb.org/macoda/ontologies/PMOEA#Roman_Sowinski"/>
        <PMOEA:isExtensionOf rdf:resource="http://www.semanticweb.org/macoda/ontologies/PMOEA#NEMO-II"/>
        <PMOEA:hasSearchAlgorithm rdf:resource="http://www.semanticweb.org/macoda/ontologies/PMOEA#NSGA-II"/>
        <PMOEA:hasDevelopingYear rdf:datatype="http://www.w3.org/2001/XMLSchema#integer">2015</PMOEA:hasDevelopingYear>
        <PMOEA:ParetoDominancePreservation rdf:datatype="http://www.w3.org/2001/XMLSchema#boolean">true</PMOEA:ParetoDominancePreservation>
        <PMOEA:hasReference>Branke, J., S. Greco, R. Slowinski and P. Zielniewicz (2015). &quot;Learning value functions in interactive evolutionary multiobjective optimization.&quot; Evolutionary Computation, IEEE Transactions on 19(1): 88-102</PMOEA:hasReference>
        <rdfs:comment>A single compatible value function is used to rank solutions in the population. Note that there is usually more than one compatible value function, so the question arises which one to pick(3 methods :MDVF,MSCVF,MSVF are used). Then the representative value function replaces the crowding distance in NSGA-II</rdfs:comment>
        <rdfs:label xml:lang="en">NEMO-0</rdfs:label>
    </owl:NamedIndividual>
    


    <!-- http://www.semanticweb.org/macoda/ontologies/PMOEA#Ricardo_Landa -->

    <owl:NamedIndividual rdf:about="http://www.semanticweb.org/macoda/ontologies/PMOEA#Ricardo_Landa">
        <rdf:type rdf:resource="http://www.semanticweb.org/macoda/ontologies/PMOEA#Researcher"/>
        <rdfs:label xml:lang="en">Ricardo Landa</rdfs:label>
    </owl:NamedIndividual>
    


    <!-- http://www.semanticweb.org/macoda/ontologies/PMOEA#IEM-CO -->

    <owl:NamedIndividual rdf:about="http://www.semanticweb.org/macoda/ontologies/PMOEA#IEM-CO">
        <rdf:type rdf:resource="http://www.semanticweb.org/macoda/ontologies/PMOEA#PMOEA"/>
        <PMOEA:hasPreferenceModel rdf:resource="http://www.semanticweb.org/macoda/ontologies/PMOEA#LinearUtilityFunction"/>
        <PMOEA:hasPreferenceInformationFromDM rdf:resource="http://www.semanticweb.org/macoda/ontologies/PMOEA#PairwiseComparison"/>
        <PMOEA:hasInteractionTime rdf:resource="http://www.semanticweb.org/macoda/ontologies/PMOEA#progressive"/>
        <PMOEA:hasPreferenceIntegration rdf:resource="http://www.semanticweb.org/macoda/ontologies/PMOEA#FrontSorting"/>
        <PMOEA:hasLearningMethod rdf:resource="http://www.semanticweb.org/macoda/ontologies/PMOEA#LinearProgramming"/>
        <PMOEA:canSolve rdf:resource="http://www.semanticweb.org/macoda/ontologies/PMOEA#Knapsack_2"/>
        <PMOEA:canSolve rdf:resource="http://www.semanticweb.org/macoda/ontologies/PMOEA#SpanningTree_3"/>
        <PMOEA:canSolve rdf:resource="http://www.semanticweb.org/macoda/ontologies/PMOEA#Knapsack_4"/>
        <PMOEA:canSolve rdf:resource="http://www.semanticweb.org/macoda/ontologies/PMOEA#SpanningTree_4"/>
        <PMOEA:canSolve rdf:resource="http://www.semanticweb.org/macoda/ontologies/PMOEA#Knapsack_3"/>
        <PMOEA:canSolve rdf:resource="http://www.semanticweb.org/macoda/ontologies/PMOEA#SpanningTree_2"/>
        <PMOEA:hasResultInfluence rdf:resource="http://www.semanticweb.org/macoda/ontologies/PMOEA#OneSolution"/>
        <PMOEA:hasAuthor rdf:resource="http://www.semanticweb.org/macoda/ontologies/PMOEA#Murat_Koeksalan"/>
        <PMOEA:hasAuthor rdf:resource="http://www.semanticweb.org/macoda/ontologies/PMOEA#Selcen_Phelps"/>
        <PMOEA:hasSearchAlgorithm rdf:resource="http://www.semanticweb.org/macoda/ontologies/PMOEA#GeneralMOEA"/>
        <PMOEA:hasDevelopingYear rdf:datatype="http://www.w3.org/2001/XMLSchema#integer">2003</PMOEA:hasDevelopingYear>
        <PMOEA:hasReference>S. P. Phelps and M. Koksalan, An interactive evolutionary metaheuristic
for multiobjective combinatorial optimization, Management Science,
vol. 49, no. 12, pp. 17261738, 2003.</PMOEA:hasReference>
        <rdfs:comment>It proposed an interactive evolutionary algorithm that periodically asks the DM to rank pairs of solutions. Assuming a linear model, these preferences are turned into constraints for possible weights. The method determines the most discriminating (in the sense of MDVF) linear value function compatible with the preference information by solving a LP. The resulting value function is then used for ranking individuals in the evolutionary algorithm that works as a single objective evolutionary algorithm between user interactions</rdfs:comment>
        <rdfs:label xml:lang="en">IEM-CO</rdfs:label>
    </owl:NamedIndividual>
    


    <!-- http://www.semanticweb.org/macoda/ontologies/PMOEA#Eun-Soo_Kim -->

    <owl:NamedIndividual rdf:about="http://www.semanticweb.org/macoda/ontologies/PMOEA#Eun-Soo_Kim">
        <rdf:type rdf:resource="http://www.semanticweb.org/macoda/ontologies/PMOEA#Researcher"/>
        <rdfs:label xml:lang="en">Eun-Soo Kim</rdfs:label>
    </owl:NamedIndividual>
    


    <!-- http://www.semanticweb.org/macoda/ontologies/PMOEA#KR-NSGA-II -->

    <owl:NamedIndividual rdf:about="http://www.semanticweb.org/macoda/ontologies/PMOEA#KR-NSGA-II">
        <rdf:type rdf:resource="http://www.semanticweb.org/macoda/ontologies/PMOEA#PMOEA"/>
        <PMOEA:hasPreferenceModel rdf:resource="http://www.semanticweb.org/macoda/ontologies/PMOEA#Knee-point"/>
        <PMOEA:hasInteractionTime rdf:resource="http://www.semanticweb.org/macoda/ontologies/PMOEA#a-priori"/>
        <PMOEA:hasInteractionTime rdf:resource="http://www.semanticweb.org/macoda/ontologies/PMOEA#progressive"/>
        <PMOEA:hasPreferenceIntegration rdf:resource="http://www.semanticweb.org/macoda/ontologies/PMOEA#CrowdingDistance"/>
        <PMOEA:canSolve rdf:resource="http://www.semanticweb.org/macoda/ontologies/PMOEA#DO2DK"/>
        <PMOEA:canSolve rdf:resource="http://www.semanticweb.org/macoda/ontologies/PMOEA#DEB2DK"/>
        <PMOEA:canSolve rdf:resource="http://www.semanticweb.org/macoda/ontologies/PMOEA#DEB3DK"/>
        <PMOEA:hasResultInfluence rdf:resource="http://www.semanticweb.org/macoda/ontologies/PMOEA#BiasedDistribution"/>
        <PMOEA:hasAuthor rdf:resource="http://www.semanticweb.org/macoda/ontologies/PMOEA#Slim_Bechikh"/>
        <PMOEA:hasAuthor rdf:resource="http://www.semanticweb.org/macoda/ontologies/PMOEA#Lamjed_Ben_Said,"/>
        <PMOEA:isExtensionOf rdf:resource="http://www.semanticweb.org/macoda/ontologies/PMOEA#R-NSGA-II"/>
        <PMOEA:hasSearchAlgorithm rdf:resource="http://www.semanticweb.org/macoda/ontologies/PMOEA#NSGA-II"/>
        <PMOEA:hasImplementationLanguage rdf:resource="http://www.semanticweb.org/macoda/ontologies/PMOEA#Matlab"/>
        <PMOEA:MultipleRegionOfInterest rdf:datatype="http://www.w3.org/2001/XMLSchema#boolean">true</PMOEA:MultipleRegionOfInterest>
        <PMOEA:SpreadControl rdf:datatype="http://www.w3.org/2001/XMLSchema#boolean">true</PMOEA:SpreadControl>
        <PMOEA:ParetoDominancePreservation rdf:datatype="http://www.w3.org/2001/XMLSchema#boolean">true</PMOEA:ParetoDominancePreservation>
        <PMOEA:hasReference>Bechikh, Slim, Lamjed Ben Said, and Khaled Ghdira. &quot;Searching for knee regions in multi-objective optimization using mobile reference points.&quot; Proceedings of the 2010 ACM symposium on applied computing. ACM, 2010.</PMOEA:hasReference>
        <rdfs:comment>KR-NSGA-II is an extension of R-NSGA-II which uses knee points as reference points</rdfs:comment>
        <rdfs:label xml:lang="en">KR-NSGA-II</rdfs:label>
    </owl:NamedIndividual>
    


    <!-- http://www.semanticweb.org/macoda/ontologies/PMOEA#GeneralAdditiveUtilityFunction -->

    <owl:NamedIndividual rdf:about="http://www.semanticweb.org/macoda/ontologies/PMOEA#GeneralAdditiveUtilityFunction">
        <rdf:type rdf:resource="http://www.semanticweb.org/macoda/ontologies/PMOEA#GeneralAdditive"/>
        <rdfs:label xml:lang="en">GeneralAdditiveUtilityFunction</rdfs:label>
    </owl:NamedIndividual>
    


    <!-- http://www.semanticweb.org/macoda/ontologies/PMOEA#Kalyanmoy_Deb -->

    <owl:NamedIndividual rdf:about="http://www.semanticweb.org/macoda/ontologies/PMOEA#Kalyanmoy_Deb">
        <rdf:type rdf:resource="http://www.semanticweb.org/macoda/ontologies/PMOEA#Researcher"/>
        <rdfs:label xml:lang="en">Kalyanmoy Deb</rdfs:label>
    </owl:NamedIndividual>
    


    <!-- http://www.semanticweb.org/macoda/ontologies/PMOEA#Jong-Hwan_Kim -->

    <owl:NamedIndividual rdf:about="http://www.semanticweb.org/macoda/ontologies/PMOEA#Jong-Hwan_Kim">
        <rdf:type rdf:resource="http://www.semanticweb.org/macoda/ontologies/PMOEA#Researcher"/>
        <rdfs:label xml:lang="en">Jong-Hwan Kim</rdfs:label>
    </owl:NamedIndividual>
    


    <!-- http://www.semanticweb.org/macoda/ontologies/PMOEA#TurningOptimizationProblem -->

    <owl:NamedIndividual rdf:about="http://www.semanticweb.org/macoda/ontologies/PMOEA#TurningOptimizationProblem">
        <rdf:type rdf:resource="http://www.semanticweb.org/macoda/ontologies/PMOEA#Realworld_Problem"/>
        <PMOEA:isContinuousProblem rdf:datatype="http://www.w3.org/2001/XMLSchema#boolean">true</PMOEA:isContinuousProblem>
        <PMOEA:ObjectiveNumber rdf:datatype="http://www.w3.org/2001/XMLSchema#integer">5</PMOEA:ObjectiveNumber>
        <PMOEA:isManyObjectiveProblem rdf:datatype="http://www.w3.org/2001/XMLSchema#boolean">true</PMOEA:isManyObjectiveProblem>
        <rdfs:label xml:lang="en">TurningOptimizationProblem</rdfs:label>
    </owl:NamedIndividual>
    


    <!-- http://www.semanticweb.org/macoda/ontologies/PMOEA#PI-EMO-VF -->

    <owl:NamedIndividual rdf:about="http://www.semanticweb.org/macoda/ontologies/PMOEA#PI-EMO-VF">
        <rdf:type rdf:resource="http://www.semanticweb.org/macoda/ontologies/PMOEA#PMOEA"/>
        <PMOEA:hasPreferenceModel rdf:resource="http://www.semanticweb.org/macoda/ontologies/PMOEA#StrictlyIncreasingPolynomialValueFunction"/>
        <PMOEA:hasPreferenceInformationFromDM rdf:resource="http://www.semanticweb.org/macoda/ontologies/PMOEA#RankSamples"/>
        <PMOEA:hasInteractionTime rdf:resource="http://www.semanticweb.org/macoda/ontologies/PMOEA#progressive"/>
        <PMOEA:hasPreferenceIntegration rdf:resource="http://www.semanticweb.org/macoda/ontologies/PMOEA#ValueFunction-dominance"/>
        <PMOEA:hasPreferenceIntegration rdf:resource="http://www.semanticweb.org/macoda/ontologies/PMOEA#LocalSearch-basedTerminationCriterion"/>
        <PMOEA:hasLearningMethod rdf:resource="http://www.semanticweb.org/macoda/ontologies/PMOEA#SequentialQuadraticProgramming"/>
        <PMOEA:canSolve rdf:resource="http://www.semanticweb.org/macoda/ontologies/PMOEA#DTLZ2_5"/>
        <PMOEA:canSolve rdf:resource="http://www.semanticweb.org/macoda/ontologies/PMOEA#DTLZ2_3"/>
        <PMOEA:canSolve rdf:resource="http://www.semanticweb.org/macoda/ontologies/PMOEA#ZDT1"/>
        <PMOEA:hasResultInfluence rdf:resource="http://www.semanticweb.org/macoda/ontologies/PMOEA#OneSolution"/>
        <PMOEA:hasAuthor rdf:resource="http://www.semanticweb.org/macoda/ontologies/PMOEA#Ankur_Sinha"/>
        <PMOEA:hasAuthor rdf:resource="http://www.semanticweb.org/macoda/ontologies/PMOEA#Jyrki_Wallenius"/>
        <PMOEA:hasAuthor rdf:resource="http://www.semanticweb.org/macoda/ontologies/PMOEA#Kalyanmoy_Deb"/>
        <PMOEA:hasAuthor rdf:resource="http://www.semanticweb.org/macoda/ontologies/PMOEA#Pekka_J._Korhonen"/>
        <PMOEA:hasSearchAlgorithm rdf:resource="http://www.semanticweb.org/macoda/ontologies/PMOEA#NSGA-II"/>
        <PMOEA:hasDevelopingYear rdf:datatype="http://www.w3.org/2001/XMLSchema#integer">2010</PMOEA:hasDevelopingYear>
        <PMOEA:ParetoDominancePreservation rdf:datatype="http://www.w3.org/2001/XMLSchema#boolean">true</PMOEA:ParetoDominancePreservation>
        <PMOEA:hasReference>Deb, K., A. Sinha, P. J. Korhonen and J. Wallenius (2010). &quot;An interactive evolutionary multiobjective optimization method based on progressively approximated value functions.&quot; Evolutionary Computation, IEEE Transactions on 14(5): 723-739</PMOEA:hasReference>
        <rdfs:comment>The DM is asked to order a given set of alternatives from best to worst. This preference information is then used to model a strictly increasing polynomial value function. The construction procedure involves solving a single-objective optimization problem to determine the optimal parameters of the value function. This constructed value function is then utilized to redefine the dominance principle, and drive the EMO approach (NSGA-II is applied) to search for preferred solutions for the subsequent iterations until the next DM call. In addition, this value function is also used to build a preference based termination criterion</rdfs:comment>
        <rdfs:label xml:lang="en">PI-EMO-VF</rdfs:label>
    </owl:NamedIndividual>
    


    <!-- http://www.semanticweb.org/macoda/ontologies/PMOEA#MOEAFramework -->

    <owl:NamedIndividual rdf:about="http://www.semanticweb.org/macoda/ontologies/PMOEA#MOEAFramework">
        <PMOEA:hasLibraryDescription>he MOEA Framework is a free and open source Java library for developing and experimenting with multiobjective evolutionary algorithms (MOEAs) and other general-purpose multiobjective optimization algorithms. The MOEA Framework supports genetic algorithms, differential evolution, particle swarm optimization, genetic programming, grammatical evolution, and more. A number of algorithms are provided out-of-the-box, including NSGA-II, NSGA-III, -MOEA, GDE3, PAES, PESA2, SPEA2, IBEA, SMS-EMOA, SMPSO, OMOPSO, CMA-ES, and MOEA/D. In addition, the MOEA Framework provides the tools necessary to rapidly design, develop, execute and statistically test optimization algorithms.</PMOEA:hasLibraryDescription>
        <rdfs:label xml:lang="en">MOEAFramework</rdfs:label>
    </owl:NamedIndividual>
    


    <!-- http://www.semanticweb.org/macoda/ontologies/PMOEA#Eckart_Zitzler -->

    <owl:NamedIndividual rdf:about="http://www.semanticweb.org/macoda/ontologies/PMOEA#Eckart_Zitzler">
        <rdf:type rdf:resource="http://www.semanticweb.org/macoda/ontologies/PMOEA#Researcher"/>
        <rdfs:label xml:lang="en">Eckart Zitzler</rdfs:label>
    </owl:NamedIndividual>
    


    <!-- http://www.semanticweb.org/macoda/ontologies/PMOEA#PegasusGasTurbinEngineOptimization -->

    <owl:NamedIndividual rdf:about="http://www.semanticweb.org/macoda/ontologies/PMOEA#PegasusGasTurbinEngineOptimization">
        <rdf:type rdf:resource="http://www.semanticweb.org/macoda/ontologies/PMOEA#Realworld_Problem"/>
        <PMOEA:isContinuousProblem rdf:datatype="http://www.w3.org/2001/XMLSchema#boolean">true</PMOEA:isContinuousProblem>
        <PMOEA:ObjectiveNumber rdf:datatype="http://www.w3.org/2001/XMLSchema#integer">4</PMOEA:ObjectiveNumber>
        <PMOEA:hasReference>Hancock,S.D.(1992).Gas Turbine Engine Controller Design Using Multi-Objective Optimization Techniques. PhD thesis, University of Wales, Bangor,UK</PMOEA:hasReference>
        <PMOEA:isManyObjectiveProblem rdf:datatype="http://www.w3.org/2001/XMLSchema#boolean">true</PMOEA:isManyObjectiveProblem>
        <rdfs:label xml:lang="en">PegasusGasTurbinEngineOptimization</rdfs:label>
    </owl:NamedIndividual>
    


    <!-- http://www.semanticweb.org/macoda/ontologies/PMOEA#SpanningTree_2 -->

    <owl:NamedIndividual rdf:about="http://www.semanticweb.org/macoda/ontologies/PMOEA#SpanningTree_2">
        <rdf:type rdf:resource="http://www.semanticweb.org/macoda/ontologies/PMOEA#Academic_Problem"/>
        <PMOEA:isDiscreteProblem rdf:datatype="http://www.w3.org/2001/XMLSchema#boolean">true</PMOEA:isDiscreteProblem>
        <PMOEA:ObjectiveNumber rdf:datatype="http://www.w3.org/2001/XMLSchema#integer">2</PMOEA:ObjectiveNumber>
        <rdfs:label xml:lang="en">SpanningTree_2</rdfs:label>
    </owl:NamedIndividual>
    


    <!-- http://www.semanticweb.org/macoda/ontologies/PMOEA#linguisticComparisonOnObjectives -->

    <owl:NamedIndividual rdf:about="http://www.semanticweb.org/macoda/ontologies/PMOEA#linguisticComparisonOnObjectives">
        <rdf:type rdf:resource="http://www.semanticweb.org/macoda/ontologies/PMOEA#ObjectiveComparison"/>
        <rdfs:comment>objective f2 is {much more important, more important, less important,equally important,don&apos;t care} than objective f1.</rdfs:comment>
        <rdfs:label xml:lang="en">linguisticComparisonOnObjectives</rdfs:label>
    </owl:NamedIndividual>
    


    <!-- http://www.semanticweb.org/macoda/ontologies/PMOEA#Dirac-typeFunction -->

    <owl:NamedIndividual rdf:about="http://www.semanticweb.org/macoda/ontologies/PMOEA#Dirac-typeFunction">
        <rdf:type rdf:resource="http://www.semanticweb.org/macoda/ontologies/PMOEA#DistributionFunctionInObjectiveSpace"/>
        <rdfs:label xml:lang="en">Dirac-typeFunction</rdfs:label>
    </owl:NamedIndividual>
    


    <!-- http://www.semanticweb.org/macoda/ontologies/PMOEA#MOEA-D -->

    <owl:NamedIndividual rdf:about="http://www.semanticweb.org/macoda/ontologies/PMOEA#MOEA-D">
        <rdf:type rdf:resource="http://www.semanticweb.org/macoda/ontologies/PMOEA#Decomposition_based"/>
        <rdfs:label xml:lang="en">MOEA/D</rdfs:label>
    </owl:NamedIndividual>
    


    <!-- http://www.semanticweb.org/macoda/ontologies/PMOEA#WFG4_2 -->

    <owl:NamedIndividual rdf:about="http://www.semanticweb.org/macoda/ontologies/PMOEA#WFG4_2">
        <rdf:type rdf:resource="http://www.semanticweb.org/macoda/ontologies/PMOEA#WFG"/>
        <PMOEA:OWLDataProperty_61d3cd95_fde4_4c1b_af08_1eaf73473aea rdf:datatype="http://www.w3.org/2001/XMLSchema#boolean">true</PMOEA:OWLDataProperty_61d3cd95_fde4_4c1b_af08_1eaf73473aea>
        <PMOEA:isContinuousProblem rdf:datatype="http://www.w3.org/2001/XMLSchema#boolean">true</PMOEA:isContinuousProblem>
        <PMOEA:ObjectiveNumber rdf:datatype="http://www.w3.org/2001/XMLSchema#integer">2</PMOEA:ObjectiveNumber>
        <rdfs:label xml:lang="en">WFG4_2</rdfs:label>
    </owl:NamedIndividual>
    


    <!-- http://www.semanticweb.org/macoda/ontologies/PMOEA#DENT -->

    <owl:NamedIndividual rdf:about="http://www.semanticweb.org/macoda/ontologies/PMOEA#DENT">
        <rdf:type rdf:resource="http://www.semanticweb.org/macoda/ontologies/PMOEA#Academic_Problem"/>
        <PMOEA:isContinuousProblem rdf:datatype="http://www.w3.org/2001/XMLSchema#boolean">true</PMOEA:isContinuousProblem>
        <PMOEA:ObjectiveNumber rdf:datatype="http://www.w3.org/2001/XMLSchema#integer">2</PMOEA:ObjectiveNumber>
        <rdfs:label xml:lang="en">DENT</rdfs:label>
    </owl:NamedIndividual>
    


    <!-- http://www.semanticweb.org/macoda/ontologies/PMOEA#Knee-point -->

    <owl:NamedIndividual rdf:about="http://www.semanticweb.org/macoda/ontologies/PMOEA#Knee-point">
        <rdf:type rdf:resource="http://www.semanticweb.org/macoda/ontologies/PMOEA#KneePoint"/>
        <rdfs:comment>This model means when no explicit DM preference is provided, the knee point is considered to be most preferred.</rdfs:comment>
        <rdfs:label xml:lang="en">Knee-point</rdfs:label>
    </owl:NamedIndividual>
    


    <!-- http://www.semanticweb.org/macoda/ontologies/PMOEA#Schaffers_f2_Function -->

    <owl:NamedIndividual rdf:about="http://www.semanticweb.org/macoda/ontologies/PMOEA#Schaffers_f2_Function">
        <rdf:type rdf:resource="http://www.semanticweb.org/macoda/ontologies/PMOEA#Academic_Problem"/>
        <PMOEA:isContinuousProblem rdf:datatype="http://www.w3.org/2001/XMLSchema#boolean">true</PMOEA:isContinuousProblem>
        <PMOEA:ObjectiveNumber rdf:datatype="http://www.w3.org/2001/XMLSchema#integer">2</PMOEA:ObjectiveNumber>
        <rdfs:label xml:lang="en">Schaffer&apos;s_f2_Function</rdfs:label>
    </owl:NamedIndividual>
    


    <!-- http://www.semanticweb.org/macoda/ontologies/PMOEA#BrushingPreferenceRegionInObjectiveSpace -->

    <owl:NamedIndividual rdf:about="http://www.semanticweb.org/macoda/ontologies/PMOEA#BrushingPreferenceRegionInObjectiveSpace">
        <rdf:type rdf:resource="http://www.semanticweb.org/macoda/ontologies/PMOEA#PreferenceRegion"/>
        <rdfs:label xml:lang="en">BrushingPreferenceRegionInObjectiveSpace</rdfs:label>
    </owl:NamedIndividual>
    


    <!-- http://www.semanticweb.org/macoda/ontologies/PMOEA#COGA -->

    <owl:NamedIndividual rdf:about="http://www.semanticweb.org/macoda/ontologies/PMOEA#COGA">
        <rdf:type rdf:resource="http://www.semanticweb.org/macoda/ontologies/PMOEA#Coevolution_based"/>
        <PMOEA:hasReference>I. C. Parmee and A. H. Watson, Preliminary airframe design using
co-evolutionary multiobjective genetic algorithms, in GECCO-99:
Proceedings of the Genetic and Evolutionary Computation Conference,
W. Banzhaf and J. Daida, Eds. San Mateo, CA: Morgan Kaufmann,
1999, pp. 16571665.</PMOEA:hasReference>
        <rdfs:label xml:lang="en">COGA</rdfs:label>
    </owl:NamedIndividual>
    


    <!-- http://www.semanticweb.org/macoda/ontologies/PMOEA#DTLZ3_2 -->

    <owl:NamedIndividual rdf:about="http://www.semanticweb.org/macoda/ontologies/PMOEA#DTLZ3_2">
        <rdf:type rdf:resource="http://www.semanticweb.org/macoda/ontologies/PMOEA#DTLZ"/>
        <PMOEA:OWLDataProperty_61d3cd95_fde4_4c1b_af08_1eaf73473aea rdf:datatype="http://www.w3.org/2001/XMLSchema#boolean">true</PMOEA:OWLDataProperty_61d3cd95_fde4_4c1b_af08_1eaf73473aea>
        <PMOEA:isContinuousProblem rdf:datatype="http://www.w3.org/2001/XMLSchema#boolean">true</PMOEA:isContinuousProblem>
        <PMOEA:ObjectiveNumber rdf:datatype="http://www.w3.org/2001/XMLSchema#integer">2</PMOEA:ObjectiveNumber>
        <rdfs:label xml:lang="en">DTLZ3_2</rdfs:label>
    </owl:NamedIndividual>
    


    <!-- http://www.semanticweb.org/macoda/ontologies/PMOEA#NSGA-II -->

    <owl:NamedIndividual rdf:about="http://www.semanticweb.org/macoda/ontologies/PMOEA#NSGA-II">
        <rdf:type rdf:resource="http://www.semanticweb.org/macoda/ontologies/PMOEA#DiversityVSConvergence_based"/>
        <rdfs:label xml:lang="en">NSGA-II</rdfs:label>
    </owl:NamedIndividual>
    


    <!-- http://www.semanticweb.org/macoda/ontologies/PMOEA#WFG9_8 -->

    <owl:NamedIndividual rdf:about="http://www.semanticweb.org/macoda/ontologies/PMOEA#WFG9_8">
        <rdf:type rdf:resource="http://www.semanticweb.org/macoda/ontologies/PMOEA#WFG"/>
        <PMOEA:OWLDataProperty_61d3cd95_fde4_4c1b_af08_1eaf73473aea rdf:datatype="http://www.w3.org/2001/XMLSchema#boolean">true</PMOEA:OWLDataProperty_61d3cd95_fde4_4c1b_af08_1eaf73473aea>
        <PMOEA:isContinuousProblem rdf:datatype="http://www.w3.org/2001/XMLSchema#boolean">true</PMOEA:isContinuousProblem>
        <PMOEA:ObjectiveNumber rdf:datatype="http://www.w3.org/2001/XMLSchema#integer">8</PMOEA:ObjectiveNumber>
        <PMOEA:isManyObjectiveProblem rdf:datatype="http://www.w3.org/2001/XMLSchema#boolean">true</PMOEA:isManyObjectiveProblem>
        <rdfs:label xml:lang="en">WFG9_8</rdfs:label>
    </owl:NamedIndividual>
    


    <!-- http://www.semanticweb.org/macoda/ontologies/PMOEA#HypE -->

    <owl:NamedIndividual rdf:about="http://www.semanticweb.org/macoda/ontologies/PMOEA#HypE">
        <rdf:type rdf:resource="http://www.semanticweb.org/macoda/ontologies/PMOEA#Indicator_based"/>
        <rdfs:label xml:lang="en">HypE</rdfs:label>
    </owl:NamedIndividual>
    


    <!-- http://www.semanticweb.org/macoda/ontologies/PMOEA#iWASF-GA -->

    <owl:NamedIndividual rdf:about="http://www.semanticweb.org/macoda/ontologies/PMOEA#iWASF-GA">
        <rdf:type rdf:resource="http://www.semanticweb.org/macoda/ontologies/PMOEA#PMOEA"/>
        <PMOEA:hasPreferenceModel rdf:resource="http://www.semanticweb.org/macoda/ontologies/PMOEA#WierzbickiASF"/>
        <PMOEA:hasPreferenceInformationFromDM rdf:resource="http://www.semanticweb.org/macoda/ontologies/PMOEA#NumberofSolutions"/>
        <PMOEA:hasPreferenceInformationFromDM rdf:resource="http://www.semanticweb.org/macoda/ontologies/PMOEA#ReferencePoint"/>
        <PMOEA:hasInteractionTime rdf:resource="http://www.semanticweb.org/macoda/ontologies/PMOEA#progressive"/>
        <PMOEA:hasPreferenceIntegration rdf:resource="http://www.semanticweb.org/macoda/ontologies/PMOEA#FrontSorting"/>
        <PMOEA:hasComparison rdf:resource="http://www.semanticweb.org/macoda/ontologies/PMOEA#iMOEA/D"/>
        <PMOEA:hasComparison rdf:resource="http://www.semanticweb.org/macoda/ontologies/PMOEA#PIE"/>
        <PMOEA:hasComparison rdf:resource="http://www.semanticweb.org/macoda/ontologies/PMOEA#iPICEA-G"/>
        <PMOEA:hasComparison rdf:resource="http://www.semanticweb.org/macoda/ontologies/PMOEA#PBEA"/>
        <PMOEA:hasComparison rdf:resource="http://www.semanticweb.org/macoda/ontologies/PMOEA#R-NSGA-II"/>
        <PMOEA:canSolve rdf:resource="http://www.semanticweb.org/macoda/ontologies/PMOEA#DTLZ2_5"/>
        <PMOEA:hasResultInfluence rdf:resource="http://www.semanticweb.org/macoda/ontologies/PMOEA#BoundedRegion"/>
        <PMOEA:hasAuthor rdf:resource="http://www.semanticweb.org/macoda/ontologies/PMOEA#Ana_Beln_Ruiz"/>
        <PMOEA:hasAuthor rdf:resource="http://www.semanticweb.org/macoda/ontologies/PMOEA#Kaisa_Miettinen"/>
        <PMOEA:hasAuthor rdf:resource="http://www.semanticweb.org/macoda/ontologies/PMOEA#Mariano_Luque"/>
        <PMOEA:hasAuthor rdf:resource="http://www.semanticweb.org/macoda/ontologies/PMOEA#Ruben_Saborido"/>
        <PMOEA:useLibrary rdf:resource="http://www.semanticweb.org/macoda/ontologies/PMOEA#jMetal"/>
        <PMOEA:hasSearchAlgorithm rdf:resource="http://www.semanticweb.org/macoda/ontologies/PMOEA#GeneralMOEA"/>
        <PMOEA:hasImplementationLanguage rdf:resource="http://www.semanticweb.org/macoda/ontologies/PMOEA#Java"/>
        <PMOEA:hasDevelopingYear rdf:datatype="http://www.w3.org/2001/XMLSchema#integer">2015</PMOEA:hasDevelopingYear>
        <PMOEA:ParetoDominancePreservation rdf:datatype="http://www.w3.org/2001/XMLSchema#boolean">true</PMOEA:ParetoDominancePreservation>
        <PMOEA:hasReference>Ruiz, A. B., M. Luque, K. Miettinen and R. Saborido (2015). An Interactive Evolutionary Multiobjective Optimization Method: Interactive WASF-GA. Evolutionary Multi-Criterion Optimization, Springer</PMOEA:hasReference>
        <rdfs:comment>interactive version of WASF-GA</rdfs:comment>
        <rdfs:label xml:lang="en">iWASF-GA</rdfs:label>
    </owl:NamedIndividual>
    


    <!-- http://www.semanticweb.org/macoda/ontologies/PMOEA#DTLZ7_2 -->

    <owl:NamedIndividual rdf:about="http://www.semanticweb.org/macoda/ontologies/PMOEA#DTLZ7_2">
        <rdf:type rdf:resource="http://www.semanticweb.org/macoda/ontologies/PMOEA#DTLZ"/>
        <PMOEA:isContinuousProblem rdf:datatype="http://www.w3.org/2001/XMLSchema#boolean">true</PMOEA:isContinuousProblem>
        <PMOEA:ObjectiveNumber rdf:datatype="http://www.w3.org/2001/XMLSchema#integer">2</PMOEA:ObjectiveNumber>
        <rdfs:label xml:lang="en">DTLZ7_2</rdfs:label>
    </owl:NamedIndividual>
    


    <!-- http://www.semanticweb.org/macoda/ontologies/PMOEA#NecessaryPreferenceRelation -->

    <owl:NamedIndividual rdf:about="http://www.semanticweb.org/macoda/ontologies/PMOEA#NecessaryPreferenceRelation">
        <rdf:type rdf:resource="http://www.semanticweb.org/macoda/ontologies/PMOEA#DominanceRelation"/>
        <rdfs:comment>x &gt;N y, if and only if x is at least as good as y according to all instances of the preference model compatible with the preference information</rdfs:comment>
        <rdfs:label xml:lang="en">NecessaryPreferenceRelation</rdfs:label>
    </owl:NamedIndividual>
    


    <!-- http://www.semanticweb.org/macoda/ontologies/PMOEA#ZDT1 -->

    <owl:NamedIndividual rdf:about="http://www.semanticweb.org/macoda/ontologies/PMOEA#ZDT1">
        <rdf:type rdf:resource="http://www.semanticweb.org/macoda/ontologies/PMOEA#ZDT"/>
        <PMOEA:isDiscreteProblem rdf:datatype="http://www.w3.org/2001/XMLSchema#boolean">false</PMOEA:isDiscreteProblem>
        <PMOEA:OWLDataProperty_61d3cd95_fde4_4c1b_af08_1eaf73473aea rdf:datatype="http://www.w3.org/2001/XMLSchema#boolean">false</PMOEA:OWLDataProperty_61d3cd95_fde4_4c1b_af08_1eaf73473aea>
        <PMOEA:isContinuousProblem rdf:datatype="http://www.w3.org/2001/XMLSchema#boolean">true</PMOEA:isContinuousProblem>
        <PMOEA:ObjectiveNumber rdf:datatype="http://www.w3.org/2001/XMLSchema#integer">2</PMOEA:ObjectiveNumber>
        <PMOEA:isManyObjectiveProblem rdf:datatype="http://www.w3.org/2001/XMLSchema#boolean">false</PMOEA:isManyObjectiveProblem>
        <rdfs:label xml:lang="en">ZDT1</rdfs:label>
    </owl:NamedIndividual>
    


    <!-- http://www.semanticweb.org/macoda/ontologies/PMOEA#Tobias_Friedrich -->

    <owl:NamedIndividual rdf:about="http://www.semanticweb.org/macoda/ontologies/PMOEA#Tobias_Friedrich">
        <rdf:type rdf:resource="http://www.semanticweb.org/macoda/ontologies/PMOEA#Researcher"/>
        <rdfs:label xml:lang="en">Tobias Friedrich</rdfs:label>
    </owl:NamedIndividual>
    


    <!-- http://www.semanticweb.org/macoda/ontologies/PMOEA#Knapsack_8 -->

    <owl:NamedIndividual rdf:about="http://www.semanticweb.org/macoda/ontologies/PMOEA#Knapsack_8">
        <rdf:type rdf:resource="http://www.semanticweb.org/macoda/ontologies/PMOEA#Knapsack"/>
        <PMOEA:isDiscreteProblem rdf:datatype="http://www.w3.org/2001/XMLSchema#boolean">true</PMOEA:isDiscreteProblem>
        <PMOEA:ObjectiveNumber rdf:datatype="http://www.w3.org/2001/XMLSchema#integer">8</PMOEA:ObjectiveNumber>
        <PMOEA:isManyObjectiveProblem rdf:datatype="http://www.w3.org/2001/XMLSchema#boolean">true</PMOEA:isManyObjectiveProblem>
        <rdfs:label xml:lang="en">Knapsack_8</rdfs:label>
    </owl:NamedIndividual>
    


    <!-- http://www.semanticweb.org/macoda/ontologies/PMOEA#C-Sharp -->

    <owl:NamedIndividual rdf:about="http://www.semanticweb.org/macoda/ontologies/PMOEA#C-Sharp">
        <rdf:type rdf:resource="http://www.semanticweb.org/macoda/ontologies/PMOEA#ProgrammingLanguage"/>
        <rdfs:label xml:lang="en">C#</rdfs:label>
    </owl:NamedIndividual>
    


    <!-- http://www.semanticweb.org/macoda/ontologies/PMOEA#DTLZ2_15 -->

    <owl:NamedIndividual rdf:about="http://www.semanticweb.org/macoda/ontologies/PMOEA#DTLZ2_15">
        <rdf:type rdf:resource="http://www.semanticweb.org/macoda/ontologies/PMOEA#DTLZ"/>
        <PMOEA:isContinuousProblem rdf:datatype="http://www.w3.org/2001/XMLSchema#boolean">true</PMOEA:isContinuousProblem>
        <PMOEA:ObjectiveNumber rdf:datatype="http://www.w3.org/2001/XMLSchema#integer">15</PMOEA:ObjectiveNumber>
        <PMOEA:isManyObjectiveProblem rdf:datatype="http://www.w3.org/2001/XMLSchema#boolean">true</PMOEA:isManyObjectiveProblem>
        <rdfs:label xml:lang="en">DTLZ2_15</rdfs:label>
    </owl:NamedIndividual>
    


    <!-- http://www.semanticweb.org/macoda/ontologies/PMOEA#PPEA-IMOP -->

    <owl:NamedIndividual rdf:about="http://www.semanticweb.org/macoda/ontologies/PMOEA#PPEA-IMOP">
        <rdf:type rdf:resource="http://www.semanticweb.org/macoda/ontologies/PMOEA#PMOEA"/>
        <PMOEA:hasPreferenceModel rdf:resource="http://www.semanticweb.org/macoda/ontologies/PMOEA#PreferenceConvexCone"/>
        <PMOEA:hasPreferenceInformationFromDM rdf:resource="http://www.semanticweb.org/macoda/ontologies/PMOEA#PicktheBestandWorst"/>
        <PMOEA:hasInteractionTime rdf:resource="http://www.semanticweb.org/macoda/ontologies/PMOEA#progressive"/>
        <PMOEA:hasPreferenceIntegration rdf:resource="http://www.semanticweb.org/macoda/ontologies/PMOEA#FrontSorting"/>
        <PMOEA:canSolve rdf:resource="http://www.semanticweb.org/macoda/ontologies/PMOEA#ZDT2"/>
        <PMOEA:canSolve rdf:resource="http://www.semanticweb.org/macoda/ontologies/PMOEA#DTLZ2_5"/>
        <PMOEA:canSolve rdf:resource="http://www.semanticweb.org/macoda/ontologies/PMOEA#ZDT6"/>
        <PMOEA:canSolve rdf:resource="http://www.semanticweb.org/macoda/ontologies/PMOEA#ZDT4"/>
        <PMOEA:canSolve rdf:resource="http://www.semanticweb.org/macoda/ontologies/PMOEA#DTLZ1_3"/>
        <PMOEA:canSolve rdf:resource="http://www.semanticweb.org/macoda/ontologies/PMOEA#DTLZ2_3"/>
        <PMOEA:canSolve rdf:resource="http://www.semanticweb.org/macoda/ontologies/PMOEA#ZDT1"/>
        <PMOEA:hasResultInfluence rdf:resource="http://www.semanticweb.org/macoda/ontologies/PMOEA#OneSolution"/>
        <PMOEA:hasAuthor rdf:resource="http://www.semanticweb.org/macoda/ontologies/PMOEA#Dunwei_Gong"/>
        <PMOEA:hasAuthor rdf:resource="http://www.semanticweb.org/macoda/ontologies/PMOEA#Jing_Sun"/>
        <PMOEA:hasAuthor rdf:resource="http://www.semanticweb.org/macoda/ontologies/PMOEA#Xinfang_Ji"/>
        <PMOEA:hasSearchAlgorithm rdf:resource="http://www.semanticweb.org/macoda/ontologies/PMOEA#NSGA-II"/>
        <PMOEA:hasImplementationLanguage rdf:resource="http://www.semanticweb.org/macoda/ontologies/PMOEA#Matlab"/>
        <PMOEA:hasDevelopingYear rdf:datatype="http://www.w3.org/2001/XMLSchema#integer">2013</PMOEA:hasDevelopingYear>
        <PMOEA:hasReference>Gong, Dunwei, Jing Sun, and Xinfang Ji. &quot;Evolutionary algorithms with preference polyhedron for interval multi-objective optimization problems.&quot; Information Sciences 233 (2013): 141-161.</PMOEA:hasReference>
        <rdfs:comment>In this study, we proposed a preference-based EA for MOPs with interval parameters by employing the framework of NSGA-II, which incorporates an optimization-cum-decision-making procedure. In order to alleviate the DMs burden in evaluations, a preference polyhedron is created to approximate the DMs value function by using convex cones [21], and is used to guide the search toward the DMs preferred region.</rdfs:comment>
        <rdfs:label xml:lang="en">PPEA-IMOP</rdfs:label>
    </owl:NamedIndividual>
    


    <!-- http://www.semanticweb.org/macoda/ontologies/PMOEA#SPAM -->

    <owl:NamedIndividual rdf:about="http://www.semanticweb.org/macoda/ontologies/PMOEA#SPAM">
        <rdf:type rdf:resource="http://www.semanticweb.org/macoda/ontologies/PMOEA#PMOEA"/>
        <PMOEA:hasPreferenceModel rdf:resource="http://www.semanticweb.org/macoda/ontologies/PMOEA#SetPreferenceRelation"/>
        <PMOEA:hasPreferenceInformationFromDM rdf:resource="http://www.semanticweb.org/macoda/ontologies/PMOEA#SetPreference"/>
        <PMOEA:hasInteractionTime rdf:resource="http://www.semanticweb.org/macoda/ontologies/PMOEA#a-priori"/>
        <PMOEA:hasPreferenceIntegration rdf:resource="http://www.semanticweb.org/macoda/ontologies/PMOEA#SetQualityIndicator"/>
        <PMOEA:canSolve rdf:resource="http://www.semanticweb.org/macoda/ontologies/PMOEA#DTLZ2_2"/>
        <PMOEA:canSolve rdf:resource="http://www.semanticweb.org/macoda/ontologies/PMOEA#DTLZ5_2"/>
        <PMOEA:canSolve rdf:resource="http://www.semanticweb.org/macoda/ontologies/PMOEA#DTLZ2_5"/>
        <PMOEA:hasResultInfluence rdf:resource="http://www.semanticweb.org/macoda/ontologies/PMOEA#SetOfSolutions"/>
        <PMOEA:hasAuthor rdf:resource="http://www.semanticweb.org/macoda/ontologies/PMOEA#Johannes Bader"/>
        <PMOEA:hasAuthor rdf:resource="http://www.semanticweb.org/macoda/ontologies/PMOEA#Lothar_Thiele"/>
        <PMOEA:hasAuthor rdf:resource="http://www.semanticweb.org/macoda/ontologies/PMOEA#Eckart_Zitzler"/>
        <PMOEA:hasSearchAlgorithm rdf:resource="http://www.semanticweb.org/macoda/ontologies/PMOEA#SPAMO"/>
        <PMOEA:hasDevelopingYear rdf:datatype="http://www.w3.org/2001/XMLSchema#integer">2010</PMOEA:hasDevelopingYear>
        <PMOEA:ParetoDominancePreservation rdf:datatype="http://www.w3.org/2001/XMLSchema#boolean">true</PMOEA:ParetoDominancePreservation>
        <PMOEA:hasReference>Zitzler, Eckart, Lothar Thiele, and Johannes Bader. &quot;On set-based multiobjective optimization.&quot; IEEE Transactions on Evolutionary Computation 14.1 (2010): 58-79.</PMOEA:hasReference>
        <rdfs:comment>This paper proposes a theory of set preference relations that clarifies how user preferences on Pareto set approximations can be formalized on the basis of quality indicators and what criteria such formalizations must fulfill; it also introduces a general set-preference based search algorithm that can be shown to converge under certain mild assumptions</rdfs:comment>
        <rdfs:label xml:lang="en">SPAM</rdfs:label>
    </owl:NamedIndividual>
    


    <!-- http://www.semanticweb.org/macoda/ontologies/PMOEA#SetPreferenceRelation -->

    <owl:NamedIndividual rdf:about="http://www.semanticweb.org/macoda/ontologies/PMOEA#SetPreferenceRelation">
        <rdf:type rdf:resource="http://www.semanticweb.org/macoda/ontologies/PMOEA#SetPreferenceRelation"/>
        <rdfs:comment>In SPAM,  the author proposes a theory of set preference relations that clarifies how user preferences on Pareto set approximations can be formalized on the basis of quality indicators and what criteria such formalizations must fulfill.</rdfs:comment>
        <rdfs:label xml:lang="en">SetPreferenceRelation</rdfs:label>
    </owl:NamedIndividual>
    


    <!-- http://www.semanticweb.org/macoda/ontologies/PMOEA#basicASF -->

    <owl:NamedIndividual rdf:about="http://www.semanticweb.org/macoda/ontologies/PMOEA#basicASF">
        <rdf:type rdf:resource="http://www.semanticweb.org/macoda/ontologies/PMOEA#AchievementScalarizingFunction"/>
        <PMOEA:hasReference>A.P. Wierzbicki, A mathematical basis for satisficing decision
making, Mathematical Modelling 3 (1982) 391405</PMOEA:hasReference>
        <rdfs:comment>WierzbickiASF divided by distance of nardiar point and utopian point</rdfs:comment>
        <rdfs:label xml:lang="en">basicASF</rdfs:label>
    </owl:NamedIndividual>
    


    <!-- http://www.semanticweb.org/macoda/ontologies/PMOEA#Longmei_Li -->

    <owl:NamedIndividual rdf:about="http://www.semanticweb.org/macoda/ontologies/PMOEA#Longmei_Li">
        <rdf:type rdf:resource="http://www.semanticweb.org/macoda/ontologies/PMOEA#Researcher"/>
        <rdfs:label xml:lang="en">Longmei Li</rdfs:label>
    </owl:NamedIndividual>
    


    <!-- http://www.semanticweb.org/macoda/ontologies/PMOEA#DTLZ7_10 -->

    <owl:NamedIndividual rdf:about="http://www.semanticweb.org/macoda/ontologies/PMOEA#DTLZ7_10">
        <rdf:type rdf:resource="http://www.semanticweb.org/macoda/ontologies/PMOEA#DTLZ"/>
        <PMOEA:isContinuousProblem rdf:datatype="http://www.w3.org/2001/XMLSchema#boolean">true</PMOEA:isContinuousProblem>
        <PMOEA:ObjectiveNumber rdf:datatype="http://www.w3.org/2001/XMLSchema#integer">10</PMOEA:ObjectiveNumber>
        <PMOEA:isManyObjectiveProblem rdf:datatype="http://www.w3.org/2001/XMLSchema#boolean">true</PMOEA:isManyObjectiveProblem>
        <rdfs:label xml:lang="en">DTLZ7_10</rdfs:label>
    </owl:NamedIndividual>
    


    <!-- http://www.semanticweb.org/macoda/ontologies/PMOEA#Seung-Hwan_Choi -->

    <owl:NamedIndividual rdf:about="http://www.semanticweb.org/macoda/ontologies/PMOEA#Seung-Hwan_Choi">
        <rdf:type rdf:resource="http://www.semanticweb.org/macoda/ontologies/PMOEA#Researcher"/>
        <rdfs:label xml:lang="en">Seung-Hwan Choi</rdfs:label>
    </owl:NamedIndividual>
    


    <!-- http://www.semanticweb.org/macoda/ontologies/PMOEA#W_HypE -->

    <owl:NamedIndividual rdf:about="http://www.semanticweb.org/macoda/ontologies/PMOEA#W_HypE">
        <rdf:type rdf:resource="http://www.semanticweb.org/macoda/ontologies/PMOEA#PMOEA"/>
        <PMOEA:hasPreferenceModel rdf:resource="http://www.semanticweb.org/macoda/ontologies/PMOEA#ObjectiveSpaceWeightDistribution"/>
        <PMOEA:hasPreferenceInformationFromDM rdf:resource="http://www.semanticweb.org/macoda/ontologies/PMOEA#ExponentialFunctionPreferOneObjective"/>
        <PMOEA:hasPreferenceInformationFromDM rdf:resource="http://www.semanticweb.org/macoda/ontologies/PMOEA#GaussianFunctionPreferOneRP"/>
        <PMOEA:hasInteractionTime rdf:resource="http://www.semanticweb.org/macoda/ontologies/PMOEA#a-priori"/>
        <PMOEA:hasPreferenceIntegration rdf:resource="http://www.semanticweb.org/macoda/ontologies/PMOEA#HypervolumeIndicator"/>
        <PMOEA:canSolve rdf:resource="http://www.semanticweb.org/macoda/ontologies/PMOEA#ZDT6"/>
        <PMOEA:canSolve rdf:resource="http://www.semanticweb.org/macoda/ontologies/PMOEA#DTLZ2_7"/>
        <PMOEA:canSolve rdf:resource="http://www.semanticweb.org/macoda/ontologies/PMOEA#ZDT3"/>
        <PMOEA:canSolve rdf:resource="http://www.semanticweb.org/macoda/ontologies/PMOEA#ZDT1"/>
        <PMOEA:hasResultInfluence rdf:resource="http://www.semanticweb.org/macoda/ontologies/PMOEA#BiasedDistribution"/>
        <PMOEA:hasAuthor rdf:resource="http://www.semanticweb.org/macoda/ontologies/PMOEA#Johannes Bader"/>
        <PMOEA:hasAuthor rdf:resource="http://www.semanticweb.org/macoda/ontologies/PMOEA#Dimo_Brockhoff"/>
        <PMOEA:hasAuthor rdf:resource="http://www.semanticweb.org/macoda/ontologies/PMOEA#Eckart_Zitzler"/>
        <PMOEA:hasAuthor rdf:resource="http://www.semanticweb.org/macoda/ontologies/PMOEA#Anne_Auger"/>
        <PMOEA:hasExtension rdf:resource="http://www.semanticweb.org/macoda/ontologies/PMOEA#W_HypE"/>
        <PMOEA:isExtensionOf rdf:resource="http://www.semanticweb.org/macoda/ontologies/PMOEA#W_IBEA"/>
        <PMOEA:hasSearchAlgorithm rdf:resource="http://www.semanticweb.org/macoda/ontologies/PMOEA#HypE"/>
        <PMOEA:hasImplementationLanguage rdf:resource="http://www.semanticweb.org/macoda/ontologies/PMOEA#Matlab"/>
        <PMOEA:hasDevelopingYear rdf:datatype="http://www.w3.org/2001/XMLSchema#integer">2009</PMOEA:hasDevelopingYear>
        <PMOEA:MultipleRegionOfInterest rdf:datatype="http://www.w3.org/2001/XMLSchema#boolean">true</PMOEA:MultipleRegionOfInterest>
        <PMOEA:SpreadControl rdf:datatype="http://www.w3.org/2001/XMLSchema#boolean">true</PMOEA:SpreadControl>
        <PMOEA:hasReference>Auger, A., et al. (2009). Articulating user preferences in many-objective problems by sampling the weighted hypervolume. Proceedings of the 11th Annual conference on Genetic and evolutionary computation, ACM.</PMOEA:hasReference>
        <rdfs:comment>W-IBEA proposed the weighted hypervolume indicator with which user-defined preferences can be articulated; other studies exist that propose to estimate the hypervolume indicator by Monte-Carlo sampling. Here, we combine these two approaches for the first time and extend them, i.e., we present an approach of sampling the weighted hypervolume to incorporate user-defined preferences into the search for problems with many objectives.</rdfs:comment>
        <rdfs:label xml:lang="en">W_HypE</rdfs:label>
    </owl:NamedIndividual>
    


    <!-- http://www.semanticweb.org/macoda/ontologies/PMOEA#F3 -->

    <owl:NamedIndividual rdf:about="http://www.semanticweb.org/macoda/ontologies/PMOEA#F3">
        <rdf:type rdf:resource="http://www.semanticweb.org/macoda/ontologies/PMOEA#Academic_Problem"/>
        <PMOEA:isContinuousProblem rdf:datatype="http://www.w3.org/2001/XMLSchema#boolean">true</PMOEA:isContinuousProblem>
        <PMOEA:ObjectiveNumber rdf:datatype="http://www.w3.org/2001/XMLSchema#integer">2</PMOEA:ObjectiveNumber>
        <rdfs:comment>Y. Jin, M. Olhofer, and B. Sendhoff. Evolutionaynamic
weighted aggregation: Why does it work and how? In
L. Spector, E. Goodman, A. Wu, W.B. Langdon, H.-
M. Voigt, M. Gen, S. Sen, M. DOrigo, S. Pezeshk,
M. Garzon, and E. Burke, editors, Proceedings of Ge-
netic and Evolutionary Computation Conference, pages
10421049, San Francisco, CA, 2001</rdfs:comment>
        <rdfs:label xml:lang="en">F3</rdfs:label>
    </owl:NamedIndividual>
    


    <!-- http://www.semanticweb.org/macoda/ontologies/PMOEA#DTLZ2_8 -->

    <owl:NamedIndividual rdf:about="http://www.semanticweb.org/macoda/ontologies/PMOEA#DTLZ2_8">
        <rdf:type rdf:resource="http://www.semanticweb.org/macoda/ontologies/PMOEA#DTLZ"/>
        <PMOEA:isContinuousProblem rdf:datatype="http://www.w3.org/2001/XMLSchema#boolean">true</PMOEA:isContinuousProblem>
        <PMOEA:ObjectiveNumber rdf:datatype="http://www.w3.org/2001/XMLSchema#integer">8</PMOEA:ObjectiveNumber>
        <PMOEA:isManyObjectiveProblem rdf:datatype="http://www.w3.org/2001/XMLSchema#boolean">true</PMOEA:isManyObjectiveProblem>
        <rdfs:label xml:lang="en">DTLZ2_8</rdfs:label>
    </owl:NamedIndividual>
    


    <!-- http://www.semanticweb.org/macoda/ontologies/PMOEA#ReferenceVectorFORIso-UtilityFunction -->

    <owl:NamedIndividual rdf:about="http://www.semanticweb.org/macoda/ontologies/PMOEA#ReferenceVectorFORIso-UtilityFunction">
        <rdf:type rdf:resource="http://www.semanticweb.org/macoda/ontologies/PMOEA#ReferenceDirection"/>
        <rdfs:comment>a reference direction vector that defines an iso-utility function, solutions that are parallel to this function are prefered. In BCD_NSGA2</rdfs:comment>
        <rdfs:label xml:lang="en">ReferenceVectorFORIso-UtilityFunction</rdfs:label>
    </owl:NamedIndividual>
    


    <!-- http://www.semanticweb.org/macoda/ontologies/PMOEA#MiniCAPS -->

    <owl:NamedIndividual rdf:about="http://www.semanticweb.org/macoda/ontologies/PMOEA#MiniCAPS">
        <rdf:type rdf:resource="http://www.semanticweb.org/macoda/ontologies/PMOEA#Realworld_Problem"/>
        <PMOEA:isContinuousProblem rdf:datatype="http://www.w3.org/2001/XMLSchema#boolean">true</PMOEA:isContinuousProblem>
        <PMOEA:ObjectiveNumber rdf:datatype="http://www.w3.org/2001/XMLSchema#integer">13</PMOEA:ObjectiveNumber>
        <PMOEA:hasReference>E. Webb, MINICAPSA simplified version of CAPS for use as a research tool, British Aerospace, Warton, U.K., Unclassified Rep. BAe-WOA-RP-GEN-11313, July 1997</PMOEA:hasReference>
        <PMOEA:isManyObjectiveProblem rdf:datatype="http://www.w3.org/2001/XMLSchema#boolean">true</PMOEA:isManyObjectiveProblem>
        <rdfs:comment>conceptual airframe design project, an industrial project developed in cooperation with British Aerospace Systems (BAE)</rdfs:comment>
        <rdfs:label xml:lang="en">MiniCAPS</rdfs:label>
    </owl:NamedIndividual>
    


    <!-- http://www.semanticweb.org/macoda/ontologies/PMOEA#SupportVectorRanking -->

    <owl:NamedIndividual rdf:about="http://www.semanticweb.org/macoda/ontologies/PMOEA#SupportVectorRanking">
        <rdf:type rdf:resource="http://www.semanticweb.org/macoda/ontologies/PMOEA#SupportVectorMachine"/>
        <rdfs:label xml:lang="en">SupportVectorRanking</rdfs:label>
    </owl:NamedIndividual>
    


    <!-- http://www.semanticweb.org/macoda/ontologies/PMOEA#Wei_Zhang -->

    <owl:NamedIndividual rdf:about="http://www.semanticweb.org/macoda/ontologies/PMOEA#Wei_Zhang">
        <rdf:type rdf:resource="http://www.semanticweb.org/macoda/ontologies/PMOEA#Researcher"/>
        <rdfs:label xml:lang="en">Wei Zhang</rdfs:label>
    </owl:NamedIndividual>
    


    <!-- http://www.semanticweb.org/macoda/ontologies/PMOEA#RODEOlib -->

    <owl:NamedIndividual rdf:about="http://www.semanticweb.org/macoda/ontologies/PMOEA#RODEOlib">
        <rdf:type rdf:resource="http://www.semanticweb.org/macoda/ontologies/PMOEA#ImplementationLibrary"/>
        <PMOEA:hasLibraryDescription>The RODEOlib, or (Ro)bust (De)sign (O)ptimization library, is a MATLAB/Octave library for (robust) optimization using Evolutionary Algorithms. It contains MATLAB/Octave code for optimization in noisy and uncertain environments.</PMOEA:hasLibraryDescription>
        <rdfs:comment>The RODEOlib, or (Ro)bust (De)sign (O)ptimization library, is a MATLAB/Octave library for (robust) optimization using Evolutionary Algorithms. It contains MATLAB/Octave code for optimization in noisy and uncertain environments.</rdfs:comment>
        <rdfs:label xml:lang="en">RODEOlib</rdfs:label>
    </owl:NamedIndividual>
    


    <!-- http://www.semanticweb.org/macoda/ontologies/PMOEA#SelectionOfNSGAII -->

    <owl:NamedIndividual rdf:about="http://www.semanticweb.org/macoda/ontologies/PMOEA#SelectionOfNSGAII">
        <rdf:type rdf:resource="http://www.semanticweb.org/macoda/ontologies/PMOEA#SelectionCriterion"/>
        <rdfs:comment>In ER-NSGA-II, It avoids to automatically select all solutions of the first front of the candidate set into the next population, instead, distance to the reference point is considered as criterion.</rdfs:comment>
        <rdfs:label xml:lang="en">SelectionOfNSGAII</rdfs:label>
    </owl:NamedIndividual>
    


    <!-- http://www.semanticweb.org/macoda/ontologies/PMOEA#Anne_Auger -->

    <owl:NamedIndividual rdf:about="http://www.semanticweb.org/macoda/ontologies/PMOEA#Anne_Auger">
        <rdf:type rdf:resource="http://www.semanticweb.org/macoda/ontologies/PMOEA#Researcher"/>
        <rdfs:label xml:lang="en">Anne Auger</rdfs:label>
    </owl:NamedIndividual>
    


    <!-- http://www.semanticweb.org/macoda/ontologies/PMOEA#ObjectiveRelativeImportance -->

    <owl:NamedIndividual rdf:about="http://www.semanticweb.org/macoda/ontologies/PMOEA#ObjectiveRelativeImportance">
        <rdf:type rdf:resource="http://www.semanticweb.org/macoda/ontologies/PMOEA#ObjectiveRelativeImportance"/>
    </owl:NamedIndividual>
    


    <!-- http://www.semanticweb.org/macoda/ontologies/PMOEA#OutrankingNeighbour -->

    <owl:NamedIndividual rdf:about="http://www.semanticweb.org/macoda/ontologies/PMOEA#OutrankingNeighbour">
        <rdf:type rdf:resource="http://www.semanticweb.org/macoda/ontologies/PMOEA#OutrankingRelation"/>
        <rdfs:comment>Light Beam Search Method: A local preference model in the form of an outranking relation S is used to obtain neighboring solutions of the current non-dominated point, or the middle point.</rdfs:comment>
        <rdfs:label>OutrankingNeighbour</rdfs:label>
    </owl:NamedIndividual>
    


    <!-- http://www.semanticweb.org/macoda/ontologies/PMOEA#PBEA -->

    <owl:NamedIndividual rdf:about="http://www.semanticweb.org/macoda/ontologies/PMOEA#PBEA">
        <rdf:type rdf:resource="http://www.semanticweb.org/macoda/ontologies/PMOEA#PMOEA"/>
        <PMOEA:hasPreferenceModel rdf:resource="http://www.semanticweb.org/macoda/ontologies/PMOEA#WierzbickiASF"/>
        <PMOEA:hasPreferenceInformationFromDM rdf:resource="http://www.semanticweb.org/macoda/ontologies/PMOEA#ReferencePoint"/>
        <PMOEA:hasInteractionTime rdf:resource="http://www.semanticweb.org/macoda/ontologies/PMOEA#a-priori"/>
        <PMOEA:hasInteractionTime rdf:resource="http://www.semanticweb.org/macoda/ontologies/PMOEA#progressive"/>
        <PMOEA:hasPreferenceIntegration rdf:resource="http://www.semanticweb.org/macoda/ontologies/PMOEA#AdditiveEpsilonIndicator"/>
        <PMOEA:canSolve rdf:resource="http://www.semanticweb.org/macoda/ontologies/PMOEA#ZDT3"/>
        <PMOEA:canSolve rdf:resource="http://www.semanticweb.org/macoda/ontologies/PMOEA#ZDT1"/>
        <PMOEA:canSolve rdf:resource="http://www.semanticweb.org/macoda/ontologies/PMOEA#PollutionMonitoringStationLocation"/>
        <PMOEA:hasResultInfluence rdf:resource="http://www.semanticweb.org/macoda/ontologies/PMOEA#BoundedRegion"/>
        <PMOEA:hasAuthor rdf:resource="http://www.semanticweb.org/macoda/ontologies/PMOEA#Julin_Molina"/>
        <PMOEA:hasAuthor rdf:resource="http://www.semanticweb.org/macoda/ontologies/PMOEA#Kaisa_Miettinen"/>
        <PMOEA:hasAuthor rdf:resource="http://www.semanticweb.org/macoda/ontologies/PMOEA#Lothar_Thiele"/>
        <PMOEA:hasAuthor rdf:resource="http://www.semanticweb.org/macoda/ontologies/PMOEA#Pekka_J._Korhonen"/>
        <PMOEA:useLibrary rdf:resource="http://www.semanticweb.org/macoda/ontologies/PMOEA#PISA"/>
        <PMOEA:hasSearchAlgorithm rdf:resource="http://www.semanticweb.org/macoda/ontologies/PMOEA#IBEA"/>
        <PMOEA:hasDevelopingYear rdf:datatype="http://www.w3.org/2001/XMLSchema#integer">2009</PMOEA:hasDevelopingYear>
        <PMOEA:MultipleRegionOfInterest rdf:datatype="http://www.w3.org/2001/XMLSchema#boolean">true</PMOEA:MultipleRegionOfInterest>
        <PMOEA:SpreadControl rdf:datatype="http://www.w3.org/2001/XMLSchema#boolean">true</PMOEA:SpreadControl>
        <PMOEA:ParetoDominancePreservation rdf:datatype="http://www.w3.org/2001/XMLSchema#boolean">true</PMOEA:ParetoDominancePreservation>
        <PMOEA:hasReference>Thiele, L., K. Miettinen, P. J. Korhonen and J. Molina (2009). &quot;A preference-based evolutionary algorithm for multi-objective optimization.&quot; Evolutionary Computation 17(3): 411-436</PMOEA:hasReference>
        <rdfs:comment>PBEA allows the DM to interactively give reference points, with which the binary quality indicator of IBEA (which measures the minimal distance by which an individual needs to be improved in each objective to become non-dominated ) is redefined using an achievement scalarizing function</rdfs:comment>
        <rdfs:label>PBEA</rdfs:label>
    </owl:NamedIndividual>
    


    <!-- http://www.semanticweb.org/macoda/ontologies/PMOEA#PR_NSGA-II -->

    <owl:NamedIndividual rdf:about="http://www.semanticweb.org/macoda/ontologies/PMOEA#PR_NSGA-II">
        <rdf:type rdf:resource="http://www.semanticweb.org/macoda/ontologies/PMOEA#PMOEA"/>
        <PMOEA:hasPreferenceModel rdf:resource="http://www.semanticweb.org/macoda/ontologies/PMOEA#TchebycheffASF"/>
        <PMOEA:hasPreferenceInformationFromDM rdf:resource="http://www.semanticweb.org/macoda/ontologies/PMOEA#ReferencePoint"/>
        <PMOEA:hasInteractionTime rdf:resource="http://www.semanticweb.org/macoda/ontologies/PMOEA#progressive"/>
        <PMOEA:hasPreferenceIntegration rdf:resource="http://www.semanticweb.org/macoda/ontologies/PMOEA#ChebyshevPreferenceRelation"/>
        <PMOEA:canSolve rdf:resource="http://www.semanticweb.org/macoda/ontologies/PMOEA#AirfoilShapeOptimization"/>
        <PMOEA:canSolve rdf:resource="http://www.semanticweb.org/macoda/ontologies/PMOEA#AirfoilShapeOptimization_3"/>
        <PMOEA:hasResultInfluence rdf:resource="http://www.semanticweb.org/macoda/ontologies/PMOEA#BoundedRegion"/>
        <PMOEA:hasAuthor rdf:resource="http://www.semanticweb.org/macoda/ontologies/PMOEA#Alfredo_Montano"/>
        <PMOEA:hasAuthor rdf:resource="http://www.semanticweb.org/macoda/ontologies/PMOEA#Antonio_Jaimes"/>
        <PMOEA:hasAuthor rdf:resource="http://www.semanticweb.org/macoda/ontologies/PMOEA#Carlos_Coello_Coello"/>
        <PMOEA:hasSearchAlgorithm rdf:resource="http://www.semanticweb.org/macoda/ontologies/PMOEA#NSGA-II"/>
        <PMOEA:hasDevelopingYear rdf:datatype="http://www.w3.org/2001/XMLSchema#integer">2011</PMOEA:hasDevelopingYear>
        <PMOEA:SpreadControl rdf:datatype="http://www.w3.org/2001/XMLSchema#boolean">true</PMOEA:SpreadControl>
        <PMOEA:ParetoDominancePreservation rdf:datatype="http://www.w3.org/2001/XMLSchema#boolean">true</PMOEA:ParetoDominancePreservation>
        <PMOEA:hasReference>Jaimes, A. L., A. A. Montano and C. A. C. Coello (2011). Preference incorporation to solve many-objective airfoil design problems. Evolutionary Computation (CEC), 2011 IEEE Congress on, IEEE</PMOEA:hasReference>
        <rdfs:comment>In this paper, we assess the convenience of applying a previously proposed interactive method to solve three aerodynamic airfoil shape optimization problems with 2, 3, and 6 objectives, respectively.
First, the search can be focused on the decision makers region of interest, saving this way, valuable function evaluations. Second, the preference relation used in the interactive method helps to deal with a large number of objectives since it is able to rank incomparable nondominated solutions.</rdfs:comment>
        <rdfs:label>PR_NAGA-II</rdfs:label>
    </owl:NamedIndividual>
    


    <!-- http://www.semanticweb.org/macoda/ontologies/PMOEA#ParametersInGaussionFunction -->

    <owl:NamedIndividual rdf:about="http://www.semanticweb.org/macoda/ontologies/PMOEA#ParametersInGaussionFunction">
        <rdf:type rdf:resource="http://www.semanticweb.org/macoda/ontologies/PMOEA#DistributionFunctionInObjectiveSpace"/>
        <rdfs:comment>center and spread vector to define a region on the hyperplane</rdfs:comment>
        <rdfs:label>GaussionFunctionOnHyperplane</rdfs:label>
    </owl:NamedIndividual>
    


    <!-- http://www.semanticweb.org/macoda/ontologies/PMOEA#Patricia_Sanchez -->

    <owl:NamedIndividual rdf:about="http://www.semanticweb.org/macoda/ontologies/PMOEA#Patricia_Sanchez">
        <rdf:type rdf:resource="http://www.semanticweb.org/macoda/ontologies/PMOEA#Researcher"/>
        <rdfs:label>Patricia Sanchez</rdfs:label>
    </owl:NamedIndividual>
    


    <!-- http://www.semanticweb.org/macoda/ontologies/PMOEA#Pekka_J._Korhonen -->

    <owl:NamedIndividual rdf:about="http://www.semanticweb.org/macoda/ontologies/PMOEA#Pekka_J._Korhonen">
        <rdf:type rdf:resource="http://www.semanticweb.org/macoda/ontologies/PMOEA#Researcher"/>
        <rdfs:label>Pekka J. Korhonen</rdfs:label>
    </owl:NamedIndividual>
    


    <!-- http://www.semanticweb.org/macoda/ontologies/PMOEA#PollutionMonitoringStationLocation -->

    <owl:NamedIndividual rdf:about="http://www.semanticweb.org/macoda/ontologies/PMOEA#PollutionMonitoringStationLocation">
        <rdf:type rdf:resource="http://www.semanticweb.org/macoda/ontologies/PMOEA#Realworld_Problem"/>
        <PMOEA:isContinuousProblem rdf:datatype="http://www.w3.org/2001/XMLSchema#boolean">true</PMOEA:isContinuousProblem>
        <PMOEA:ObjectiveNumber rdf:datatype="http://www.w3.org/2001/XMLSchema#integer">5</PMOEA:ObjectiveNumber>
        <PMOEA:hasReference>Miettinen, K., Lotov, A.V., Kamenev, G.K., Berezkin, V.E.: Integration of two
multiobjective optimization methods for nonlinear problems. Optimization Method and Software 18(1), 6380 (2003)</PMOEA:hasReference>
        <rdfs:label>PollutionMonitoringStationLocation</rdfs:label>
    </owl:NamedIndividual>
    


    <!-- http://www.semanticweb.org/macoda/ontologies/PMOEA#PreferencePoint -->

    <owl:NamedIndividual rdf:about="http://www.semanticweb.org/macoda/ontologies/PMOEA#PreferencePoint">
        <rdf:type rdf:resource="http://www.semanticweb.org/macoda/ontologies/PMOEA#PreferencePoint"/>
    </owl:NamedIndividual>
    


    <!-- http://www.semanticweb.org/macoda/ontologies/PMOEA#ProjectPortfolioProblem_9 -->

    <owl:NamedIndividual rdf:about="http://www.semanticweb.org/macoda/ontologies/PMOEA#ProjectPortfolioProblem_9">
        <rdf:type rdf:resource="http://www.semanticweb.org/macoda/ontologies/PMOEA#Realworld_Problem"/>
        <PMOEA:isDiscreteProblem rdf:datatype="http://www.w3.org/2001/XMLSchema#boolean">true</PMOEA:isDiscreteProblem>
        <PMOEA:ObjectiveNumber rdf:datatype="http://www.w3.org/2001/XMLSchema#integer">9</PMOEA:ObjectiveNumber>
        <PMOEA:isManyObjectiveProblem rdf:datatype="http://www.w3.org/2001/XMLSchema#boolean">true</PMOEA:isManyObjectiveProblem>
        <rdfs:label>ProjectPortfolioProblem_9</rdfs:label>
    </owl:NamedIndividual>
    


    <!-- http://www.semanticweb.org/macoda/ontologies/PMOEA#R-NSGA-II -->

    <owl:NamedIndividual rdf:about="http://www.semanticweb.org/macoda/ontologies/PMOEA#R-NSGA-II">
        <rdf:type rdf:resource="http://www.semanticweb.org/macoda/ontologies/PMOEA#PMOEA"/>
        <PMOEA:hasPreferenceModel rdf:resource="http://www.semanticweb.org/macoda/ontologies/PMOEA#PreferencePoint"/>
        <PMOEA:hasPreferenceModel rdf:resource="http://www.semanticweb.org/macoda/ontologies/PMOEA#WeightedEuclideanDistanceASF"/>
        <PMOEA:hasPreferenceInformationFromDM rdf:resource="http://www.semanticweb.org/macoda/ontologies/PMOEA#weights"/>
        <PMOEA:hasPreferenceInformationFromDM rdf:resource="http://www.semanticweb.org/macoda/ontologies/PMOEA#ReferencePoint"/>
        <PMOEA:hasInteractionTime rdf:resource="http://www.semanticweb.org/macoda/ontologies/PMOEA#a-priori"/>
        <PMOEA:hasPreferenceIntegration rdf:resource="http://www.semanticweb.org/macoda/ontologies/PMOEA#CrowdingDistance"/>
        <PMOEA:canSolve rdf:resource="http://www.semanticweb.org/macoda/ontologies/PMOEA#DTLZ2_10"/>
        <PMOEA:canSolve rdf:resource="http://www.semanticweb.org/macoda/ontologies/PMOEA#ZDT2"/>
        <PMOEA:canSolve rdf:resource="http://www.semanticweb.org/macoda/ontologies/PMOEA#DTLZ2_5"/>
        <PMOEA:canSolve rdf:resource="http://www.semanticweb.org/macoda/ontologies/PMOEA#ZDT3"/>
        <PMOEA:canSolve rdf:resource="http://www.semanticweb.org/macoda/ontologies/PMOEA#DTLZ2_3"/>
        <PMOEA:canSolve rdf:resource="http://www.semanticweb.org/macoda/ontologies/PMOEA#ZDT1"/>
        <PMOEA:canSolve rdf:resource="http://www.semanticweb.org/macoda/ontologies/PMOEA#SpringDesignProblem"/>
        <PMOEA:canSolve rdf:resource="http://www.semanticweb.org/macoda/ontologies/PMOEA#WeldedBeamDesign"/>
        <PMOEA:hasResultInfluence rdf:resource="http://www.semanticweb.org/macoda/ontologies/PMOEA#BoundedRegion"/>
        <PMOEA:hasAuthor rdf:resource="http://www.semanticweb.org/macoda/ontologies/PMOEA#J._Sundar"/>
        <PMOEA:hasAuthor rdf:resource="http://www.semanticweb.org/macoda/ontologies/PMOEA#Kalyanmoy_Deb"/>
        <PMOEA:hasSearchAlgorithm rdf:resource="http://www.semanticweb.org/macoda/ontologies/PMOEA#NSGA-II"/>
        <PMOEA:hasDevelopingYear rdf:datatype="http://www.w3.org/2001/XMLSchema#integer">2006</PMOEA:hasDevelopingYear>
        <PMOEA:MultipleRegionOfInterest rdf:datatype="http://www.w3.org/2001/XMLSchema#boolean">true</PMOEA:MultipleRegionOfInterest>
        <PMOEA:SpreadControl rdf:datatype="http://www.w3.org/2001/XMLSchema#boolean">true</PMOEA:SpreadControl>
        <PMOEA:ParetoDominancePreservation rdf:datatype="http://www.w3.org/2001/XMLSchema#boolean">true</PMOEA:ParetoDominancePreservation>
        <PMOEA:hasReference>Deb, K., et al. (2006). &quot;Reference point based multi-objective optimization using evolutionary algorithms.&quot; International Journal of Computational Intelligence Research 2(3): 273-286</PMOEA:hasReference>
        <rdfs:comment>The crowding distance used in NSGA-II is replaced by a preference distance.  Reference point is not applied in a classical way, i.e. together with an achievement scalarizing function, but rather to establish a biased crowding scheme. Specifically, solutions near reference points are emphasized by the selection mechanisms. The extent and the distribution of the solutions is maintained by an additional parameter.</rdfs:comment>
        <rdfs:label>R-NSGA-II</rdfs:label>
    </owl:NamedIndividual>
    


    <!-- http://www.semanticweb.org/macoda/ontologies/PMOEA#RIO-EMO -->

    <owl:NamedIndividual rdf:about="http://www.semanticweb.org/macoda/ontologies/PMOEA#RIO-EMO">
        <rdf:type rdf:resource="http://www.semanticweb.org/macoda/ontologies/PMOEA#PMOEA"/>
        <PMOEA:hasPreferenceModel rdf:resource="http://www.semanticweb.org/macoda/ontologies/PMOEA#ObjectiveRelativeImportance"/>
        <PMOEA:hasPreferenceInformationFromDM rdf:resource="http://www.semanticweb.org/macoda/ontologies/PMOEA#RelativeImportanceOfObjectives"/>
        <PMOEA:hasInteractionTime rdf:resource="http://www.semanticweb.org/macoda/ontologies/PMOEA#a-priori"/>
        <PMOEA:hasInteractionTime rdf:resource="http://www.semanticweb.org/macoda/ontologies/PMOEA#progressive"/>
        <PMOEA:hasPreferenceIntegration rdf:resource="http://www.semanticweb.org/macoda/ontologies/PMOEA#CrowdingDistance"/>
        <PMOEA:hasPreferenceIntegration rdf:resource="http://www.semanticweb.org/macoda/ontologies/PMOEA#FrontSorting"/>
        <PMOEA:hasPreferenceIntegration rdf:resource="http://www.semanticweb.org/macoda/ontologies/PMOEA#constraints"/>
        <PMOEA:canSolve rdf:resource="http://www.semanticweb.org/macoda/ontologies/PMOEA#DTLZ2_6"/>
        <PMOEA:canSolve rdf:resource="http://www.semanticweb.org/macoda/ontologies/PMOEA#DTLZ3_3"/>
        <PMOEA:canSolve rdf:resource="http://www.semanticweb.org/macoda/ontologies/PMOEA#DTLZ3_4"/>
        <PMOEA:canSolve rdf:resource="http://www.semanticweb.org/macoda/ontologies/PMOEA#DTLZ3_6"/>
        <PMOEA:canSolve rdf:resource="http://www.semanticweb.org/macoda/ontologies/PMOEA#DTLZ4_4"/>
        <PMOEA:canSolve rdf:resource="http://www.semanticweb.org/macoda/ontologies/PMOEA#DTLZ4_6"/>
        <PMOEA:canSolve rdf:resource="http://www.semanticweb.org/macoda/ontologies/PMOEA#DTLZ5_3"/>
        <PMOEA:canSolve rdf:resource="http://www.semanticweb.org/macoda/ontologies/PMOEA#DTLZ5_4"/>
        <PMOEA:canSolve rdf:resource="http://www.semanticweb.org/macoda/ontologies/PMOEA#DTLZ5_6"/>
        <PMOEA:canSolve rdf:resource="http://www.semanticweb.org/macoda/ontologies/PMOEA#ZDT2"/>
        <PMOEA:canSolve rdf:resource="http://www.semanticweb.org/macoda/ontologies/PMOEA#DTLZ4_3"/>
        <PMOEA:canSolve rdf:resource="http://www.semanticweb.org/macoda/ontologies/PMOEA#DTLZ2_4"/>
        <PMOEA:canSolve rdf:resource="http://www.semanticweb.org/macoda/ontologies/PMOEA#DTLZ1_3"/>
        <PMOEA:canSolve rdf:resource="http://www.semanticweb.org/macoda/ontologies/PMOEA#DTLZ1_4"/>
        <PMOEA:canSolve rdf:resource="http://www.semanticweb.org/macoda/ontologies/PMOEA#DTLZ1_6"/>
        <PMOEA:canSolve rdf:resource="http://www.semanticweb.org/macoda/ontologies/PMOEA#ZDT3"/>
        <PMOEA:canSolve rdf:resource="http://www.semanticweb.org/macoda/ontologies/PMOEA#DTLZ2_3"/>
        <PMOEA:canSolve rdf:resource="http://www.semanticweb.org/macoda/ontologies/PMOEA#ZDT1"/>
        <PMOEA:hasResultInfluence rdf:resource="http://www.semanticweb.org/macoda/ontologies/PMOEA#BiasedDistribution"/>
        <PMOEA:hasResultInfluence rdf:resource="http://www.semanticweb.org/macoda/ontologies/PMOEA#BoundedRegion"/>
        <PMOEA:hasAuthor rdf:resource="http://www.semanticweb.org/macoda/ontologies/PMOEA#Dipti_Srinivasan"/>
        <PMOEA:hasAuthor rdf:resource="http://www.semanticweb.org/macoda/ontologies/PMOEA#Lily_Rachmawati"/>
        <PMOEA:hasSearchAlgorithm rdf:resource="http://www.semanticweb.org/macoda/ontologies/PMOEA#NSGA-II"/>
        <PMOEA:hasImplementationLanguage rdf:resource="http://www.semanticweb.org/macoda/ontologies/PMOEA#C"/>
        <PMOEA:hasDevelopingYear rdf:datatype="http://www.w3.org/2001/XMLSchema#integer">2010</PMOEA:hasDevelopingYear>
        <PMOEA:ParetoDominancePreservation rdf:datatype="http://www.w3.org/2001/XMLSchema#boolean">true</PMOEA:ParetoDominancePreservation>
        <PMOEA:hasReference>Rachmawati, L. and D. Srinivasan (2010). &quot;Incorporating the notion of relative importance of objectives in evolutionary multiobjective optimization.&quot; Evolutionary Computation, IEEE Transactions on 14(4): 530-546</PMOEA:hasReference>
        <rdfs:comment>The axiomatic model proposed here formalizes the notion of relative importance of objectives as a partial order that supports strict preference, equality of importance, and incomparability between objective pairs. Unlike most approaches, the proposed model does not encode relative importance as a set of real-valued parameters. Instead, the approach provides a functional correspondence between a coherent overall preference with a subset of the Pareto-optimal front.Three techniques of integrating explicated preference information into the NSGA-II (constraints,rank penalty, crowding distance)are proposed.</rdfs:comment>
        <rdfs:label>RIO-EMO</rdfs:label>
    </owl:NamedIndividual>
    


    <!-- http://www.semanticweb.org/macoda/ontologies/PMOEA#RPSO-SS -->

    <owl:NamedIndividual rdf:about="http://www.semanticweb.org/macoda/ontologies/PMOEA#RPSO-SS">
        <rdf:type rdf:resource="http://www.semanticweb.org/macoda/ontologies/PMOEA#PMOEA"/>
        <PMOEA:hasPreferenceModel rdf:resource="http://www.semanticweb.org/macoda/ontologies/PMOEA#TchebycheffASF"/>
        <PMOEA:hasPreferenceInformationFromDM rdf:resource="http://www.semanticweb.org/macoda/ontologies/PMOEA#ReferencePoint"/>
        <PMOEA:hasInteractionTime rdf:resource="http://www.semanticweb.org/macoda/ontologies/PMOEA#a-priori"/>
        <PMOEA:hasPreferenceIntegration rdf:resource="http://www.semanticweb.org/macoda/ontologies/PMOEA#LeaderParticleSelection"/>
        <PMOEA:canSolve rdf:resource="http://www.semanticweb.org/macoda/ontologies/PMOEA#DTLZ6_3"/>
        <PMOEA:canSolve rdf:resource="http://www.semanticweb.org/macoda/ontologies/PMOEA#ZDT2"/>
        <PMOEA:canSolve rdf:resource="http://www.semanticweb.org/macoda/ontologies/PMOEA#ZDT4"/>
        <PMOEA:canSolve rdf:resource="http://www.semanticweb.org/macoda/ontologies/PMOEA#ZDT3"/>
        <PMOEA:canSolve rdf:resource="http://www.semanticweb.org/macoda/ontologies/PMOEA#DTLZ2_3"/>
        <PMOEA:canSolve rdf:resource="http://www.semanticweb.org/macoda/ontologies/PMOEA#ZDT1"/>
        <PMOEA:hasResultInfluence rdf:resource="http://www.semanticweb.org/macoda/ontologies/PMOEA#BoundedRegion"/>
        <PMOEA:hasAuthor rdf:resource="http://www.semanticweb.org/macoda/ontologies/PMOEA#Juergen_Branke"/>
        <PMOEA:hasAuthor rdf:resource="http://www.semanticweb.org/macoda/ontologies/PMOEA#Richard_Allmendinger"/>
        <PMOEA:hasAuthor rdf:resource="http://www.semanticweb.org/macoda/ontologies/PMOEA#Xiaodong_Li"/>
        <PMOEA:hasSearchAlgorithm rdf:resource="http://www.semanticweb.org/macoda/ontologies/PMOEA#MOPSO"/>
        <PMOEA:hasDevelopingYear rdf:datatype="http://www.w3.org/2001/XMLSchema#integer">2008</PMOEA:hasDevelopingYear>
        <PMOEA:MultipleRegionOfInterest rdf:datatype="http://www.w3.org/2001/XMLSchema#boolean">true</PMOEA:MultipleRegionOfInterest>
        <PMOEA:SpreadControl rdf:datatype="http://www.w3.org/2001/XMLSchema#boolean">true</PMOEA:SpreadControl>
        <PMOEA:ParetoDominancePreservation rdf:datatype="http://www.w3.org/2001/XMLSchema#boolean">true</PMOEA:ParetoDominancePreservation>
        <PMOEA:hasReference>Allmendinger, R., X. Li and J. Branke (2008). Reference point-based particle swarm optimization using a steady-state approach. Simulated Evolution and Learning, Springer: 200-209</PMOEA:hasReference>
        <rdfs:comment>We propose a multi-objective PSO algorithm that employs a preference-based method in order to find a set of preferred Pareto-optimal solutions near user-provided reference points.</rdfs:comment>
        <rdfs:label>RPSO-SS</rdfs:label>
    </owl:NamedIndividual>
    


    <!-- http://www.semanticweb.org/macoda/ontologies/PMOEA#Rafael_Caballero -->

    <owl:NamedIndividual rdf:about="http://www.semanticweb.org/macoda/ontologies/PMOEA#Rafael_Caballero">
        <rdf:type rdf:resource="http://www.semanticweb.org/macoda/ontologies/PMOEA#Researcher"/>
        <rdfs:label>Rafael Caballero</rdfs:label>
    </owl:NamedIndividual>
    


    <!-- http://www.semanticweb.org/macoda/ontologies/PMOEA#ReferencePoint -->

    <owl:NamedIndividual rdf:about="http://www.semanticweb.org/macoda/ontologies/PMOEA#ReferencePoint">
        <rdf:type rdf:resource="http://www.semanticweb.org/macoda/ontologies/PMOEA#ReferencePoint"/>
        <rdfs:label>ReferencePoint</rdfs:label>
    </owl:NamedIndividual>
    


    <!-- http://www.semanticweb.org/macoda/ontologies/PMOEA#RelativeImportanceOfObjectives -->

    <owl:NamedIndividual rdf:about="http://www.semanticweb.org/macoda/ontologies/PMOEA#RelativeImportanceOfObjectives">
        <rdf:type rdf:resource="http://www.semanticweb.org/macoda/ontologies/PMOEA#ObjectiveComparison"/>
        <rdfs:comment>strict preference, equality of importance, and incomparability between objective pairs</rdfs:comment>
        <rdfs:label>RelativeImportanceOfObjectives</rdfs:label>
    </owl:NamedIndividual>
    


    <!-- http://www.semanticweb.org/macoda/ontologies/PMOEA#Richard_Allmendinger -->

    <owl:NamedIndividual rdf:about="http://www.semanticweb.org/macoda/ontologies/PMOEA#Richard_Allmendinger">
        <rdf:type rdf:resource="http://www.semanticweb.org/macoda/ontologies/PMOEA#Researcher"/>
        <rdfs:label>Richard Allmendinger</rdfs:label>
    </owl:NamedIndividual>
    


    <!-- http://www.semanticweb.org/macoda/ontologies/PMOEA#Sergio_Bernal -->

    <owl:NamedIndividual rdf:about="http://www.semanticweb.org/macoda/ontologies/PMOEA#Sergio_Bernal">
        <rdf:type rdf:resource="http://www.semanticweb.org/macoda/ontologies/PMOEA#Researcher"/>
        <rdfs:label>Sergio Bernal</rdfs:label>
    </owl:NamedIndividual>
    


    <!-- http://www.semanticweb.org/macoda/ontologies/PMOEA#Slim_Bechikh -->

    <owl:NamedIndividual rdf:about="http://www.semanticweb.org/macoda/ontologies/PMOEA#Slim_Bechikh">
        <rdf:type rdf:resource="http://www.semanticweb.org/macoda/ontologies/PMOEA#Researcher"/>
        <rdfs:label>Slim Bechikh</rdfs:label>
    </owl:NamedIndividual>
    


    <!-- http://www.semanticweb.org/macoda/ontologies/PMOEA#SortSampleIntoCategory -->

    <owl:NamedIndividual rdf:about="http://www.semanticweb.org/macoda/ontologies/PMOEA#SortSampleIntoCategory">
        <rdf:type rdf:resource="http://www.semanticweb.org/macoda/ontologies/PMOEA#SampleSorts"/>
        <rdfs:comment>sorting some solutions in the current population into relatively good and others</rdfs:comment>
        <rdfs:label>SortSampleIntoCategory</rdfs:label>
    </owl:NamedIndividual>
    


    <!-- http://www.semanticweb.org/macoda/ontologies/PMOEA#SpringDesignProblem -->

    <owl:NamedIndividual rdf:about="http://www.semanticweb.org/macoda/ontologies/PMOEA#SpringDesignProblem">
        <rdf:type rdf:resource="http://www.semanticweb.org/macoda/ontologies/PMOEA#Realworld_Problem"/>
        <PMOEA:isMixedInteger rdf:datatype="http://www.w3.org/2001/XMLSchema#boolean">true</PMOEA:isMixedInteger>
        <PMOEA:ObjectiveNumber rdf:datatype="http://www.w3.org/2001/XMLSchema#integer">2</PMOEA:ObjectiveNumber>
        <rdfs:label>SpringDesignProblem</rdfs:label>
    </owl:NamedIndividual>
    


    <!-- http://www.semanticweb.org/macoda/ontologies/PMOEA#THESEUS -->

    <owl:NamedIndividual rdf:about="http://www.semanticweb.org/macoda/ontologies/PMOEA#THESEUS">
        <rdf:type rdf:resource="http://www.semanticweb.org/macoda/ontologies/PMOEA#OutrankingRelation"/>
        <rdfs:comment>Proposed by Fernandez and Navarro [Fernandez, E., Navarro, J.: A new approach to multicriteria sorting problems based on fuzzy outranking relations: the THESEUS method. Eur. J. Oper. Res. 213, 405413 (2011)].
 It utilizes a new way of evaluating the assignment of an object to an element of the set of ordered categories that were previously defined. This way is based on comparing every possible assignment with the information from various preference relations that are derived from a fuzzy outranking relation defined on the universe of objects</rdfs:comment>
        <rdfs:label>THESEUS</rdfs:label>
    </owl:NamedIndividual>
    


    <!-- http://www.semanticweb.org/macoda/ontologies/PMOEA#TSP_4 -->

    <owl:NamedIndividual rdf:about="http://www.semanticweb.org/macoda/ontologies/PMOEA#TSP_4">
        <rdf:type rdf:resource="http://www.semanticweb.org/macoda/ontologies/PMOEA#Academic_Problem"/>
        <PMOEA:isDiscreteProblem rdf:datatype="http://www.w3.org/2001/XMLSchema#boolean">true</PMOEA:isDiscreteProblem>
        <PMOEA:ObjectiveNumber rdf:datatype="http://www.w3.org/2001/XMLSchema#integer">4</PMOEA:ObjectiveNumber>
        <PMOEA:isManyObjectiveProblem rdf:datatype="http://www.w3.org/2001/XMLSchema#boolean">true</PMOEA:isManyObjectiveProblem>
    </owl:NamedIndividual>
    


    <!-- http://www.semanticweb.org/macoda/ontologies/PMOEA#TSP_5 -->

    <owl:NamedIndividual rdf:about="http://www.semanticweb.org/macoda/ontologies/PMOEA#TSP_5">
        <rdf:type rdf:resource="http://www.semanticweb.org/macoda/ontologies/PMOEA#Academic_Problem"/>
        <PMOEA:isDiscreteProblem rdf:datatype="http://www.w3.org/2001/XMLSchema#boolean">true</PMOEA:isDiscreteProblem>
        <PMOEA:ObjectiveNumber rdf:datatype="http://www.w3.org/2001/XMLSchema#integer">5</PMOEA:ObjectiveNumber>
        <PMOEA:isManyObjectiveProblem rdf:datatype="http://www.w3.org/2001/XMLSchema#boolean">true</PMOEA:isManyObjectiveProblem>
    </owl:NamedIndividual>
    


    <!-- http://www.semanticweb.org/macoda/ontologies/PMOEA#TSP_6 -->

    <owl:NamedIndividual rdf:about="http://www.semanticweb.org/macoda/ontologies/PMOEA#TSP_6">
        <rdf:type rdf:resource="http://www.semanticweb.org/macoda/ontologies/PMOEA#Academic_Problem"/>
        <PMOEA:isContinuousProblem rdf:datatype="http://www.w3.org/2001/XMLSchema#boolean">true</PMOEA:isContinuousProblem>
        <PMOEA:ObjectiveNumber rdf:datatype="http://www.w3.org/2001/XMLSchema#integer">6</PMOEA:ObjectiveNumber>
        <PMOEA:isManyObjectiveProblem rdf:datatype="http://www.w3.org/2001/XMLSchema#boolean">true</PMOEA:isManyObjectiveProblem>
    </owl:NamedIndividual>
    


    <!-- http://www.semanticweb.org/macoda/ontologies/PMOEA#TchebycheffASF -->

    <owl:NamedIndividual rdf:about="http://www.semanticweb.org/macoda/ontologies/PMOEA#TchebycheffASF">
        <rdf:type rdf:resource="http://www.semanticweb.org/macoda/ontologies/PMOEA#AchievementScalarizingFunction"/>
        <rdfs:comment>max</rdfs:comment>
        <rdfs:label>TchebycheffASF</rdfs:label>
    </owl:NamedIndividual>
    


    <!-- http://www.semanticweb.org/macoda/ontologies/PMOEA#WASF-GA -->

    <owl:NamedIndividual rdf:about="http://www.semanticweb.org/macoda/ontologies/PMOEA#WASF-GA">
        <rdf:type rdf:resource="http://www.semanticweb.org/macoda/ontologies/PMOEA#PMOEA"/>
        <PMOEA:hasPreferenceModel rdf:resource="http://www.semanticweb.org/macoda/ontologies/PMOEA#WierzbickiASF"/>
        <PMOEA:hasPreferenceInformationFromDM rdf:resource="http://www.semanticweb.org/macoda/ontologies/PMOEA#ReferencePoint"/>
        <PMOEA:hasInteractionTime rdf:resource="http://www.semanticweb.org/macoda/ontologies/PMOEA#a-priori"/>
        <PMOEA:hasPreferenceIntegration rdf:resource="http://www.semanticweb.org/macoda/ontologies/PMOEA#FrontSorting"/>
        <PMOEA:hasComparison rdf:resource="http://www.semanticweb.org/macoda/ontologies/PMOEA#PMOGA"/>
        <PMOEA:hasComparison rdf:resource="http://www.semanticweb.org/macoda/ontologies/PMOEA#R-NSGA-II"/>
        <PMOEA:hasComparison rdf:resource="http://www.semanticweb.org/macoda/ontologies/PMOEA#g-NSGA-II"/>
        <PMOEA:hasComparison rdf:resource="http://www.semanticweb.org/macoda/ontologies/PMOEA#r-NSGA-II"/>
        <PMOEA:hasInteractiveVersion rdf:resource="http://www.semanticweb.org/macoda/ontologies/PMOEA#iWASF-GA"/>
        <PMOEA:canSolve rdf:resource="http://www.semanticweb.org/macoda/ontologies/PMOEA#DTLZ7_3"/>
        <PMOEA:canSolve rdf:resource="http://www.semanticweb.org/macoda/ontologies/PMOEA#LZ09_F6"/>
        <PMOEA:canSolve rdf:resource="http://www.semanticweb.org/macoda/ontologies/PMOEA#WFG1_3"/>
        <PMOEA:canSolve rdf:resource="http://www.semanticweb.org/macoda/ontologies/PMOEA#WFG1_2"/>
        <PMOEA:canSolve rdf:resource="http://www.semanticweb.org/macoda/ontologies/PMOEA#ZDT2"/>
        <PMOEA:canSolve rdf:resource="http://www.semanticweb.org/macoda/ontologies/PMOEA#ZDT3"/>
        <PMOEA:canSolve rdf:resource="http://www.semanticweb.org/macoda/ontologies/PMOEA#DTLZ2_3"/>
        <PMOEA:canSolve rdf:resource="http://www.semanticweb.org/macoda/ontologies/PMOEA#LZ09_F1"/>
        <PMOEA:canSolve rdf:resource="http://www.semanticweb.org/macoda/ontologies/PMOEA#ZDT1"/>
        <PMOEA:hasResultInfluence rdf:resource="http://www.semanticweb.org/macoda/ontologies/PMOEA#BoundedRegion"/>
        <PMOEA:hasAuthor rdf:resource="http://www.semanticweb.org/macoda/ontologies/PMOEA#Ana_Beln_Ruiz"/>
        <PMOEA:hasAuthor rdf:resource="http://www.semanticweb.org/macoda/ontologies/PMOEA#Mariano_Luque"/>
        <PMOEA:hasAuthor rdf:resource="http://www.semanticweb.org/macoda/ontologies/PMOEA#Ruben_Saborido"/>
        <PMOEA:useLibrary rdf:resource="http://www.semanticweb.org/macoda/ontologies/PMOEA#jMetal"/>
        <PMOEA:hasSearchAlgorithm rdf:resource="http://www.semanticweb.org/macoda/ontologies/PMOEA#GeneralMOEA"/>
        <PMOEA:hasImplementationLanguage rdf:resource="http://www.semanticweb.org/macoda/ontologies/PMOEA#Java"/>
        <PMOEA:hasDevelopingYear rdf:datatype="http://www.w3.org/2001/XMLSchema#integer">2014</PMOEA:hasDevelopingYear>
        <PMOEA:ParetoDominancePreservation rdf:datatype="http://www.w3.org/2001/XMLSchema#boolean">true</PMOEA:ParetoDominancePreservation>
        <PMOEA:hasReference>Ruiz, A. B., Saborido, R., &amp; Luque, M. (2014). A preference-based evolutionary algorithm for multiobjective optimization: the weighting achievement scalarizing function genetic algorithm. Journal of Global Optimization, 62(1), 101-129</PMOEA:hasReference>
        <rdfs:comment>The proposed approach is based on the use of an achievement scalarizing function (ASF) and on the classification of the individuals into several fronts. At each generation of WASF-GA, this classification is done according to the values that each solution takes on the ASF for the reference point and using different weight vectors. These vectors of weights are selected so that the vectors formed by their inverse components constitute a well-distributed representation of the weight vectors space. The main purpose of WASF-GA is to generate a well-distributed set of nondominated objective vectors approximating the region of interest of the Pareto optimal front defined by the reference point.</rdfs:comment>
        <rdfs:label>WASF-GA</rdfs:label>
    </owl:NamedIndividual>
    


    <!-- http://www.semanticweb.org/macoda/ontologies/PMOEA#WeightedEuclideanDistanceASF -->

    <owl:NamedIndividual rdf:about="http://www.semanticweb.org/macoda/ontologies/PMOEA#WeightedEuclideanDistanceASF">
        <rdf:type rdf:resource="http://www.semanticweb.org/macoda/ontologies/PMOEA#AchievementScalarizingFunction"/>
        <rdfs:comment>used in R-NSGA-II</rdfs:comment>
        <rdfs:label>WeightedEuclideanDistanceASF</rdfs:label>
    </owl:NamedIndividual>
    


    <!-- http://www.semanticweb.org/macoda/ontologies/PMOEA#WeldedBeamDesign -->

    <owl:NamedIndividual rdf:about="http://www.semanticweb.org/macoda/ontologies/PMOEA#WeldedBeamDesign">
        <rdf:type rdf:resource="http://www.semanticweb.org/macoda/ontologies/PMOEA#Realworld_Problem"/>
        <PMOEA:isContinuousProblem rdf:datatype="http://www.w3.org/2001/XMLSchema#boolean">true</PMOEA:isContinuousProblem>
        <PMOEA:ObjectiveNumber rdf:datatype="http://www.w3.org/2001/XMLSchema#integer">2</PMOEA:ObjectiveNumber>
        <PMOEA:hasReference>K. Deb, J. Sundar, N. Uday, and S. Chaudhuri. Reference point
based multi-objective optimization using evolutionary algorithms. International Journal of Computational Intelligence Research (IJCIR),
2(6):273286, 2006.</PMOEA:hasReference>
        <rdfs:label>WeldedBeamDesign</rdfs:label>
    </owl:NamedIndividual>
    


    <!-- http://www.semanticweb.org/macoda/ontologies/PMOEA#Xiaodong_Li -->

    <owl:NamedIndividual rdf:about="http://www.semanticweb.org/macoda/ontologies/PMOEA#Xiaodong_Li">
        <rdf:type rdf:resource="http://www.semanticweb.org/macoda/ontologies/PMOEA#Researcher"/>
        <rdfs:label>Xiaodong Li</rdfs:label>
    </owl:NamedIndividual>
    


    <!-- http://www.semanticweb.org/macoda/ontologies/PMOEA#Yu_Setoguchi -->

    <owl:NamedIndividual rdf:about="http://www.semanticweb.org/macoda/ontologies/PMOEA#Yu_Setoguchi">
        <rdf:type rdf:resource="http://www.semanticweb.org/macoda/ontologies/PMOEA#Researcher"/>
        <rdfs:label>Yu Setoguchi</rdfs:label>
    </owl:NamedIndividual>
    


    <!-- http://www.semanticweb.org/macoda/ontologies/PMOEA#Yuki_Tanigaki -->

    <owl:NamedIndividual rdf:about="http://www.semanticweb.org/macoda/ontologies/PMOEA#Yuki_Tanigaki">
        <rdf:type rdf:resource="http://www.semanticweb.org/macoda/ontologies/PMOEA#Researcher"/>
        <rdfs:label>Yuki Tanigaki</rdfs:label>
    </owl:NamedIndividual>
    


    <!-- http://www.semanticweb.org/macoda/ontologies/PMOEA#chapAllmendingerKnowles21 -->

    <owl:NamedIndividual rdf:about="http://www.semanticweb.org/macoda/ontologies/PMOEA#chapAllmendingerKnowles21">
        <rdf:type rdf:resource="http://www.semanticweb.org/macoda/ontologies/PMOEA#Publication"/>
        <rdfs:comment>Richard Allmendinger (lead), Joshua Knowles: Heterogenous Objectives: In Many-Criteria Optimization and Decision Analysis, D. Brockhoff, M. Emmerich, B. Naujoks, R. Purshouse (editors). Springer, (to be published)</rdfs:comment>
    </owl:NamedIndividual>
    


    <!-- http://www.semanticweb.org/macoda/ontologies/PMOEA#constraints -->

    <owl:NamedIndividual rdf:about="http://www.semanticweb.org/macoda/ontologies/PMOEA#constraints">
        <rdf:type rdf:resource="http://www.semanticweb.org/macoda/ontologies/PMOEA#Constraints"/>
        <rdfs:label>constraints</rdfs:label>
    </owl:NamedIndividual>
    


    <!-- http://www.semanticweb.org/macoda/ontologies/PMOEA#g-NSGA-II -->

    <owl:NamedIndividual rdf:about="http://www.semanticweb.org/macoda/ontologies/PMOEA#g-NSGA-II">
        <rdf:type rdf:resource="http://www.semanticweb.org/macoda/ontologies/PMOEA#PMOEA"/>
        <PMOEA:hasPreferenceModel rdf:resource="http://www.semanticweb.org/macoda/ontologies/PMOEA#PreferencePoint"/>
        <PMOEA:hasPreferenceInformationFromDM rdf:resource="http://www.semanticweb.org/macoda/ontologies/PMOEA#ReferencePoint"/>
        <PMOEA:hasInteractionTime rdf:resource="http://www.semanticweb.org/macoda/ontologies/PMOEA#a-priori"/>
        <PMOEA:hasInteractionTime rdf:resource="http://www.semanticweb.org/macoda/ontologies/PMOEA#progressive"/>
        <PMOEA:hasPreferenceIntegration rdf:resource="http://www.semanticweb.org/macoda/ontologies/PMOEA#g-dominance"/>
        <PMOEA:canSolve rdf:resource="http://www.semanticweb.org/macoda/ontologies/PMOEA#Deb32"/>
        <PMOEA:canSolve rdf:resource="http://www.semanticweb.org/macoda/ontologies/PMOEA#ZDT1"/>
        <PMOEA:hasResultInfluence rdf:resource="http://www.semanticweb.org/macoda/ontologies/PMOEA#BoundedRegion"/>
        <PMOEA:hasAuthor rdf:resource="http://www.semanticweb.org/macoda/ontologies/PMOEA#Alfredo_G._Hernndez-Daz"/>
        <PMOEA:hasAuthor rdf:resource="http://www.semanticweb.org/macoda/ontologies/PMOEA#Carlos_Coello_Coello"/>
        <PMOEA:hasAuthor rdf:resource="http://www.semanticweb.org/macoda/ontologies/PMOEA#Julin_Molina"/>
        <PMOEA:hasAuthor rdf:resource="http://www.semanticweb.org/macoda/ontologies/PMOEA#Luis_V._Santana"/>
        <PMOEA:hasAuthor rdf:resource="http://www.semanticweb.org/macoda/ontologies/PMOEA#Rafael_Caballero"/>
        <PMOEA:hasSearchAlgorithm rdf:resource="http://www.semanticweb.org/macoda/ontologies/PMOEA#NSGA-II"/>
        <PMOEA:hasDevelopingYear rdf:datatype="http://www.w3.org/2001/XMLSchema#integer">2009</PMOEA:hasDevelopingYear>
        <PMOEA:MultipleRegionOfInterest rdf:datatype="http://www.w3.org/2001/XMLSchema#boolean">true</PMOEA:MultipleRegionOfInterest>
        <PMOEA:SpreadControl rdf:datatype="http://www.w3.org/2001/XMLSchema#boolean">false</PMOEA:SpreadControl>
        <PMOEA:ParetoDominancePreservation rdf:datatype="http://www.w3.org/2001/XMLSchema#boolean">false</PMOEA:ParetoDominancePreservation>
        <PMOEA:hasReference>Molina, J., L. V. Santana, A. G. Hernndez-Daz, C. A. C. Coello and R. Caballero (2009). &quot;g-dominance: Reference point based dominance for multiobjective metaheuristics.&quot; European Journal of Operational Research 197(2): 685-692</PMOEA:hasReference>
        <rdfs:comment>In this paper, a new dominance relation called g-dominance is suggested based on a reference point. In the new relation, objective vectors satisfying all the aspiration values and objective vectors fulfilling none of them are preferred over objective vectors satisfying some of the aspiration levels. The main advantage of the g-dominance is that it can be incorporated in any metaheuristic algorithm, given that it does not modify the architecture of the algorithm. However, the g-dominance does not preserve the Pareto dominance</rdfs:comment>
        <rdfs:label>g-NSGA-II</rdfs:label>
    </owl:NamedIndividual>
    


    <!-- http://www.semanticweb.org/macoda/ontologies/PMOEA#generalHeterogeneousObjectives -->

    <owl:NamedIndividual rdf:about="http://www.semanticweb.org/macoda/ontologies/PMOEA#generalHeterogeneousObjectives">
        <rdf:type rdf:resource="http://www.semanticweb.org/macoda/ontologies/PMOEA#HeterogeneousObjectives"/>
        <PMOEA:discussedIn rdf:resource="http://www.semanticweb.org/macoda/ontologies/PMOEA#chapAllmendingerKnowles21"/>
    </owl:NamedIndividual>
    


    <!-- http://www.semanticweb.org/macoda/ontologies/PMOEA#iPMA -->

    <owl:NamedIndividual rdf:about="http://www.semanticweb.org/macoda/ontologies/PMOEA#iPMA">
        <rdf:type rdf:resource="http://www.semanticweb.org/macoda/ontologies/PMOEA#PMOEA"/>
        <PMOEA:hasPreferenceModel rdf:resource="http://www.semanticweb.org/macoda/ontologies/PMOEA#LinearUtilityFunction"/>
        <PMOEA:hasPreferenceInformationFromDM rdf:resource="http://www.semanticweb.org/macoda/ontologies/PMOEA#PairwiseComparison"/>
        <PMOEA:hasInteractionTime rdf:resource="http://www.semanticweb.org/macoda/ontologies/PMOEA#progressive"/>
        <PMOEA:hasPreferenceIntegration rdf:resource="http://www.semanticweb.org/macoda/ontologies/PMOEA#WeightsInASF"/>
        <PMOEA:canSolve rdf:resource="http://www.semanticweb.org/macoda/ontologies/PMOEA#TSP_4"/>
        <PMOEA:canSolve rdf:resource="http://www.semanticweb.org/macoda/ontologies/PMOEA#TSP_5"/>
        <PMOEA:canSolve rdf:resource="http://www.semanticweb.org/macoda/ontologies/PMOEA#TSP_6"/>
        <PMOEA:hasResultInfluence rdf:resource="http://www.semanticweb.org/macoda/ontologies/PMOEA#BoundedRegion"/>
        <PMOEA:hasAuthor rdf:resource="http://www.semanticweb.org/macoda/ontologies/PMOEA#Andrzej_Jaszkiewicz"/>
        <PMOEA:hasSearchAlgorithm rdf:resource="http://www.semanticweb.org/macoda/ontologies/PMOEA#PMA"/>
        <PMOEA:hasDevelopingYear rdf:datatype="http://www.w3.org/2001/XMLSchema#integer">2007</PMOEA:hasDevelopingYear>
        <PMOEA:hasReference>Jaszkiewicz, A. (2007). &quot;Interactive multiobjective optimization with the Pareto memetic algorithm.&quot; Foundations of Computing and Decision Sciences 32: 15-31</PMOEA:hasReference>
        <rdfs:comment>The DM preference is elicited from pairwise comparison of solutions. However, this strategy does not aim to identify a single most likely utility function but, rather, simultaneously maintains a range of utility functions compatible with the elicited preferences. In other words, the preference information is not applied to create a single compatible weight vector but it is to reduce the set of possible weight vectors</rdfs:comment>
        <rdfs:label>iPMA</rdfs:label>
    </owl:NamedIndividual>
    


    <!-- http://www.semanticweb.org/macoda/ontologies/PMOEA#r-Dominance -->

    <owl:NamedIndividual rdf:about="http://www.semanticweb.org/macoda/ontologies/PMOEA#r-Dominance">
        <rdf:type rdf:resource="http://www.semanticweb.org/macoda/ontologies/PMOEA#DominanceRelation"/>
        <rdfs:comment>This new dominance relation distinguishes objective vectors according to their Euclidean distance to a reference point given by the DM, emphasizing those closer to the reference point. In r-NSGA-II</rdfs:comment>
        <rdfs:label>r-dominance</rdfs:label>
    </owl:NamedIndividual>
    


    <!-- http://www.semanticweb.org/macoda/ontologies/PMOEA#r-NSGA-II -->

    <owl:NamedIndividual rdf:about="http://www.semanticweb.org/macoda/ontologies/PMOEA#r-NSGA-II">
        <rdf:type rdf:resource="http://www.semanticweb.org/macoda/ontologies/PMOEA#PMOEA"/>
        <PMOEA:hasPreferenceModel rdf:resource="http://www.semanticweb.org/macoda/ontologies/PMOEA#WeightedEuclideanDistanceASF"/>
        <PMOEA:hasPreferenceInformationFromDM rdf:resource="http://www.semanticweb.org/macoda/ontologies/PMOEA#ReferencePoint"/>
        <PMOEA:hasInteractionTime rdf:resource="http://www.semanticweb.org/macoda/ontologies/PMOEA#a-priori"/>
        <PMOEA:hasInteractionTime rdf:resource="http://www.semanticweb.org/macoda/ontologies/PMOEA#progressive"/>
        <PMOEA:hasPreferenceIntegration rdf:resource="http://www.semanticweb.org/macoda/ontologies/PMOEA#r-Dominance"/>
        <PMOEA:hasComparison rdf:resource="http://www.semanticweb.org/macoda/ontologies/PMOEA#PBEA"/>
        <PMOEA:hasComparison rdf:resource="http://www.semanticweb.org/macoda/ontologies/PMOEA#R-NSGA-II"/>
        <PMOEA:hasComparison rdf:resource="http://www.semanticweb.org/macoda/ontologies/PMOEA#g-NSGA-II"/>
        <PMOEA:canSolve rdf:resource="http://www.semanticweb.org/macoda/ontologies/PMOEA#DTLZ2_10"/>
        <PMOEA:canSolve rdf:resource="http://www.semanticweb.org/macoda/ontologies/PMOEA#DTLZ7_3"/>
        <PMOEA:canSolve rdf:resource="http://www.semanticweb.org/macoda/ontologies/PMOEA#Fonseca_test"/>
        <PMOEA:canSolve rdf:resource="http://www.semanticweb.org/macoda/ontologies/PMOEA#ZDT3"/>
        <PMOEA:canSolve rdf:resource="http://www.semanticweb.org/macoda/ontologies/PMOEA#DTLZ2_3"/>
        <PMOEA:hasResultInfluence rdf:resource="http://www.semanticweb.org/macoda/ontologies/PMOEA#BoundedRegion"/>
        <PMOEA:hasAuthor rdf:resource="http://www.semanticweb.org/macoda/ontologies/PMOEA#Khaled_Ghdira"/>
        <PMOEA:hasAuthor rdf:resource="http://www.semanticweb.org/macoda/ontologies/PMOEA#Slim_Bechikh"/>
        <PMOEA:hasAuthor rdf:resource="http://www.semanticweb.org/macoda/ontologies/PMOEA#Lamjed_Ben_Said,"/>
        <PMOEA:hasSearchAlgorithm rdf:resource="http://www.semanticweb.org/macoda/ontologies/PMOEA#NSGA-II"/>
        <PMOEA:hasImplementationLanguage rdf:resource="http://www.semanticweb.org/macoda/ontologies/PMOEA#Matlab"/>
        <PMOEA:hasDevelopingYear rdf:datatype="http://www.w3.org/2001/XMLSchema#integer">2010</PMOEA:hasDevelopingYear>
        <PMOEA:MultipleRegionOfInterest rdf:datatype="http://www.w3.org/2001/XMLSchema#boolean">true</PMOEA:MultipleRegionOfInterest>
        <PMOEA:SpreadControl rdf:datatype="http://www.w3.org/2001/XMLSchema#boolean">true</PMOEA:SpreadControl>
        <PMOEA:ParetoDominancePreservation rdf:datatype="http://www.w3.org/2001/XMLSchema#boolean">true</PMOEA:ParetoDominancePreservation>
        <PMOEA:hasReference>Ben Said, L., S. Bechikh and K. Ghdira (2010). &quot;The r-dominance: a new dominance relation for interactive evolutionary multicriteria decision making.&quot; Evolutionary Computation, IEEE Transactions on 14(5): 801-818</PMOEA:hasReference>
        <rdfs:comment>In this paper, we introduce a new variant of the Pareto dominance relation, called r-dominance, which has the ability to create a strict partial order among Pareto-equivalent solutions. This fact makes such a relation able to guide the search toward the interesting parts of the Pareto optimal region based on the decision makers preferences expressed as a set of aspiration levels</rdfs:comment>
        <rdfs:label>r-NSGA-II</rdfs:label>
    </owl:NamedIndividual>
    


    <!-- http://www.semanticweb.org/macoda/ontologies/PMOEA#Fernando_Lopez, -->

    <owl:NamedIndividual rdf:about="http://www.semanticweb.org/macoda/ontologies/PMOEA#Fernando_Lopez,">
        <rdf:type rdf:resource="http://www.semanticweb.org/macoda/ontologies/PMOEA#Researcher"/>
        <rdfs:label>Fernando Lopez</rdfs:label>
    </owl:NamedIndividual>
    


    <!-- http://www.semanticweb.org/macoda/ontologies/PMOEA#Lamjed_Ben_Said, -->

    <owl:NamedIndividual rdf:about="http://www.semanticweb.org/macoda/ontologies/PMOEA#Lamjed_Ben_Said,">
        <rdf:type rdf:resource="http://www.semanticweb.org/macoda/ontologies/PMOEA#Researcher"/>
        <rdfs:label>Lamjed Ben Said</rdfs:label>
    </owl:NamedIndividual>
    


    <!-- 
    ///////////////////////////////////////////////////////////////////////////////////////
    //
    // Annotations
    //
    ///////////////////////////////////////////////////////////////////////////////////////
     -->

    <rdf:Description rdf:about="http://www.semanticweb.org/macoda/ontologies/PMOEA#LightBeamSearch">
        <rdfs:label>LightBeamSearch</rdfs:label>
        <rdfs:comment>The light beam search uses a reference direction and additional thresholds which are then used to find some possibly interesting neighboring solutions around the most preferred solution.The hybrid procedure has the ability to find the part of the Pareto optimal region illuminated by the light beam emanating from the starting point to the aspiration point with a span controlled by the veto threshold</rdfs:comment>
    </rdf:Description>
    <rdf:Description rdf:about="http://www.semanticweb.org/macoda/ontologies/PMOEA#ObjectiveRelativeImportance">
        <rdfs:label>ObjectiveRelativeImportance</rdfs:label>
        <rdfs:comment>The preference model is unique in that it allows incomparability between objectives, results in a partial ranking of objectives and provides an explicit functional correspondence between explicated decision maker preference and the target region in the objective space</rdfs:comment>
    </rdf:Description>
    <rdf:Description rdf:about="http://www.semanticweb.org/macoda/ontologies/PMOEA#PreferencePoint">
        <rdfs:comment>PreferencePoint means this model wants to find set of solutions around the point given by the DM</rdfs:comment>
        <rdfs:label>PreferencePoint</rdfs:label>
    </rdf:Description>
    


    <!-- 
    ///////////////////////////////////////////////////////////////////////////////////////
    //
    // General axioms
    //
    ///////////////////////////////////////////////////////////////////////////////////////
     -->

    <rdf:Description>
        <rdf:type rdf:resource="http://www.w3.org/2002/07/owl#AllDisjointClasses"/>
        <owl:members rdf:parseType="Collection">
            <rdf:Description rdf:about="http://www.semanticweb.org/macoda/ontologies/PMOEA#GeneralAdditive"/>
            <rdf:Description rdf:about="http://www.semanticweb.org/macoda/ontologies/PMOEA#ChoquetIntegral"/>
            <rdf:Description rdf:about="http://www.semanticweb.org/macoda/ontologies/PMOEA#Linear"/>
            <rdf:Description rdf:about="http://www.semanticweb.org/macoda/ontologies/PMOEA#AdditivePiecewiseLinear"/>
            <rdf:Description rdf:about="http://www.semanticweb.org/macoda/ontologies/PMOEA#DesirabilityFunction"/>
            <rdf:Description rdf:about="http://www.semanticweb.org/macoda/ontologies/PMOEA#Polynomial"/>
        </owl:members>
    </rdf:Description>
    <rdf:Description>
        <rdf:type rdf:resource="http://www.w3.org/2002/07/owl#AllDisjointClasses"/>
        <owl:members rdf:parseType="Collection">
            <rdf:Description rdf:about="http://www.semanticweb.org/macoda/ontologies/PMOEA#DiversityVSConvergence_based"/>
            <rdf:Description rdf:about="http://www.semanticweb.org/macoda/ontologies/PMOEA#PSO_based"/>
            <rdf:Description rdf:about="http://www.semanticweb.org/macoda/ontologies/PMOEA#Decomposition_based"/>
            <rdf:Description rdf:about="http://www.semanticweb.org/macoda/ontologies/PMOEA#ACO_based"/>
            <rdf:Description rdf:about="http://www.semanticweb.org/macoda/ontologies/PMOEA#Coevolution_based"/>
            <rdf:Description rdf:about="http://www.semanticweb.org/macoda/ontologies/PMOEA#Indicator_based"/>
        </owl:members>
    </rdf:Description>
    <rdf:Description>
        <rdf:type rdf:resource="http://www.w3.org/2002/07/owl#AllDisjointClasses"/>
        <owl:members rdf:parseType="Collection">
            <rdf:Description rdf:about="http://www.semanticweb.org/macoda/ontologies/PMOEA#PolyhedralConeBased"/>
            <rdf:Description rdf:about="http://www.semanticweb.org/macoda/ontologies/PMOEA#UtilityFunction"/>
            <rdf:Description rdf:about="http://www.semanticweb.org/macoda/ontologies/PMOEA#DecisionRules"/>
            <rdf:Description rdf:about="http://www.semanticweb.org/macoda/ontologies/PMOEA#AchievementScalarizingFunction"/>
            <rdf:Description rdf:about="http://www.semanticweb.org/macoda/ontologies/PMOEA#OutrankingRelation"/>
            <rdf:Description rdf:about="http://www.semanticweb.org/macoda/ontologies/PMOEA#WeightFunctionInObjectiveSpace"/>
        </owl:members>
    </rdf:Description>
    <rdf:Description>
        <rdf:type rdf:resource="http://www.w3.org/2002/07/owl#AllDisjointClasses"/>
        <owl:members rdf:parseType="Collection">
            <rdf:Description rdf:about="http://www.semanticweb.org/macoda/ontologies/PMOEA#OrdinalRegression"/>
            <rdf:Description rdf:about="http://www.semanticweb.org/macoda/ontologies/PMOEA#LinearProgramming"/>
            <rdf:Description rdf:about="http://www.semanticweb.org/macoda/ontologies/PMOEA#NeuralNetwork"/>
            <rdf:Description rdf:about="http://www.semanticweb.org/macoda/ontologies/PMOEA#SupportVectorMachine"/>
        </owl:members>
    </rdf:Description>
    <rdf:Description>
        <rdf:type rdf:resource="http://www.w3.org/2002/07/owl#AllDisjointClasses"/>
        <owl:members rdf:parseType="Collection">
            <rdf:Description rdf:about="http://www.semanticweb.org/macoda/ontologies/PMOEA#FrontSorting"/>
            <rdf:Description rdf:about="http://www.semanticweb.org/macoda/ontologies/PMOEA#TerminationCriterion"/>
            <rdf:Description rdf:about="http://www.semanticweb.org/macoda/ontologies/PMOEA#ASF"/>
            <rdf:Description rdf:about="http://www.semanticweb.org/macoda/ontologies/PMOEA#DominanceRelation"/>
            <rdf:Description rdf:about="http://www.semanticweb.org/macoda/ontologies/PMOEA#SetQualityIndicator"/>
            <rdf:Description rdf:about="http://www.semanticweb.org/macoda/ontologies/PMOEA#CrowdingDistance"/>
        </owl:members>
    </rdf:Description>
    <rdf:Description>
        <rdf:type rdf:resource="http://www.w3.org/2002/07/owl#AllDisjointClasses"/>
        <owl:members rdf:parseType="Collection">
            <rdf:Description rdf:about="http://www.semanticweb.org/macoda/ontologies/PMOEA#PreferenceInformationFromDM"/>
            <rdf:Description rdf:about="http://www.semanticweb.org/macoda/ontologies/PMOEA#PMOEA"/>
            <rdf:Description rdf:about="http://www.semanticweb.org/macoda/ontologies/PMOEA#PreferenceModel"/>
            <rdf:Description rdf:about="http://www.semanticweb.org/macoda/ontologies/PMOEA#PreferenceIntegration"/>
        </owl:members>
    </rdf:Description>
    <rdf:Description>
        <rdf:type rdf:resource="http://www.w3.org/2002/07/owl#AllDisjointClasses"/>
        <owl:members rdf:parseType="Collection">
            <rdf:Description rdf:about="http://www.semanticweb.org/macoda/ontologies/PMOEA#a-priori"/>
            <rdf:Description rdf:about="http://www.semanticweb.org/macoda/ontologies/PMOEA#a-posteriori"/>
            <rdf:Description rdf:about="http://www.semanticweb.org/macoda/ontologies/PMOEA#progressive"/>
        </owl:members>
    </rdf:Description>
    <rdf:Description>
        <rdf:type rdf:resource="http://www.w3.org/2002/07/owl#AllDifferent"/>
        <owl:distinctMembers rdf:parseType="Collection">
            <rdf:Description rdf:about="http://www.semanticweb.org/macoda/ontologies/PMOEA#W_HypE"/>
            <rdf:Description rdf:about="http://www.semanticweb.org/macoda/ontologies/PMOEA#iTDEA"/>
            <rdf:Description rdf:about="http://www.semanticweb.org/macoda/ontologies/PMOEA#W_IBEA"/>
            <rdf:Description rdf:about="http://www.semanticweb.org/macoda/ontologies/PMOEA#iW_HypE"/>
            <rdf:Description rdf:about="http://www.semanticweb.org/macoda/ontologies/PMOEA#W_HypE"/>
        </owl:distinctMembers>
    </rdf:Description>
    <rdf:Description>
        <rdf:type rdf:resource="http://www.w3.org/2002/07/owl#AllDifferent"/>
        <owl:distinctMembers rdf:parseType="Collection">
            <rdf:Description rdf:about="http://www.semanticweb.org/macoda/ontologies/PMOEA#Knapsack_2"/>
            <rdf:Description rdf:about="http://www.semanticweb.org/macoda/ontologies/PMOEA#LZ09_F1"/>
        </owl:distinctMembers>
    </rdf:Description>
    <rdf:Description>
        <rdf:type rdf:resource="http://www.w3.org/2002/07/owl#AllDifferent"/>
        <owl:distinctMembers rdf:parseType="Collection">
            <rdf:Description rdf:about="http://www.semanticweb.org/macoda/ontologies/PMOEA#IBEA"/>
            <rdf:Description rdf:about="http://www.semanticweb.org/macoda/ontologies/PMOEA#R2_EMOA"/>
            <rdf:Description rdf:about="http://www.semanticweb.org/macoda/ontologies/PMOEA#SMS-EMOA"/>
            <rdf:Description rdf:about="http://www.semanticweb.org/macoda/ontologies/PMOEA#HypE"/>
        </owl:distinctMembers>
    </rdf:Description>
    <rdf:Description>
        <rdf:type rdf:resource="http://www.w3.org/2002/07/owl#AllDifferent"/>
        <owl:distinctMembers rdf:parseType="Collection">
            <rdf:Description rdf:about="http://www.semanticweb.org/macoda/ontologies/PMOEA#DTLZ2_2"/>
            <rdf:Description rdf:about="http://www.semanticweb.org/macoda/ontologies/PMOEA#DTLZ2_5"/>
            <rdf:Description rdf:about="http://www.semanticweb.org/macoda/ontologies/PMOEA#DTLZ1_3"/>
            <rdf:Description rdf:about="http://www.semanticweb.org/macoda/ontologies/PMOEA#DTLZ2_7"/>
            <rdf:Description rdf:about="http://www.semanticweb.org/macoda/ontologies/PMOEA#DTLZ2_3"/>
        </owl:distinctMembers>
    </rdf:Description>
    <rdf:Description>
        <rdf:type rdf:resource="http://www.w3.org/2002/07/owl#AllDifferent"/>
        <owl:distinctMembers rdf:parseType="Collection">
            <rdf:Description rdf:about="http://www.semanticweb.org/macoda/ontologies/PMOEA#a-priori"/>
            <rdf:Description rdf:about="http://www.semanticweb.org/macoda/ontologies/PMOEA#progressive"/>
            <rdf:Description rdf:about="http://www.semanticweb.org/macoda/ontologies/PMOEA#a-posteriori"/>
        </owl:distinctMembers>
    </rdf:Description>
    <rdf:Description>
        <rdf:type rdf:resource="http://www.w3.org/2002/07/owl#AllDifferent"/>
        <owl:distinctMembers rdf:parseType="Collection">
            <rdf:Description rdf:about="http://www.semanticweb.org/macoda/ontologies/PMOEA#Souhila_Kaci"/>
            <rdf:Description rdf:about="http://www.semanticweb.org/macoda/ontologies/PMOEA#Heike_Trautmann"/>
            <rdf:Description rdf:about="http://www.semanticweb.org/macoda/ontologies/PMOEA#Boris_Naujoks"/>
            <rdf:Description rdf:about="http://www.semanticweb.org/macoda/ontologies/PMOEA#Michael_Emmerich"/>
            <rdf:Description rdf:about="http://www.semanticweb.org/macoda/ontologies/PMOEA#Johannes Bader"/>
            <rdf:Description rdf:about="http://www.semanticweb.org/macoda/ontologies/PMOEA#Lothar_Thiele"/>
            <rdf:Description rdf:about="http://www.semanticweb.org/macoda/ontologies/PMOEA#Juergen_Branke"/>
            <rdf:Description rdf:about="http://www.semanticweb.org/macoda/ontologies/PMOEA#Tobias_Wagner"/>
            <rdf:Description rdf:about="http://www.semanticweb.org/macoda/ontologies/PMOEA#Youssef_Hamadi"/>
            <rdf:Description rdf:about="http://www.semanticweb.org/macoda/ontologies/PMOEA#Dimo_Brockhoff"/>
            <rdf:Description rdf:about="http://www.semanticweb.org/macoda/ontologies/PMOEA#Kalyanmoy_Deb"/>
            <rdf:Description rdf:about="http://www.semanticweb.org/macoda/ontologies/PMOEA#Anne_Auger"/>
        </owl:distinctMembers>
    </rdf:Description>
    <rdf:Description>
        <rdf:type rdf:resource="http://www.w3.org/2002/07/owl#AllDifferent"/>
        <owl:distinctMembers rdf:parseType="Collection">
            <rdf:Description rdf:about="http://www.semanticweb.org/macoda/ontologies/PMOEA#ZDT6"/>
            <rdf:Description rdf:about="http://www.semanticweb.org/macoda/ontologies/PMOEA#DTLZ2_7"/>
            <rdf:Description rdf:about="http://www.semanticweb.org/macoda/ontologies/PMOEA#ZDT3"/>
            <rdf:Description rdf:about="http://www.semanticweb.org/macoda/ontologies/PMOEA#DTLZ2_3"/>
            <rdf:Description rdf:about="http://www.semanticweb.org/macoda/ontologies/PMOEA#ZDT1"/>
        </owl:distinctMembers>
    </rdf:Description>
</rdf:RDF>



<!-- Generated by the OWL API (version 4.5.9.2019-02-01T07:24:44Z) https://github.com/owlcs/owlapi -->
